@prefix : <https://w3id.org/i40/sto/iot/concerns/> .
@prefix ns1: <https://www.w3.org/ns/> .
@prefix ns10: <http://purl.org/vocab/vann/> .
@prefix ns11: <http://usefulinc.com/ns/doap#> .
@prefix ns12: <http://purl.org/dc/elements/1.1/> .
@prefix ns2: <http://purl.org/dc/terms/> .
@prefix ns3: <http://www.ontologydesignpatterns.org/ont/dul/DUL.owl#> .
@prefix ns4: <https://w3id.org/i40/sto#> .
@prefix ns5: <https://w3id.org/i40/sto/iot#> .
@prefix ns6: <http://www.w3.org/2004/02/skos/core#> .
@prefix ns7: <http://voag.linkedmodel.org/voag#> .
@prefix ns8: <http://xmlns.com/foaf/0.1/> .
@prefix ns9: <http://creativecommons.org/ns#> .
@prefix owl: <http://www.w3.org/2002/07/owl#> .
@prefix rdf: <http://www.w3.org/1999/02/22-rdf-syntax-ns#> .
@prefix rdfs: <http://www.w3.org/2000/01/rdf-schema#> .
@prefix xsd: <http://www.w3.org/2001/XMLSchema#> .

ns9:attributionName a owl:DatatypeProperty .

ns9:attributionURL a owl:DatatypeProperty .

<http://example.org/iira#CrosscuttingFunction> a owl:Class ;
    rdfs:label "IIRA Crosscutting Function"@en ;
    ns2:creator "sebastian"@en ;
    rdfs:comment "Often these enabling functions, the so-called crosscutting functions, need to be made available across many of the system functional components. For Reference Architecture 6: Functional Viewpoint example, system functions need to be connected so they can interact with each other to complete functionality at the system level."@en ;
    rdfs:subClassOf [ a owl:Restriction ;
            owl:hasValue <http://example.org/iira#FunctionalViewpoint> ;
            owl:onProperty ns3:isPartOf ],
        ns4:StandardClassification .

<http://example.org/iira#FunctionalDomain> a owl:Class ;
    rdfs:label "IIRA Functional Domain"@en ;
    rdfs:subClassOf [ a owl:Restriction ;
            owl:hasValue ns4:IIRA ;
            owl:onProperty ns4:isDescribedin ],
        ns4:StandardClassification .

<http://example.org/iira#SystemCharacteristics> a owl:Class ;
    rdfs:label "IIRA System Characteristic"@en ;
    rdfs:subClassOf [ a owl:Restriction ;
            owl:hasValue <http://example.org/iira#FunctionalViewpoint> ;
            owl:onProperty ns3:isPartOf ],
        ns4:StandardClassification .

ns2:LicenseDocument a owl:Class ;
    rdfs:label "License Document"@en ;
    rdfs:comment "A legal document giving official permission to do something with a Resource."@en ;
    rdfs:isDefinedBy ns2: .

ns2:creator rdfs:label "Creator"@en ;
    ns2:description "Examples of a Creator include a person, an organization, or a service."@en ;
    ns2:hasVersion <http://dublincore.org/usage/terms/history/#creatorT-002> ;
    ns2:issued "2008-01-14"^^xsd:date ;
    ns2:modified "2010-10-11"^^xsd:date ;
    rdfs:comment "An entity primarily responsible for making the resource."@en ;
    rdfs:isDefinedBy ns2: ;
    rdfs:range ns2:Agent ;
    rdfs:subPropertyOf ns12:creator,
        ns2:contributor ;
    owl:equivalentProperty ns8:maker .

ns2:description rdfs:label "Description"@en ;
    ns2:description "Description may include but is not limited to: an abstract, a table of contents, a graphical representation, or a free-text account of the resource."@en ;
    ns2:hasVersion <http://dublincore.org/usage/terms/history/#descriptionT-001> ;
    ns2:issued "2008-01-14"^^xsd:date ;
    ns2:modified "2008-01-14"^^xsd:date ;
    rdfs:comment "An account of the resource."@en ;
    rdfs:isDefinedBy ns2: ;
    rdfs:subPropertyOf ns12:description .

ns2:format a owl:AnnotationProperty .

ns2:hasVersion rdfs:label "Has Version"@en ;
    ns2:hasVersion <http://dublincore.org/usage/terms/history/#hasVersion-003> ;
    ns2:issued "2000-07-11"^^xsd:date ;
    ns2:modified "2008-01-14"^^xsd:date ;
    rdfs:comment "A related resource that is a version, edition, or adaptation of the described resource."@en ;
    rdfs:isDefinedBy ns2: ;
    rdfs:subPropertyOf ns12:relation,
        ns2:relation ;
    ns6:note "This term is intended to be used with non-literal values as defined in the DCMI Abstract Model (http://dublincore.org/documents/abstract-model/).  As of December 2007, the DCMI Usage Board is seeking a way to express this intention with a formal range declaration."@en .

ns2:issued rdfs:label "Date Issued"@en ;
    ns2:hasVersion <http://dublincore.org/usage/terms/history/#issued-003> ;
    ns2:issued "2000-07-11"^^xsd:date ;
    ns2:modified "2008-01-14"^^xsd:date ;
    rdfs:comment "Date of formal issuance (e.g., publication) of the resource."@en ;
    rdfs:isDefinedBy ns2: ;
    rdfs:range rdfs:Literal ;
    rdfs:subPropertyOf ns12:date,
        ns2:date .

ns2:modified rdfs:label "Date Modified"@en ;
    ns2:hasVersion <http://dublincore.org/usage/terms/history/#modified-003> ;
    ns2:issued "2000-07-11"^^xsd:date ;
    ns2:modified "2008-01-14"^^xsd:date ;
    rdfs:comment "Date on which the resource was changed."@en ;
    rdfs:isDefinedBy ns2: ;
    rdfs:range rdfs:Literal ;
    rdfs:subPropertyOf ns12:date,
        ns2:date .

ns2:title rdfs:label "Title"@en ;
    ns2:hasVersion <http://dublincore.org/usage/terms/history/#titleT-002> ;
    ns2:issued "2008-01-14"^^xsd:date ;
    ns2:modified "2010-10-11"^^xsd:date ;
    rdfs:comment "A name given to the resource."@en ;
    rdfs:isDefinedBy ns2: ;
    rdfs:range rdfs:Literal ;
    rdfs:subPropertyOf ns12:title .

ns7:hasStakeholder a owl:AnnotationProperty .

<http://w3id.org/ids/ram/Perspective> a owl:Class ;
    rdfs:label "IDS RAM Perspective"@en ;
    rdfs:subClassOf ns4:StandardClassification ;
    owl:equivalentClass [ a owl:Class ;
            owl:oneOf ( <https://w3id.org/ids/ram/Certification> <https://w3id.org/ids/ram/Governance> <https://w3id.org/ids/ram/Security> ) ] .

<http://www.ontology-of-units-of-measure.org/resource/om-2/hasNumericalValue> a owl:DatatypeProperty ;
    rdfs:label "has numerical value"@en ;
    rdfs:domain [ a owl:Class ] .

<http://www.ontology-of-units-of-measure.org/resource/om-2/hasUnit> a owl:ObjectProperty ;
    rdfs:label "has unit"@en ;
    rdfs:domain <http://org.semanticweb.owlapi/error#Error1> ;
    rdfs:range <http://www.ontology-of-units-of-measure.org/resource/om-2/Unit> .

ns3:isComponentOf a owl:ObjectProperty ;
    rdfs:label "is Component Of"@en ;
    rdfs:comment "Represents Standards that are component of other Standards. This relation is not transitive"@en ;
    rdfs:domain ns4:Standard ;
    rdfs:isDefinedBy <http://www.ontologydesignpatterns.org/ont/dul/DUL.owl> ;
    rdfs:range [ a owl:Class ;
            owl:unionOf ( ns4:Standard ns4:StandardPart ) ] ;
    rdfs:subPropertyOf ns4:relatedTo .

ns3:isMemberOf a owl:ObjectProperty ;
    rdfs:label "is member of"@en,
        "è membro di"@it ;
    rdfs:comment "A relation between collections and entities, e.g. 'the Night Watch by Rembrandt is in the Rijksmuseum collection'; 'Davide is member of the Pen Club', 'Igor is one the subjects chosen for the experiment'."@en ;
    rdfs:domain ns3:Entity ;
    rdfs:isDefinedBy <http://www.ontologydesignpatterns.org/ont/dul/DUL.owl> ;
    rdfs:range ns3:Collection ;
    rdfs:subPropertyOf ns3:associatedWith .

rdf:value a owl:AnnotationProperty .

ns6:altLabel a owl:AnnotationProperty ;
    rdfs:label "alternative label"@en .

ns6:definition a owl:AnnotationProperty ;
    rdfs:label "definition"@en .

ns6:narrower a owl:AnnotationProperty .

ns6:note a owl:AnnotationProperty ;
    rdfs:label "note"@en .

ns6:prefLabel a owl:AnnotationProperty ;
    rdfs:label "preferred label"@en .

<http://www.w3.org/ns/prov#wasGeneratedBy> a owl:ObjectProperty ;
    rdfs:label "was Generated By"@en ;
    rdfs:comment "Standard A has influences in Standard B. For example, IEC_61499 hasInfluenceIn IEC_61804-2(EDDL)"@en ;
    rdfs:isDefinedBy "https://www.w3.org/TR/prov-o/#wasGeneratedBy"@en ;
    rdfs:subPropertyOf ns4:relatedTo .

ns8:familyName a owl:property ;
    rdfs:label "Family Name"@en ;
    rdfs:domain ns8:person .

ns8:mbox a owl:property ;
    rdfs:label "mbox"@en ;
    rdfs:domain ns8:Agent ;
    rdfs:range ns8:thing .

ns8:name a owl:property ;
    rdfs:label "name"@en ;
    rdfs:domain ns8:thing .

<https://w3id.org/i40/rami#RAMILifeCycleLayer> a owl:Class ;
    rdfs:label "RAMI Life Cycle Layer"@en ;
    rdfs:seeAlso "http://www.zvei.org/en/subjects/Industry-40/Pages/The-Reference-Architectural-Model-RAMI-40-and-the-Industrie-40-Component.aspx" ;
    rdfs:subClassOf ns4:StandardClassification ;
    ns6:definition "It describes the different Life Cycle and Value Stream layers for the RAMI model according to the IEC 62890 Standard."@en ;
    ns6:prefLabel "RAMI Life Cycle Layer"@en .

ns4:AMQP a owl:NamedIndividual,
        ns8:Document,
        ns4:Publication,
        ns4:TechnicalSpecification ;
    rdfs:label "AMQP"@en ;
    ns2:creator ns4:sebastian ;
    rdfs:comment "AMQP (Advanced Message Queuing Protocol): An open standard application layer protocol for message-oriented middleware. The defining features of AMQP are message orientation, queuing, routing (including point-to-point and publish-and-subscribe), reliability and security. (source: https://www.postscapes.com/internet-of-things-protocols/)"@en ;
    ns4:hasOfficialResource <http://www.amqp.org/> .

ns4:Access_Rights_for_IoT-Cloud a owl:NamedIndividual,
        ns4:Concern ;
    rdfs:label "Access Rights for IoT-Cloud"@en ;
    ns2:creator ns4:MuhammadUsman ;
    rdfs:seeAlso <https://ieeexplore.ieee.org/document/7919553> ;
    ns6:note "TODO what is the IoT Cloud?" ;
    ns4:hasWikipediaArticle <https://en.wikipedia.org/wiki/Access_rights> ;
    ns5:supports ns4:Cloud_Connectivity .

ns4:Accountability a owl:NamedIndividual,
        ns4:Concern ;
    rdfs:label "Accountability"@en ;
    rdfs:comment "A system built using the ARM shall support the reversing of the pseudonymization processes in order to guarantee mutual accountability"@en ;
    rdfs:seeAlso "IoT-A Requirement UNI.605" .

ns4:Adaptability a owl:NamedIndividual,
        ns4:Concern ;
    rdfs:label "Adaptability"@en ;
    ns2:creator ns4:MuhammadUsman ;
    rdfs:comment """Because of clients' need and time's requirements, there ought to be constant change in the system of associated devices for Internet of Things. Adaptability is
continuously a need for survival and development of Internet of Things."""@en ;
    rdfs:seeAlso <https://ieeexplore.ieee.org/document/6188257> ;
    ns6:note "TODO merge with programmability or evolveability" ;
    ns4:hasWikipediaArticle <https://en.wikipedia.org/wiki/Adaptability> ;
    ns5:supports ns4:IoT .

ns4:Aeron a owl:NamedIndividual,
        ns8:Document,
        ns4:Publication,
        ns4:TechnicalSpecification ;
    rdfs:label "Aeron"@en ;
    ns2:creator ns4:sebastian ;
    rdfs:comment "Aeron - Efficient reliable UDP unicast, UDP multicast, and IPC message transport. (source: https://www.postscapes.com/internet-of-things-protocols/)"@en ;
    ns4:hasOfficialResource <https://github.com/real-logic/Aeron> .

ns4:AiiDataAnno a owl:NamedIndividual,
        ns1:oaAnnotation ;
    ns1:oahasBody ns4:AiiData ;
    ns1:oahasTarget [ a ns1:oaSpecificResource ;
            ns1:oahasSelector [ a ns1:oaRangeSelector ;
                    ns1:oahasEndSelector [ a ns1:oaXPathSelector ;
                            rdf:value "Page 32" ] ;
                    ns1:oahasStartSelector [ a ns1:oaXPathSelector ;
                            rdf:value "Page 25" ] ] ;
            ns1:oahasSource ns4:Industrial_Internet_Architecture_Version_1 ] .

ns4:AiiNetworkAnno a owl:NamedIndividual,
        ns1:oaAnnotation ;
    ns1:oahasBody ns4:AiiNetwork ;
    ns1:oahasTarget [ a ns1:oaSpecificResource ;
            ns2:format "pdf" ;
            ns1:oahasSelector [ a ns1:oaRangeSelector ;
                    ns1:oahasEndSelector [ a ns1:oaXPathSelector ;
                            rdf:value "Page 25" ] ;
                    ns1:oahasStartSelector [ a ns1:oaXPathSelector ;
                            rdf:value "Page 10" ] ] ;
            ns1:oahasSource ns4:Industrial_Internet_Architecture_Version_1 ] .

ns4:AiiSecurityAnno a owl:NamedIndividual,
        ns1:oaAnnotation ;
    ns1:oahasBody ns4:AiiSecurity ;
    ns1:oahasTarget [ a ns1:oaSpecificResource ;
            ns2:format "pdf" ;
            ns1:oahasSelector [ a ns1:oaRangeSelector ;
                    ns1:oahasEndSelector [ a ns1:oaXPathSelector ;
                            rdf:value "Page 37" ] ;
                    ns1:oahasStartSelector [ a ns1:oaXPathSelector ;
                            rdf:value "Page 32" ] ] ;
            ns1:oahasSource ns4:Industrial_Internet_Architecture_Version_1 ] .

ns4:AllSeenAlliance a owl:NamedIndividual,
        ns8:Organization,
        ns4:IIoTConsortium ;
    rdfs:label "AllSeen Alliance"@en ;
    ns2:creator ns4:sebastian ;
    rdfs:comment "The AllSeen Alliance is a nonprofit consortium dedicated to enabling and driving the widespread adoption of products, systems and services that support the Internet of Everything with an open, universal development framework supported by a vibrant ecosystem and thriving technical community' (source: https://www.postscapes.com/internet-of-things-protocols/)"@en ;
    ns4:hasOfficialResource <https://allseenalliance.org/> .

ns4:AllianceIndustrieDuFutur a owl:NamedIndividual,
        ns4:IIoTConsortium ;
    rdfs:label "Alliance Industrie du Futur"@en ;
    ns4:hasHeadquaterIn ns4:France ;
    ns4:hasOfficialResource <http://www.industrie-dufutur.org/> .

ns4:Alljoyn a owl:NamedIndividual,
        ns8:Document,
        ns4:Publication,
        ns4:TechnicalSpecification ;
    rdfs:label "Alljoyn"@en ;
    ns2:creator ns4:sebastian ;
    rdfs:comment "Alljoyn - An open source software framework that makes it easy for devices and apps to discover and communicate with each other. (source: https://www.postscapes.com/internet-of-things-protocols/)"@en ;
    ns4:hasOfficialResource <https://allseenalliance.org/framework> .

ns4:AnnoActuation a owl:NamedIndividual,
        ns1:oaAnnotation ;
    ns1:oahasBody ns4:Actuation ;
    ns1:oahasTarget [ a ns1:oaSpecificResource ;
            ns2:format "pdf" ;
            ns1:oahasSelector [ a ns1:oaRangeSelector ;
                    ns1:oahasEndSelector [ a ns1:oaXPathSelector ;
                            rdf:value "Page 29" ] ;
                    ns1:oahasStartSelector [ a ns1:oaXPathSelector ;
                            rdf:value "Page 28" ] ] ;
            ns1:oahasSource ns4:IIC_PUB_G1_V1_80_20170131 ],
        [ a ns1:oaSpecificResource ;
            ns2:format "pdf" ;
            ns1:oahasSelector [ a ns1:oaRangeSelector ;
                    ns1:oahasEndSelector [ a ns1:oaXPathSelector ;
                            rdf:value "Page 29" ] ;
                    ns1:oahasStartSelector [ a ns1:oaXPathSelector ;
                            rdf:value "Page 28" ] ] ;
            ns1:oahasSource ns4:IIC_PUB_G1_V1_80_20170131 ] .

ns4:AnnoAiiClassification a owl:NamedIndividual,
        ns1:oaAnnotation ;
    ns1:oahasBody ns4:AiiClassification ;
    ns1:oahasTarget [ a ns1:oaSpecificResource ;
            ns2:format "pdf" ;
            ns1:oahasSource ns4:Industrial_Internet_Architecture_Version_1 ],
        [ a ns1:oaSpecificResource ;
            ns2:format "pdf" ;
            ns1:oahasSource ns4:Industrial_Internet_Architecture_Version_1 ] .

ns4:AoutonomousCommunication rdfs:seeAlso "IoT-A Requirement UNI.247" .

ns4:ArrowheadFramework a owl:NamedIndividual,
        ns4:IIoTConsortium,
        ns4:StandardizationFramework ;
    rdfs:label "Arrowhead Framework" ;
    ns4:hasPublisher ns4:ArrowheadProject ;
    ns4:seeAlso <http://www.arrowhead.eu/> .

ns4:Auto_Scaling a owl:NamedIndividual,
        ns4:Concern ;
    rdfs:label "Auto Scaling"@en ;
    ns2:creator ns4:MuhammadUsman ;
    rdfs:comment "Autoscaling, also spelled auto scaling or auto-scaling, and sometimes also called automatic scaling, is a method used in cloud computing, whereby the amount of computational resources in a server farm, typically measured in terms of the number of active servers, scales automatically based on the load on the farm. It is closely related to, and builds upon, the idea of load balancing."@en ;
    ns6:note "TODO already covered by scalability?"@en ;
    ns4:hasWikipediaArticle <https://en.wikipedia.org/wiki/Autoscaling> ;
    ns5:supports ns4:Scalability .

ns4:Awareness a owl:NamedIndividual,
        ns4:Concern ;
    rdfs:label "Awareness"@en ;
    ns2:creator ns4:MuhammadUsman ;
    rdfs:comment "Awareness is the ability to directly know and perceive, to feel, or to be cognizant of events. More broadly, it is the state of being conscious of something. Another definition describes it as a state wherein a subject is aware of some information when that information is directly available to bring to bear in the direction of a wide range of behavioral processes. The concept is often synonymous to consciousness and is also understood as being consciousness itself."@en ;
    rdfs:seeAlso <https://ieeexplore.ieee.org/document/7488250> ;
    ns4:hasWikipediaArticle <https://en.wikipedia.org/wiki/Awareness> ;
    ns5:supports ns4:EdgeComputing .

ns4:Bandwidth a owl:NamedIndividual,
        ns4:Concern ;
    rdfs:label "Bandwidth"@en ;
    ns2:creator ns4:MuhammadUsman ;
    rdfs:comment "In computing, bandwidth is the maximum rate of data transfer across a given path. Bandwidth may be characterized as network bandwidth, data bandwidth, or digital bandwidth."@en ;
    rdfs:seeAlso <https://ieeexplore.ieee.org/document/6188257>,
        <https://ieeexplore.ieee.org/document/7488250> ;
    ns4:hasWikipediaArticle <https://en.wikipedia.org/wiki/Bandwidth_(computing)> ;
    ns5:supports ns4:Communication .

ns4:BdvaCloudAndHighPerformanceComputingAnno a owl:NamedIndividual,
        ns1:oaAnnotation ;
    ns1:oahasBody ns4:BdvaCloudAndHighPerformanceComputing ;
    ns1:oahasTarget [ a ns1:oaSpecificResource ;
            ns1:oahasSelector [ a ns1:oaRangeSelector ;
                    ns1:oahasEndSelector [ a ns1:oaXPathSelector ;
                            rdf:value "Page 40" ] ;
                    ns1:oahasStartSelector [ a ns1:oaXPathSelector ;
                            rdf:value "Page 37" ] ] ;
            ns1:oahasSource ns4:European_BDV_SRIA_version_4_0 ],
        [ a ns1:oaSpecificResource ;
            ns1:oahasSelector [ a ns1:oaRangeSelector ;
                    ns1:oahasEndSelector [ a ns1:oaXPathSelector ;
                            rdf:value "Page 40" ] ;
                    ns1:oahasStartSelector [ a ns1:oaXPathSelector ;
                            rdf:value "Page 37" ] ] ;
            ns1:oahasSource ns4:European_BDV_SRIA_version_4_0 ] .

ns4:BdvaCommunicationConnectivityAnno a owl:NamedIndividual,
        ns1:oaAnnotation ;
    ns1:oahasBody ns4:BdvaCommunicationConnectivity ;
    ns1:oahasTarget [ a ns1:oaSpecificResource ;
            ns1:oahasSelector [ a ns1:oaRangeSelector ;
                    ns1:oahasEndSelector [ a ns1:oaXPathSelector ;
                            rdf:value "Page 40" ] ;
                    ns1:oahasStartSelector [ a ns1:oaXPathSelector ;
                            rdf:value "Page 37" ] ] ;
            ns1:oahasSource ns4:European_BDV_SRIA_version_4_0 ],
        [ a ns1:oaSpecificResource ;
            ns1:oahasSelector [ a ns1:oaRangeSelector ;
                    ns1:oahasEndSelector [ a ns1:oaXPathSelector ;
                            rdf:value "Page 40" ] ;
                    ns1:oahasStartSelector [ a ns1:oaXPathSelector ;
                            rdf:value "Page 37" ] ] ;
            ns1:oahasSource ns4:European_BDV_SRIA_version_4_0 ] .

ns4:BdvaConcernAnno a owl:NamedIndividual,
        ns1:oaAnnotation ;
    ns1:oahasBody ns4:BdvaConcern ;
    ns1:oahasTarget [ a ns1:oaSpecificResource ;
            ns1:oahasSelector [ a ns1:oaRangeSelector ;
                    ns1:oahasEndSelector [ a ns1:oaXPathSelector ;
                            rdf:value "Page 40" ] ;
                    ns1:oahasStartSelector [ a ns1:oaXPathSelector ;
                            rdf:value "Page 37" ] ] ;
            ns1:oahasSource ns4:European_BDV_SRIA_version_4_0 ],
        [ a ns1:oaSpecificResource ;
            ns1:oahasSelector [ a ns1:oaRangeSelector ;
                    ns1:oahasEndSelector [ a ns1:oaXPathSelector ;
                            rdf:value "Page 40" ] ;
                    ns1:oahasStartSelector [ a ns1:oaXPathSelector ;
                            rdf:value "Page 38" ] ] ;
            ns1:oahasSource ns4:European_BDV_SRIA_version_4_0 ],
        [ a ns1:oaSpecificResource ;
            ns1:oahasSelector [ a ns1:oaRangeSelector ;
                    ns1:oahasEndSelector [ a ns1:oaXPathSelector ;
                            rdf:value "Page 40" ] ;
                    ns1:oahasStartSelector [ a ns1:oaXPathSelector ;
                            rdf:value "Page 37" ] ] ;
            ns1:oahasSource ns4:European_BDV_SRIA_version_4_0 ] .

ns4:BdvaCyberSecurityTrustAnno a owl:NamedIndividual,
        ns1:oaAnnotation ;
    ns1:oahasBody ns4:BdvaCyberSecurityTrust ;
    ns1:oahasTarget [ a ns1:oaSpecificResource ;
            ns1:oahasSelector [ a ns1:oaRangeSelector ;
                    ns1:oahasEndSelector [ a ns1:oaXPathSelector ;
                            rdf:value "Page 40" ] ;
                    ns1:oahasStartSelector [ a ns1:oaXPathSelector ;
                            rdf:value "Page 37" ] ] ;
            ns1:oahasSource ns4:European_BDV_SRIA_version_4_0 ],
        [ a ns1:oaSpecificResource ;
            ns1:oahasSelector [ a ns1:oaRangeSelector ;
                    ns1:oahasEndSelector [ a ns1:oaXPathSelector ;
                            rdf:value "Page 40" ] ;
                    ns1:oahasStartSelector [ a ns1:oaXPathSelector ;
                            rdf:value "Page 37" ] ] ;
            ns1:oahasSource ns4:European_BDV_SRIA_version_4_0 ] .

ns4:BdvaDataAnalyticsAnno a owl:NamedIndividual,
        ns1:oaAnnotation ;
    ns1:oahasBody ns4:BdvaDataAnalytics ;
    ns1:oahasTarget [ a ns1:oaSpecificResource ;
            ns1:oahasSelector [ a ns1:oaRangeSelector ;
                    ns1:oahasEndSelector [ a ns1:oaXPathSelector ;
                            rdf:value "Page 40" ] ;
                    ns1:oahasStartSelector [ a ns1:oaXPathSelector ;
                            rdf:value "Page 37" ] ] ;
            ns1:oahasSource ns4:European_BDV_SRIA_version_4_0 ],
        [ a ns1:oaSpecificResource ;
            ns1:oahasSelector [ a ns1:oaRangeSelector ;
                    ns1:oahasEndSelector [ a ns1:oaXPathSelector ;
                            rdf:value "Page 40" ] ;
                    ns1:oahasStartSelector [ a ns1:oaXPathSelector ;
                            rdf:value "Page 37" ] ] ;
            ns1:oahasSource ns4:European_BDV_SRIA_version_4_0 ] .

ns4:BdvaDataManagementAnno a owl:NamedIndividual,
        ns1:oaAnnotation ;
    ns1:oahasBody ns4:BdvaDataManagement ;
    ns1:oahasTarget [ a ns1:oaSpecificResource ;
            ns1:oahasSelector [ a ns1:oaRangeSelector ;
                    ns1:oahasEndSelector [ a ns1:oaXPathSelector ;
                            rdf:value "Page 40" ] ;
                    ns1:oahasStartSelector [ a ns1:oaXPathSelector ;
                            rdf:value "Page 37" ] ] ;
            ns1:oahasSource ns4:European_BDV_SRIA_version_4_0 ],
        [ a ns1:oaSpecificResource ;
            ns1:oahasSelector [ a ns1:oaRangeSelector ;
                    ns1:oahasEndSelector [ a ns1:oaXPathSelector ;
                            rdf:value "Page 40" ] ;
                    ns1:oahasStartSelector [ a ns1:oaXPathSelector ;
                            rdf:value "Page 37" ] ] ;
            ns1:oahasSource ns4:European_BDV_SRIA_version_4_0 ] .

ns4:BdvaDataProcessingArchitecturesAnno a owl:NamedIndividual,
        ns1:oaAnnotation ;
    ns1:oahasBody ns4:BdvaDataProcessingArchitectures ;
    ns1:oahasTarget [ a ns1:oaSpecificResource ;
            ns1:oahasSelector [ a ns1:oaRangeSelector ;
                    ns1:oahasEndSelector [ a ns1:oaXPathSelector ;
                            rdf:value "Page 40" ] ;
                    ns1:oahasStartSelector [ a ns1:oaXPathSelector ;
                            rdf:value "Page 37" ] ] ;
            ns1:oahasSource ns4:European_BDV_SRIA_version_4_0 ],
        [ a ns1:oaSpecificResource ;
            ns1:oahasSelector [ a ns1:oaRangeSelector ;
                    ns1:oahasEndSelector [ a ns1:oaXPathSelector ;
                            rdf:value "Page 40" ] ;
                    ns1:oahasStartSelector [ a ns1:oaXPathSelector ;
                            rdf:value "Page 37" ] ] ;
            ns1:oahasSource ns4:European_BDV_SRIA_version_4_0 ] .

ns4:BdvaDataProtectionAnno a owl:NamedIndividual,
        ns1:oaAnnotation ;
    ns1:oahasBody ns4:BdvaDataProtection ;
    ns1:oahasTarget [ a ns1:oaSpecificResource ;
            ns1:oahasSelector [ a ns1:oaRangeSelector ;
                    ns1:oahasEndSelector [ a ns1:oaXPathSelector ;
                            rdf:value "Page 40" ] ;
                    ns1:oahasStartSelector [ a ns1:oaXPathSelector ;
                            rdf:value "Page 37" ] ] ;
            ns1:oahasSource ns4:European_BDV_SRIA_version_4_0 ],
        [ a ns1:oaSpecificResource ;
            ns1:oahasSelector [ a ns1:oaRangeSelector ;
                    ns1:oahasEndSelector [ a ns1:oaXPathSelector ;
                            rdf:value "Page 40" ] ;
                    ns1:oahasStartSelector [ a ns1:oaXPathSelector ;
                            rdf:value "Page 37" ] ] ;
            ns1:oahasSource ns4:European_BDV_SRIA_version_4_0 ] .

ns4:BdvaDataSharingPlatformsAnno a owl:NamedIndividual,
        ns1:oaAnnotation ;
    ns1:oahasBody ns4:BdvaDataSharingPlatforms ;
    ns1:oahasTarget [ a ns1:oaSpecificResource ;
            ns1:oahasSelector [ a ns1:oaRangeSelector ;
                    ns1:oahasEndSelector [ a ns1:oaXPathSelector ;
                            rdf:value "Page 40" ] ;
                    ns1:oahasStartSelector [ a ns1:oaXPathSelector ;
                            rdf:value "Page 37" ] ] ;
            ns1:oahasSource ns4:European_BDV_SRIA_version_4_0 ],
        [ a ns1:oaSpecificResource ;
            ns1:oahasSelector [ a ns1:oaRangeSelector ;
                    ns1:oahasEndSelector [ a ns1:oaXPathSelector ;
                            rdf:value "Page 40" ] ;
                    ns1:oahasStartSelector [ a ns1:oaXPathSelector ;
                            rdf:value "Page 37" ] ] ;
            ns1:oahasSource ns4:European_BDV_SRIA_version_4_0 ] .

ns4:BdvaDataVisualizationAndUserInteractionAnno a owl:NamedIndividual,
        ns1:oaAnnotation ;
    ns1:oahasBody ns4:BdvaDataVisualizationAndUserInteraction ;
    ns1:oahasTarget [ a ns1:oaSpecificResource ;
            ns1:oahasSelector [ a ns1:oaRangeSelector ;
                    ns1:oahasEndSelector [ a ns1:oaXPathSelector ;
                            rdf:value "Page 40" ] ;
                    ns1:oahasStartSelector [ a ns1:oaXPathSelector ;
                            rdf:value "Page 37" ] ] ;
            ns1:oahasSource ns4:European_BDV_SRIA_version_4_0 ],
        [ a ns1:oaSpecificResource ;
            ns1:oahasSelector [ a ns1:oaRangeSelector ;
                    ns1:oahasEndSelector [ a ns1:oaXPathSelector ;
                            rdf:value "Page 40" ] ;
                    ns1:oahasStartSelector [ a ns1:oaXPathSelector ;
                            rdf:value "Page 37" ] ] ;
            ns1:oahasSource ns4:European_BDV_SRIA_version_4_0 ] .

ns4:BdvaDevelopmentEngineeringAnno a owl:NamedIndividual,
        ns1:oaAnnotation ;
    ns1:oahasBody ns4:BdvaDevelopmentEngineering ;
    ns1:oahasTarget [ a ns1:oaSpecificResource ;
            ns1:oahasSelector [ a ns1:oaRangeSelector ;
                    ns1:oahasEndSelector [ a ns1:oaXPathSelector ;
                            rdf:value "Page 40" ] ;
                    ns1:oahasStartSelector [ a ns1:oaXPathSelector ;
                            rdf:value "Page 37" ] ] ;
            ns1:oahasSource ns4:European_BDV_SRIA_version_4_0 ],
        [ a ns1:oaSpecificResource ;
            ns1:oahasSelector [ a ns1:oaRangeSelector ;
                    ns1:oahasEndSelector [ a ns1:oaXPathSelector ;
                            rdf:value "Page 40" ] ;
                    ns1:oahasStartSelector [ a ns1:oaXPathSelector ;
                            rdf:value "Page 37" ] ] ;
            ns1:oahasSource ns4:European_BDV_SRIA_version_4_0 ] .

ns4:BdvaSiraAnno a owl:NamedIndividual,
        ns1:oaAnnotation ;
    ns1:oahasBody ns4:BdvaSira ;
    ns1:oahasTarget [ a ns1:oaSpecificResource ;
            ns1:oahasSelector [ a ns1:oaRangeSelector ;
                    ns1:oahasEndSelector [ a ns1:oaXPathSelector ;
                            rdf:value "Page 106" ] ;
                    ns1:oahasStartSelector [ a ns1:oaXPathSelector ;
                            rdf:value "Page 1" ] ] ;
            ns1:oahasSource ns4:European_BDV_SRIA_version_4_0 ],
        [ a ns1:oaSpecificResource ;
            ns1:oahasSelector [ a ns1:oaRangeSelector ;
                    ns1:oahasEndSelector [ a ns1:oaXPathSelector ;
                            rdf:value "Page 106" ] ;
                    ns1:oahasStartSelector [ a ns1:oaXPathSelector ;
                            rdf:value "Page 1" ] ] ;
            ns1:oahasSource ns4:European_BDV_SRIA_version_4_0 ] .

ns4:BdvaStandardsAnno a owl:NamedIndividual,
        ns1:oaAnnotation ;
    ns1:oahasBody ns4:BdvaStandards ;
    ns1:oahasTarget [ a ns1:oaSpecificResource ;
            ns1:oahasSelector [ a ns1:oaRangeSelector ;
                    ns1:oahasEndSelector [ a ns1:oaXPathSelector ;
                            rdf:value "Page 40" ] ;
                    ns1:oahasStartSelector [ a ns1:oaXPathSelector ;
                            rdf:value "Page 37" ] ] ;
            ns1:oahasSource ns4:European_BDV_SRIA_version_4_0 ],
        [ a ns1:oaSpecificResource ;
            ns1:oahasSelector [ a ns1:oaRangeSelector ;
                    ns1:oahasEndSelector [ a ns1:oaXPathSelector ;
                            rdf:value "Page 40" ] ;
                    ns1:oahasStartSelector [ a ns1:oaXPathSelector ;
                            rdf:value "Page 37" ] ] ;
            ns1:oahasSource ns4:European_BDV_SRIA_version_4_0 ] .

ns4:BdvaThingsAssetsSensorsActuatorsAnno a owl:NamedIndividual,
        ns1:oaAnnotation ;
    ns1:oahasBody ns4:BdvaThingsAssetsSensorsActuators ;
    ns1:oahasTarget [ a ns1:oaSpecificResource ;
            ns1:oahasSelector [ a ns1:oaRangeSelector ;
                    ns1:oahasEndSelector [ a ns1:oaXPathSelector ;
                            rdf:value "Page 40" ] ;
                    ns1:oahasStartSelector [ a ns1:oaXPathSelector ;
                            rdf:value "Page 37" ] ] ;
            ns1:oahasSource ns4:European_BDV_SRIA_version_4_0 ],
        [ a ns1:oaSpecificResource ;
            ns1:oahasSelector [ a ns1:oaRangeSelector ;
                    ns1:oahasEndSelector [ a ns1:oaXPathSelector ;
                            rdf:value "Page 40" ] ;
                    ns1:oahasStartSelector [ a ns1:oaXPathSelector ;
                            rdf:value "Page 37" ] ] ;
            ns1:oahasSource ns4:European_BDV_SRIA_version_4_0 ] .

ns4:Bluetooth a owl:NamedIndividual,
        ns8:Document,
        ns4:Publication,
        ns4:TechnicalSpecification ;
    rdfs:label "Bluetooth"@en ;
    ns2:creator ns4:sebastian ;
    rdfs:comment "Bluetooth works in the 2.4 GHz ISM band and uses frequency hopping. With a data rate up to 3 Mbps and maximum range of 100m. Each application type which can use Bluetooth has its own profile.  (source: https://www.postscapes.com/internet-of-things-protocols/)"@en ;
    ns4:hasClassification ns4:RAMICommunicationLayer ;
    ns4:hasOfficialResource <http://www.bluetooth.com/Pages/Bluetooth-Home.aspx> .

ns4:BusinessCycleSCM a owl:Class ;
    rdfs:label "Business Cycle SCM"@en ;
    rdfs:comment "Suply Chain Management Business Cycle."@en ;
    rdfs:isDefinedBy <http://nvlpubs.nist.gov/nistpubs/ir/2016/NIST.IR.8107.pdf> ;
    rdfs:seeAlso <https://en.wikipedia.org/wiki/Supply_chain_management>,
        "https://en.wikipedia.org/wiki/Supply_chain_management" ;
    rdfs:subClassOf ns4:StandardClassification .

ns4:BusinessManager rdfs:label "Business Manager"@en ;
    rdfs:comment " A business manager is responsible for the running of the business and to make large profits." ;
    rdfs:seeAlso "IIC:PUB:G1:V1.80:20170131" ;
    ns6:note "Publications referred: 'IIC:PUB:G1:V1.80:20170131' '1.5 AUDIENCE' 'Page 7' " ;
    ns4:hasWikipediaArticle <https://en.wikipedia.org/wiki/Business_manager> .

ns4:BusinessProcessManagement a owl:NamedIndividual,
        ns4:Concern ;
    rdfs:label "BPM"@en ;
    ns2:title "Business process management"@en ;
    rdfs:comment "Business process management (BPM) is a field in operations management that focuses on improving corporate performance by managing and optimizing a company's business processes. It can therefore be described as a \"process optimization process.\" It is argued that BPM enables organizations to be more efficient, more effective and more capable of change than a functionally focused, traditional hierarchical management approach. These processes can impact the cost and revenue generation of an organization. As a policy-making approach, BPM sees processes as important assets of an organization that must be understood, managed, and developed to announce value-added products and services to clients or customers. This approach closely resembles other total quality management or continual improvement process methodologies and BPM proponents also claim that this approach can be supported, or enabled, through technology. As such, many BPM articles and scholars frequently discuss BPM from one of two viewpoints: people and/or technology. (source: wikipedia)"@en ;
    rdfs:seeAlso "IoT-A Requirement UNI.211",
        "IoT-A Requirement UNI.212",
        "IoT-A Requirement UNI.214",
        "IoT-A Requirement UNI.215",
        "IoT-A Requirement UNI.229" ;
    ns4:hasDBpediaResource <http://dbpedia.org/resource/Business_process_management> ;
    ns5:supports ns4:BusinessContext .

ns4:ComplexEventProcessing a owl:NamedIndividual,
        ns4:Concern ;
    rdfs:label "CEP"@en ;
    ns2:title "Complex Event Processing"@en ;
    rdfs:comment "Event processing is a method of tracking and analyzing (processing) streams of information (data) about things that happen (events), and deriving a conclusion from them. Complex event processing, or CEP, is event processing that combines data from multiple sources to infer events or patterns that suggest more complicated circumstances. The goal of complex event processing is to identify meaningful events (such as opportunities or threats) and respond to them as quickly as possible. (source: wikipedia)"@en ;
    rdfs:seeAlso "IoT-A Requirement UNI.232" ;
    ns4:hasDBpediaResource <http://dbpedia.org/page/Complex_event_processing> ;
    ns5:supports ns4:DataAnalytics .

ns4:Confidentiality a owl:NamedIndividual,
        ns4:Concern ;
    rdfs:label "Confidentiality"@en ;
    ns2:creator ns4:MuhammadUsman ;
    rdfs:comment "Confidentiality involves a set of rules or a promise usually executed through confidentiality agreements that limits access or places restrictions on certain types of information."@en ;
    rdfs:seeAlso <https://dl.acm.org/citation.cfm?doid=3108421.3108426>,
        <https://ieeexplore.ieee.org/document/8327600> ;
    ns4:hasWikipediaArticle <https://en.wikipedia.org/wiki/Confidentiality> ;
    ns5:supports ns4:Privacy .

ns4:ConnectivityLayer a owl:Class ;
    rdfs:label "Connectivity Layer"@en ;
    rdfs:comment "Connectivity Layer of the Internet Connectivity Framework"@en ;
    rdfs:isDefinedBy <https://www.iiconsortium.org/pdf/IIC_PUB_G5_V1.01_PB_20180228.pdf> ;
    rdfs:subClassOf ns4:StandardClassification .

ns4:ConstrainedDevices a owl:NamedIndividual,
        ns4:Concern ;
    rdfs:label "Constrained Devices"@en ;
    ns2:creator ns4:sebastian ;
    ns7:hasStakeholder "System Architect TODO"@en ;
    rdfs:comment "Data-memory-constrained devices must be able to participate in communication. This means that a system built using the ARM shall support communication stacks with small data footprint."@en,
        "Small devices with limited CPU, memory, and power resources, so-called \"constrained devices\" (often used as sensors/actuators, smart objects, or smart devices) can form a network, becoming \"constrained nodes\" in that network.  Such a network may itself exhibit constraints, e.g., with unreliable or lossy channels, limited and unpredictable bandwidth, and a highly dynamic topology. (source: https://tools.ietf.org/html/rfc7228)"@en ;
    rdfs:seeAlso "IoT-A Requirement UNI.306",
        "IoT-A Requirement UNI.307",
        "UNI.306"@en ;
    ns5:supports ns4:IoT .

ns4:CostEfficiency a owl:NamedIndividual,
        ns4:Concern ;
    rdfs:label "Cost Efficiency"@en,
        "DataRecovery"@en ;
    ns2:creator ns4:SebastianBader ;
    rdfs:comment ""@en ;
    rdfs:seeAlso <https://dl.acm.org/citation.cfm?doid=3266237.3266263> ;
    ns5:supports ns4:BusinessContext .

ns4:Customer a ns7:StakeholderGroup,
        owl:NamedIndividual .

ns4:Customization a owl:NamedIndividual,
        ns4:Concern ;
    rdfs:label "Customization"@en ;
    ns2:creator ns4:MuhammadUsman ;
    rdfs:comment "The resources sharing by contrasting users keeps cloud service provider from having the capacity to customize their services to meet the diverse necessities of customers"@en ;
    rdfs:seeAlso <https://dl.acm.org/citation.cfm?doid=3108421.3108426> ;
    ns4:hasWikipediaArticle <https://en.wikipedia.org/wiki/Customization> ;
    ns5:supports ns4:BusinessContext,
        ns4:Scalability .

ns4:DIN_77005_P1 a owl:NamedIndividual,
        ns4:Standard ;
    rdfs:label "DIN 77005-1:2018-09"@en ;
    ns5:frames ns4:DataLifecycleManagment .

ns4:DIN_EN_50128 a owl:NamedIndividual,
        ns4:Standard ;
    ns5:frames ns4:Safety .

ns4:DIN_EN_50129 a owl:NamedIndividual,
        ns4:Standard ;
    rdfs:label "DIN EN 50129"@en ;
    ns4:hasClassification ns4:IDSRAMCertification ;
    ns5:hasTargetConcern ns4:Safety .

ns4:DIN_EN_50155 a owl:NamedIndividual,
        ns4:Standard ;
    rdfs:label "DIN EN 50155"@en ;
    ns4:hasClassification ns4:IDSRAMCertification ;
    ns5:hasTargetConcern ns4:Safety .

ns4:DIN_EN_50159 a owl:NamedIndividual,
        ns4:Standard ;
    ns4:hasClassification ns4:IDSRAMCertification ;
    ns5:hasTargetConcern ns4:Safety .

ns4:DIN_EN_61511 a owl:NamedIndividual,
        ns4:Standard ;
    rdfs:label "DIN EN 61511"@en ;
    ns4:hasClassification ns4:IDSRAMCertification ;
    ns5:hasTargetConcern ns4:Safety .

ns4:DIN_EN_ISO_13849 a owl:NamedIndividual,
        ns4:Standard ;
    ns4:hasClassification ns4:IDSRAMCertification ;
    ns5:hasTargetConcern ns4:Safety .

ns4:DIN_EN_ISO_IEC_17025 a owl:NamedIndividual,
        ns4:Standard ;
    ns4:hasClassification ns4:IDSRAMCertification .

ns4:DIN_ISO_14638 a owl:NamedIndividual,
        ns4:Standard ;
    ns5:frames ns4:ThingDescription .

ns4:DIN_SPEC_16593_P1 a owl:NamedIndividual,
        ns4:Standard ;
    ns5:frames ns4:ServiceDescription .

ns4:DIN_SPEC_92222 a owl:NamedIndividual,
        ns4:Standard ;
    ns5:frames ns4:CloudComputing,
        ns4:communication,
        ns4:interoperability .

ns4:DataAggregation a owl:NamedIndividual,
        ns4:Concern ;
    rdfs:label "Data Aggregation"@en ;
    rdfs:comment "Data Aggregation is the compiling the data before Data Processing"@en ;
    rdfs:seeAlso <https://ieeexplore.ieee.org/document/7566346>,
        <https://www.researchgate.net/publication/319283535_Data_aggregation_mechanisms_in_the_Internet_of_things_A_systematic_review_of_the_literature_and_recommendations_for_future_research> ;
    ns6:narrower ns4:DataProcessing ;
    ns4:hasWikipediaArticle <https://en.wikipedia.org/wiki/Data_aggregation> .

ns4:DataEncryption a owl:NamedIndividual,
        ns4:Concern ;
    rdfs:label "Customization"@en,
        "Data secrecy and encryption"@en ;
    ns2:creator ns4:MuhammadUsman ;
    rdfs:comment ""@en,
        "The resources sharing by contrasting users keeps cloud service provider from having the capacity to customize their services to meet the diverse necessities of customers"@en ;
    rdfs:seeAlso <https://dl.acm.org/citation.cfm?doid=3108421.3108426>,
        <https://ieeexplore.ieee.org/document/6188257> ;
    ns4:hasWikipediaArticle <https://en.wikipedia.org/wiki/Customization>,
        <https://en.wikipedia.org/wiki/Encryption> ;
    ns5:supports ns4:BusinessContext,
        ns4:SecureCommunication .

ns4:DataIsolation a owl:NamedIndividual,
        ns4:Concern ;
    rdfs:label "Data Isolation"@en ;
    rdfs:comment "Isolation is one of the ACID (Atomicity, Consistency, Isolation, Durability) properties adopted by the database systems"@en ;
    ns6:narrower ns4:Isolation ;
    ns4:hasWikipediaArticle <https://en.wikipedia.org/wiki/Isolation_(database_systems)> ;
    ns5:supports ns4:DataIntegrity .

ns4:DataLifecycleManagement rdfs:seeAlso "IoT-A Requirement UNI.097" .

ns4:DataLocation a owl:NamedIndividual,
        ns4:Concern ;
    rdfs:label "Data Location"@en ;
    ns2:creator ns4:MuhammadUsman ;
    rdfs:comment "One of the features of cloud computing is geodistribution of data among several servers. But this can be an issue for the enterprise, as the location of the data is unknown to the user."@en ;
    rdfs:seeAlso <https://dl.acm.org/citation.cfm?doid=2735399.2735405>,
        <https://dl.acm.org/citation.cfm?doid=3286606.3286865>,
        <https://ieeexplore.ieee.org/document/8249113> ;
    ns5:supports ns4:DataUsageControl .

ns4:DataMarkets a owl:NamedIndividual,
        ns4:Concern ;
    rdfs:label "Data Markets"@en ;
    ns2:creator ns4:sebastian ;
    rdfs:comment "Data as an economic good; it's offered, demanded, and priced."@en ;
    ns5:supports ns4:DataEconomy .

ns4:DataOwnership a owl:NamedIndividual,
        ns4:Concern ;
    rdfs:label "Data Ownership"@en ;
    ns2:creator ns4:sebastian ;
    rdfs:comment "Data Ownership declare the possesion on an information resource that is independent of its location, e.g. personal data belongs to the related person no matter where it is stored."@en ;
    ns4:hasDBpediaResource <http://dbpedia.org/resource/Data_ownership> ;
    ns5:supports ns4:Privacy .

ns4:DataTransferProjectAnno a owl:NamedIndividual,
        ns1:oaAnnotation ;
    ns1:oahasBody ns4:DataTransferProject ;
    ns1:oahasTarget [ a ns1:oaSpecificResource ;
            ns1:oahasSource ns4:Data_Transfer_Project_Overview_and_Fundamentals ] .

ns4:DataTransferProjectWhitepaper a owl:NamedIndividual,
        ns8:Document,
        ns4:Publication ;
    rdfs:label "Data Transfer Project Whitepaper"@en ;
    ns2:creator ns4:DataTransferProject,
        ns4:sebastian ;
    rdfs:comment "The Data Transfer Project Whitepaper provides a brief overview on the intends of the Data Transfer Project and the targeted approach."@en ;
    ns8:maker ns4:DataTransferProject ;
    ns4:hasClassification ns4:DtpDeploymentView,
        ns4:DtpEcosystemView,
        ns4:DtpSecurityPrivacy,
        ns4:DtpSystemView ;
    ns4:hasDBpediaResource <http://dbpedia.org/page/Data_Transfer_Project> ;
    ns4:hasDeveloper ns4:DataTransferProject ;
    ns4:hasPublisher ns4:DataTransferProject ;
    ns4:hasWikipediaArticle <https://en.wikipedia.org/wiki/Data_Transfer_Project> ;
    ns5:hasTargetConcern ns4:DataSovereignty,
        ns4:IdentityManagement,
        ns4:Privacy,
        ns4:SecureCommunication,
        ns4:UserPreferences .

ns4:Data_Confidentiality a owl:NamedIndividual,
        ns4:Concern ;
    rdfs:label "Data Confidentiality"@en ;
    ns2:creator ns4:MuhammadUsman ;
    rdfs:comment "In edge computing, user private data is outsourced to the edge server and its ownership and control are separated, which causes users to lose their physical control over the outsourced data."@en ;
    rdfs:seeAlso <https://ieeexplore.ieee.org/document/6188257>,
        <https://ieeexplore.ieee.org/document/8327600> ;
    ns5:supports ns4:Privacy .

ns4:Device_Authentication a owl:NamedIndividual,
        ns4:Concern ;
    rdfs:label "Device Authentication"@en ;
    ns2:creator ns4:MuhammadUsman ;
    rdfs:seeAlso <https://ieeexplore.ieee.org/document/7919553> ;
    ns4:hasWikipediaArticle <https://en.wikipedia.org/wiki/Authentication> ;
    ns5:supports ns4:Authentication .

ns4:DmaArchitecture a owl:NamedIndividual,
        ns4:ArchitectureDescription,
        ns4:StandardizationFramework ;
    rdfs:label "DMA Architecture"@en ;
    ns2:creator ns4:sebastian ;
    ns4:hasPublisher ns4:DataMarketAustria .

ns4:DmaServiceTechnologySpecificationAndDevelopmentRoadmap a owl:NamedIndividual,
        ns8:Document,
        ns4:Publication,
        ns4:StandardizationFramework ;
    rdfs:label "DMA Service Technology Specification and Development Roadmap"@en ;
    ns2:creator ns4:DataMarketAustria ;
    ns3:associatedWith ns4:Blockchain,
        ns4:REST,
        ns4:RFC_6750 ;
    rdfs:comment """This document presents the DMA Data Technology Specification and Development Roadmap regarding the ongoing work in WP6 of the DMA project. The document relates to deliverable D2.2 “D2.2 Community-driven Data-Services Ecosystem Requirements (1st version)” which formulates
the requirements of the DMA community. It will be explained in what way the requirements formulated in D2.2 are going to be addressed. The document gives an overview about the components which are going to be developed in WP6 and how these components are planned to be employed to provide DMA core services. The expected outputs of these services are described and a procedure of describing a 3rd party service for DMA platform is addressed."""@en ;
    ns8:maker ns4:DataMarketAustria ;
    ns4:hasOfficialResource <https://datamarket.at/wp-content/uploads/2017/10/DMA_Deliverable_D6.1_FINAL_v01.pdf> ;
    ns4:hasPublisher ns4:DataMarketAustria ;
    ns5:hasTargetConcern ns4:Authentication,
        ns4:Authorization,
        ns4:BigDataApplications,
        ns4:Billing,
        ns4:CloudComputing,
        ns4:DataAccess,
        ns4:DataQuality,
        ns4:Privacy,
        ns4:SecureCommunication,
        ns4:Security,
        ns4:SemanticInteroperability,
        ns4:StreamProcessing,
        ns4:SyntacticInteroperability,
        ns4:Trustworthiness .

ns4:DynamicDiscovery a owl:NamedIndividual,
        ns4:Concern ;
    rdfs:label "Dynamic Discovery"@en ;
    rdfs:comment "A systems ability to retrive according information on required assets and components on-the-fly."@en ;
    rdfs:seeAlso "IoT-A Requirement UNI.418",
        "IoT-A Requirement UNI.419",
        "IoT-A Requirement UNI.420",
        "IoT-A Requirement UNI.421" ;
    ns5:supports ns4:DataDiscovery,
        ns4:ServiceDiscovery .

ns4:EdgecrossEdgeComputingLayerAnno a owl:NamedIndividual,
        ns1:oaAnnotation ;
    ns1:oahasBody ns4:EdgecrossEdgeComputingLayer ;
    ns1:oahasTarget [ a ns1:oaSpecificResource ;
            ns2:format "pdf" ;
            ns1:oahasSelector [ a ns1:oaRangeSelector ;
                    ns1:oahasEndSelector [ a ns1:oaXPathSelector ;
                            rdf:value "Page 15" ] ;
                    ns1:oahasStartSelector [ a ns1:oaXPathSelector ;
                            rdf:value "Page 9" ] ] ;
            ns1:oahasSource ns4:Edgecross_Consortium_to_Address_Edge_Integration_in_IIoT_enabled_Architectures ],
        [ a ns1:oaSpecificResource ;
            ns2:format "pdf" ;
            ns1:oahasSelector [ a ns1:oaRangeSelector ;
                    ns1:oahasEndSelector [ a ns1:oaXPathSelector ;
                            rdf:value "Page 15" ] ;
                    ns1:oahasStartSelector [ a ns1:oaXPathSelector ;
                            rdf:value "Page 9" ] ] ;
            ns1:oahasSource ns4:Edgecross_Consortium_to_Address_Edge_Integration_in_IIoT_enabled_Architectures ] .

ns4:EdgecrossFacilityLayerAnno a owl:NamedIndividual,
        ns1:oaAnnotation ;
    ns1:oahasBody ns4:EdgecrossFacilityLayer ;
    ns1:oahasTarget [ a ns1:oaSpecificResource ;
            ns2:format "pdf" ;
            ns1:oahasSelector [ a ns1:oaRangeSelector ;
                    ns1:oahasEndSelector [ a ns1:oaXPathSelector ;
                            rdf:value "Page 15" ] ;
                    ns1:oahasStartSelector [ a ns1:oaXPathSelector ;
                            rdf:value "Page 9" ] ] ;
            ns1:oahasSource ns4:Edgecross_Consortium_to_Address_Edge_Integration_in_IIoT_enabled_Architectures ],
        [ a ns1:oaSpecificResource ;
            ns2:format "pdf" ;
            ns1:oahasSelector [ a ns1:oaRangeSelector ;
                    ns1:oahasEndSelector [ a ns1:oaXPathSelector ;
                            rdf:value "Page 15" ] ;
                    ns1:oahasStartSelector [ a ns1:oaXPathSelector ;
                            rdf:value "Page 9" ] ] ;
            ns1:oahasSource ns4:Edgecross_Consortium_to_Address_Edge_Integration_in_IIoT_enabled_Architectures ] .

ns4:EdgecrossItSystemsLayerAnno a owl:NamedIndividual,
        ns1:oaAnnotation ;
    ns1:oahasBody ns4:EdgecrossItSystemsLayer ;
    ns1:oahasTarget [ a ns1:oaSpecificResource ;
            ns2:format "pdf" ;
            ns1:oahasSelector [ a ns1:oaRangeSelector ;
                    ns1:oahasEndSelector [ a ns1:oaXPathSelector ;
                            rdf:value "Page 15" ] ;
                    ns1:oahasStartSelector [ a ns1:oaXPathSelector ;
                            rdf:value "Page 9" ] ] ;
            ns1:oahasSource ns4:Edgecross_Consortium_to_Address_Edge_Integration_in_IIoT_enabled_Architectures ],
        [ a ns1:oaSpecificResource ;
            ns2:format "pdf" ;
            ns1:oahasSelector [ a ns1:oaRangeSelector ;
                    ns1:oahasEndSelector [ a ns1:oaXPathSelector ;
                            rdf:value "Page 15" ] ;
                    ns1:oahasStartSelector [ a ns1:oaXPathSelector ;
                            rdf:value "Page 9" ] ] ;
            ns1:oahasSource ns4:Edgecross_Consortium_to_Address_Edge_Integration_in_IIoT_enabled_Architectures ] .

ns4:EdgecrossLayerAnno a owl:NamedIndividual,
        ns1:oaAnnotation ;
    ns1:oahasBody ns4:EdgecrossLayer ;
    ns1:oahasTarget [ a ns1:oaSpecificResource ;
            ns2:format "pdf" ;
            ns1:oahasSource ns4:Edgecross_Consortium_to_Address_Edge_Integration_in_IIoT_enabled_Architectures ],
        [ a ns1:oaSpecificResource ;
            ns2:format "pdf" ;
            ns1:oahasSource ns4:Edgecross_Consortium_to_Address_Edge_Integration_in_IIoT_enabled_Architectures ] .

ns4:EdgecrossWhitepaper a owl:NamedIndividual,
        ns8:Document,
        ns4:Publication ;
    rdfs:label "Edgecross Whitepaper"@en ;
    ns2:creator ns4:EdgecrossConsortium ;
    ns8:maker ns4:EdgecrossConsortium ;
    ns4:hasClassification ns4:EdgecrossEdgeComputingLayer,
        ns4:EdgecrossFacilityLayer,
        ns4:EdgecrossItSystemsLayer ;
    ns4:hasOfficialResource <https://www.edgecross.org/ja/data-download/pdf/Edgecross_Consortium_WP(E).pdf> ;
    ns4:hasPublisher ns4:EdgecrossConsortium ;
    ns5:hasTargetConcern ns4:EdgeComputing,
        ns4:Interoperability .

ns4:ExecutionVariability a owl:NamedIndividual,
        ns4:Concern ;
    rdfs:label "Execution Variability"@en ;
    ns2:creator ns4:sebastian ;
    rdfs:comment "The system's ability to flexibly connect/adjust data flows in order to reach a defined target."@en .

ns4:Extensibility a owl:NamedIndividual,
        ns4:Concern ;
    rdfs:label "Extensibility"@en ;
    ns2:creator ns4:MuhammadUsman ;
    rdfs:comment "\"Extensibility could be a huge challenge at the edge of the network, unlike a mobile system, the things in the IoT could be very dynamic. When the owner purchases a new thing, can it be easily added to the current service without any problem? Or when one thing is replaced due to wearing out, can the previous service adopt a new node easily? These problems should be solved with a flexible and extensible design of service management layer in the edgeOS.\""@en ;
    rdfs:seeAlso <https://ieeexplore.ieee.org/document/7488250> ;
    ns4:hasWikipediaArticle <https://en.wikipedia.org/wiki/Extensibility> ;
    ns5:supports ns4:Evolvability .

ns4:FIWAREAnno a owl:NamedIndividual,
        ns1:oaAnnotation ;
    ns1:oahasBody ns4:FIWARE ;
    ns1:oahasTarget [ a ns1:oaSpecificResource ;
            ns1:oahasSource <https://forge.fiware.org/plugins/mediawiki/wiki/fiware/index.php/Summary_of_FI-WARE_Open_Specifications> ],
        [ a ns1:oaSpecificResource ;
            ns1:oahasSource <https://forge.fiware.org/plugins/mediawiki/wiki/fiware/index.php/Summary_of_FI-WARE_Open_Specifications> ] .

ns4:Fairness a owl:NamedIndividual,
        ns4:Concern ;
    rdfs:label "Fairness"@en ;
    ns2:creator ns4:MuhammadUsman ;
    rdfs:comment "How can a fair and non-discriminating access to (compute and storage) resources be established?"@en ;
    rdfs:seeAlso <https://dl.acm.org/citation.cfm?doid=3098208.3098210> ;
    ns4:hasWikipediaArticle <https://en.wikipedia.org/wiki/Fairness> ;
    ns5:supports ns4:BusinessContext .

ns4:FaultTolerance a owl:NamedIndividual,
        ns4:Concern ;
    rdfs:label "Fault Tolerance"@en ;
    ns2:creator ns4:MuhammadUsman ;
    rdfs:comment "Fault tolerance is the property that enables a system to continue operating properly in the event of the failure of some (one or more faults within) of its components. If its operating quality decreases at all, the decrease is proportional to the severity of the failure, as compared to a naively designed system in which even a small failure can cause total breakdown."@en ;
    rdfs:seeAlso <https://dl.acm.org/citation.cfm?doid=2508075.2508082>,
        <https://ieeexplore.ieee.org/document/6188257>,
        <https://ieeexplore.ieee.org/document/8304465> ;
    ns4:hasDBpediaResource <http://dbpedia.org/page/Category:Fault-tolerant_computer_systems> ;
    ns4:hasWikipediaArticle <https://en.wikipedia.org/wiki/Fault_tolerance> ;
    ns5:supports ns4:Availability .

ns4:FiwareAdvancedUiAnno a owl:NamedIndividual,
        ns1:oaAnnotation ;
    ns1:oahasBody ns4:FiwareAdvancedUi ;
    ns1:oahasTarget [ a ns1:oaSpecificResource ;
            ns1:oahasSource <https://forge.fiware.org/plugins/mediawiki/wiki/fiware/index.php/Advanced_Middleware_and_Web_UI_Architecture> ],
        [ a ns1:oaSpecificResource ;
            ns1:oahasSource <https://forge.fiware.org/plugins/mediawiki/wiki/fiware/index.php/Advanced_Middleware_and_Web_UI_Architecture> ] .

ns4:FiwareApplicationsServicesAndDataDeliveryAnno a owl:NamedIndividual,
        ns1:oaAnnotation ;
    ns1:oahasBody ns4:FiwareApplicationsServicesAndDataDelivery ;
    ns1:oahasTarget [ a ns1:oaSpecificResource ;
            ns1:oahasSource <https://forge.fiware.org/plugins/mediawiki/wiki/fiware/index.php/Architecture_of_Applications,_Services_and_Data_Delivery_R3> ],
        [ a ns1:oaSpecificResource ;
            ns1:oahasSource <https://forge.fiware.org/plugins/mediawiki/wiki/fiware/index.php/Architecture_of_Applications,_Services_and_Data_Delivery_R3> ] .

ns4:FiwareChapterAnno a owl:NamedIndividual,
        ns1:oaAnnotation ;
    ns1:oahasBody ns4:FiwareChapter ;
    ns1:oahasTarget [ a ns1:oaSpecificResource ;
            ns1:oahasSource <https://forge.fiware.org/plugins/mediawiki/wiki/fiware/index.php/Summary_of_FI-WARE_Open_Specifications> ] .

ns4:FiwareCloudHostingAnno a owl:NamedIndividual,
        ns1:oaAnnotation ;
    ns1:oahasBody ns4:FiwareCloudHosting ;
    ns1:oahasTarget [ a ns1:oaSpecificResource ;
            ns1:oahasSource <https://forge.fiware.org/plugins/mediawiki/wiki/fiware/index.php/Cloud_Hosting_Architecture_R3> ],
        [ a ns1:oaSpecificResource ;
            ns1:oahasSource <https://forge.fiware.org/plugins/mediawiki/wiki/fiware/index.php/Cloud_Hosting_Architecture_R3> ] .

ns4:FiwareDataContextManagementAnno a owl:NamedIndividual,
        ns1:oaAnnotation ;
    ns1:oahasBody ns4:FiwareDataContextManagement ;
    ns1:oahasTarget [ a ns1:oaSpecificResource ;
            ns1:oahasSource <https://forge.fiware.org/plugins/mediawiki/wiki/fiware/index.php/Data/Context_Management_Architecture_R3> ],
        [ a ns1:oaSpecificResource ;
            ns1:oahasSource <https://forge.fiware.org/plugins/mediawiki/wiki/fiware/index.php/Data/Context_Management_Architecture_R3> ] .

ns4:FiwareIotServicesEnablementAnno a owl:NamedIndividual,
        ns1:oaAnnotation ;
    ns1:oahasBody ns4:FiwareIotServicesEnablement ;
    ns1:oahasTarget [ a ns1:oaSpecificResource ;
            ns1:oahasSource <https://forge.fiware.org/plugins/mediawiki/wiki/fiware/index.php/Internet_of_Things_(IoT)_Services_Enablement_Architecture_R3> ],
        [ a ns1:oaSpecificResource ;
            ns1:oahasSource <https://forge.fiware.org/plugins/mediawiki/wiki/fiware/index.php/Internet_of_Things_(IoT)_Services_Enablement_Architecture_R3> ] .

ns4:FiwareSecurityAnno a owl:NamedIndividual,
        ns1:oaAnnotation ;
    ns1:oahasBody ns4:FiwareSecurity ;
    ns1:oahasTarget [ a ns1:oaSpecificResource ;
            ns1:oahasSource <https://forge.fiware.org/plugins/mediawiki/wiki/fiware/index.php/Security_Architecture_R3> ],
        [ a ns1:oaSpecificResource ;
            ns1:oahasSource <https://forge.fiware.org/plugins/mediawiki/wiki/fiware/index.php/Security_Architecture_R3> ] .

ns4:GeoTracking a owl:NamedIndividual,
        ns4:Concern ;
    rdfs:label "Geo tracking"@en ;
    ns7:hasStakeholder <http://purl.oclc.org/NET/mvco.owl#EndUser> ;
    rdfs:comment "A system built using the ARM shall support physical entity location tracking (geo spatial and/or logical location)"@en ;
    rdfs:seeAlso "IoT-A Requirement UNI.016" ;
    ns4:hasDBpediaResource <http://dbpedia.org/resource/Track_and_trace> ;
    ns5:supports ns4:ContextAwareness .

ns4:GeospatialQuery rdfs:seeAlso "IoT-A Requirement UNI.401" .

ns4:Greening_of_IoT a owl:NamedIndividual,
        ns4:Concern ;
    rdfs:label "Greening of IoT"@en ;
    ns2:creator ns4:MuhammadUsman ;
    rdfs:comment """The system energy consumption is expanding at a high rate because of increment in information rates, an increment in quantity of Internet-empowered services
and fast development of Internet associated edgedevices. The future IoT will cause a critical increase in the network energy consumption."""@en ;
    rdfs:seeAlso <https://ieeexplore.ieee.org/document/6188257> ;
    ns4:hasWikipediaArticle <https://en.wikipedia.org/wiki/Green_computing> ;
    ns5:supports ns4:EnergyControl .

ns4:ID4me a owl:NamedIndividual,
        ns4:TechnicalSpecification ;
    ns5:hasTargetConcern ns4:Identification,
        ns4:IdentityManagement .

ns4:IDSRAMBusinessLayerAnno a owl:NamedIndividual,
        ns1:oaAnnotation ;
    ns1:oahasBody ns4:IDSRAMBusinessLayer ;
    ns1:oahasTarget [ a ns1:oaSpecificResource ;
            ns2:format "pdf" ;
            ns1:oahasSelector [ a ns1:oaRangeSelector ;
                    ns1:oahasEndSelector [ a ns1:oaXPathSelector ;
                            rdf:value "Page 21" ] ;
                    ns1:oahasStartSelector [ a ns1:oaXPathSelector ;
                            rdf:value "Page 17" ] ] ;
            ns1:oahasSource ns4:IDS_REFERENCE_ARCHITECTURE_MODEL_INDUSTRIAL_DATA_SPACE_VERSION_2_0 ] .

ns4:IDSRAMCertificationAnno a owl:NamedIndividual,
        ns1:oaAnnotation ;
    ns1:oahasBody ns4:IDSRAMCertification ;
    ns1:oahasTarget [ a ns1:oaSpecificResource ;
            ns2:format "pdf" ;
            ns1:oahasSelector [ a ns1:oaRangeSelector ;
                    ns1:oahasEndSelector [ a ns1:oaXPathSelector ;
                            rdf:value "Page 84" ] ;
                    ns1:oahasStartSelector [ a ns1:oaXPathSelector ;
                            rdf:value "Page 79" ] ] ;
            ns1:oahasSource ns4:IDS_REFERENCE_ARCHITECTURE_MODEL_INDUSTRIAL_DATA_SPACE_VERSION_2_0 ] .

ns4:IDSRAMDataMarket a owl:NamedIndividual,
        ns4:StandardClassification ;
    rdfs:label "IDS Data Market"@en ;
    ns4:isDescribedin ns4:IDSRAMReferenceArchitectureModel .

ns4:IDSRAMFunctionalLayerAnno a owl:NamedIndividual,
        ns1:oaAnnotation ;
    ns1:oahasBody ns4:IDSRAMFunctionalLayer ;
    ns1:oahasTarget [ a ns1:oaSpecificResource ;
            ns2:format "pdf" ;
            ns1:oahasSelector [ a ns1:oaRangeSelector ;
                    ns1:oahasEndSelector [ a ns1:oaXPathSelector ;
                            rdf:value "Page 25" ] ;
                    ns1:oahasStartSelector [ a ns1:oaXPathSelector ;
                            rdf:value "Page 21" ] ] ;
            ns1:oahasSource ns4:IDS_REFERENCE_ARCHITECTURE_MODEL_INDUSTRIAL_DATA_SPACE_VERSION_2_0 ] .

ns4:IDSRAMGovernanceAnno a owl:NamedIndividual,
        ns1:oaAnnotation ;
    ns1:oahasBody ns4:IDSRAMGovernance ;
    ns1:oahasTarget [ a ns1:oaSpecificResource ;
            ns2:format "pdf" ;
            ns1:oahasSelector [ a ns1:oaRangeSelector ;
                    ns1:oahasEndSelector [ a ns1:oaXPathSelector ;
                            rdf:value "Page 88" ] ;
                    ns1:oahasStartSelector [ a ns1:oaXPathSelector ;
                            rdf:value "Page 84" ] ] ;
            ns1:oahasSource ns4:IDS_REFERENCE_ARCHITECTURE_MODEL_INDUSTRIAL_DATA_SPACE_VERSION_2_0 ] .

ns4:IDSRAMInformationLayerAnno a owl:NamedIndividual,
        ns1:oaAnnotation ;
    ns1:oahasBody ns4:IDSRAMInformationLayer ;
    ns1:oahasTarget [ a ns1:oaSpecificResource ;
            ns2:format "pdf" ;
            ns1:oahasSelector [ a ns1:oaRangeSelector ;
                    ns1:oahasEndSelector [ a ns1:oaXPathSelector ;
                            rdf:value "Page 56" ] ;
                    ns1:oahasStartSelector [ a ns1:oaXPathSelector ;
                            rdf:value "Page 32" ] ] ;
            ns1:oahasSource ns4:IDS_REFERENCE_ARCHITECTURE_MODEL_INDUSTRIAL_DATA_SPACE_VERSION_2_0 ] .

ns4:IDSRAMLayerAnno a owl:NamedIndividual,
        ns1:oaAnnotation ;
    ns1:oahasBody ns4:IDSRAMLayer ;
    ns1:oahasTarget [ a ns1:oaSpecificResource ;
            ns2:format "pdf" ;
            ns1:oahasSource ns4:IDS_REFERENCE_ARCHITECTURE_MODEL_INDUSTRIAL_DATA_SPACE_VERSION_2_0 ],
        [ a ns1:oaSpecificResource ;
            ns2:format "pdf" ;
            ns1:oahasSource ns4:IDS_REFERENCE_ARCHITECTURE_MODEL_INDUSTRIAL_DATA_SPACE_VERSION_2_0 ] .

ns4:IDSRAMProcessLayerAnno a owl:NamedIndividual,
        ns1:oaAnnotation ;
    ns1:oahasBody ns4:IDSRAMProcessLayer ;
    ns1:oahasTarget [ a ns1:oaSpecificResource ;
            ns2:format "pdf" ;
            ns1:oahasSelector [ a ns1:oaRangeSelector ;
                    ns1:oahasEndSelector [ a ns1:oaXPathSelector ;
                            rdf:value "Page 32" ] ;
                    ns1:oahasStartSelector [ a ns1:oaXPathSelector ;
                            rdf:value "Page 25" ] ] ;
            ns1:oahasSource ns4:IDS_REFERENCE_ARCHITECTURE_MODEL_INDUSTRIAL_DATA_SPACE_VERSION_2_0 ] .

ns4:IDSRAMSecurityAnno a owl:NamedIndividual,
        ns1:oaAnnotation ;
    ns1:oahasBody ns4:IDSRAMSecurity ;
    ns1:oahasTarget [ a ns1:oaSpecificResource ;
            ns2:format "pdf" ;
            ns1:oahasSelector [ a ns1:oaRangeSelector ;
                    ns1:oahasEndSelector [ a ns1:oaXPathSelector ;
                            rdf:value "Page 79" ] ;
                    ns1:oahasStartSelector [ a ns1:oaXPathSelector ;
                            rdf:value "Page 63" ] ] ;
            ns1:oahasSource ns4:IDS_REFERENCE_ARCHITECTURE_MODEL_INDUSTRIAL_DATA_SPACE_VERSION_2_0 ] .

ns4:IDSRAMSystemLayerAnno a owl:NamedIndividual,
        ns1:oaAnnotation ;
    ns1:oahasBody ns4:IDSRAMSystemLayer ;
    ns1:oahasTarget [ a ns1:oaSpecificResource ;
            ns2:format "pdf" ;
            ns1:oahasSelector [ a ns1:oaRangeSelector ;
                    ns1:oahasEndSelector [ a ns1:oaXPathSelector ;
                            rdf:value "Page 62" ] ;
                    ns1:oahasStartSelector [ a ns1:oaXPathSelector ;
                            rdf:value "Page 56" ] ] ;
            ns1:oahasSource ns4:IDS_REFERENCE_ARCHITECTURE_MODEL_INDUSTRIAL_DATA_SPACE_VERSION_2_0 ] .

ns4:IEC_29115 a owl:NamedIndividual,
        ns4:Standard ;
    ns4:hasClassification ns4:IIRASecurity ;
    ns5:hasTargetConcern ns4:Authentication,
        ns4:Identification .

ns4:IEC_61508 a owl:NamedIndividual,
        ns4:Standard ;
    ns4:hasClassification ns4:IDSRAMCertification,
        ns4:Safety ;
    ns5:hasTargetConcern ns4:Safety .

ns4:IEC_61511 a owl:NamedIndividual,
        ns4:Standard ;
    ns4:hasClassification ns4:IDSRAMCertification ;
    ns5:hasTargetConcern ns4:Safety .

ns4:IEC_61804_P3 a owl:NamedIndividual,
        ns4:Standard ;
    ns5:frames ns4:ThingDescription .

ns4:IEC_61804_P4 a owl:NamedIndividual,
        ns4:Standard ;
    ns5:frames ns4:ThingDescription .

ns4:IEC_61804_P5 a owl:NamedIndividual,
        ns4:Standard ;
    ns5:frames ns4:ThingDescription .

ns4:IEC_61804_P6 a owl:NamedIndividual,
        ns4:TechnicalReport ;
    ns5:frames ns4:ThingDescription .

ns4:IEC_62264_P6 a owl:NamedIndividual,
        ns4:Standard ;
    ns5:frames ns4:Communication .

ns4:IICFFrameworkLayerAnno a owl:NamedIndividual,
        ns1:oaAnnotation ;
    ns1:oahasBody ns4:IICFFrameworkLayer ;
    ns1:oahasTarget [ a ns1:oaSpecificResource ;
            ns2:format "pdf" ;
            ns1:oahasSelector [ a ns1:oaRangeSelector ;
                    ns1:oahasEndSelector [ a ns1:oaXPathSelector ;
                            rdf:value "Page 17" ] ;
                    ns1:oahasStartSelector [ a ns1:oaXPathSelector ;
                            rdf:value "Page 14" ] ] ;
            ns1:oahasSource ns4:The_Industrial_Internet_of_Things_Volume_G5_Connectivity_Framework ],
        [ a ns1:oaSpecificResource ;
            ns2:format "pdf" ;
            ns1:oahasSelector [ a ns1:oaRangeSelector ;
                    ns1:oahasEndSelector [ a ns1:oaXPathSelector ;
                            rdf:value "Page 17" ] ;
                    ns1:oahasStartSelector [ a ns1:oaXPathSelector ;
                            rdf:value "Page 14" ] ] ;
            ns1:oahasSource ns4:The_Industrial_Internet_of_Things_Volume_G5_Connectivity_Framework ] .

ns4:IICFLinkLayerAnno a owl:NamedIndividual,
        ns1:oaAnnotation ;
    ns1:oahasBody ns4:IICFLinkLayer ;
    ns1:oahasTarget [ a ns1:oaSpecificResource ;
            ns2:format "pdf" ;
            ns1:oahasSelector [ a ns1:oaRangeSelector ;
                    ns1:oahasEndSelector [ a ns1:oaXPathSelector ;
                            rdf:value "Page 17" ] ;
                    ns1:oahasStartSelector [ a ns1:oaXPathSelector ;
                            rdf:value "Page 14" ] ] ;
            ns1:oahasSource ns4:The_Industrial_Internet_of_Things_Volume_G5_Connectivity_Framework ],
        [ a ns1:oaSpecificResource ;
            ns2:format "pdf" ;
            ns1:oahasSelector [ a ns1:oaRangeSelector ;
                    ns1:oahasEndSelector [ a ns1:oaXPathSelector ;
                            rdf:value "Page 17" ] ;
                    ns1:oahasStartSelector [ a ns1:oaXPathSelector ;
                            rdf:value "Page 14" ] ] ;
            ns1:oahasSource ns4:The_Industrial_Internet_of_Things_Volume_G5_Connectivity_Framework ] .

ns4:IICFNetworkLayerAnno a owl:NamedIndividual,
        ns1:oaAnnotation ;
    ns1:oahasBody ns4:IICFNetworkLayer ;
    ns1:oahasTarget [ a ns1:oaSpecificResource ;
            ns2:format "pdf" ;
            ns1:oahasSelector [ a ns1:oaRangeSelector ;
                    ns1:oahasEndSelector [ a ns1:oaXPathSelector ;
                            rdf:value "Page 17" ] ;
                    ns1:oahasStartSelector [ a ns1:oaXPathSelector ;
                            rdf:value "Page 14" ] ] ;
            ns1:oahasSource ns4:The_Industrial_Internet_of_Things_Volume_G5_Connectivity_Framework ],
        [ a ns1:oaSpecificResource ;
            ns2:format "pdf" ;
            ns1:oahasSelector [ a ns1:oaRangeSelector ;
                    ns1:oahasEndSelector [ a ns1:oaXPathSelector ;
                            rdf:value "Page 17" ] ;
                    ns1:oahasStartSelector [ a ns1:oaXPathSelector ;
                            rdf:value "Page 14" ] ] ;
            ns1:oahasSource ns4:The_Industrial_Internet_of_Things_Volume_G5_Connectivity_Framework ] .

ns4:IICFPhysicalLayerAnno a owl:NamedIndividual,
        ns1:oaAnnotation ;
    ns1:oahasBody ns4:IICFPhysicalLayer ;
    ns1:oahasTarget [ a ns1:oaSpecificResource ;
            ns2:format "pdf" ;
            ns1:oahasSelector [ a ns1:oaRangeSelector ;
                    ns1:oahasEndSelector [ a ns1:oaXPathSelector ;
                            rdf:value "Page 17" ] ;
                    ns1:oahasStartSelector [ a ns1:oaXPathSelector ;
                            rdf:value "Page 14" ] ] ;
            ns1:oahasSource ns4:The_Industrial_Internet_of_Things_Volume_G5_Connectivity_Framework ],
        [ a ns1:oaSpecificResource ;
            ns2:format "pdf" ;
            ns1:oahasSelector [ a ns1:oaRangeSelector ;
                    ns1:oahasEndSelector [ a ns1:oaXPathSelector ;
                            rdf:value "Page 17" ] ;
                    ns1:oahasStartSelector [ a ns1:oaXPathSelector ;
                            rdf:value "Page 14" ] ] ;
            ns1:oahasSource ns4:The_Industrial_Internet_of_Things_Volume_G5_Connectivity_Framework ] .

ns4:IICFTansportLayerAnno a owl:NamedIndividual,
        ns1:oaAnnotation ;
    ns1:oahasBody ns4:IICFTansportLayer ;
    ns1:oahasTarget [ a ns1:oaSpecificResource ;
            ns2:format "pdf" ;
            ns1:oahasSelector [ a ns1:oaRangeSelector ;
                    ns1:oahasEndSelector [ a ns1:oaXPathSelector ;
                            rdf:value "Page 17" ] ;
                    ns1:oahasStartSelector [ a ns1:oaXPathSelector ;
                            rdf:value "Page 14" ] ] ;
            ns1:oahasSource ns4:The_Industrial_Internet_of_Things_Volume_G5_Connectivity_Framework ],
        [ a ns1:oaSpecificResource ;
            ns2:format "pdf" ;
            ns1:oahasSelector [ a ns1:oaRangeSelector ;
                    ns1:oahasEndSelector [ a ns1:oaXPathSelector ;
                            rdf:value "Page 17" ] ;
                    ns1:oahasStartSelector [ a ns1:oaXPathSelector ;
                            rdf:value "Page 14" ] ] ;
            ns1:oahasSource ns4:The_Industrial_Internet_of_Things_Volume_G5_Connectivity_Framework ] .

ns4:IICVocabulary a owl:NamedIndividual,
        ns8:Document,
        ns4:Publication,
        ns4:StandardClassification ;
    rdfs:label "IIC Vocabulary"@en ;
    ns2:creator ns4:IIC,
        ns4:sebastian ;
    ns3:associatedWith ns4:IDSRAMInformationLayer ;
    ns8:maker ns4:IIC ;
    ns4:hasPublisher ns4:IIC ;
    ns4:isDescribedin ns4:IIRA ;
    ns5:alignsWith ns4:IDSRAMInformationLayer .

ns4:IIRAApplicationDomainAnno a owl:NamedIndividual,
        ns1:oaAnnotation ;
    ns1:oahasBody ns4:IIRAApplicationDomain ;
    ns1:oahasTarget [ a ns1:oaSpecificResource ;
            ns2:format "pdf" ;
            ns1:oahasSelector [ a ns1:oaRangeSelector ;
                    ns1:oahasEndSelector [ a ns1:oaXPathSelector ;
                            rdf:value "Page 35" ] ;
                    ns1:oahasStartSelector [ a ns1:oaXPathSelector ;
                            rdf:value "Page 34" ] ] ;
            ns1:oahasSource ns4:The_Industrial_Internet_of_Things_Volume_G1_Reference_Architecture ],
        [ a ns1:oaSpecificResource ;
            ns2:format "pdf" ;
            ns1:oahasSelector [ a ns1:oaRangeSelector ;
                    ns1:oahasEndSelector [ a ns1:oaXPathSelector ;
                            rdf:value "Page 35" ] ;
                    ns1:oahasStartSelector [ a ns1:oaXPathSelector ;
                            rdf:value "Page 34" ] ] ;
            ns1:oahasSource ns4:The_Industrial_Internet_of_Things_Volume_G1_Reference_Architecture ] .

ns4:IIRABusinessDomainAnno a owl:NamedIndividual,
        ns1:oaAnnotation ;
    ns1:oahasBody ns4:IIRABusinessDomain ;
    ns1:oahasTarget [ a ns1:oaSpecificResource ;
            ns2:format "pdf" ;
            ns1:oahasSelector [ a ns1:oaRangeSelector ;
                    ns1:oahasEndSelector [ a ns1:oaXPathSelector ;
                            rdf:value "Page 35" ] ;
                    ns1:oahasStartSelector [ a ns1:oaXPathSelector ;
                            rdf:value "Page 34" ] ] ;
            ns1:oahasSource ns4:The_Industrial_Internet_of_Things_Volume_G1_Reference_Architecture ],
        [ a ns1:oaSpecificResource ;
            ns2:format "pdf" ;
            ns1:oahasSelector [ a ns1:oaRangeSelector ;
                    ns1:oahasEndSelector [ a ns1:oaXPathSelector ;
                            rdf:value "Page 35" ] ;
                    ns1:oahasStartSelector [ a ns1:oaXPathSelector ;
                            rdf:value "Page 34" ] ] ;
            ns1:oahasSource ns4:The_Industrial_Internet_of_Things_Volume_G1_Reference_Architecture ] .

ns4:IIRABusinessViewpointAnno a owl:NamedIndividual,
        ns1:oaAnnotation ;
    ns1:oahasBody ns4:IIRABusinessViewpoint ;
    ns1:oahasTarget [ a ns1:oaSpecificResource ;
            ns2:format "pdf" ;
            ns1:oahasSelector [ a ns1:oaRangeSelector ;
                    ns1:oahasEndSelector [ a ns1:oaXPathSelector ;
                            rdf:value "Page 22" ] ;
                    ns1:oahasStartSelector [ a ns1:oaXPathSelector ;
                            rdf:value "Page 20" ] ] ;
            ns1:oahasSource ns4:The_Industrial_Internet_of_Things_Volume_G1_Reference_Architecture ],
        [ a ns1:oaSpecificResource ;
            ns2:format "pdf" ;
            ns1:oahasSelector [ a ns1:oaRangeSelector ;
                    ns1:oahasEndSelector [ a ns1:oaXPathSelector ;
                            rdf:value "Page 22" ] ;
                    ns1:oahasStartSelector [ a ns1:oaXPathSelector ;
                            rdf:value "Page 20" ] ] ;
            ns1:oahasSource ns4:The_Industrial_Internet_of_Things_Volume_G1_Reference_Architecture ] .

ns4:IIRAConnectivityAnno a owl:NamedIndividual,
        ns1:oaAnnotation ;
    ns1:oahasBody ns4:IIRAConnectivity ;
    ns1:oahasTarget [ a ns1:oaSpecificResource ;
            ns2:format "pdf" ;
            ns1:oahasSelector [ a ns1:oaRangeSelector ;
                    ns1:oahasEndSelector [ a ns1:oaXPathSelector ;
                            rdf:value "Page 127" ] ;
                    ns1:oahasStartSelector [ a ns1:oaXPathSelector ;
                            rdf:value "Page 8" ] ] ;
            ns1:oahasSource ns4:The_Industrial_Internet_of_Things_Volume_G5_Connectivity_Framework ],
        [ a ns1:oaSpecificResource ;
            ns2:format "pdf" ;
            ns1:oahasSelector [ a ns1:oaRangeSelector ;
                    ns1:oahasEndSelector [ a ns1:oaXPathSelector ;
                            rdf:value "Page 127" ] ;
                    ns1:oahasStartSelector [ a ns1:oaXPathSelector ;
                            rdf:value "Page 8" ] ] ;
            ns1:oahasSource ns4:The_Industrial_Internet_of_Things_Volume_G5_Connectivity_Framework ] .

ns4:IIRAControlDomainAnno a owl:NamedIndividual,
        ns1:oaAnnotation ;
    ns1:oahasBody ns4:IIRAControlDomain ;
    ns1:oahasTarget [ a ns1:oaSpecificResource ;
            ns2:format "pdf" ;
            ns1:oahasSelector [ a ns1:oaRangeSelector ;
                    ns1:oahasEndSelector [ a ns1:oaXPathSelector ;
                            rdf:value "Page 30" ] ;
                    ns1:oahasStartSelector [ a ns1:oaXPathSelector ;
                            rdf:value "Page 27" ] ] ;
            ns1:oahasSource ns4:The_Industrial_Internet_of_Things_Volume_G1_Reference_Architecture ],
        [ a ns1:oaSpecificResource ;
            ns2:format "pdf" ;
            ns1:oahasSelector [ a ns1:oaRangeSelector ;
                    ns1:oahasEndSelector [ a ns1:oaXPathSelector ;
                            rdf:value "Page 30" ] ;
                    ns1:oahasStartSelector [ a ns1:oaXPathSelector ;
                            rdf:value "Page 27" ] ] ;
            ns1:oahasSource ns4:The_Industrial_Internet_of_Things_Volume_G1_Reference_Architecture ] .

ns4:IIRACrosscuttingFunctionAnno a owl:NamedIndividual,
        ns1:oaAnnotation ;
    ns1:oahasBody ns4:IIRACrosscuttingFunction ;
    ns1:oahasTarget [ a ns1:oaSpecificResource ;
            ns2:format "pdf" ;
            ns1:oahasSelector [ a ns1:oaRangeSelector ;
                    ns1:oahasEndSelector [ a ns1:oaXPathSelector ;
                            rdf:value "Page 36" ] ;
                    ns1:oahasStartSelector [ a ns1:oaXPathSelector ;
                            rdf:value "Page 34" ] ] ;
            ns1:oahasSource ns4:The_Industrial_Internet_of_Things_Volume_G1_Reference_Architecture ],
        [ a ns1:oaSpecificResource ;
            ns2:format "pdf" ;
            ns1:oahasSelector [ a ns1:oaRangeSelector ;
                    ns1:oahasEndSelector [ a ns1:oaXPathSelector ;
                            rdf:value "Page 36" ] ;
                    ns1:oahasStartSelector [ a ns1:oaXPathSelector ;
                            rdf:value "Page 34" ] ] ;
            ns1:oahasSource ns4:The_Industrial_Internet_of_Things_Volume_G1_Reference_Architecture ] .

ns4:IIRAFunctionalViewpointAnno a owl:NamedIndividual,
        ns1:oaAnnotation ;
    ns1:oahasBody ns4:IIRAFunctionalViewpoint ;
    ns1:oahasTarget [ a ns1:oaSpecificResource ;
            ns2:format "pdf" ;
            ns1:oahasSelector [ a ns1:oaRangeSelector ;
                    ns1:oahasEndSelector [ a ns1:oaXPathSelector ;
                            rdf:value "Page 38" ] ;
                    ns1:oahasStartSelector [ a ns1:oaXPathSelector ;
                            rdf:value "Page 25" ] ] ;
            ns1:oahasSource ns4:The_Industrial_Internet_of_Things_Volume_G1_Reference_Architecture ],
        [ a ns1:oaSpecificResource ;
            ns2:format "pdf" ;
            ns1:oahasSelector [ a ns1:oaRangeSelector ;
                    ns1:oahasEndSelector [ a ns1:oaXPathSelector ;
                            rdf:value "Page 38" ] ;
                    ns1:oahasStartSelector [ a ns1:oaXPathSelector ;
                            rdf:value "Page 25" ] ] ;
            ns1:oahasSource ns4:The_Industrial_Internet_of_Things_Volume_G1_Reference_Architecture ] .

ns4:IIRAImplementationViewpointAnno a owl:NamedIndividual,
        ns1:oaAnnotation ;
    ns1:oahasBody ns4:IIRAImplementationViewpoint ;
    ns1:oahasTarget [ a ns1:oaSpecificResource ;
            ns2:format "pdf" ;
            ns1:oahasSelector [ a ns1:oaRangeSelector ;
                    ns1:oahasEndSelector [ a ns1:oaXPathSelector ;
                            rdf:value "Page 47" ] ;
                    ns1:oahasStartSelector [ a ns1:oaXPathSelector ;
                            rdf:value "Page 38" ] ] ;
            ns1:oahasSource ns4:The_Industrial_Internet_of_Things_Volume_G1_Reference_Architecture ],
        [ a ns1:oaSpecificResource ;
            ns2:format "pdf" ;
            ns1:oahasSelector [ a ns1:oaRangeSelector ;
                    ns1:oahasEndSelector [ a ns1:oaXPathSelector ;
                            rdf:value "Page 47" ] ;
                    ns1:oahasStartSelector [ a ns1:oaXPathSelector ;
                            rdf:value "Page 38" ] ] ;
            ns1:oahasSource ns4:The_Industrial_Internet_of_Things_Volume_G1_Reference_Architecture ] .

ns4:IIRAIndustrialAnalytics a owl:NamedIndividual,
        ns4:IIRACrosscuttingFunction,
        ns4:StandardClassification ;
    ns3:isPartOf ns4:IIRAFunctionalViewpoint ;
    ns4:isDescribedin ns4:IIRA .

ns4:IIRAInformationDomainAnno a owl:NamedIndividual,
        ns1:oaAnnotation ;
    ns1:oahasBody ns4:IIRAInformationDomain ;
    ns1:oahasTarget [ a ns1:oaSpecificResource ;
            ns2:format "pdf" ;
            ns1:oahasSelector [ a ns1:oaRangeSelector ;
                    ns1:oahasEndSelector [ a ns1:oaXPathSelector ;
                            rdf:value "Page 34" ] ;
                    ns1:oahasStartSelector [ a ns1:oaXPathSelector ;
                            rdf:value "Page 32" ] ] ;
            ns1:oahasSource ns4:The_Industrial_Internet_of_Things_Volume_G1_Reference_Architecture ],
        [ a ns1:oaSpecificResource ;
            ns2:format "pdf" ;
            ns1:oahasSelector [ a ns1:oaRangeSelector ;
                    ns1:oahasEndSelector [ a ns1:oaXPathSelector ;
                            rdf:value "Page 34" ] ;
                    ns1:oahasStartSelector [ a ns1:oaXPathSelector ;
                            rdf:value "Page 32" ] ] ;
            ns1:oahasSource ns4:The_Industrial_Internet_of_Things_Volume_G1_Reference_Architecture ] .

ns4:IIRAIntelligentAndResilientControl a owl:NamedIndividual,
        ns4:IIRACrosscuttingFunction,
        ns4:StandardClassification ;
    rdfs:label "IIRA Intelligent and Resilient Control"@en ;
    ns3:isPartOf ns4:IIRAFunctionalViewpoint ;
    rdfs:comment """There is a renewed movement to distribute computational capability toward the network peripheries, away from concentrated computation centers, to benefit from a reduction in movement of data and communication latency, and enhancement in local intelligent control and, more importantly, resilience.
source: Industrial Internet Reference Archietcture"""@en ;
    ns4:isDescribedin ns4:IIRA .

ns4:IIRAOperationsDomainAnno a owl:NamedIndividual,
        ns1:oaAnnotation ;
    ns1:oahasBody ns4:IIRAOperationsDomain ;
    ns1:oahasTarget [ a ns1:oaSpecificResource ;
            ns2:format "pdf" ;
            ns1:oahasSelector [ a ns1:oaRangeSelector ;
                    ns1:oahasEndSelector [ a ns1:oaXPathSelector ;
                            rdf:value "Page 32" ] ;
                    ns1:oahasStartSelector [ a ns1:oaXPathSelector ;
                            rdf:value "Page 30" ] ] ;
            ns1:oahasSource ns4:The_Industrial_Internet_of_Things_Volume_G1_Reference_Architecture ],
        [ a ns1:oaSpecificResource ;
            ns2:format "pdf" ;
            ns1:oahasSelector [ a ns1:oaRangeSelector ;
                    ns1:oahasEndSelector [ a ns1:oaXPathSelector ;
                            rdf:value "Page 32" ] ;
                    ns1:oahasStartSelector [ a ns1:oaXPathSelector ;
                            rdf:value "Page 30" ] ] ;
            ns1:oahasSource ns4:The_Industrial_Internet_of_Things_Volume_G1_Reference_Architecture ] .

ns4:IIRAReliabilityAnno a owl:NamedIndividual,
        ns1:oaAnnotation ;
    ns1:oahasBody ns4:IIRAReliability ;
    ns1:oahasTarget [ a ns1:oaSpecificResource ;
            ns2:format "pdf" ;
            ns1:oahasSelector [ a ns1:oaRangeSelector ;
                    ns1:oahasEndSelector [ a ns1:oaXPathSelector ;
                            rdf:value "Page 19" ] ;
                    ns1:oahasStartSelector [ a ns1:oaXPathSelector ;
                            rdf:value "Page 18" ] ] ;
            ns1:oahasSource ns4:Industrial_Internet_of_Things_Volume_G4_Security_Framework ],
        [ a ns1:oaSpecificResource ;
            ns2:format "pdf" ;
            ns1:oahasSelector [ a ns1:oaRangeSelector ;
                    ns1:oahasEndSelector [ a ns1:oaXPathSelector ;
                            rdf:value "Page 19" ] ;
                    ns1:oahasStartSelector [ a ns1:oaXPathSelector ;
                            rdf:value "Page 18" ] ] ;
            ns1:oahasSource ns4:Industrial_Internet_of_Things_Volume_G4_Security_Framework ] .

ns4:IIRAResilienceAnno a owl:NamedIndividual,
        ns1:oaAnnotation ;
    ns1:oahasBody ns4:IIRAResilience ;
    ns1:oahasTarget [ a ns1:oaSpecificResource ;
            ns2:format "pdf" ;
            ns1:oahasSelector [ a ns1:oaRangeSelector ;
                    ns1:oahasEndSelector [ a ns1:oaXPathSelector ;
                            rdf:value "Page 20" ] ;
                    ns1:oahasStartSelector [ a ns1:oaXPathSelector ;
                            rdf:value "Page 19" ] ] ;
            ns1:oahasSource ns4:Industrial_Internet_of_Things_Volume_G4_Security_Framework ],
        [ a ns1:oaSpecificResource ;
            ns2:format "pdf" ;
            ns1:oahasSelector [ a ns1:oaRangeSelector ;
                    ns1:oahasEndSelector [ a ns1:oaXPathSelector ;
                            rdf:value "Page 19" ] ;
                    ns1:oahasStartSelector [ a ns1:oaXPathSelector ;
                            rdf:value "Page 18" ] ] ;
            ns1:oahasSource ns4:Industrial_Internet_of_Things_Volume_G4_Security_Framework ],
        [ a ns1:oaSpecificResource ;
            ns2:format "pdf" ;
            ns1:oahasSelector [ a ns1:oaRangeSelector ;
                    ns1:oahasEndSelector [ a ns1:oaXPathSelector ;
                            rdf:value "Page 19" ] ;
                    ns1:oahasStartSelector [ a ns1:oaXPathSelector ;
                            rdf:value "Page 18" ] ] ;
            ns1:oahasSource ns4:Industrial_Internet_of_Things_Volume_G4_Security_Framework ],
        [ a ns1:oaSpecificResource ;
            ns2:format "pdf" ;
            ns1:oahasSelector [ a ns1:oaRangeSelector ;
                    ns1:oahasEndSelector [ a ns1:oaXPathSelector ;
                            rdf:value "Page 20" ] ;
                    ns1:oahasStartSelector [ a ns1:oaXPathSelector ;
                            rdf:value "Page 19" ] ] ;
            ns1:oahasSource ns4:Industrial_Internet_of_Things_Volume_G4_Security_Framework ] .

ns4:IIRASafetyAnno a owl:NamedIndividual,
        ns1:oaAnnotation ;
    ns1:oahasBody ns4:IIRASafety ;
    ns1:oahasTarget [ a ns1:oaSpecificResource ;
            ns2:format "pdf" ;
            ns1:oahasSelector [ a ns1:oaRangeSelector ;
                    ns1:oahasEndSelector [ a ns1:oaXPathSelector ;
                            rdf:value "Page 18" ] ;
                    ns1:oahasStartSelector [ a ns1:oaXPathSelector ;
                            rdf:value "Page 17" ] ] ;
            ns1:oahasSource ns4:Industrial_Internet_of_Things_Volume_G4_Security_Framework ],
        [ a ns1:oaSpecificResource ;
            ns2:format "pdf" ;
            ns1:oahasSelector [ a ns1:oaRangeSelector ;
                    ns1:oahasEndSelector [ a ns1:oaXPathSelector ;
                            rdf:value "Page 18" ] ;
                    ns1:oahasStartSelector [ a ns1:oaXPathSelector ;
                            rdf:value "Page 17" ] ] ;
            ns1:oahasSource ns4:Industrial_Internet_of_Things_Volume_G4_Security_Framework ] .

ns4:IIRASecurityAnno a owl:NamedIndividual,
        ns1:oaAnnotation ;
    ns1:oahasBody ns4:IIRASecurity ;
    ns1:oahasTarget [ a ns1:oaSpecificResource ;
            ns2:format "pdf" ;
            ns1:oahasSelector [ a ns1:oaRangeSelector ;
                    ns1:oahasEndSelector [ a ns1:oaXPathSelector ;
                            rdf:value "Page 121" ] ;
                    ns1:oahasStartSelector [ a ns1:oaXPathSelector ;
                            rdf:value "Page 11" ] ] ;
            ns1:oahasSource ns4:Industrial_Internet_of_Things_Volume_G4_Security_Framework ],
        [ a ns1:oaSpecificResource ;
            ns2:format "pdf" ;
            ns1:oahasSelector [ a ns1:oaRangeSelector ;
                    ns1:oahasEndSelector [ a ns1:oaXPathSelector ;
                            rdf:value "Page 121" ] ;
                    ns1:oahasStartSelector [ a ns1:oaXPathSelector ;
                            rdf:value "Page 11" ] ] ;
            ns1:oahasSource ns4:Industrial_Internet_of_Things_Volume_G4_Security_Framework ] .

ns4:IIRASecurityFrameworkAnno a owl:NamedIndividual,
        ns1:oaAnnotation ;
    ns1:oahasBody ns4:IIRASecurityFramework ;
    ns1:oahasTarget [ a ns1:oaSpecificResource ;
            ns2:format "pdf" ;
            ns1:oahasSelector [ a ns1:oaRangeSelector ;
                    ns1:oahasEndSelector [ a ns1:oaXPathSelector ;
                            rdf:value "Page 121" ] ;
                    ns1:oahasStartSelector [ a ns1:oaXPathSelector ;
                            rdf:value "Page 11" ] ] ;
            ns1:oahasSource ns4:Industrial_Internet_of_Things_Volume_G4_Security_Framework ],
        [ a ns1:oaSpecificResource ;
            ns2:format "pdf" ;
            ns1:oahasSelector [ a ns1:oaRangeSelector ;
                    ns1:oahasEndSelector [ a ns1:oaXPathSelector ;
                            rdf:value "Page 121" ] ;
                    ns1:oahasStartSelector [ a ns1:oaXPathSelector ;
                            rdf:value "Page 11" ] ] ;
            ns1:oahasSource ns4:Industrial_Internet_of_Things_Volume_G4_Security_Framework ],
        [ a ns1:oaSpecificResource ;
            ns2:format "pdf" ;
            ns1:oahasSelector [ a ns1:oaRangeSelector ;
                    ns1:oahasEndSelector [ a ns1:oaXPathSelector ;
                            rdf:value "Page 121" ] ;
                    ns1:oahasStartSelector [ a ns1:oaXPathSelector ;
                            rdf:value "Page 11" ] ] ;
            ns1:oahasSource ns4:Industrial_Internet_of_Things_Volume_G4_Security_Framework ],
        [ a ns1:oaSpecificResource ;
            ns2:format "pdf" ;
            ns1:oahasSelector [ a ns1:oaRangeSelector ;
                    ns1:oahasEndSelector [ a ns1:oaXPathSelector ;
                            rdf:value "Page 121" ] ;
                    ns1:oahasStartSelector [ a ns1:oaXPathSelector ;
                            rdf:value "Page 11" ] ] ;
            ns1:oahasSource ns4:Industrial_Internet_of_Things_Volume_G4_Security_Framework ] .

ns4:IIRAUsageViewpointAnno a owl:NamedIndividual,
        ns1:oaAnnotation ;
    ns1:oahasBody ns4:IIRAUsageViewpoint ;
    ns1:oahasTarget [ a ns1:oaSpecificResource ;
            ns2:format "pdf" ;
            ns1:oahasSelector [ a ns1:oaRangeSelector ;
                    ns1:oahasEndSelector [ a ns1:oaXPathSelector ;
                            rdf:value "Page 25" ] ;
                    ns1:oahasStartSelector [ a ns1:oaXPathSelector ;
                            rdf:value "Page 22" ] ] ;
            ns1:oahasSource ns4:The_Industrial_Internet_of_Things_Volume_G1_Reference_Architecture ],
        [ a ns1:oaSpecificResource ;
            ns2:format "pdf" ;
            ns1:oahasSelector [ a ns1:oaRangeSelector ;
                    ns1:oahasEndSelector [ a ns1:oaXPathSelector ;
                            rdf:value "Page 25" ] ;
                    ns1:oahasStartSelector [ a ns1:oaXPathSelector ;
                            rdf:value "Page 22" ] ] ;
            ns1:oahasSource ns4:The_Industrial_Internet_of_Things_Volume_G1_Reference_Architecture ] .

ns4:IIRC a owl:NamedIndividual,
        ns4:StandardizationFramework ;
    rdfs:label "IICF"@en ;
    rdfs:comment "Industrial Internet Connectivity Framework"@en ;
    rdfs:isDefinedBy <https://www.iiconsortium.org/IICF.htm> ;
    rdfs:seeAlso <https://www.iiconsortium.org/pdf/IIC_PUB_G5_V1.01_PB_20180228.pdf> .

ns4:IPSO a owl:NamedIndividual,
        ns8:Organization,
        ns4:IIoTConsortium ;
    rdfs:label "IPSO"@en ;
    ns2:creator ns4:sebastian ;
    rdfs:comment "The Alliance is a global non-profit organization serving the various communities seeking to establish the Internet Protocol as the network for the connection of Smart Objects by providing coordinated marketing efforts available to the general public. (source: https://www.postscapes.com/internet-of-things-protocols/)"@en ;
    ns4:hasOfficialResource <http://www.ipso-alliance.org/> .

ns4:ISO_13485 a owl:NamedIndividual,
        ns4:Standard ;
    ns5:hasTargetConcern ns4:QualityOfService .

ns4:ISO_13849 a owl:NamedIndividual,
        ns4:Standard ;
    ns4:hasClassification ns4:IDSRAMCertification,
        ns4:IIRASecurity ;
    ns5:hasTargetConcern ns4:Safety .

ns4:ISO_19941 a owl:NamedIndividual,
        ns4:Standard ;
    ns5:hasTargetConcern ns4:CloudComputing .

ns4:ISO_20140_P1 a owl:NamedIndividual,
        ns4:Standard ;
    ns5:frames ns4:EnergyEfficiency .

ns4:ISO_29115 a owl:NamedIndividual,
        ns4:Standard ;
    rdfs:label "ISO/IEC 29115"@en ;
    ns5:hasTargetConcern ns4:Authentication,
        ns4:Identification .

ns4:ISO_50001 a owl:NamedIndividual,
        ns4:Standard ;
    rdfs:label "ISO 50001"@en ;
    ns5:hasTargetConcern ns4:Energy_management .

ns4:ISO_9000 a owl:NamedIndividual,
        ns4:Standard ;
    rdfs:label "ISO 9000"@en ;
    ns4:hasClassification ns4:CrossLevel,
        ns4:IDSRAMCertification ;
    ns5:hasTargetConcern ns4:QualityOfService .

ns4:ISO_9594-8 a owl:NamedIndividual,
        ns4:Standard ;
    rdfs:label "ISO/IEC 9594-8"@en ;
    ns4:hasClassification ns4:DataSovereignty,
        ns4:IDSRAMCertification,
        ns4:IDSRAMSecurity .

ns4:ITManager rdfs:label "IT Manager"@en ;
    rdfs:comment " An IT manager is responsible for the functioning of the IT services of an organisation." ;
    rdfs:seeAlso "IIC:PUB:G1:V1.80:20170131" ;
    ns6:note "Publications referred: 'IIC:PUB:G1:V1.80:20170131' '1.5 AUDIENCE' 'Page 7' " ;
    ns4:hasWikipediaArticle <https://en.wikipedia.org/wiki/Information_technology_management#IT_managers> .

ns4:IicfConnectivityLayerAnno a owl:NamedIndividual,
        ns1:oaAnnotation ;
    ns1:oahasBody ns4:IicfConnectivityLayer ;
    ns1:oahasTarget [ a ns1:oaSpecificResource ;
            ns2:format "pdf" ;
            ns1:oahasSelector [ a ns1:oaRangeSelector ;
                    ns1:oahasEndSelector [ a ns1:oaXPathSelector ;
                            rdf:value "Page 17" ] ;
                    ns1:oahasStartSelector [ a ns1:oaXPathSelector ;
                            rdf:value "Page 14" ] ] ;
            ns1:oahasSource ns4:The_Industrial_Internet_of_Things_Volume_G5_Connectivity_Framework ],
        [ a ns1:oaSpecificResource ;
            ns2:format "pdf" ;
            ns1:oahasSelector [ a ns1:oaRangeSelector ;
                    ns1:oahasEndSelector [ a ns1:oaXPathSelector ;
                            rdf:value "Page 17" ] ;
                    ns1:oahasStartSelector [ a ns1:oaXPathSelector ;
                            rdf:value "Page 14" ] ] ;
            ns1:oahasSource ns4:The_Industrial_Internet_of_Things_Volume_G5_Connectivity_Framework ] .

ns4:IndustrialDataSpace a owl:NamedIndividual,
        ns4:StandardizationFramework .

ns4:InformationSecurity a owl:NamedIndividual,
        ns4:Concern ;
    rdfs:label "Information Security"@en ;
    ns2:creator ns4:SebastianBader ;
    rdfs:comment ""@en ;
    rdfs:seeAlso <https://ieeexplore.ieee.org/document/8552311> ;
    ns5:supports ns4:Security .

ns4:Information_Privacy a owl:NamedIndividual,
        ns4:Concern ;
    rdfs:label "Information Privacy"@en ;
    ns2:creator ns4:MuhammadUsman ;
    rdfs:comment """The IoT utilizes different sort of object distinguishing proof advancements, e.g., RFID, 2D-standardized tags and so forth. Since each kind of day by day use articles
will convey these recognizable proof labels and insert the particular object data, it is important to take legal protection measures and prevent unauthorized access."""@en ;
    rdfs:seeAlso <https://ieeexplore.ieee.org/document/6188257> ;
    ns4:hasWikipediaArticle <https://en.wikipedia.org/wiki/Information_privacy> ;
    ns5:supports ns4:Privacy .

ns4:InterfaceNetworksDevicesAnno a owl:NamedIndividual,
        ns1:oaAnnotation ;
    ns1:oahasBody ns4:InterfaceNetworksDevices ;
    ns1:oahasTarget [ a ns1:oaSpecificResource ;
            ns1:oahasSource <https://forge.fiware.org/plugins/mediawiki/wiki/fiware/index.php/Interface_to_Networks_and_Devices_(I2ND)_Architecture_R3> ],
        [ a ns1:oaSpecificResource ;
            ns1:oahasSource <https://forge.fiware.org/plugins/mediawiki/wiki/fiware/index.php/Interface_to_Networks_and_Devices_(I2ND)_Architecture_R3> ] .

ns4:IoTivity a owl:NamedIndividual,
        ns8:Document,
        ns4:Publication,
        ns4:TechnicalSpecification ;
    rdfs:label "IoTivity"@en ;
    ns2:creator ns4:sebastian ;
    rdfs:comment "IoTivity is an open source project hosted by the Linux Foundation, and sponsored by the OIC. (source: https://www.postscapes.com/internet-of-things-protocols/)"@en ;
    ns4:hasOfficialResource <https://www.iotivity.org/> .

ns4:IotaAvailabilityResilienceAnno a owl:NamedIndividual,
        ns1:oaAnnotation ;
    ns1:oahasBody ns4:IotaAvailabilityResilience ;
    ns1:oahasTarget [ a ns1:oaSpecificResource ;
            ns2:format "pdf" ;
            ns1:oahasSelector [ a ns1:oaRangeSelector ;
                    ns1:oahasEndSelector [ a ns1:oaXPathSelector ;
                            rdf:value "Page 156" ] ;
                    ns1:oahasStartSelector [ a ns1:oaXPathSelector ;
                            rdf:value "Page 155" ] ] ;
            ns1:oahasSource ns4:Final_architectural_reference_model_for_the_IoT_v3_0 ],
        [ a ns1:oaSpecificResource ;
            ns2:format "pdf" ;
            ns1:oahasSelector [ a ns1:oaRangeSelector ;
                    ns1:oahasEndSelector [ a ns1:oaXPathSelector ;
                            rdf:value "Page 156" ] ;
                    ns1:oahasStartSelector [ a ns1:oaXPathSelector ;
                            rdf:value "Page 155" ] ] ;
            ns1:oahasSource ns4:Final_architectural_reference_model_for_the_IoT_v3_0 ] .

ns4:IotaDeploymentOperationViewpointAnno a owl:NamedIndividual,
        ns1:oaAnnotation ;
    ns1:oahasBody ns4:IotaDeploymentOperationViewpoint ;
    ns1:oahasTarget [ a ns1:oaSpecificResource ;
            ns2:format "pdf" ;
            ns1:oahasSelector [ a ns1:oaRangeSelector ;
                    ns1:oahasEndSelector [ a ns1:oaXPathSelector ;
                            rdf:value "Page 149" ] ;
                    ns1:oahasStartSelector [ a ns1:oaXPathSelector ;
                            rdf:value "Page 141" ] ] ;
            ns1:oahasSource ns4:Final_architectural_reference_model_for_the_IoT_v3_0 ],
        [ a ns1:oaSpecificResource ;
            ns2:format "pdf" ;
            ns1:oahasSelector [ a ns1:oaRangeSelector ;
                    ns1:oahasEndSelector [ a ns1:oaXPathSelector ;
                            rdf:value "Page 149" ] ;
                    ns1:oahasStartSelector [ a ns1:oaXPathSelector ;
                            rdf:value "Page 141" ] ] ;
            ns1:oahasSource ns4:Final_architectural_reference_model_for_the_IoT_v3_0 ] .

ns4:IotaEvolutionInteroperabilityAnno a owl:NamedIndividual,
        ns1:oaAnnotation ;
    ns1:oahasBody ns4:IotaEvolutionInteroperability ;
    ns1:oahasTarget [ a ns1:oaSpecificResource ;
            ns2:format "pdf" ;
            ns1:oahasSelector [ a ns1:oaRangeSelector ;
                    ns1:oahasEndSelector [ a ns1:oaXPathSelector ;
                            rdf:value "Page 151" ] ;
                    ns1:oahasStartSelector [ a ns1:oaXPathSelector ;
                            rdf:value "Page 150" ] ] ;
            ns1:oahasSource ns4:Final_architectural_reference_model_for_the_IoT_v3_0 ],
        [ a ns1:oaSpecificResource ;
            ns2:format "pdf" ;
            ns1:oahasSelector [ a ns1:oaRangeSelector ;
                    ns1:oahasEndSelector [ a ns1:oaXPathSelector ;
                            rdf:value "Page 151" ] ;
                    ns1:oahasStartSelector [ a ns1:oaXPathSelector ;
                            rdf:value "Page 150" ] ] ;
            ns1:oahasSource ns4:Final_architectural_reference_model_for_the_IoT_v3_0 ] .

ns4:IotaFunctionalViewpointAnno a owl:NamedIndividual,
        ns1:oaAnnotation ;
    ns1:oahasBody ns4:IotaFunctionalViewpoint ;
    ns1:oahasTarget [ a ns1:oaSpecificResource ;
            ns2:format "pdf" ;
            ns1:oahasSelector [ a ns1:oaRangeSelector ;
                    ns1:oahasEndSelector [ a ns1:oaXPathSelector ;
                            rdf:value "Page 126" ] ;
                    ns1:oahasStartSelector [ a ns1:oaXPathSelector ;
                            rdf:value "Page 105" ] ] ;
            ns1:oahasSource ns4:Final_architectural_reference_model_for_the_IoT_v3_0 ],
        [ a ns1:oaSpecificResource ;
            ns2:format "pdf" ;
            ns1:oahasSelector [ a ns1:oaRangeSelector ;
                    ns1:oahasEndSelector [ a ns1:oaXPathSelector ;
                            rdf:value "Page 126" ] ;
                    ns1:oahasStartSelector [ a ns1:oaXPathSelector ;
                            rdf:value "Page 105" ] ] ;
            ns1:oahasSource ns4:Final_architectural_reference_model_for_the_IoT_v3_0 ] .

ns4:IotaInformationViewpointAnno a owl:NamedIndividual,
        ns1:oaAnnotation ;
    ns1:oahasBody ns4:IotaInformationViewpoint ;
    ns1:oahasTarget [ a ns1:oaSpecificResource ;
            ns2:format "pdf" ;
            ns1:oahasSelector [ a ns1:oaRangeSelector ;
                    ns1:oahasEndSelector [ a ns1:oaXPathSelector ;
                            rdf:value "Page 141" ] ;
                    ns1:oahasStartSelector [ a ns1:oaXPathSelector ;
                            rdf:value "Page 126" ] ] ;
            ns1:oahasSource ns4:Final_architectural_reference_model_for_the_IoT_v3_0 ],
        [ a ns1:oaSpecificResource ;
            ns2:format "pdf" ;
            ns1:oahasSelector [ a ns1:oaRangeSelector ;
                    ns1:oahasEndSelector [ a ns1:oaXPathSelector ;
                            rdf:value "Page 141" ] ;
                    ns1:oahasStartSelector [ a ns1:oaXPathSelector ;
                            rdf:value "Page 126" ] ] ;
            ns1:oahasSource ns4:Final_architectural_reference_model_for_the_IoT_v3_0 ] .

ns4:IotaPerformanceScalabilityAnno a owl:NamedIndividual,
        ns1:oaAnnotation ;
    ns1:oahasBody ns4:IotaPerformanceScalability ;
    ns1:oahasTarget [ a ns1:oaSpecificResource ;
            ns2:format "pdf" ;
            ns1:oahasSelector [ a ns1:oaRangeSelector ;
                    ns1:oahasEndSelector [ a ns1:oaXPathSelector ;
                            rdf:value "Page 152" ] ;
                    ns1:oahasStartSelector [ a ns1:oaXPathSelector ;
                            rdf:value "Page 151" ] ] ;
            ns1:oahasSource ns4:Final_architectural_reference_model_for_the_IoT_v3_0 ],
        [ a ns1:oaSpecificResource ;
            ns2:format "pdf" ;
            ns1:oahasSelector [ a ns1:oaRangeSelector ;
                    ns1:oahasEndSelector [ a ns1:oaXPathSelector ;
                            rdf:value "Page 152" ] ;
                    ns1:oahasStartSelector [ a ns1:oaXPathSelector ;
                            rdf:value "Page 151" ] ] ;
            ns1:oahasSource ns4:Final_architectural_reference_model_for_the_IoT_v3_0 ] .

ns4:IotaPerspectiveAnno a owl:NamedIndividual,
        ns1:oaAnnotation ;
    ns1:oahasBody ns4:IotaPerspective ;
    ns1:oahasTarget [ a ns1:oaSpecificResource ;
            ns2:format "pdf" ;
            ns1:oahasSelector [ a ns1:oaRangeSelector ;
                    ns1:oahasEndSelector [ a ns1:oaXPathSelector ;
                            rdf:value "Page 156" ] ;
                    ns1:oahasStartSelector [ a ns1:oaXPathSelector ;
                            rdf:value "Page 149" ] ] ;
            ns1:oahasSource ns4:Final_architectural_reference_model_for_the_IoT_v3_0 ],
        [ a ns1:oaSpecificResource ;
            ns2:format "pdf" ;
            ns1:oahasSelector [ a ns1:oaRangeSelector ;
                    ns1:oahasEndSelector [ a ns1:oaXPathSelector ;
                            rdf:value "Page 156" ] ;
                    ns1:oahasStartSelector [ a ns1:oaXPathSelector ;
                            rdf:value "Page 149" ] ] ;
            ns1:oahasSource ns4:Final_architectural_reference_model_for_the_IoT_v3_0 ] .

ns4:IotaReferenceArchitectureAnno a owl:NamedIndividual,
        ns1:oaAnnotation ;
    ns1:oahasBody ns4:IotaReferenceArchitecture ;
    ns1:oahasTarget [ a ns1:oaSpecificResource ;
            ns2:format "pdf" ;
            ns1:oahasSelector [ a ns1:oaRangeSelector ;
                    ns1:oahasEndSelector [ a ns1:oaXPathSelector ;
                            rdf:value "Page 482" ] ;
                    ns1:oahasStartSelector [ a ns1:oaXPathSelector ;
                            rdf:value "Page 1" ] ] ;
            ns1:oahasSource ns4:Final_architectural_reference_model_for_the_IoT_v3_0 ],
        [ a ns1:oaSpecificResource ;
            ns2:format "pdf" ;
            ns1:oahasSelector [ a ns1:oaRangeSelector ;
                    ns1:oahasEndSelector [ a ns1:oaXPathSelector ;
                            rdf:value "Page 482" ] ;
                    ns1:oahasStartSelector [ a ns1:oaXPathSelector ;
                            rdf:value "Page 1" ] ] ;
            ns1:oahasSource ns4:Final_architectural_reference_model_for_the_IoT_v3_0 ] .

ns4:IotaTrustSecurityPrivacyAnno a owl:NamedIndividual,
        ns1:oaAnnotation ;
    ns1:oahasBody ns4:IotaTrustSecurityPrivacy ;
    ns1:oahasTarget [ a ns1:oaSpecificResource ;
            ns2:format "pdf" ;
            ns1:oahasSelector [ a ns1:oaRangeSelector ;
                    ns1:oahasEndSelector [ a ns1:oaXPathSelector ;
                            rdf:value "Page 155" ] ;
                    ns1:oahasStartSelector [ a ns1:oaXPathSelector ;
                            rdf:value "Page 152" ] ] ;
            ns1:oahasSource ns4:Final_architectural_reference_model_for_the_IoT_v3_0 ],
        [ a ns1:oaSpecificResource ;
            ns2:format "pdf" ;
            ns1:oahasSelector [ a ns1:oaRangeSelector ;
                    ns1:oahasEndSelector [ a ns1:oaXPathSelector ;
                            rdf:value "Page 155" ] ;
                    ns1:oahasStartSelector [ a ns1:oaXPathSelector ;
                            rdf:value "Page 152" ] ] ;
            ns1:oahasSource ns4:Final_architectural_reference_model_for_the_IoT_v3_0 ] .

ns4:IpsoAppFramework a owl:NamedIndividual,
        ns8:Document,
        ns4:Publication,
        ns4:TechnicalSpecification ;
    rdfs:label "IPSO App Framework"@en ;
    ns2:creator ns4:sebastian ;
    rdfs:comment "IPSO Application Framework (PDF): This design defines sets of REST interfaces that may be used by a smart object to represent its available resources, interact with other smart objects and backend services. This framework is designed to be complementary to existing Web profiles including SEP2 and oBIX. (source: https://www.postscapes.com/internet-of-things-protocols/)"@en ;
    ns4:hasOfficialResource <http://www.ipso-alliance.org/wp-content/media/draft-ipso-app-framework-04.pdf> .

ns4:IviActivityLayerAnno a owl:NamedIndividual,
        ns1:oaAnnotation ;
    ns1:oahasBody ns4:IviActivityLayer ;
    ns1:oahasTarget [ a ns1:oaSpecificResource ;
            ns2:format "pdf" ;
            ns1:oahasSelector [ a ns1:oaRangeSelector ;
                    ns1:oahasEndSelector [ a ns1:oaXPathSelector ;
                            rdf:value "Page 5" ] ;
                    ns1:oahasStartSelector [ a ns1:oaXPathSelector ;
                            rdf:value "Page 4" ] ] ;
            ns1:oahasSource ns4:Industrial_Value_Chain_Reference_Architecture_IVRA_Next ],
        [ a ns1:oaSpecificResource ;
            ns2:format "pdf" ;
            ns1:oahasSelector [ a ns1:oaRangeSelector ;
                    ns1:oahasEndSelector [ a ns1:oaXPathSelector ;
                            rdf:value "Page 6" ] ;
                    ns1:oahasStartSelector [ a ns1:oaXPathSelector ;
                            rdf:value "Page 5" ] ] ;
            ns1:oahasSource ns4:Industrial_Value_Chain_Reference_Architecture_IVRA_Next ] .

ns4:IviActivityViewAnno a owl:NamedIndividual,
        ns1:oaAnnotation ;
    ns1:oahasBody ns4:IviActivityView ;
    ns1:oahasTarget [ a ns1:oaSpecificResource ;
            ns2:format "pdf" ;
            ns1:oahasSelector [ a ns1:oaRangeSelector ;
                    ns1:oahasEndSelector [ a ns1:oaXPathSelector ;
                            rdf:value "Page 3" ] ;
                    ns1:oahasStartSelector [ a ns1:oaXPathSelector ;
                            rdf:value "Page 2" ] ] ;
            ns1:oahasSource ns4:Industrial_Value_Chain_Reference_Architecture_IVRA ],
        [ a ns1:oaSpecificResource ;
            ns2:format "pdf" ;
            ns1:oahasSelector [ a ns1:oaRangeSelector ;
                    ns1:oahasEndSelector [ a ns1:oaXPathSelector ;
                            rdf:value "Page 4" ] ;
                    ns1:oahasStartSelector [ a ns1:oaXPathSelector ;
                            rdf:value "Page 2" ] ] ;
            ns1:oahasSource ns4:Industrial_Value_Chain_Reference_Architecture_IVRA ] .

ns4:IviAssetViewAnno a owl:NamedIndividual,
        ns1:oaAnnotation ;
    ns1:oahasBody ns4:IviAssetView ;
    ns1:oahasTarget [ a ns1:oaSpecificResource ;
            ns2:format "pdf" ;
            ns1:oahasSelector [ a ns1:oaRangeSelector ;
                    ns1:oahasEndSelector [ a ns1:oaXPathSelector ;
                            rdf:value "Page 2" ] ;
                    ns1:oahasStartSelector [ a ns1:oaXPathSelector ;
                            rdf:value "Page 1" ] ] ;
            ns1:oahasSource ns4:Industrial_Value_Chain_Reference_Architecture_IVRA ],
        [ a ns1:oaSpecificResource ;
            ns2:format "pdf" ;
            ns1:oahasSelector [ a ns1:oaRangeSelector ;
                    ns1:oahasEndSelector [ a ns1:oaXPathSelector ;
                            rdf:value "Page 2" ] ;
                    ns1:oahasStartSelector [ a ns1:oaXPathSelector ;
                            rdf:value "Page 1" ] ] ;
            ns1:oahasSource ns4:Industrial_Value_Chain_Reference_Architecture_IVRA ] .

ns4:IviBusinessLayerAnno a owl:NamedIndividual,
        ns1:oaAnnotation ;
    ns1:oahasBody ns4:IviBusinessLayer ;
    ns1:oahasTarget [ a ns1:oaSpecificResource ;
            ns2:format "pdf" ;
            ns1:oahasSelector [ a ns1:oaRangeSelector ;
                    ns1:oahasEndSelector [ a ns1:oaXPathSelector ;
                            rdf:value "Page 5" ] ;
                    ns1:oahasStartSelector [ a ns1:oaXPathSelector ;
                            rdf:value "Page 4" ] ] ;
            ns1:oahasSource ns4:Industrial_Value_Chain_Reference_Architecture_IVRA_Next ],
        [ a ns1:oaSpecificResource ;
            ns2:format "pdf" ;
            ns1:oahasSelector [ a ns1:oaRangeSelector ;
                    ns1:oahasEndSelector [ a ns1:oaXPathSelector ;
                            rdf:value "Page 6" ] ;
                    ns1:oahasStartSelector [ a ns1:oaXPathSelector ;
                            rdf:value "Page 5" ] ] ;
            ns1:oahasSource ns4:Industrial_Value_Chain_Reference_Architecture_IVRA_Next ] .

ns4:IviManagementViewAnno a owl:NamedIndividual,
        ns1:oaAnnotation ;
    ns1:oahasBody ns4:IviManagementView ;
    ns1:oahasTarget [ a ns1:oaSpecificResource ;
            ns2:format "pdf" ;
            ns1:oahasSelector [ a ns1:oaRangeSelector ;
                    ns1:oahasEndSelector [ a ns1:oaXPathSelector ;
                            rdf:value "Page 4" ] ;
                    ns1:oahasStartSelector [ a ns1:oaXPathSelector ;
                            rdf:value "Page 3" ] ] ;
            ns1:oahasSource ns4:Industrial_Value_Chain_Reference_Architecture_IVRA ],
        [ a ns1:oaSpecificResource ;
            ns2:format "pdf" ;
            ns1:oahasSelector [ a ns1:oaRangeSelector ;
                    ns1:oahasEndSelector [ a ns1:oaXPathSelector ;
                            rdf:value "Page 4" ] ;
                    ns1:oahasStartSelector [ a ns1:oaXPathSelector ;
                            rdf:value "Page 3" ] ] ;
            ns1:oahasSource ns4:Industrial_Value_Chain_Reference_Architecture_IVRA ] .

ns4:IviSpecificationLayerAnno a owl:NamedIndividual,
        ns1:oaAnnotation ;
    ns1:oahasBody ns4:IviSpecificationLayer ;
    ns1:oahasTarget [ a ns1:oaSpecificResource ;
            ns2:format "pdf" ;
            ns1:oahasSelector [ a ns1:oaRangeSelector ;
                    ns1:oahasEndSelector [ a ns1:oaXPathSelector ;
                            rdf:value "Page 5" ] ;
                    ns1:oahasStartSelector [ a ns1:oaXPathSelector ;
                            rdf:value "Page 4" ] ] ;
            ns1:oahasSource ns4:Industrial_Value_Chain_Reference_Architecture_IVRA_Next ],
        [ a ns1:oaSpecificResource ;
            ns2:format "pdf" ;
            ns1:oahasSelector [ a ns1:oaRangeSelector ;
                    ns1:oahasEndSelector [ a ns1:oaXPathSelector ;
                            rdf:value "Page 6" ] ;
                    ns1:oahasStartSelector [ a ns1:oaXPathSelector ;
                            rdf:value "Page 5" ] ] ;
            ns1:oahasSource ns4:Industrial_Value_Chain_Reference_Architecture_IVRA_Next ] .

ns4:JMS a owl:NamedIndividual,
        ns8:Document,
        ns4:Publication,
        ns4:TechnicalSpecification ;
    rdfs:label "JMS"@en ;
    ns2:creator ns4:sebastian ;
    rdfs:comment "JMS (Java Message Service) - A Java Message Oriented Middleware (MOM) API for sending messages between two or more clients. (source: https://www.postscapes.com/internet-of-things-protocols/)"@en .

ns4:Jurisdictional_Issues a owl:NamedIndividual,
        ns4:Concern ;
    rdfs:label "Jurisdictional Issues"@en ;
    ns2:creator ns4:MuhammadUsman ;
    rdfs:comment "It is often challenging to alter resources, for example, the server or data centres to a particular geographic area. Load balancing service provider of the cloud, the availability of the network, or the performance of the data centre are few factors that determine where the data is stored. Accordingly, an organization data might be stored in a different location with various legal jurisdictions and diverse laws concerning the security issues, such as the protection and interruptions of the data"@en ;
    rdfs:seeAlso <https://dl.acm.org/citation.cfm?doid=3108421.3108426> ;
    ns4:hasWikipediaArticle <https://en.wikipedia.org/wiki/Jurisdiction> ;
    ns5:supports ns4:CloudComputing .

ns4:KeyRock a owl:NamedIndividual,
        ns8:Document,
        ns4:Publication,
        ns4:TechnicalSpecification ;
    ns3:associatedWith ns4:FiwareDataContextManagement,
        ns4:FiwareSecurity ;
    ns5:hasTargetConcern ns4:IdentityManagement .

ns4:LatencyReduction a owl:NamedIndividual,
        ns4:Concern ;
    rdfs:label "LatencyReduction"@en ;
    ns2:creator ns4:MuhammadUsman ;
    rdfs:comment "Latency is a time interval between the stimulation and response, or, from a more general point of view, a time delay between the cause and the effect of some physical change in the system being observed."@en ;
    rdfs:seeAlso <https://ieeexplore.ieee.org/document/7488250> ;
    ns4:hasWikipediaArticle <https://en.wikipedia.org/wiki/Latency_(engineering)> ;
    ns5:supports ns4:Communication .

ns4:Layer a owl:Class ;
    rdfs:label "Layer"@en ;
    rdfs:comment "Describes the layers of the standardization frameworks. In some cases, the layers are connected to dimensions of the frameworks. "@en .

ns4:LoWPAN a owl:NamedIndividual,
        ns8:Document,
        ns4:Publication,
        ns4:TechnicalSpecification ;
    rdfs:label "6LoWPAN"@en ;
    ns2:creator ns4:IETF,
        ns4:sebastian ;
    rdfs:comment "6LoWPAN is an acronym of IPv6 over Low power Wireless Personal Area Networks. It is an adaption layer for IPv6 over IEEE802.15.4 links. This protocol operates only in the 2.4 GHz frequency range with 250 kbps transfer rate. (source: https://www.postscapes.com/internet-of-things-protocols/)"@en ;
    ns8:maker ns4:IETF ;
    ns4:hasClassification ns4:IIRAConnectivity,
        ns4:RAMICommunicationlayer ;
    ns4:hasDBpediaResource <http://dbpedia.org/resource/6LoWPAN> ;
    ns4:hasDeveloper ns4:IETF ;
    ns4:hasPublisher ns4:IETF ;
    ns4:hasWikipediaArticle <https://en.wikipedia.org/wiki/6LoWPAN> ;
    ns5:hasTargetConcern ns4:Communication .

ns4:LocalDataConfidentiality a owl:NamedIndividual,
        ns4:Concern ;
    rdfs:label "Local Data Confidentiality"@en ;
    ns2:creator ns4:sebastian ;
    rdfs:comment "Describes the means by which local data is protected."@en .

ns4:Logging a owl:NamedIndividual,
        ns4:Concern ;
    rdfs:label "Logging"@en ;
    rdfs:comment "The process of recording incidents and events regarding a specific service, data resource or device in order to make status changes transparent."@en ;
    rdfs:seeAlso "IoT-A Requirement UNI.409",
        "IoT-A Requirement UNI.710" ;
    ns4:hasDBpediaResource <http://dbpedia.org/resource/Data_logger> ;
    ns5:supports ns4:DataUsageControl,
        ns4:ServiceAccessControl .

ns4:Long_Term_Business_Sustainability a owl:NamedIndividual,
        ns4:Concern ;
    rdfs:label "Long Term Business Sustainability"@en ;
    ns2:creator ns4:MuhammadUsman ;
    rdfs:comment "The provider should not go broke, be financially in a close-fitting corner or close down the business. Organizations should be sure and know how to move your data to another cloud provider. And should know how to have a backup at another public cloud of data for redundancy"@en ;
    rdfs:seeAlso <https://dl.acm.org/citation.cfm?doid=3286606.3286865> ;
    ns4:hasWikipediaArticle <https://en.wikipedia.org/wiki/Sustainability> ;
    ns5:supports ns4:BusinessContext .

ns4:LowPowerWiFi a owl:NamedIndividual,
        ns8:Document,
        ns4:Publication,
        ns4:TechnicalSpecification .

ns4:MessagePriority a owl:NamedIndividual,
        ns4:Concern ;
    rdfs:label "Message precedence"@en ;
    ns7:hasStakeholder <https://www.wikidata.org/wiki/Q1548249>,
        <owl:Developer> ;
    rdfs:comment "Message precedence is an indicator attached to a message indicating its level of urgency. (source: wikipedia)"@en ;
    rdfs:seeAlso "IoT-A Requirement UNI.028" ;
    ns4:hasDBpediaResource <http://dbpedia.org/resource/Message_precedence> ;
    ns5:supports ns4:Communication .

ns4:MobilDevices a owl:NamedIndividual,
        ns4:Concern ;
    rdfs:label "Mobil Devices"@en ;
    ns2:creator ns4:MuhammadUsman ;
    rdfs:comment """How to handle the massive mobility of vehicles? In the case of an application scenario that involves connected vehicles, mobility is a major issue and includes data consumer as well as data producer. In this particular case, one of the influencing factors is the potential speed of a vehicle. High-speed mobility may
lead to situations in which a request for data or a service may not be answered before the vehicle disconnects and re-connects to another network entry point. This leads to unfulfilled requests and potential duplication of efforts."""@en ;
    rdfs:seeAlso <https://dl.acm.org/citation.cfm?doid=3098208.3098210>,
        <https://en.wikipedia.org/wiki/Connected_car>,
        <https://ieeexplore.ieee.org/document/6188257> ;
    ns5:supports ns4:IoT .

ns4:Multicast rdfs:seeAlso "IoT-A Requirement UNI.302",
        "IoT-A Requirement UNI.303",
        "IoT-A Requirement UNI.304",
        "IoT-A Requirement UNI.305" .

ns4:MultipleIdenities rdfs:seeAlso "IoT-A Requirement UNI.320" .

ns4:MultipleIdentities a owl:NamedIndividual,
        ns4:Concern ;
    rdfs:label "Multiple Identities"@en ;
    ns2:creator ns4:sebastian ;
    rdfs:comment "Devices must be able to switch between different networks without losing connections (Network handover/handoff support)."@en ;
    rdfs:seeAlso "UNI.320"@en ;
    ns5:supports ns4:IdentityManagement .

ns4:NGSI a owl:NamedIndividual,
        ns8:Document,
        ns4:Publication,
        ns4:TechnicalSpecification ;
    rdfs:label "NGSI"@en ;
    ns2:creator ns4:FIWARE,
        ns4:sebastian ;
    ns2:title "Next Generation Service Interface"@en ;
    rdfs:comment """The FIWARE NGSI (Next Generation Service Interface) API defines
-    a data model for context information, based on a simple information model using the notion of context entities
-    a context data interface for exchanging information by means of query, subscription, and update operations
-    a context availability interface for exchanging information on how to obtain context information (whether to separate the two interfaces is currently under discussion)."""@en ;
    ns8:maker ns4:FIWARE ;
    ns4:hasOfficialResource <http://fiware.github.io/specifications/ngsiv2/stable/> ;
    ns4:hasPublisher ns4:FIWARE .

ns4:NetworkSecurity a owl:NamedIndividual,
        ns4:Concern ;
    rdfs:label "network security"@en ;
    ns2:creator ns4:SebastianBader ;
    rdfs:comment """Data flow is an integral part of any cloud service over the network of computers or
clusters of systems using internet. Any intruder can analyze the data packet to detect any weakness in the system and can gain access to applications and data
using some kind of remote access mechanism and injection like SQL and some bad command, Denial of Service (DoS), Distributed DoS (DDoS), man in the
middle attacks, social networking attacks and some unauthorized attacks are the major entrance level attacks in cloud computing environment."""@en ;
    rdfs:seeAlso <https://ieeexplore.ieee.org/document/6188257>,
        <https://ieeexplore.ieee.org/document/8249113>,
        <https://ieeexplore.ieee.org/document/8552311> ;
    ns4:hasWikipediaArticle <https://en.wikipedia.org/wiki/Audit>,
        <https://en.wikipedia.org/wiki/Network_security> ;
    ns5:supports ns4:Security .

ns4:NetworkVirtualization a owl:NamedIndividual,
        ns4:Concern ;
    rdfs:label "Network Virtualization"@en ;
    ns2:creator ns4:sebastian ;
    rdfs:comment "The system shall support network virtualisation, i.e. the usage of virtual overlay networks."@en ;
    rdfs:seeAlso "IoT-A Requirement UNI.328",
        "UNI.328"@en ;
    ns4:hasWikipediaArticle <https://en.wikipedia.org/wiki/Network_virtualization> ;
    ns5:supports ns4:Communication .

ns4:ODRL a owl:NamedIndividual,
        ns8:Document,
        ns4:Publication,
        ns4:Standard ;
    rdfs:label "ODRL"@en,
        "Open Digital Rights Language"@en ;
    ns2:creator ns4:W3C ;
    rdfs:comment """The Open Digital Rights Language (ODRL) is a policy expression language that provides a flexible and interoperable information model, vocabulary, and encoding mechanisms for representing statements about the usage of content and services. The ODRL Information Model describes the underlying concepts, entities, and relationships that form the foundational basis for the semantics of the ODRL policies.
Policies are used to represent permitted and prohibited actions over a certain asset, as well as the obligations required to be meet by stakeholders. In addition, policies may be limited by constraints (e.g., temporal or spatial constraints) and duties (e.g. payments) may be imposed on permissions."""@en ;
    ns8:maker ns4:W3C ;
    ns4:hasClassification ns4:IDSRAMInformationLayer,
        ns4:IDSRAMSecurity ;
    ns4:hasOfficialResource <https://www.w3.org/TR/odrl-model/> ;
    ns4:hasPublisher ns4:W3C .

ns4:OFRAAgilityPillarAnno a owl:NamedIndividual,
        ns1:oaAnnotation ;
    ns1:oahasBody ns4:OFRAAgilityPillar ;
    ns1:oahasTarget [ a ns1:oaSpecificResource ;
            ns2:format "pdf" ;
            ns1:oahasSelector [ a ns1:oaRangeSelector ;
                    ns1:oahasEndSelector [ a ns1:oaXPathSelector ;
                            rdf:value "Page 32" ] ;
                    ns1:oahasStartSelector [ a ns1:oaXPathSelector ;
                            rdf:value "Page 31" ] ] ;
            ns1:oahasSource ns4:OpenFog_Reference_Architecture_for_Fog_Computing ],
        [ a ns1:oaSpecificResource ;
            ns2:format "pdf" ;
            ns1:oahasSelector [ a ns1:oaRangeSelector ;
                    ns1:oahasEndSelector [ a ns1:oaXPathSelector ;
                            rdf:value "Page 32" ] ;
                    ns1:oahasStartSelector [ a ns1:oaXPathSelector ;
                            rdf:value "Page 31" ] ] ;
            ns1:oahasSource ns4:OpenFog_Reference_Architecture_for_Fog_Computing ] .

ns4:OFRAAutonomyPillarAnno a owl:NamedIndividual,
        ns1:oaAnnotation ;
    ns1:oahasBody ns4:OFRAAutonomyPillar ;
    ns1:oahasTarget [ a ns1:oaSpecificResource ;
            ns2:format "pdf" ;
            ns1:oahasSelector [ a ns1:oaRangeSelector ;
                    ns1:oahasEndSelector [ a ns1:oaXPathSelector ;
                            rdf:value "Page 29" ] ;
                    ns1:oahasStartSelector [ a ns1:oaXPathSelector ;
                            rdf:value "Page 27" ] ] ;
            ns1:oahasSource ns4:OpenFog_Reference_Architecture_for_Fog_Computing ],
        [ a ns1:oaSpecificResource ;
            ns2:format "pdf" ;
            ns1:oahasSelector [ a ns1:oaRangeSelector ;
                    ns1:oahasEndSelector [ a ns1:oaXPathSelector ;
                            rdf:value "Page 29" ] ;
                    ns1:oahasStartSelector [ a ns1:oaXPathSelector ;
                            rdf:value "Page 27" ] ] ;
            ns1:oahasSource ns4:OpenFog_Reference_Architecture_for_Fog_Computing ] .

ns4:OFRADataAnalyticsAndControlPerspectiveAnno a owl:NamedIndividual,
        ns1:oaAnnotation ;
    ns1:oahasBody ns4:OFRADataAnalyticsAndControlPerspective ;
    ns1:oahasTarget [ a ns1:oaSpecificResource ;
            ns2:format "pdf" ;
            ns1:oahasSelector [ a ns1:oaRangeSelector ;
                    ns1:oahasEndSelector [ a ns1:oaXPathSelector ;
                            rdf:value "Page 56" ] ;
                    ns1:oahasStartSelector [ a ns1:oaXPathSelector ;
                            rdf:value "Page 54" ] ] ;
            ns1:oahasSource ns4:OpenFog_Reference_Architecture_for_Fog_Computing ],
        [ a ns1:oaSpecificResource ;
            ns2:format "pdf" ;
            ns1:oahasSelector [ a ns1:oaRangeSelector ;
                    ns1:oahasEndSelector [ a ns1:oaXPathSelector ;
                            rdf:value "Page 56" ] ;
                    ns1:oahasStartSelector [ a ns1:oaXPathSelector ;
                            rdf:value "Page 54" ] ] ;
            ns1:oahasSource ns4:OpenFog_Reference_Architecture_for_Fog_Computing ] .

ns4:OFRADeploymentViewpointAnno a owl:NamedIndividual,
        ns1:oaAnnotation ;
    ns1:oahasBody ns4:OFRADeploymentViewpoint ;
    ns1:oahasTarget [ a ns1:oaSpecificResource ;
            ns2:format "pdf" ;
            ns1:oahasSelector [ a ns1:oaRangeSelector ;
                    ns1:oahasEndSelector [ a ns1:oaXPathSelector ;
                            rdf:value "Page 40" ] ;
                    ns1:oahasStartSelector [ a ns1:oaXPathSelector ;
                            rdf:value "Page 39" ] ] ;
            ns1:oahasSource ns4:OpenFog_Reference_Architecture_for_Fog_Computing ],
        [ a ns1:oaSpecificResource ;
            ns2:format "pdf" ;
            ns1:oahasSelector [ a ns1:oaRangeSelector ;
                    ns1:oahasEndSelector [ a ns1:oaXPathSelector ;
                            rdf:value "Page 40" ] ;
                    ns1:oahasStartSelector [ a ns1:oaXPathSelector ;
                            rdf:value "Page 39" ] ] ;
            ns1:oahasSource ns4:OpenFog_Reference_Architecture_for_Fog_Computing ] .

ns4:OFRAFunctionalViewpointAnno a owl:NamedIndividual,
        ns1:oaAnnotation ;
    ns1:oahasBody ns4:OFRAFunctionalViewpoint ;
    ns1:oahasTarget [ a ns1:oaSpecificResource ;
            ns2:format "pdf" ;
            ns1:oahasSelector [ a ns1:oaRangeSelector ;
                    ns1:oahasEndSelector [ a ns1:oaXPathSelector ;
                            rdf:value "Page 39" ] ;
                    ns1:oahasStartSelector [ a ns1:oaXPathSelector ;
                            rdf:value "Page 38" ] ] ;
            ns1:oahasSource ns4:OpenFog_Reference_Architecture_for_Fog_Computing ],
        [ a ns1:oaSpecificResource ;
            ns2:format "pdf" ;
            ns1:oahasSelector [ a ns1:oaRangeSelector ;
                    ns1:oahasEndSelector [ a ns1:oaXPathSelector ;
                            rdf:value "Page 39" ] ;
                    ns1:oahasStartSelector [ a ns1:oaXPathSelector ;
                            rdf:value "Page 38" ] ] ;
            ns1:oahasSource ns4:OpenFog_Reference_Architecture_for_Fog_Computing ] .

ns4:OFRAHierarchyPillarAnno a owl:NamedIndividual,
        ns1:oaAnnotation ;
    ns1:oahasBody ns4:OFRAHierarchyPillar ;
    ns1:oahasTarget [ a ns1:oaSpecificResource ;
            ns2:format "pdf" ;
            ns1:oahasSelector [ a ns1:oaRangeSelector ;
                    ns1:oahasEndSelector [ a ns1:oaXPathSelector ;
                            rdf:value "Page 34" ] ;
                    ns1:oahasStartSelector [ a ns1:oaXPathSelector ;
                            rdf:value "Page 31" ] ] ;
            ns1:oahasSource ns4:OpenFog_Reference_Architecture_for_Fog_Computing ],
        [ a ns1:oaSpecificResource ;
            ns2:format "pdf" ;
            ns1:oahasSelector [ a ns1:oaRangeSelector ;
                    ns1:oahasEndSelector [ a ns1:oaXPathSelector ;
                            rdf:value "Page 34" ] ;
                    ns1:oahasStartSelector [ a ns1:oaXPathSelector ;
                            rdf:value "Page 31" ] ] ;
            ns1:oahasSource ns4:OpenFog_Reference_Architecture_for_Fog_Computing ] .

ns4:OFRAItBusinessAndCrossFogApplicationsPerspectiveAnno a owl:NamedIndividual,
        ns1:oaAnnotation ;
    ns1:oahasBody ns4:OFRAItBusinessAndCrossFogApplicationsPerspective ;
    ns1:oahasTarget [ a ns1:oaSpecificResource ;
            ns2:format "pdf" ;
            ns1:oahasSelector [ a ns1:oaRangeSelector ;
                    ns1:oahasEndSelector [ a ns1:oaXPathSelector ;
                            rdf:value "Page 57" ] ;
                    ns1:oahasStartSelector [ a ns1:oaXPathSelector ;
                            rdf:value "Page 56" ] ] ;
            ns1:oahasSource ns4:OpenFog_Reference_Architecture_for_Fog_Computing ],
        [ a ns1:oaSpecificResource ;
            ns2:format "pdf" ;
            ns1:oahasSelector [ a ns1:oaRangeSelector ;
                    ns1:oahasEndSelector [ a ns1:oaXPathSelector ;
                            rdf:value "Page 57" ] ;
                    ns1:oahasStartSelector [ a ns1:oaXPathSelector ;
                            rdf:value "Page 56" ] ] ;
            ns1:oahasSource ns4:OpenFog_Reference_Architecture_for_Fog_Computing ] .

ns4:OFRAManageabilityPerspectiveAnno a owl:NamedIndividual,
        ns1:oaAnnotation ;
    ns1:oahasBody ns4:OFRAManageabilityPerspective ;
    ns1:oahasTarget [ a ns1:oaSpecificResource ;
            ns2:format "pdf" ;
            ns1:oahasSelector [ a ns1:oaRangeSelector ;
                    ns1:oahasEndSelector [ a ns1:oaXPathSelector ;
                            rdf:value "Page 54" ] ;
                    ns1:oahasStartSelector [ a ns1:oaXPathSelector ;
                            rdf:value "Page 51" ] ] ;
            ns1:oahasSource ns4:OpenFog_Reference_Architecture_for_Fog_Computing ],
        [ a ns1:oaSpecificResource ;
            ns2:format "pdf" ;
            ns1:oahasSelector [ a ns1:oaRangeSelector ;
                    ns1:oahasEndSelector [ a ns1:oaXPathSelector ;
                            rdf:value "Page 54" ] ;
                    ns1:oahasStartSelector [ a ns1:oaXPathSelector ;
                            rdf:value "Page 51" ] ] ;
            ns1:oahasSource ns4:OpenFog_Reference_Architecture_for_Fog_Computing ] .

ns4:OFRANodeViewAnno a owl:NamedIndividual,
        ns1:oaAnnotation ;
    ns1:oahasBody ns4:OFRANodeView ;
    ns1:oahasTarget [ a ns1:oaSpecificResource ;
            ns2:format "pdf" ;
            ns1:oahasSelector [ a ns1:oaRangeSelector ;
                    ns1:oahasEndSelector [ a ns1:oaXPathSelector ;
                            rdf:value "Page 73" ] ;
                    ns1:oahasStartSelector [ a ns1:oaXPathSelector ;
                            rdf:value "Page 56" ] ] ;
            ns1:oahasSource ns4:OpenFog_Reference_Architecture_for_Fog_Computing ],
        [ a ns1:oaSpecificResource ;
            ns2:format "pdf" ;
            ns1:oahasSelector [ a ns1:oaRangeSelector ;
                    ns1:oahasEndSelector [ a ns1:oaXPathSelector ;
                            rdf:value "Page 73" ] ;
                    ns1:oahasStartSelector [ a ns1:oaXPathSelector ;
                            rdf:value "Page 56" ] ] ;
            ns1:oahasSource ns4:OpenFog_Reference_Architecture_for_Fog_Computing ] .

ns4:OFRAOpennessPillarAnno a owl:NamedIndividual,
        ns1:oaAnnotation ;
    ns1:oahasBody ns4:OFRAOpennessPillar ;
    ns1:oahasTarget [ a ns1:oaSpecificResource ;
            ns2:format "pdf" ;
            ns1:oahasSelector [ a ns1:oaRangeSelector ;
                    ns1:oahasEndSelector [ a ns1:oaXPathSelector ;
                            rdf:value "Page 27" ] ;
                    ns1:oahasStartSelector [ a ns1:oaXPathSelector ;
                            rdf:value "Page 26" ] ] ;
            ns1:oahasSource ns4:OpenFog_Reference_Architecture_for_Fog_Computing ],
        [ a ns1:oaSpecificResource ;
            ns2:format "pdf" ;
            ns1:oahasSelector [ a ns1:oaRangeSelector ;
                    ns1:oahasEndSelector [ a ns1:oaXPathSelector ;
                            rdf:value "Page 27" ] ;
                    ns1:oahasStartSelector [ a ns1:oaXPathSelector ;
                            rdf:value "Page 26" ] ] ;
            ns1:oahasSource ns4:OpenFog_Reference_Architecture_for_Fog_Computing ] .

ns4:OFRAPerformancePerspectiveAnno a owl:NamedIndividual,
        ns1:oaAnnotation ;
    ns1:oahasBody ns4:OFRAPerformancePerspective ;
    ns1:oahasTarget [ a ns1:oaSpecificResource ;
            ns2:format "pdf" ;
            ns1:oahasSelector [ a ns1:oaRangeSelector ;
                    ns1:oahasEndSelector [ a ns1:oaXPathSelector ;
                            rdf:value "Page 47" ] ;
                    ns1:oahasStartSelector [ a ns1:oaXPathSelector ;
                            rdf:value "Page 46" ] ] ;
            ns1:oahasSource ns4:OpenFog_Reference_Architecture_for_Fog_Computing ],
        [ a ns1:oaSpecificResource ;
            ns2:format "pdf" ;
            ns1:oahasSelector [ a ns1:oaRangeSelector ;
                    ns1:oahasEndSelector [ a ns1:oaXPathSelector ;
                            rdf:value "Page 47" ] ;
                    ns1:oahasStartSelector [ a ns1:oaXPathSelector ;
                            rdf:value "Page 46" ] ] ;
            ns1:oahasSource ns4:OpenFog_Reference_Architecture_for_Fog_Computing ] .

ns4:OFRAProgrammabilityPillarAnno a owl:NamedIndividual,
        ns1:oaAnnotation ;
    ns1:oahasBody ns4:OFRAProgrammabilityPillar ;
    ns1:oahasTarget [ a ns1:oaSpecificResource ;
            ns2:format "pdf" ;
            ns1:oahasSelector [ a ns1:oaRangeSelector ;
                    ns1:oahasEndSelector [ a ns1:oaXPathSelector ;
                            rdf:value "Page 30" ] ;
                    ns1:oahasStartSelector [ a ns1:oaXPathSelector ;
                            rdf:value "Page 29" ] ] ;
            ns1:oahasSource ns4:OpenFog_Reference_Architecture_for_Fog_Computing ],
        [ a ns1:oaSpecificResource ;
            ns2:format "pdf" ;
            ns1:oahasSelector [ a ns1:oaRangeSelector ;
                    ns1:oahasEndSelector [ a ns1:oaXPathSelector ;
                            rdf:value "Page 30" ] ;
                    ns1:oahasStartSelector [ a ns1:oaXPathSelector ;
                            rdf:value "Page 29" ] ] ;
            ns1:oahasSource ns4:OpenFog_Reference_Architecture_for_Fog_Computing ] .

ns4:OFRAScalabilityPillarAnno a owl:NamedIndividual,
        ns1:oaAnnotation ;
    ns1:oahasBody ns4:OFRAScalabilityPillar ;
    ns1:oahasTarget [ a ns1:oaSpecificResource ;
            ns2:format "pdf" ;
            ns1:oahasSelector [ a ns1:oaRangeSelector ;
                    ns1:oahasEndSelector [ a ns1:oaXPathSelector ;
                            rdf:value "Page 26" ] ;
                    ns1:oahasStartSelector [ a ns1:oaXPathSelector ;
                            rdf:value "Page 24" ] ] ;
            ns1:oahasSource ns4:OpenFog_Reference_Architecture_for_Fog_Computing ],
        [ a ns1:oaSpecificResource ;
            ns2:format "pdf" ;
            ns1:oahasSelector [ a ns1:oaRangeSelector ;
                    ns1:oahasEndSelector [ a ns1:oaXPathSelector ;
                            rdf:value "Page 26" ] ;
                    ns1:oahasStartSelector [ a ns1:oaXPathSelector ;
                            rdf:value "Page 24" ] ] ;
            ns1:oahasSource ns4:OpenFog_Reference_Architecture_for_Fog_Computing ] .

ns4:OFRASecurityPerspectiveAnno a owl:NamedIndividual,
        ns1:oaAnnotation ;
    ns1:oahasBody ns4:OFRASecurityPerspective ;
    ns1:oahasTarget [ a ns1:oaSpecificResource ;
            ns2:format "pdf" ;
            ns1:oahasSelector [ a ns1:oaRangeSelector ;
                    ns1:oahasEndSelector [ a ns1:oaXPathSelector ;
                            rdf:value "Page 51" ] ;
                    ns1:oahasStartSelector [ a ns1:oaXPathSelector ;
                            rdf:value "Page 47" ] ] ;
            ns1:oahasSource ns4:OpenFog_Reference_Architecture_for_Fog_Computing ],
        [ a ns1:oaSpecificResource ;
            ns2:format "pdf" ;
            ns1:oahasSelector [ a ns1:oaRangeSelector ;
                    ns1:oahasEndSelector [ a ns1:oaXPathSelector ;
                            rdf:value "Page 51" ] ;
                    ns1:oahasStartSelector [ a ns1:oaXPathSelector ;
                            rdf:value "Page 47" ] ] ;
            ns1:oahasSource ns4:OpenFog_Reference_Architecture_for_Fog_Computing ] .

ns4:OFRASecurityPillarAnno a owl:NamedIndividual,
        ns1:oaAnnotation ;
    ns1:oahasBody ns4:OFRASecurityPillar ;
    ns1:oahasTarget [ a ns1:oaSpecificResource ;
            ns2:format "pdf" ;
            ns1:oahasSelector [ a ns1:oaRangeSelector ;
                    ns1:oahasEndSelector [ a ns1:oaXPathSelector ;
                            rdf:value "Page 24" ] ;
                    ns1:oahasStartSelector [ a ns1:oaXPathSelector ;
                            rdf:value "Page 23" ] ] ;
            ns1:oahasSource ns4:OpenFog_Reference_Architecture_for_Fog_Computing ],
        [ a ns1:oaSpecificResource ;
            ns2:format "pdf" ;
            ns1:oahasSelector [ a ns1:oaRangeSelector ;
                    ns1:oahasEndSelector [ a ns1:oaXPathSelector ;
                            rdf:value "Page 24" ] ;
                    ns1:oahasStartSelector [ a ns1:oaXPathSelector ;
                            rdf:value "Page 23" ] ] ;
            ns1:oahasSource ns4:OpenFog_Reference_Architecture_for_Fog_Computing ],
        [ a ns1:oaSpecificResource ;
            ns2:format "pdf" ;
            ns1:oahasSelector [ a ns1:oaRangeSelector ;
                    ns1:oahasEndSelector [ a ns1:oaXPathSelector ;
                            rdf:value "Page 24" ] ;
                    ns1:oahasStartSelector [ a ns1:oaXPathSelector ;
                            rdf:value "Page 23" ] ] ;
            ns1:oahasSource ns4:OpenFog_Reference_Architecture_for_Fog_Computing ],
        [ a ns1:oaSpecificResource ;
            ns2:format "pdf" ;
            ns1:oahasSelector [ a ns1:oaRangeSelector ;
                    ns1:oahasEndSelector [ a ns1:oaXPathSelector ;
                            rdf:value "Page 24" ] ;
                    ns1:oahasStartSelector [ a ns1:oaXPathSelector ;
                            rdf:value "Page 23" ] ] ;
            ns1:oahasSource ns4:OpenFog_Reference_Architecture_for_Fog_Computing ] .

ns4:OFRASoftwareViewAnno a owl:NamedIndividual,
        ns1:oaAnnotation ;
    ns1:oahasBody ns4:OFRASoftwareView ;
    ns1:oahasTarget [ a ns1:oaSpecificResource ;
            ns2:format "pdf" ;
            ns1:oahasSelector [ a ns1:oaRangeSelector ;
                    ns1:oahasEndSelector [ a ns1:oaXPathSelector ;
                            rdf:value "Page 89" ] ;
                    ns1:oahasStartSelector [ a ns1:oaXPathSelector ;
                            rdf:value "Page 77" ] ] ;
            ns1:oahasSource ns4:OpenFog_Reference_Architecture_for_Fog_Computing ],
        [ a ns1:oaSpecificResource ;
            ns2:format "pdf" ;
            ns1:oahasSelector [ a ns1:oaRangeSelector ;
                    ns1:oahasEndSelector [ a ns1:oaXPathSelector ;
                            rdf:value "Page 89" ] ;
                    ns1:oahasStartSelector [ a ns1:oaXPathSelector ;
                            rdf:value "Page 77" ] ] ;
            ns1:oahasSource ns4:OpenFog_Reference_Architecture_for_Fog_Computing ] .

ns4:OFRASystemViewAnno a owl:NamedIndividual,
        ns1:oaAnnotation ;
    ns1:oahasBody ns4:OFRASystemView ;
    ns1:oahasTarget [ a ns1:oaSpecificResource ;
            ns2:format "pdf" ;
            ns1:oahasSelector [ a ns1:oaRangeSelector ;
                    ns1:oahasEndSelector [ a ns1:oaXPathSelector ;
                            rdf:value "Page 78" ] ;
                    ns1:oahasStartSelector [ a ns1:oaXPathSelector ;
                            rdf:value "Page 73" ] ] ;
            ns1:oahasSource ns4:OpenFog_Reference_Architecture_for_Fog_Computing ],
        [ a ns1:oaSpecificResource ;
            ns2:format "pdf" ;
            ns1:oahasSelector [ a ns1:oaRangeSelector ;
                    ns1:oahasEndSelector [ a ns1:oaXPathSelector ;
                            rdf:value "Page 78" ] ;
                    ns1:oahasStartSelector [ a ns1:oaXPathSelector ;
                            rdf:value "Page 73" ] ] ;
            ns1:oahasSource ns4:OpenFog_Reference_Architecture_for_Fog_Computing ] .

ns4:OFRA_RASPillarAnno a owl:NamedIndividual,
        ns1:oaAnnotation ;
    ns1:oahasBody ns4:OFRA_RASPillar ;
    ns1:oahasTarget [ a ns1:oaSpecificResource ;
            ns2:format "pdf" ;
            ns1:oahasSelector [ a ns1:oaRangeSelector ;
                    ns1:oahasEndSelector [ a ns1:oaXPathSelector ;
                            rdf:value "Page 31" ] ;
                    ns1:oahasStartSelector [ a ns1:oaXPathSelector ;
                            rdf:value "Page 29" ] ] ;
            ns1:oahasSource ns4:OpenFog_Reference_Architecture_for_Fog_Computing ],
        [ a ns1:oaSpecificResource ;
            ns2:format "pdf" ;
            ns1:oahasSelector [ a ns1:oaRangeSelector ;
                    ns1:oahasEndSelector [ a ns1:oaXPathSelector ;
                            rdf:value "Page 31" ] ;
                    ns1:oahasStartSelector [ a ns1:oaXPathSelector ;
                            rdf:value "Page 29" ] ] ;
            ns1:oahasSource ns4:OpenFog_Reference_Architecture_for_Fog_Computing ] .

ns4:OMA a owl:NamedIndividual,
        ns8:Organization,
        ns4:IIoTConsortium ;
    rdfs:label "Open Mobile Alliance"@en ;
    ns2:creator ns4:sebastian ;
    rdfs:comment "OMA (Open Mobile Alliance) is the Leading Industry Forum for Developing Market Driven, Interoperable Mobile Service Enablers (source: https://www.postscapes.com/internet-of-things-protocols/)"@en ;
    ns4:hasOfficialResource <http://openmobilealliance.org/about-oma/work-program/m2m-enablers/> .

ns4:OMALightweightM2M a owl:NamedIndividual,
        ns8:Document,
        ns4:Publication,
        ns4:TechnicalSpecification ;
    rdfs:label "Lightweight M2M v1.0"@en ;
    ns2:creator ns4:sebastian ;
    rdfs:comment "The motivation of LightweightM2M is to develop a fast deployable client-server specification to provide machine to machine service.<br> LightweightM2M is principly a device management protocol, but it should be designed to be able to extend to meet the requirements of applications. LightweightM2M is not restricted to device management, it should be able transfer service / application data. (source: https://www.postscapes.com/internet-of-things-protocols/)"@en ;
    ns4:hasOfficialResource <http://technical.openmobilealliance.org/Technical/release_program/lightweightM2M_v1_0.aspx> .

ns4:OceanBusinessViewpointAnno a owl:NamedIndividual,
        ns1:oaAnnotation ;
    ns1:oahasBody ns4:OceanBusinessViewpoint ;
    ns1:oahasTarget [ a ns1:oaSpecificResource ;
            ns1:oahasSelector [ a ns1:oaRangeSelector ;
                    ns1:oahasEndSelector [ a ns1:oaXPathSelector ;
                            rdf:value "Page 41" ] ;
                    ns1:oahasStartSelector [ a ns1:oaXPathSelector ;
                            rdf:value "Page 1" ] ] ;
            ns1:oahasSource ns4:Ocean_Protocol_Business_Strategy_Oct_2017 ],
        [ a ns1:oaSpecificResource ;
            ns1:oahasSelector [ a ns1:oaRangeSelector ;
                    ns1:oahasEndSelector [ a ns1:oaXPathSelector ;
                            rdf:value "Page 41" ] ;
                    ns1:oahasStartSelector [ a ns1:oaXPathSelector ;
                            rdf:value "Page 1" ] ] ;
            ns1:oahasSource ns4:Ocean_Protocol_Business_Strategy_Oct_2017 ] .

ns4:OceanMarketplaceViewpointAnno a owl:NamedIndividual,
        ns1:oaAnnotation ;
    ns1:oahasBody ns4:OceanMarketplaceViewpoint ;
    ns1:oahasTarget [ a ns1:oaSpecificResource ;
            ns1:oahasSelector [ a ns1:oaRangeSelector ;
                    ns1:oahasEndSelector [ a ns1:oaXPathSelector ;
                            rdf:value "Page 27" ] ;
                    ns1:oahasStartSelector [ a ns1:oaXPathSelector ;
                            rdf:value "Page 1" ] ] ;
            ns1:oahasSource ns4:Ocean_Protocol_Reference_Marketplace_Framework_Feb_2019 ],
        [ a ns1:oaSpecificResource ;
            ns1:oahasSelector [ a ns1:oaRangeSelector ;
                    ns1:oahasEndSelector [ a ns1:oaXPathSelector ;
                            rdf:value "Page 27" ] ;
                    ns1:oahasStartSelector [ a ns1:oaXPathSelector ;
                            rdf:value "Page 1" ] ] ;
            ns1:oahasSource ns4:Ocean_Protocol_Reference_Marketplace_Framework_Feb_2019 ] .

ns4:OceanSystemViewpointAnno a owl:NamedIndividual,
        ns1:oaAnnotation ;
    ns1:oahasBody ns4:OceanSystemViewpoint ;
    ns1:oahasTarget [ a ns1:oaSpecificResource ;
            ns1:oahasSelector [ a ns1:oaRangeSelector ;
                    ns1:oahasEndSelector [ a ns1:oaXPathSelector ;
                            rdf:value "Page 59" ] ;
                    ns1:oahasStartSelector [ a ns1:oaXPathSelector ;
                            rdf:value "Page 1" ] ] ;
            ns1:oahasSource ns4:Ocean_Protocol_Technical_Whitepaper_Apr_2019 ],
        [ a ns1:oaSpecificResource ;
            ns1:oahasSelector [ a ns1:oaRangeSelector ;
                    ns1:oahasEndSelector [ a ns1:oaXPathSelector ;
                            rdf:value "Page 59" ] ;
                    ns1:oahasStartSelector [ a ns1:oaXPathSelector ;
                            rdf:value "Page 1" ] ] ;
            ns1:oahasSource ns4:Ocean_Protocol_Technical_Whitepaper_Apr_2019 ] .

ns4:OcfCoreFrameworkAnno a owl:NamedIndividual,
        ns1:oaAnnotation ;
    ns1:oahasBody ns4:OcfCoreFramework ;
    ns1:oahasTarget [ a ns1:oaSpecificResource ;
            ns1:oahasSelector [ a ns1:oaRangeSelector ;
                    ns1:oahasEndSelector [ a ns1:oaXPathSelector ;
                            rdf:value "Page 14" ] ;
                    ns1:oahasStartSelector [ a ns1:oaXPathSelector ;
                            rdf:value "Page 11" ] ] ;
            ns1:oahasSource ns4:OCF_Core_Specification_VERSION_2_0_1 ] .

ns4:OcfDataModelsAnno a owl:NamedIndividual,
        ns1:oaAnnotation ;
    ns1:oahasBody ns4:OcfDataModels ;
    ns1:oahasTarget [ a ns1:oaSpecificResource ;
            ns1:oahasSelector [ a ns1:oaRangeSelector ;
                    ns1:oahasEndSelector [ a ns1:oaXPathSelector ;
                            rdf:value "Page 14" ] ;
                    ns1:oahasStartSelector [ a ns1:oaXPathSelector ;
                            rdf:value "Page 11" ] ] ;
            ns1:oahasSource ns4:OCF_Core_Specification_VERSION_2_0_1 ] .

ns4:OcfFrameworkAnno a owl:NamedIndividual,
        ns1:oaAnnotation ;
    ns1:oahasBody ns4:OcfFramework ;
    ns1:oahasTarget [ a ns1:oaSpecificResource ;
            ns1:oahasSelector [ a ns1:oaRangeSelector ;
                    ns1:oahasEndSelector [ a ns1:oaXPathSelector ;
                            rdf:value "Page 14" ] ;
                    ns1:oahasStartSelector [ a ns1:oaXPathSelector ;
                            rdf:value "Page 11" ] ] ;
            ns1:oahasSource ns4:OCF_Core_Specification_VERSION_2_0_1 ] .

ns4:OcfL2ConnectivityAnno a owl:NamedIndividual,
        ns1:oaAnnotation ;
    ns1:oahasBody ns4:OcfL2Connectivity ;
    ns1:oahasTarget [ a ns1:oaSpecificResource ;
            ns1:oahasSelector [ a ns1:oaRangeSelector ;
                    ns1:oahasEndSelector [ a ns1:oaXPathSelector ;
                            rdf:value "Page 14" ] ;
                    ns1:oahasStartSelector [ a ns1:oaXPathSelector ;
                            rdf:value "Page 11" ] ] ;
            ns1:oahasSource ns4:OCF_Core_Specification_VERSION_2_0_1 ] .

ns4:OcfNetworkingAnno a owl:NamedIndividual,
        ns1:oaAnnotation ;
    ns1:oahasBody ns4:OcfNetworking ;
    ns1:oahasTarget [ a ns1:oaSpecificResource ;
            ns1:oahasSelector [ a ns1:oaRangeSelector ;
                    ns1:oahasEndSelector [ a ns1:oaXPathSelector ;
                            rdf:value "Page 14" ] ;
                    ns1:oahasStartSelector [ a ns1:oaXPathSelector ;
                            rdf:value "Page 11" ] ] ;
            ns1:oahasSource ns4:OCF_Core_Specification_VERSION_2_0_1 ] .

ns4:OcfSecurityAnno a owl:NamedIndividual,
        ns1:oaAnnotation ;
    ns1:oahasBody ns4:OcfSecurity ;
    ns1:oahasTarget [ a ns1:oaSpecificResource ;
            ns1:oahasSelector [ a ns1:oaRangeSelector ;
                    ns1:oahasEndSelector [ a ns1:oaXPathSelector ;
                            rdf:value "Page 14" ] ;
                    ns1:oahasStartSelector [ a ns1:oaXPathSelector ;
                            rdf:value "Page 11" ] ] ;
            ns1:oahasSource ns4:OCF_Core_Specification_VERSION_2_0_1 ] .

ns4:OpenApi a owl:NamedIndividual,
        ns8:Document,
        ns4:Publication,
        ns4:TechnicalSpecification ;
    rdfs:label "OpenAPI"@en ;
    ns2:creator ns4:sebastian ;
    rdfs:comment "The OpenAPI Specification (originally known as the Swagger Specification) is a specification for machine-readable interface files for describing, producing, consuming, and visualizing RESTful web services. A variety of tools can generate code, documentation and test cases given an interface file. Development of the OpenAPI Specification (OAS) is overseen by the Open API Initiative, an open source collaborative project of the Linux Foundation. (source: wikipedia)"@en ;
    ns4:hasDBpediaResource <http://dbpedia.org/resource/OpenAPI_Specification> .

ns4:OpenFogNodeView a owl:NamedIndividual .

ns4:OrionContextBroker a owl:NamedIndividual,
        ns8:Document,
        ns4:Publication,
        ns4:TechnicalSpecification ;
    rdfs:label "ORION Context Broker"@en ;
    ns2:creator ns4:sebastian ;
    ns3:associatedWith ns4:FIWARE .

ns4:Performance a owl:NamedIndividual,
        ns4:Concern ;
    rdfs:label "Performance"@en ;
    ns2:creator ns4:MuhammadUsman ;
    rdfs:comment "Performance is completion of a task with application of knowledge, skills and abilities"@en ;
    rdfs:seeAlso <https://ieeexplore.ieee.org/document/8249113>,
        <https://ieeexplore.ieee.org/document/8463303> ;
    ns4:hasWikipediaArticle <https://en.wikipedia.org/wiki/Performance> ;
    ns5:supports ns4:BusinessContext .

ns4:PeriodicCommunication a owl:NamedIndividual,
        ns4:Concern ;
    rdfs:label "Periodic Communication"@en ;
    ns7:hasStakeholder <https://www.wikidata.org/wiki/Q1548249> ;
    rdfs:seeAlso "IoT-A Requirement UNI.005" ;
    ns5:supports ns4:EventDrivenMessaging .

ns4:PhysicalWeb a owl:NamedIndividual,
        ns8:Document,
        ns4:Publication,
        ns4:TechnicalSpecification ;
    rdfs:label "Physical Web"@en ;
    ns2:creator ns4:sebastian ;
    rdfs:comment "Physical Web - The Physical Web enables you to see a list of URLs being broadcast by objects in the environment around you with a Bluetooth Low Energy (BLE) beacon. (source: https://www.postscapes.com/internet-of-things-protocols/)"@en ;
    ns4:hasOfficialResource <https://google.github.io/physical-web/faq> .

ns4:PlantManager rdfs:label "Plant Manager"@en ;
    rdfs:comment " A plant manager is responsible for the functioning of a plant/facility." ;
    rdfs:seeAlso "IIC:PUB:G1:V1.80:20170131" ;
    ns6:altLabel "Facility Manager"@en ;
    ns6:note "Publications referred: 'IIC:PUB:G1:V1.80:20170131' '1.5 AUDIENCE' 'Page 7' " ;
    ns4:hasWikipediaArticle <https://en.wikipedia.org/wiki/Facility_management#Role_of_the_facilities_manager> .

ns4:ProcessIsolation a owl:NamedIndividual,
        ns4:Concern ;
    rdfs:label "Isolation"@en ;
    ns2:creator ns4:MuhammadUsman ;
    rdfs:comment "\"Isolation would be another issue at the edge of the network. In mobile OS, if an application fails or crashes, the whole system will usually crash and reboot. Or in a distributed system the shared resource could be managed with different synchronization mechanisms such as a lock or token ring. \""@en ;
    rdfs:seeAlso <https://ieeexplore.ieee.org/document/7488250> ;
    ns4:hasWikipediaArticle <https://en.wikipedia.org/wiki/Process_isolation> ;
    ns5:supports ns4:IntegrityProtection .

ns4:ProductDevelopmentLifeCycle a owl:Class ;
    rdfs:label "Product Development Life Cycle"@en ;
    rdfs:comment "PLM is the process of managing the entire lifecycle of a product from inception, through engineering design and manufacture, to service and disposal of manufactured products. Related areas are PLMManagement, Modeling Practice, Product Model Data exchange, Manufacturing Model Data, Product Catalog Data."@en,
        "Product Development Life-Cycle Phase"@en ;
    rdfs:isDefinedBy "https://en.wikipedia.org/wiki/Product_lifecycle" ;
    rdfs:subClassOf ns4:StandardClassification .

ns4:ProductionSystemLifeCycle a owl:Class ;
    rdfs:label "Production System Life Cycle"@en ;
    rdfs:comment "Collections of machines, equipment, and auxiliary systems organized to create goods and services from various resources."@en ;
    rdfs:isDefinedBy <http://nvlpubs.nist.gov/nistpubs/ir/2016/NIST.IR.8107.pdf> ;
    rdfs:subClassOf ns4:StandardClassification .

ns4:ProjectManager a ns7:StakeholderGroup,
        owl:NamedIndividual .

ns4:Pseudonimity a owl:NamedIndividual,
        ns4:Concern ;
    rdfs:label "Pseudonimity"@en ;
    ns2:creator ns4:sebastian ;
    rdfs:comment "While complete anonymity is not feasibe in an IoT scenario, pseudonimity should be supported."@en ;
    rdfs:seeAlso "IoT-A Requirement UNI.624" ;
    ns4:hasDBpediaResource <http://dbpedia.org/resource/Pseudonymity> ;
    ns5:supports ns4:Anonymity .

ns4:RAMIAssetlayerAnno a owl:NamedIndividual,
        ns1:oaAnnotation ;
    ns1:oahasBody ns4:RAMIAssetlayer ;
    ns1:oahasTarget [ a ns1:oaSpecificResource ;
            ns2:format "pdf" ;
            ns1:oahasSelector [ a ns1:oaRangeSelector ;
                    ns1:oahasEndSelector [ a ns1:oaXPathSelector ;
                            rdf:value "Page 23" ] ;
                    ns1:oahasStartSelector [ a ns1:oaXPathSelector ;
                            rdf:value "Page 22" ] ] ;
            ns1:oahasSource ns4:DIN_SPEC_91345 ],
        [ a ns1:oaSpecificResource ;
            ns2:format "pdf" ;
            ns1:oahasSelector [ a ns1:oaRangeSelector ;
                    ns1:oahasEndSelector [ a ns1:oaXPathSelector ;
                            rdf:value "Page 23" ] ;
                    ns1:oahasStartSelector [ a ns1:oaXPathSelector ;
                            rdf:value "Page 22" ] ] ;
            ns1:oahasSource ns4:DIN_SPEC_91345 ] .

ns4:RAMIBodyAnno a owl:NamedIndividual,
        ns1:oaAnnotation ;
    ns1:oahasBody ns4:RAMIBody ;
    ns1:oahasTarget [ a ns1:oaSpecificResource ;
            ns2:format "pdf" ;
            ns1:oahasSelector [ a ns1:oaRangeSelector ;
                    ns1:oahasEndSelector [ a ns1:oaXPathSelector ;
                            rdf:value "Page 31" ] ;
                    ns1:oahasStartSelector [ a ns1:oaXPathSelector ;
                            rdf:value "Page 30" ] ] ;
            ns1:oahasSource ns4:DIN_SPEC_91345 ],
        [ a ns1:oaSpecificResource ;
            ns2:format "pdf" ;
            ns1:oahasSelector [ a ns1:oaRangeSelector ;
                    ns1:oahasEndSelector [ a ns1:oaXPathSelector ;
                            rdf:value "Page 31" ] ;
                    ns1:oahasStartSelector [ a ns1:oaXPathSelector ;
                            rdf:value "Page 30" ] ] ;
            ns1:oahasSource ns4:DIN_SPEC_91345 ] .

ns4:RAMIBusinessLayerAnno a owl:NamedIndividual,
        ns1:oaAnnotation ;
    ns1:oahasBody ns4:RAMIBusinessLayer ;
    ns1:oahasTarget [ a ns1:oaSpecificResource ;
            ns2:format "pdf" ;
            ns1:oahasSelector [ a ns1:oaRangeSelector ;
                    ns1:oahasEndSelector [ a ns1:oaXPathSelector ;
                            rdf:value "Page 21" ] ;
                    ns1:oahasStartSelector [ a ns1:oaXPathSelector ;
                            rdf:value "Page 20" ] ] ;
            ns1:oahasSource ns4:DIN_SPEC_91345 ],
        [ a ns1:oaSpecificResource ;
            ns2:format "pdf" ;
            ns1:oahasSelector [ a ns1:oaRangeSelector ;
                    ns1:oahasEndSelector [ a ns1:oaXPathSelector ;
                            rdf:value "Page 21" ] ;
                    ns1:oahasStartSelector [ a ns1:oaXPathSelector ;
                            rdf:value "Page 20" ] ] ;
            ns1:oahasSource ns4:DIN_SPEC_91345 ] .

ns4:RAMICommunicationlayerAnno a owl:NamedIndividual,
        ns1:oaAnnotation ;
    ns1:oahasBody ns4:RAMICommunicationlayer ;
    ns1:oahasTarget [ a ns1:oaSpecificResource ;
            ns2:format "pdf" ;
            ns1:oahasSelector [ a ns1:oaRangeSelector ;
                    ns1:oahasEndSelector [ a ns1:oaXPathSelector ;
                            rdf:value "Page 22" ] ;
                    ns1:oahasStartSelector [ a ns1:oaXPathSelector ;
                            rdf:value "Page 21" ] ] ;
            ns1:oahasSource ns4:DIN_SPEC_91345 ],
        [ a ns1:oaSpecificResource ;
            ns2:format "pdf" ;
            ns1:oahasSelector [ a ns1:oaRangeSelector ;
                    ns1:oahasEndSelector [ a ns1:oaXPathSelector ;
                            rdf:value "Page 22" ] ;
                    ns1:oahasStartSelector [ a ns1:oaXPathSelector ;
                            rdf:value "Page 21" ] ] ;
            ns1:oahasSource ns4:DIN_SPEC_91345 ] .

ns4:RAMIConnectedWorldAnno a owl:NamedIndividual,
        ns1:oaAnnotation ;
    ns1:oahasBody ns4:RAMIConnectedWorld ;
    ns1:oahasTarget [ a ns1:oaSpecificResource ;
            ns2:format "pdf" ;
            ns1:oahasSelector [ a ns1:oaRangeSelector ;
                    ns1:oahasEndSelector [ a ns1:oaXPathSelector ;
                            rdf:value "Page 24" ] ;
                    ns1:oahasStartSelector [ a ns1:oaXPathSelector ;
                            rdf:value "Page 23" ] ] ;
            ns1:oahasSource ns4:DIN_SPEC_91345 ],
        [ a ns1:oaSpecificResource ;
            ns2:format "pdf" ;
            ns1:oahasSelector [ a ns1:oaRangeSelector ;
                    ns1:oahasEndSelector [ a ns1:oaXPathSelector ;
                            rdf:value "Page 24" ] ;
                    ns1:oahasStartSelector [ a ns1:oaXPathSelector ;
                            rdf:value "Page 23" ] ] ;
            ns1:oahasSource ns4:DIN_SPEC_91345 ] .

ns4:RAMIControlDeviceAnno a owl:NamedIndividual,
        ns1:oaAnnotation ;
    ns1:oahasBody ns4:RAMIControlDevice ;
    ns1:oahasTarget [ a ns1:oaSpecificResource ;
            ns2:format "pdf" ;
            ns1:oahasSelector [ a ns1:oaRangeSelector ;
                    ns1:oahasEndSelector [ a ns1:oaXPathSelector ;
                            rdf:value "Page 24" ] ;
                    ns1:oahasStartSelector [ a ns1:oaXPathSelector ;
                            rdf:value "Page 23" ] ] ;
            ns1:oahasSource ns4:DIN_SPEC_91345 ],
        [ a ns1:oaSpecificResource ;
            ns2:format "pdf" ;
            ns1:oahasSelector [ a ns1:oaRangeSelector ;
                    ns1:oahasEndSelector [ a ns1:oaXPathSelector ;
                            rdf:value "Page 24" ] ;
                    ns1:oahasStartSelector [ a ns1:oaXPathSelector ;
                            rdf:value "Page 23" ] ] ;
            ns1:oahasSource ns4:DIN_SPEC_91345 ] .

ns4:RAMIEnterpriseAnno a owl:NamedIndividual,
        ns1:oaAnnotation ;
    ns1:oahasBody ns4:RAMIEnterprise ;
    ns1:oahasTarget [ a ns1:oaSpecificResource ;
            ns2:format "pdf" ;
            ns1:oahasSelector [ a ns1:oaRangeSelector ;
                    ns1:oahasEndSelector [ a ns1:oaXPathSelector ;
                            rdf:value "Page 24" ] ;
                    ns1:oahasStartSelector [ a ns1:oaXPathSelector ;
                            rdf:value "Page 23" ] ] ;
            ns1:oahasSource ns4:DIN_SPEC_91345 ],
        [ a ns1:oaSpecificResource ;
            ns2:format "pdf" ;
            ns1:oahasSelector [ a ns1:oaRangeSelector ;
                    ns1:oahasEndSelector [ a ns1:oaXPathSelector ;
                            rdf:value "Page 24" ] ;
                    ns1:oahasStartSelector [ a ns1:oaXPathSelector ;
                            rdf:value "Page 23" ] ] ;
            ns1:oahasSource ns4:DIN_SPEC_91345 ] .

ns4:RAMIFieldDeviceAnno a owl:NamedIndividual,
        ns1:oaAnnotation ;
    ns1:oahasBody ns4:RAMIFieldDevice ;
    ns1:oahasTarget [ a ns1:oaSpecificResource ;
            ns2:format "pdf" ;
            ns1:oahasSelector [ a ns1:oaRangeSelector ;
                    ns1:oahasEndSelector [ a ns1:oaXPathSelector ;
                            rdf:value "Page 24" ] ;
                    ns1:oahasStartSelector [ a ns1:oaXPathSelector ;
                            rdf:value "Page 23" ] ] ;
            ns1:oahasSource ns4:DIN_SPEC_91345 ],
        [ a ns1:oaSpecificResource ;
            ns2:format "pdf" ;
            ns1:oahasSelector [ a ns1:oaRangeSelector ;
                    ns1:oahasEndSelector [ a ns1:oaXPathSelector ;
                            rdf:value "Page 24" ] ;
                    ns1:oahasStartSelector [ a ns1:oaXPathSelector ;
                            rdf:value "Page 23" ] ] ;
            ns1:oahasSource ns4:DIN_SPEC_91345 ] .

ns4:RAMIFunctionalLayerAnno a owl:NamedIndividual,
        ns1:oaAnnotation ;
    ns1:oahasBody ns4:RAMIFunctionalLayer ;
    ns1:oahasTarget [ a ns1:oaSpecificResource ;
            ns2:format "pdf" ;
            ns1:oahasSelector [ a ns1:oaRangeSelector ;
                    ns1:oahasEndSelector [ a ns1:oaXPathSelector ;
                            rdf:value "Page 21" ] ;
                    ns1:oahasStartSelector [ a ns1:oaXPathSelector ;
                            rdf:value "Page 20" ] ] ;
            ns1:oahasSource ns4:DIN_SPEC_91345 ],
        [ a ns1:oaSpecificResource ;
            ns2:format "pdf" ;
            ns1:oahasSelector [ a ns1:oaRangeSelector ;
                    ns1:oahasEndSelector [ a ns1:oaXPathSelector ;
                            rdf:value "Page 21" ] ;
                    ns1:oahasStartSelector [ a ns1:oaXPathSelector ;
                            rdf:value "Page 20" ] ] ;
            ns1:oahasSource ns4:DIN_SPEC_91345 ] .

ns4:RAMIHeaderAnno a owl:NamedIndividual,
        ns1:oaAnnotation ;
    ns1:oahasBody ns4:RAMIHeader ;
    ns1:oahasTarget [ a ns1:oaSpecificResource ;
            ns2:format "pdf" ;
            ns1:oahasSelector [ a ns1:oaRangeSelector ;
                    ns1:oahasEndSelector [ a ns1:oaXPathSelector ;
                            rdf:value "Page 31" ] ;
                    ns1:oahasStartSelector [ a ns1:oaXPathSelector ;
                            rdf:value "Page 30" ] ] ;
            ns1:oahasSource ns4:DIN_SPEC_91345 ],
        [ a ns1:oaSpecificResource ;
            ns2:format "pdf" ;
            ns1:oahasSelector [ a ns1:oaRangeSelector ;
                    ns1:oahasEndSelector [ a ns1:oaXPathSelector ;
                            rdf:value "Page 31" ] ;
                    ns1:oahasStartSelector [ a ns1:oaXPathSelector ;
                            rdf:value "Page 30" ] ] ;
            ns1:oahasSource ns4:DIN_SPEC_91345 ] .

ns4:RAMIInformationLayerAnno a owl:NamedIndividual,
        ns1:oaAnnotation ;
    ns1:oahasBody ns4:RAMIInformationLayer ;
    ns1:oahasTarget [ a ns1:oaSpecificResource ;
            ns2:format "pdf" ;
            ns1:oahasSelector [ a ns1:oaRangeSelector ;
                    ns1:oahasEndSelector [ a ns1:oaXPathSelector ;
                            rdf:value "Page 22" ] ;
                    ns1:oahasStartSelector [ a ns1:oaXPathSelector ;
                            rdf:value "Page 21" ] ] ;
            ns1:oahasSource ns4:DIN_SPEC_91345 ],
        [ a ns1:oaSpecificResource ;
            ns2:format "pdf" ;
            ns1:oahasSelector [ a ns1:oaRangeSelector ;
                    ns1:oahasEndSelector [ a ns1:oaXPathSelector ;
                            rdf:value "Page 22" ] ;
                    ns1:oahasStartSelector [ a ns1:oaXPathSelector ;
                            rdf:value "Page 21" ] ] ;
            ns1:oahasSource ns4:DIN_SPEC_91345 ] .

ns4:RAMIIntegrationLayerAnno a owl:NamedIndividual,
        ns1:oaAnnotation ;
    ns1:oahasBody ns4:RAMIIntegrationLayer ;
    ns1:oahasTarget [ a ns1:oaSpecificResource ;
            ns2:format "pdf" ;
            ns1:oahasSelector [ a ns1:oaRangeSelector ;
                    ns1:oahasEndSelector [ a ns1:oaXPathSelector ;
                            rdf:value "Page 23" ] ;
                    ns1:oahasStartSelector [ a ns1:oaXPathSelector ;
                            rdf:value "Page 22" ] ] ;
            ns1:oahasSource ns4:DIN_SPEC_91345 ],
        [ a ns1:oaSpecificResource ;
            ns2:format "pdf" ;
            ns1:oahasSelector [ a ns1:oaRangeSelector ;
                    ns1:oahasEndSelector [ a ns1:oaXPathSelector ;
                            rdf:value "Page 23" ] ;
                    ns1:oahasStartSelector [ a ns1:oaXPathSelector ;
                            rdf:value "Page 22" ] ] ;
            ns1:oahasSource ns4:DIN_SPEC_91345 ] .

ns4:RAMIProductAnno a owl:NamedIndividual,
        ns1:oaAnnotation ;
    ns1:oahasBody ns4:RAMIProduct ;
    ns1:oahasTarget [ a ns1:oaSpecificResource ;
            ns2:format "pdf" ;
            ns1:oahasSelector [ a ns1:oaRangeSelector ;
                    ns1:oahasEndSelector [ a ns1:oaXPathSelector ;
                            rdf:value "Page 24" ] ;
                    ns1:oahasStartSelector [ a ns1:oaXPathSelector ;
                            rdf:value "Page 23" ] ] ;
            ns1:oahasSource ns4:DIN_SPEC_91345 ],
        [ a ns1:oaSpecificResource ;
            ns2:format "pdf" ;
            ns1:oahasSelector [ a ns1:oaRangeSelector ;
                    ns1:oahasEndSelector [ a ns1:oaXPathSelector ;
                            rdf:value "Page 24" ] ;
                    ns1:oahasStartSelector [ a ns1:oaXPathSelector ;
                            rdf:value "Page 23" ] ] ;
            ns1:oahasSource ns4:DIN_SPEC_91345 ] .

ns4:RAMIStationAnno a owl:NamedIndividual,
        ns1:oaAnnotation ;
    ns1:oahasBody ns4:RAMIStation ;
    ns1:oahasTarget [ a ns1:oaSpecificResource ;
            ns2:format "pdf" ;
            ns1:oahasSelector [ a ns1:oaRangeSelector ;
                    ns1:oahasEndSelector [ a ns1:oaXPathSelector ;
                            rdf:value "Page 24" ] ;
                    ns1:oahasStartSelector [ a ns1:oaXPathSelector ;
                            rdf:value "Page 23" ] ] ;
            ns1:oahasSource ns4:DIN_SPEC_91345 ],
        [ a ns1:oaSpecificResource ;
            ns2:format "pdf" ;
            ns1:oahasSelector [ a ns1:oaRangeSelector ;
                    ns1:oahasEndSelector [ a ns1:oaXPathSelector ;
                            rdf:value "Page 24" ] ;
                    ns1:oahasStartSelector [ a ns1:oaXPathSelector ;
                            rdf:value "Page 23" ] ] ;
            ns1:oahasSource ns4:DIN_SPEC_91345 ] .

ns4:RFC_1122 a owl:NamedIndividual,
        ns8:Document,
        ns4:Publication,
        ns4:Standard ;
    rdfs:label "RFC 1122"@en ;
    ns2:creator ns4:IETF ;
    ns2:title "Requirements for Internet Hosts -- Communication Layers"@en ;
    rdfs:comment "This is one RFC of a pair that defines and discusses the requirements for Internet host software.  This RFC covers the communications protocol layers: link layer, IP layer, and transport layer; its companion RFC-1123 covers the application and support protocols."@en ;
    ns8:maker ns4:IETF ;
    ns4:hasClassification ns4:IIRAConnectivity,
        ns4:NetworkLayer ;
    ns4:hasOfficialResource <https://tools.ietf.org/html/rfc1122> ;
    ns4:hasPublisher ns4:IETF .

ns4:RFC_2818 a owl:NamedIndividual,
        ns8:Document,
        ns4:Publication,
        ns4:Standard ;
    rdfs:label "HTTPS"@en,
        "RFC 2818"@en ;
    ns2:creator ns4:IETF ;
    rdfs:comment "This memo describes how to use TLS to secure HTTP connections over  the Internet. Current practice is to layer HTTP over SSL (the predecessor to TLS), distinguishing secured traffic from insecure traffic by the use of a different server port. This document documents that practice using TLS. A companion document describes a method for using HTTP/TLS over the same port as normal HTTP [RFC2817]."@en ;
    ns8:maker ns4:IETF ;
    ns4:hasClassification ns4:IDSRAMSecurity,
        ns4:IDSRAMSystemLayer ;
    ns4:hasPublisher ns4:IETF .

ns4:RFC_4511 a owl:NamedIndividual,
        ns8:Document,
        ns4:Publication,
        ns4:TechnicalSpecification ;
    rdfs:label "LDAP"@en ;
    ns2:creator ns4:IETF,
        ns4:sebastian ;
    ns2:title "Lightweight Directory Access Protocol"@en ;
    ns8:maker ns4:IETF ;
    ns4:hasDeveloper ns4:IETF ;
    ns4:hasOfficialResource <https://tools.ietf.org/html/rfc4511> ;
    ns4:hasPublisher ns4:IETF ;
    ns4:hasWikipediaArticle <https://en.wikipedia.org/wiki/Lightweight_Directory_Access_Protocol> ;
    ns5:hasTargetConcern ns4:CrossDomainIdentityManagement .

ns4:RFC_7252 a owl:NamedIndividual,
        ns8:Document,
        ns4:Publication,
        ns4:Standard ;
    rdfs:label "RFC 7252"@en ;
    ns2:creator ns4:IETF ;
    ns2:title "The Constrained Application Protocol"@en ;
    rdfs:comment "The Constrained Application Protocol (CoAP) is a specialized web transfer protocol for use with constrained nodes and constrained (e.g., low-power, lossy) networks.  The nodes often have 8-bit microcontrollers with small amounts of ROM and RAM, while constrained networks such as IPv6 over Low-Power Wireless Personal Area Networks (6LoWPANs) often have high packet error rates and a typical throughput of 10s of kbit/s.  The protocol is designed for machine-to-machine (M2M) applications such as smart energy and building automation."@en ;
    ns6:altLabel "CoAP"@en ;
    ns8:maker ns4:IETF ;
    ns4:hasClassification ns4:IIRAOperationsDomain,
        ns4:TansportLayer ;
    ns4:hasOfficialResource <https://tools.ietf.org/html/rfc7252> ;
    ns4:hasPublicationDate "2014-06-01"^^xsd:date ;
    ns4:hasPublisher ns4:IETF .

ns4:RFC_7540 a owl:NamedIndividual,
        ns8:Document,
        ns4:Publication,
        ns4:Standard ;
    rdfs:label "HTTP/2"@en,
        "RFC 7540"@en ;
    ns2:creator ns4:IETF ;
    rdfs:comment """This specification describes an optimized expression of the semantics of the Hypertext Transfer Protocol (HTTP), referred to as HTTP version 2 (HTTP/2).  HTTP/2 enables a more efficient use of network resources and a reduced perception of latency by introducing header field compression and allowing multiple concurrent exchanges on the same connection.  It also introduces unsolicited push of  representations from servers to clients.

This specification is an alternative to, but does not obsolete, the HTTP/1.1 message syntax.  HTTP's existing semantics remain unchanged."""@en ;
    ns8:maker ns4:IETF ;
    ns4:hasClassification ns4:IDSRAMInteroperability,
        ns4:IDSRAMSystemLayer,
        ns4:IIRAFunctionalViewpoint,
        ns4:RAMICommunicationlayer,
        ns4:TansportLayer ;
    ns4:hasPublisher ns4:IETF .

ns4:RFC_768 a owl:NamedIndividual,
        ns4:Standard ;
    rdfs:label "RFC 768"@en ;
    ns2:creator ns4:IETF ;
    ns2:title "User Datagram Protocol (UDP)"@en ;
    rdfs:comment "In computer networking, the User Datagram Protocol (UDP) is one of the core members of the Internet protocol suite. The protocol was designed by David P. Reed in 1980 and formally defined in RFC 768. With UDP, computer applications can send messages, in this case referred to as datagrams, to other hosts on an Internet Protocol (IP) network. Prior communications are not required in order to set up communication channels or data paths."@en ;
    ns8:maker ns4:IETF ;
    ns4:hasClassification ns4:TansportLayer ;
    ns4:hasDBpediaResource <http://dbpedia.org/resource/User_Datagram_Protocol> ;
    ns4:hasOfficialResource <https://tools.ietf.org/html/rfc768> ;
    ns4:hasPublisher ns4:IETF ;
    ns4:hasWikipediaArticle <https://en.wikipedia.org/wiki/User_Datagram_Protocol> .

ns4:ROLL a owl:NamedIndividual,
        ns8:Document,
        ns4:Publication,
        ns4:TechnicalSpecification ;
    rdfs:label "ROLL"@en ;
    ns2:creator ns4:sebastian ;
    rdfs:comment "ROLL / RPL (IPv6 routing for low power/lossy networks) (source: https://www.postscapes.com/internet-of-things-protocols/)"@en ;
    ns4:hasOfficialResource <https://datatracker.ietf.org/wg/roll/> .

ns4:RPMA a owl:NamedIndividual,
        ns8:Document,
        ns4:Publication,
        ns4:TechnicalSpecification ;
    rdfs:label "RPMA"@en ;
    ns2:creator ns4:sebastian ;
    rdfs:comment "RPMA (Random phase multiple access) A technology communication system employing direct-sequence spread spectrum (DSSS) with multiple access. (source: https://www.postscapes.com/internet-of-things-protocols/)"@en ;
    ns4:hasWikipediaArticle <https://en.wikipedia.org/wiki/Random_phase_multiple_access> .

ns4:RadioActivityControl a owl:NamedIndividual,
        ns4:Concern ;
    rdfs:label "Radio activity control"@en ;
    ns7:hasStakeholder <http://dbpedia.org/ontology/developer> ;
    rdfs:comment "The user shall be able to control the radio activity of the system."@en ;
    rdfs:seeAlso "IoT-A Requirement UNI.021" ;
    ns5:supports ns4:EnergyControl .

ns4:ReactiveStreams a owl:NamedIndividual,
        ns8:Document,
        ns4:Publication,
        ns4:TechnicalSpecification ;
    rdfs:label "Reactive Streams"@en ;
    ns2:creator ns4:sebastian ;
    rdfs:comment "A standard for asynchronous stream processing with non-blocking back pressure on the JVM. (source: https://www.postscapes.com/internet-of-things-protocols/)"@en ;
    ns4:hasOfficialResource <http://www.reactive-streams.org/> .

ns4:Regulatory_Compliance a owl:NamedIndividual,
        ns4:Concern ;
    rdfs:label "Regulatory Compliance"@en ;
    ns2:creator ns4:MuhammadUsman ;
    rdfs:comment "Organizations are ultimately legally responsible for their process compliance and data security, Even though the data is in a public cloud."@en ;
    rdfs:seeAlso <https://dl.acm.org/citation.cfm?doid=3286606.3286865> ;
    ns6:narrower ns4:Compliance ;
    ns4:hasWikipediaArticle <https://en.wikipedia.org/wiki/Regulatory_compliance> .

ns4:RiskManagement a owl:NamedIndividual,
        ns4:Concern ;
    rdfs:label "Risk Management"@en ;
    ns2:creator ns4:MuhammadUsman ;
    rdfs:comment """Organizations will be generally exposed to a broad range of different risks, by adopting the cloud computing. Managing these risks is very important concern, as the successful implementation of cloud computing relies upon the appropriate managing, reducing, as well as mitigating these risks linked to
cloud computing"""@en ;
    rdfs:seeAlso <https://dl.acm.org/citation.cfm?doid=3108421.3108426> ;
    ns4:hasDBpediaResource <http://dbpedia.org/page/Risk_management> ;
    ns4:hasWikipediaArticle <https://en.wikipedia.org/wiki/Risk_management> ;
    ns5:supports ns4:BusinessContext .

ns4:SCIM a owl:NamedIndividual,
        ns8:Document,
        ns4:Publication,
        ns4:TechnicalSpecification ;
    rdfs:label "SCIM"@en ;
    ns2:creator ns4:irlan,
        ns4:sebastian ;
    ns2:title "IETF System for Cross-domain Identity Management (SCIM) 2.0"@en ;
    ns3:associatedWith ns4:FiwareSecurity,
        ns4:RFC_7642,
        ns4:RFC_7643,
        ns4:RFC_7644 ;
    rdfs:comment "The System for Cross-domain Identity Management (SCIM) specification is designed to make managing user identities in cloud-based applications and services easier. The specification suite seeks to build upon experience with existing schemas and deployments, placing specific emphasis on simplicity of development and integration, while applying existing authentication, authorization, and privacy models. Its intent is to reduce the cost and complexity of user management operations by providing a common user schema and extension model, as well as binding documents to provide patterns for exchanging this schema using standard protocols. In essence: make it fast, cheap, and easy to move users in to, out of, and around the cloud."@en ;
    ns8:maker ns4:IETF ;
    ns4:hasDBpediaResource <http://dbpedia.org/resource/System_for_Cross-domain_Identity_Management> ;
    ns4:hasPublisher ns4:IETF ;
    ns4:hasWikipediaArticle <https://en.wikipedia.org/wiki/System_for_Cross-domain_Identity_Management> ;
    ns5:hasTargetConcern ns4:CrossDomainIdentityManagement .

ns4:SelectionOfServiceProvider a owl:NamedIndividual,
        ns4:Concern ;
    rdfs:label "Selection of Service Provider"@en ;
    ns2:creator ns4:MuhammadUsman ;
    rdfs:comment """Due to the diversity of cloud computing service suppliers, it is a challenge for organizations to pick am appropriate service supplier. In selection of a cloud provider, organizations ought to look at different elements, like the reputation and size of the company of service supplier, in terms of number of employees,
share of the market, as well as their other resources"""@en ;
    rdfs:seeAlso <https://dl.acm.org/citation.cfm?doid=3108421.3108426> ;
    ns4:hasWikipediaArticle <https://en.wikipedia.org/wiki/Service_provider> ;
    ns5:supports ns4:BusinessContext,
        ns4:CloudComputing .

ns4:ServiceDescriptions rdfs:seeAlso "IoT-A Requirement UNI.244" .

ns4:Service_Recovery a owl:NamedIndividual,
        ns4:Concern ;
    rdfs:label "Service Recovery"@en ;
    ns2:creator ns4:MuhammadUsman ;
    rdfs:comment "Organizations should make sure that the cloud provider imitates the data and provides services in case the major site is down. Find out the time to restore services and the data loss if any, in case the chief site goes down."@en ;
    rdfs:seeAlso <https://dl.acm.org/citation.cfm?doid=3286606.3286865> ;
    ns4:hasWikipediaArticle <https://en.wikipedia.org/wiki/Service_recovery> ;
    ns5:supports ns4:CloudComputing,
        ns4:Reliability .

ns4:Software_Updates a owl:NamedIndividual,
        ns4:Concern ;
    rdfs:label "Software Updates"@en ;
    ns2:creator ns4:MuhammadUsman ;
    rdfs:comment "Software update is the process that prevents compromise an IoT based  system. Organizations are yet to be geared up with mechanisms to Remotely Patch Connected Devices."@en ;
    rdfs:seeAlso <https://ieeexplore.ieee.org/document/7919553> ;
    ns4:hasWikipediaArticle <https://en.wikipedia.org/wiki/Wikipedia:Software_updates> ;
    ns5:supports ns4:Evolvability .

ns4:SpatialModeling a owl:NamedIndividual,
        ns4:Concern ;
    rdfs:label "Spatial modeling"@en ;
    rdfs:comment "A system shall have a semantic understanding of distance and location."@en ;
    rdfs:seeAlso "IoT-A Requirement UNI.098" ;
    ns4:hasDBpediaResource <http://dbpedia.org/resource/Spatial_analysis> ;
    ns5:supports ns4:DataDescription,
        ns4:SemanticInteroperability .

ns4:SyntacticInteroperablity rdfs:seeAlso "IoT-A Requirement UNI.311",
        "IoT-A Requirement UNI.312",
        "IoT-A Requirement UNI.313",
        "IoT-A Requirement UNI.315" .

ns4:SystemEvolution a owl:NamedIndividual,
        ns4:Concern ;
    rdfs:label "System evolution"@en ;
    ns2:creator ns4:sebastian ;
    rdfs:comment "Software evolution is the term used in software engineering (specifically software maintenance) to refer to the process of developing software initially, then repeatedly updating it for various reasons. (source: wikipedia)"@en ;
    rdfs:seeAlso "IoT-A Requirement UNI.211",
        "IoT-A Requirement UNI.229" ;
    ns4:hasDBpediaResource <http://dbpedia.org/resource/Software_evolution> ;
    ns5:supports ns4:Evolvability .

ns4:SystemRecovery a owl:NamedIndividual,
        ns4:Concern ;
    rdfs:label "System Recovery"@en ;
    ns2:creator ns4:sebastian ;
    rdfs:comment ""@en ;
    ns5:supports ns4:Reliability .

ns4:ThingMobility a owl:NamedIndividual,
        ns4:Concern ;
    rdfs:label "Thing mobility"@en ;
    ns2:creator ns4:sebastian ;
    rdfs:comment "A Thing in terms of Internet of Things (IoT) needs to be moveable."@en ;
    rdfs:seeAlso "IoT-A Requirement UNI.050",
        "IoT-A Requirement UNI.233" ;
    ns5:supports ns4:DataAccess,
        ns4:IoT,
        ns4:ServiceDeployment .

ns4:TrustedConnector a owl:NamedIndividual,
        ns4:Technology ;
    rdfs:label "IDS Trusted Connector"@en ;
    ns2:creator ns4:sebastian ;
    ns3:associatedWith ns4:DIN_SPEC_27070,
        ns4:IDSRAMReferenceArchitectureModel ;
    rdfs:comment "The advent of the Industrial Internet of Things (IIoT) also raises challenges with respect to security and privacy of sensitive and personal data that is created by sensors and processed by services hosted in different administrative domains. The Industrial Data Space initiative addresses these challenges and proposes a secure edge gateway platform named \"Trusted Connector\". In this report, we introduce the main security building blocks of the Trusted Connector and point out how they help protecting business-critical data and preserving the user's privacy."@en ;
    ns4:hasOfficialResource <https://arxiv.org/abs/1804.09442> ;
    ns5:alignsWith ns4:DIN_SPEC_27070 .

ns4:UnreliableNetwork a owl:NamedIndividual,
        ns4:Concern ;
    rdfs:label "Unreliable Network"@en ;
    ns2:creator ns4:sebastian ;
    ns7:hasStakeholder "Developer"@en,
        "System Architect"@en ;
    rdfs:comment "Productive systems must inherently cover issues caused by unreliable networks."@en ;
    rdfs:seeAlso "IoT-A Requirement UNI.308",
        "IoT-A Requirement UNI.318" ;
    ns5:supports ns4:Reliability .

ns4:VendorLockin a owl:NamedIndividual,
        ns4:Concern ;
    rdfs:label "Vendor Lockin"@en ;
    ns2:creator ns4:MuhammadUsman ;
    rdfs:comment """There is a lot of competition among vendors to dominate the cloud market. According to Columbus’ report, a study conducted by IDG Cloud Computing
Study realized that Cloud investment rose by 19% in larger scale enterprises consisting of more than a thousand employees who spend a mean of $3.3 million
annually."""@en ;
    rdfs:seeAlso <https://ieeexplore.ieee.org/document/7987175> ;
    ns4:hasWikipediaArticle <https://en.wikipedia.org/wiki/Vendor_lock-in> ;
    ns5:supports ns4:BusinessContext,
        ns4:CloudComputing .

ns4:VirtualEntities rdfs:seeAlso "IoT-A Requirement UNI.409" .

ns4:abbreviation a owl:DatatypeProperty ;
    rdfs:label "has Abbreviated Name"@en ;
    rdfs:comment "Abbreviated  name of the thing."@en ;
    rdfs:domain owl:Thing ;
    rdfs:range rdf:PlainLiteral .

ns4:alignesWith a owl:ObjectProperty,
        owl:SymmetricProperty ;
    rdfs:label "alignes With"@en ;
    rdfs:comment "indicates that some Standard Classification entity has a similar scope as another. This property most probably is symmetric but not transitive."@en ;
    rdfs:domain ns4:StandardClassification ;
    rdfs:range ns4:StandardClassification ;
    rdfs:subPropertyOf ns3:associatedWith .

ns4:belongsTo a owl:ObjectProperty ;
    rdfs:label "belongs To"@en ;
    ns2:creator ns4:irlan ;
    rdfs:comment "A Standard Organization that belongs to the country"@en ;
    rdfs:domain ns4:StandardOrganization ;
    rdfs:range <http://dbpedia.org/ontology#Country> .

ns4:domainName a owl:DatatypeProperty ;
    rdfs:label "has Domain Name"@en ;
    rdfs:comment "Points the Standard with the name of the Industrial Domain"@en ;
    rdfs:domain ns4:Domain ;
    rdfs:range rdf:PlainLiteral .

ns4:formationDate a owl:DatatypeProperty,
        owl:FunctionalProperty ;
    rdfs:label "has Formation Date"@en ;
    rdfs:comment "Formation date of the Organization"@en ;
    rdfs:domain ns4:StandardOrganization ;
    rdfs:range xsd:date .

ns4:frames a owl:ObjectProperty ;
    rdfs:label "frames"@en ;
    rdfs:comment "A relation specifying that a vewpoint regards a Concern."@en ;
    rdfs:domain ns4:Viewpoint ;
    rdfs:range ns4:Concern ;
    rdfs:subPropertyOf ns3:associatedWith ;
    ns4:hasOfficialResource <http://www.iso-architecture.org/42010/> .

ns4:hasAvailableLanguage a owl:ObjectProperty ;
    rdfs:label "has Available Language"@en,
        "hasAvailableLanguage"@en ;
    ns2:creator ns4:irlan ;
    rdfs:comment "Languages in which the document of the Standard is available, e.g., English, French, Spanish"@en,
        "Points to Languages in which the standard document is available, e.g., English, French, etc. Defined as subProperty of dcterms:language"@en ;
    rdfs:domain ns8:Document ;
    rdfs:range ns2:LinguisticSystem ;
    rdfs:subPropertyOf ns2:language .

ns4:hasClassification a owl:ObjectProperty ;
    rdfs:label "has Classification"@en ;
    ns2:creator ns4:irlan ;
    rdfs:comment "An Standard is isCategorizedBy a given Categorization Area which is connected to a specific Standarization Initiative"@en ;
    rdfs:domain ns4:Standard ;
    rdfs:range ns4:StandardClassification .

ns4:hasDBpediaResource a owl:DatatypeProperty .

ns4:hasDeveloper a owl:ObjectProperty ;
    rdfs:label "has Developer"@en ;
    ns2:creator ns4:irlan ;
    rdfs:comment "The organization that developed this Standard"@en ;
    rdfs:domain ns4:Publication ;
    rdfs:range ns4:StandardOrganization ;
    rdfs:subPropertyOf ns8:maker .

ns4:hasDomain a owl:ObjectProperty ;
    ns2:creator ns4:irlan ;
    rdfs:domain ns4:Publication ;
    rdfs:range ns4:Domain .

ns4:hasEdition a owl:DatatypeProperty ;
    rdfs:label "has Edition"@en ;
    rdfs:comment "Indicates the current Edition/Version number of the document."@en ;
    rdfs:domain ns8:Document ;
    rdfs:range xsd:float .

ns4:hasFileSize a owl:ObjectProperty ;
    rdfs:label "has File Size"@en ;
    ns2:creator ns4:irlan ;
    rdfs:comment "The size of document file in some unit, e.g., 104 Kilobyte."@en ;
    rdfs:domain ns8:Document ;
    rdfs:range <http://www.ontology-of-units-of-measure.org/resource/om-2/Measure> ;
    rdfs:seeAlso <https://webstore.iec.ch/webstore/webstore.nsf/xpFAQ.xsp?Open&id=ADMN-7NALM5> ;
    ns6:note """1. Reference for om2:Measure <http://www.ontology-of-units-of-measure.org/page/om-2/Measure>
                         2. om2:Measure om2:hasNumericalValue xsd:float;
                         3. om2:Measure om2:hasUnit om2:Unit;
                         4. om2:hasUnit om2:InformationCapacityUnit; is another possibility for range that could not be verified.
                         5. rdfs:seeAlso <http://www.ontology-of-units-of-measure.org/page/om-2/kilobyte> 
                         6. Documentation on Measure <https://github.com/HajoRijgersberg/OM>""" .

ns4:hasHeadquaterIn a owl:ObjectProperty ;
    rdfs:label "has Headquater In"@en ;
    ns2:creator ns4:irlan ;
    rdfs:comment "Denotes the countries in which the Headquarter of the organization who publishes the Standart"@en ;
    rdfs:domain ns4:StandardOrganization ;
    rdfs:range <http://dbpedia.org/ontology#Place> .

ns4:hasICS a owl:ObjectProperty ;
    rdfs:label "has ICS"@en ;
    rdfs:comment "Serves as a catalogue of International Classification For Standards"@en ;
    rdfs:domain ns4:Publication ;
    rdfs:range ns4:InternationalClassificationForStandards .

ns4:hasImplementationFormat a owl:DatatypeProperty ;
    rdfs:label "has Implementation Format"@en ;
    rdfs:comment "Describes the name of the implementation or serialization format of the Publication, e.g., XML, Document, binary, batch"@en ;
    rdfs:domain ns4:Publication ;
    rdfs:range rdfs:Literal .

ns4:hasMotivation a owl:ObjectProperty ;
    rdfs:domain ns4:Publication ;
    rdfs:range <http://purl.org/spar/deo/Motivation> .

ns4:hasObjective a owl:DatatypeProperty ;
    rdfs:label "has Objective"@en ;
    rdfs:comment "Specifies the objectives for the different ISA 95 levels."@en ;
    rdfs:domain ns4:ISA95Level ;
    rdfs:range xsd:string .

ns4:hasOfficialResource a owl:DatatypeProperty ;
    rdfs:domain ns4:Publication ;
    rdfs:range xsd:anyURI .

ns4:hasOntology a owl:DatatypeProperty ;
    rdfs:label "has Ontology"@en ;
    rdfs:comment "Point to the URL of a recognized Ontology representation of the Standard"@en ;
    rdfs:domain ns4:Publication ;
    rdfs:range xsd:anyURI .

ns4:hasOpenResource a owl:AnnotationProperty .

ns4:hasPages a owl:DatatypeProperty ;
    rdfs:label "has Pages"@en ;
    rdfs:comment "Indicates the number of pages in the document."@en ;
    rdfs:domain ns8:Document ;
    rdfs:range xsd:integer .

ns4:hasPreviousVersion a owl:ObjectProperty ;
    rdfs:label "has Previous Version"@en ;
    rdfs:comment "Indicates the list of Standards that are previous versions of a Standard. For example,IEC 60038:2009 has IEC 60038:1983+AMD1:1994+AMD2:1997,IEC 60038:1983/AMD2:1997,IEC 60038:1983/AMD1:1994,IEC 60038:1983,IEC 60038:1975/AMD1:1977,IEC 60038:1975,IEC 60038:1967,IEC 60038:1954,IEC 60038:1938,IEC 60038:1927 as previous versions."@en ;
    rdfs:subPropertyOf ns4:relatedTo .

ns4:hasPublicationDate a owl:DatatypeProperty ;
    rdfs:label "has Publication Date"@en ;
    rdfs:comment "Publication date of the Publication"@en ;
    rdfs:domain ns4:Publication ;
    rdfs:range xsd:date .

ns4:hasPublisher a owl:ObjectProperty ;
    rdfs:label "has Publisher"@en ;
    ns2:creator ns4:irlan ;
    rdfs:comment "The organization that published this Standard"@en ;
    rdfs:domain ns4:Publication ;
    rdfs:range ns4:StandardOrganization ;
    rdfs:subPropertyOf ns8:maker .

ns4:hasStabilityDate a owl:DatatypeProperty ;
    rdfs:label "has Stability Date"@en ;
    rdfs:comment "Stability date of a publication. Publications are valid for a certain period, i.e., the Stability Period. This property defines the end of the stability period."@en ;
    rdfs:domain ns4:Publication ;
    rdfs:range xsd:gYear ;
    rdfs:seeAlso <https://webstore.iec.ch/webstore/webstore.nsf/xpFAQ.xsp?Open&id=ADMN-7NALM5> ;
    ns6:note "The data specified is not actually a Date but an Year" .

ns4:hasStatus a owl:DatatypeProperty ;
    rdfs:label "has Status"@en ;
    rdfs:comment "Publication status of the Standard, e.g., Valid, Revised, Published, under preparation, Released"@en ;
    rdfs:domain ns4:Publication ;
    rdfs:range rdfs:Literal .

ns4:hasTag a owl:DatatypeProperty ;
    rdfs:range <http://purl.org/muto/core#Tag>,
        rdfs:Literal .

ns4:hasTargetConcern a owl:ObjectProperty ;
    rdfs:label "has Target Concern"@en ;
    rdfs:comment "The relation declaring that a standard is relevant or targets a certain concern."@en ;
    rdfs:domain ns4:Standard ;
    rdfs:range ns4:Concern ;
    rdfs:subPropertyOf ns3:associatedWith .

ns4:hasTask a owl:DatatypeProperty ;
    rdfs:label "has Task"@en ;
    rdfs:comment "Specifies the tasks for the different ISA 95 levels."@en ;
    rdfs:domain ns4:ISA95Level ;
    rdfs:range xsd:string .

ns4:hasTechnicalCommittee a owl:ObjectProperty ;
    rdfs:label "has Technical Committee"@en ;
    rdfs:comment "Specifies the Technical Committee or a Sub-Committee that is responsible for creation and maintenance of a standard"@en ;
    rdfs:domain ns4:Publication ;
    rdfs:range ns4:TechnicalCommittee .

ns4:hasWikipediaArticle a owl:DatatypeProperty .

ns4:iShare a owl:NamedIndividual,
        ns8:Organization ;
    rdfs:label "iShare"@en ;
    ns3:associatedWith ns4:HTTP,
        ns4:ISO_9594,
        ns4:REST,
        ns4:RFC_5246,
        ns4:RFC_7519,
        ns4:XACML ;
    rdfs:comment "iSHARE is a uniform set of agreements or a scheme for identification, authentication and authorization. All companies that join the iSHARE Scheme comply with the set of agreements. They all use the same methods to both provide and gain access to data. (source: iShare: 'It is not a platform…')"@en ;
    ns4:hasOfficialResource <https://www.ishareworks.org/> ;
    ns5:hasTargetConcern ns4:Identification,
        ns4:Interoperability .

ns4:introductionXtee a owl:NamedIndividual,
        ns8:Document,
        ns4:Publication,
        ns4:TechnicalReport ;
    rdfs:label "Introduction of X-tee"@en ;
    ns2:creator ns4:EstonianInformationSystemAuthority ;
    rdfs:comment "It is a guide intended for those who want to acquaint themselves more thoroughly with the X-tee (e.g. theose who are working for an organisation which will soon join the X-tee). It introduces the X-tee’s complex terminological system slowly and in a comprehensible way, so that the reader can painlessly achieve the preliminary familiarity with the X-tee necessary to engage with more explicitly technical and complex manuals. (source: https://www.ria.ee/en/state-information-system/x-tee/introduction-x-tee.html)"@en ;
    ns8:maker ns4:EstonianInformationSystemAuthority ;
    ns4:hasClassification ns4:xRoadDeploymentView,
        ns4:xRoadProtocolsInterfaces,
        ns4:xRoadSystemComponents,
        ns4:xRoadTechnologyMatrix ;
    ns4:hasOfficialResource <https://www.ria.ee/en/state-information-system/x-tee/introduction-x-tee.html> ;
    ns4:hasPublisher ns4:EstonianInformationSystemAuthority .

ns4:isImplementationOf a owl:ObjectProperty ;
    rdfs:label "is Implementation Of"@en ;
    ns2:creator ns4:irlan ;
    rdfs:comment "Represent the relation that connects two standards when standard A is the implementation of standard B, e.g., B2MML isImplementationOf ISA-95."@en ;
    rdfs:subPropertyOf ns4:relatedTo .

ns4:orgName a owl:DatatypeProperty ;
    rdfs:label "Org Name"@en ;
    rdfs:comment "Name of the Organization"@en ;
    rdfs:domain ns4:StandardOrganization ;
    rdfs:range rdf:PlainLiteral .

ns4:seeAlso a owl:AnnotationProperty .

ns4:stoPartName a owl:DatatypeProperty ;
    rdfs:label "std Part Name"@en ;
    rdfs:comment "Name of the standard part."@en ;
    rdfs:domain ns4:StandardPart ;
    rdfs:range xsd:string .

ns4:useStructureOf a owl:ObjectProperty ;
    rdfs:label "use Structure Of"@en ;
    ns2:creator ns4:irlan ;
    rdfs:comment "Standard A uses the structure of Standard B. For example, OPC UA uses Structure Of IEC_61804 (EDDL)"@en ;
    rdfs:subPropertyOf ns4:relatedTo .

ns4:uses a owl:ObjectProperty ;
    rdfs:label "uses"@en ;
    ns2:creator ns4:irlan ;
    rdfs:comment "Defines that Standard A uses Standard B. For example, IEC_62714(AML) uses MathML."@en ;
    rdfs:subPropertyOf ns4:relatedTo .

ns4:xRoadDeploymentViewAnno a owl:NamedIndividual,
        ns1:oaAnnotation ;
    ns1:oahasBody ns4:xRoadDeploymentView ;
    ns1:oahasTarget [ a ns1:oaSpecificResource ;
            ns1:oahasSelector [ a ns1:oaRangeSelector ;
                    ns1:oahasEndSelector [ a ns1:oaXPathSelector ;
                            rdf:value "Page 16" ] ;
                    ns1:oahasStartSelector [ a ns1:oaXPathSelector ;
                            rdf:value "Page 15" ] ] ;
            ns1:oahasSource ns4:X_Road_Architecture_Technical_Specification ] .

ns4:xRoadProtocolsInterfacesAnno a owl:NamedIndividual,
        ns1:oaAnnotation ;
    ns1:oahasBody ns4:xRoadProtocolsInterfaces ;
    ns1:oahasTarget [ a ns1:oaSpecificResource ;
            ns1:oahasSelector [ a ns1:oaRangeSelector ;
                    ns1:oahasEndSelector [ a ns1:oaXPathSelector ;
                            rdf:value "Page 14" ] ;
                    ns1:oahasStartSelector [ a ns1:oaXPathSelector ;
                            rdf:value "Page 10" ] ] ;
            ns1:oahasSource ns4:X_Road_Architecture_Technical_Specification ] .

ns4:xRoadSystemComponentsAnno a owl:NamedIndividual,
        ns1:oaAnnotation ;
    ns1:oahasBody ns4:xRoadSystemComponents ;
    ns1:oahasTarget [ a ns1:oaSpecificResource ;
            ns1:oahasSelector [ a ns1:oaRangeSelector ;
                    ns1:oahasEndSelector [ a ns1:oaXPathSelector ;
                            rdf:value "Page 10" ] ;
                    ns1:oahasStartSelector [ a ns1:oaXPathSelector ;
                            rdf:value "Page 7" ] ] ;
            ns1:oahasSource ns4:X_Road_Architecture_Technical_Specification ] .

ns4:xRoadTechnologyMatrixAnno a owl:NamedIndividual,
        ns1:oaAnnotation ;
    ns1:oahasBody ns4:xRoadTechnologyMatrix ;
    ns1:oahasTarget [ a ns1:oaSpecificResource ;
            ns1:oahasSelector [ a ns1:oaRangeSelector ;
                    ns1:oahasEndSelector [ a ns1:oaXPathSelector ;
                            rdf:value "Page 15" ] ;
                    ns1:oahasStartSelector [ a ns1:oaXPathSelector ;
                            rdf:value "Page 14" ] ] ;
            ns1:oahasSource ns4:X_Road_Architecture_Technical_Specification ] .

ns5:frames a owl:ObjectProperty ;
    rdfs:label "frames"@en ;
    rdfs:comment "A relation specifying that a vewpoint regards a Concern."@en ;
    rdfs:domain ns4:StandardClassification ;
    rdfs:range ns4:Concern ;
    rdfs:subPropertyOf ns3:associatedWith ;
    ns4:hasOfficialResource <http://www.iso-architecture.org/42010/> .

ns5:hasTargetConcern a owl:AnnotationProperty,
        owl:ObjectProperty ;
    rdfs:label "has Target Concern"@en ;
    rdfs:comment "The relation declaring that a standard is relevant or targets a certain concern."@en ;
    rdfs:domain [ a owl:Class ;
            owl:unionOf ( ns4:Standard ns4:StandardizationFramework ) ] ;
    rdfs:range ns4:Concern ;
    rdfs:subPropertyOf ns3:associatedWith .

ns5:supports a owl:ObjectProperty ;
    rdfs:label "supports" ;
    rdfs:comment "A relation between two different concerns where dealing with the subject Concern supports in achieving the object concern"@en ;
    rdfs:domain ns4:Concern ;
    rdfs:range ns4:Concern .

: a owl:Ontology ;
    ns2:created "2017-01-25"^^xsd:date,
        "2019-06-09"^^xsd:date ;
    ns2:creator <http://data.semanticweb.org/person/steffen-lohmann>,
        <http://http://sda.cs.uni-bonn.de/people/irlan-grangel-gonzalez/>,
        ns4:Priyanka,
        ns4:sebastian,
        <https://www.linkedin.com/in/paul-baptista-601177b2> ;
    ns2:modified "2017-09-08"^^xsd:date,
        "2019-06-09"^^xsd:date,
        "2019-07-21"^^xsd:date ;
    ns2:publisher <http://de.dbpedia.org/resource/Fraunhofer-Gesellschaft> ;
    ns2:rights "This work is distributed under a Creative Commons Attribution License (http://creativecommons.org/licenses/by/3.0/)."@en ;
    ns2:title "Industrial IoT Architecture Ontology"@en,
        "Standards Ontology"@en ;
    ns10:preferredNamespacePrefix "sto",
        "sto_iot" ;
    ns10:preferredNamespaceUri "https://w3id.org/i40/sto#" ;
    ns11:repository <https://github.com/i40-Tools/StandardsOntology> ;
    rdfs:comment "An ontology to describe standards related to Industry 4.0 and Smart Manufacturing"@en,
        "An ontology to describe the landscape of IIoT, Industry 4.0 and Smart Manufacturing"@en,
        "The Internet of things (IoT) is the network of devices such as vehicles, and home appliances that contain electronics, software, sensors, actuators, and connectivity which allows these things to connect, interact and exchange data."@en ;
    owl:imports <https://raw.githubusercontent.com/i40-Tools/StandardOntology/master/concerns.ttl>,
        <https://raw.githubusercontent.com/i40-Tools/StandardOntology/master/sto.ttl> ;
    owl:versionIRI <https://w3id.org/i40/sto/iot/0.1/concerns/> ;
    owl:versionInfo "0.2",
        "0.3" ;
    ns4:hasDBpediaResource <http://dbpedia.org/page/Internet_of_things> ;
    ns4:hasOfficialResource <https://webstore.iec.ch/publication/153> ;
    ns4:hasWikipediaArticle <https://en.wikipedia.org/wiki/Internet_of_things> .

<https://w3id.org/ids/ram/Layer> a owl:Class ;
    rdfs:label "IDS RAM Layer"@en ;
    rdfs:subClassOf ns4:StandardClassification ;
    owl:equivalentClass [ a owl:Class ;
            owl:oneOf ( <https://w3id.org/ids/ram/BusinessLayer> <https://w3id.org/ids/ram/FunctionalLayer> <https://w3id.org/ids/ram/InformationLayer> <https://w3id.org/ids/ram/ProcessLayer> <https://w3id.org/ids/ram/SystemLayer> ) ] .

ns1:oahasBody a owl:AnnotationProperty .

ns1:oahasEndSelector a owl:AnnotationProperty .

ns1:oahasSelector a owl:AnnotationProperty .

ns1:oahasSource a owl:AnnotationProperty .

ns1:oahasStartSelector a owl:AnnotationProperty .

ns1:oahasTarget a owl:AnnotationProperty .

<n0151a891b36b43b2a7b8a60f988e2dafb1> rdfs:label "n0151a891b36b43b2a7b8a60f988e2dafb1" .

<n0151a891b36b43b2a7b8a60f988e2dafb11> rdfs:label "n0151a891b36b43b2a7b8a60f988e2dafb11" .

<n0151a891b36b43b2a7b8a60f988e2dafb15> rdfs:label "n0151a891b36b43b2a7b8a60f988e2dafb15" .

<n0151a891b36b43b2a7b8a60f988e2dafb23> rdfs:label "n0151a891b36b43b2a7b8a60f988e2dafb23" .

<n0151a891b36b43b2a7b8a60f988e2dafb31> rdfs:label "n0151a891b36b43b2a7b8a60f988e2dafb31" .

<n0151a891b36b43b2a7b8a60f988e2dafb4> rdfs:label "n0151a891b36b43b2a7b8a60f988e2dafb4" .

<n0151a891b36b43b2a7b8a60f988e2dafb42> rdfs:label "n0151a891b36b43b2a7b8a60f988e2dafb42" .

<n0151a891b36b43b2a7b8a60f988e2dafb49> rdfs:label "n0151a891b36b43b2a7b8a60f988e2dafb49" .

<n0151a891b36b43b2a7b8a60f988e2dafb7> rdfs:label "n0151a891b36b43b2a7b8a60f988e2dafb7" .

<http://dbpedia.org/ontology#Country> a owl:Class ;
    rdfs:label "Country" .

<http://dbpedia.org/ontology#Place> a owl:Class ;
    rdfs:label "Place" .

<http://org.semanticweb.owlapi/error#Error1> a owl:Class ;
    rdfs:label "Error1" .

ns12:description rdfs:label "Description"@en ;
    ns2:description "Description may include but is not limited to: an abstract, a table of contents, a graphical representation, or a free-text account of the resource."@en ;
    ns2:hasVersion <http://dublincore.org/usage/terms/history/#description-006> ;
    ns2:issued "1999-07-02"^^xsd:date ;
    ns2:modified "2008-01-14"^^xsd:date ;
    rdfs:comment "An account of the resource."@en ;
    rdfs:isDefinedBy ns12: ;
    ns6:note "A second property with the same name as this property has been declared in the dcterms: namespace (http://purl.org/dc/terms/).  See the Introduction to the document \"DCMI Metadata Terms\" (http://dublincore.org/documents/dcmi-terms/) for an explanation."@en .

ns12:title rdfs:label "Title"@en ;
    ns2:hasVersion <http://dublincore.org/usage/terms/history/#title-006> ;
    ns2:issued "1999-07-02"^^xsd:date ;
    ns2:modified "2008-01-14"^^xsd:date ;
    rdfs:comment "A name given to the resource."@en ;
    rdfs:isDefinedBy ns12: ;
    ns6:note "A second property with the same name as this property has been declared in the dcterms: namespace (http://purl.org/dc/terms/).  See the Introduction to the document \"DCMI Metadata Terms\" (http://dublincore.org/documents/dcmi-terms/) for an explanation."@en .

ns2:Agent a owl:Class ;
    rdfs:label "Agent" .

ns2:LinguisticSystem a owl:Class ;
    rdfs:label "Linguistic System" .

ns2:language a owl:ObjectProperty .

<http://purl.org/muto/core#Tag> a rdfs:Datatype,
        owl:Class ;
    rdfs:label "Tag" .

<http://purl.org/spar/deo/Motivation> a owl:Class ;
    rdfs:label "Motivation" .

<http://www.ontology-of-units-of-measure.org/resource/om-2/Measure> a owl:Class ;
    rdfs:label "Measure" .

<http://www.ontology-of-units-of-measure.org/resource/om-2/Unit> a owl:Class ;
    rdfs:label "Unit" .

ns3:Collection a owl:Class ;
    rdfs:label "Collection" .

ns3:Entity a owl:Class ;
    rdfs:label "Entity" .

xsd:gYear a rdfs:Datatype .

ns8:Agent a owl:Class ;
    rdfs:label "Agent" .

ns8:person a owl:Class ;
    rdfs:label "person" .

ns4:Agility a owl:NamedIndividual,
        ns4:Concern ;
    rdfs:comment """Agility as a key pillar that enables quick and astute business operational decisions for an OpenFog System. The predicted scale of the data generated by IoT means that it is highly unlikely that humans alone will be able to comprehend the data, derive knowledge and make wise decisions about how to best leverage their IoT assets for the benefit of their businesses. In the OpenFog architecture the agility pillar is about making sure that the valuable data generated in the IoT can be rapidly transformed into actionable insights that drive rapid decisions and further levels of automation to support business interest.
Spurce: OpenFog Consortum Architecture Whitepaper"""@en ;
    ns6:note "Publications referred: '<https://www.openfogconsortium.org/wp-content/uploads/OpenFog_Reference_Architecture_2_09_17-FINAL.pdf> OPFRA001.020817' '4.7 Agility Pillar' 'Page 31' " ;
    ns5:supports ns4:BusinessContext .

ns4:AiiData a owl:NamedIndividual,
        ns4:AiiClassification ;
    rdfs:label "AII Data Classification"@en ;
    ns4:isDescribedin ns4:IndustrialInternetArchitecture ;
    ns5:alignsWith ns4:IDSRAMInformationLayer,
        ns4:InformationDomain ;
    ns5:frames ns4:DataAnalytics,
        ns4:DataProcessing,
        ns4:Data_Collection,
        ns4:EdgeComputing,
        ns4:SemanticInteroperability .

ns4:AiiNetwork a owl:NamedIndividual,
        ns4:AiiClassification ;
    rdfs:label "AII Network Classification"@en ;
    ns4:isDescribedin ns4:IndustrialInternetArchitecture ;
    ns5:alignsWith ns4:IDSRAMSystemLayer,
        ns4:IIRAConnectivity,
        ns4:RAMICommunicationlayer,
        ns4:RAMIIntegrationLayer ;
    ns5:frames ns4:Communication,
        ns4:Connectivity,
        ns4:Identification,
        ns4:SyntacticInteroperability .

ns4:AiiSecurity a owl:NamedIndividual,
        ns4:AiiClassification ;
    rdfs:label "AII Security Classification"@en ;
    ns4:isDescribedin ns4:IndustrialInternetArchitecture ;
    ns5:alignsWith ns4:IDSRAMSecurity,
        ns4:IIRASecurity ;
    ns5:frames ns4:DataAccess,
        ns4:Security .

ns4:AllianceOfIndustrialInternet a owl:NamedIndividual,
        ns4:IIoTConsortium ;
    rdfs:label "Alliance of Industrial Internet"@en ;
    ns6:altLabel "工业互联网产业联盟"@cn ;
    ns4:hasHeadquaterIn <http://dbpedia.org/resource#China> ;
    ns4:seeAlso <http://www.aii-alliance.org/> .

ns4:Anonymity a owl:NamedIndividual,
        ns4:Concern ;
    rdfs:label "Anonymity"@en ;
    ns7:hasStakeholder <http://purl.oclc.org/NET/mvco.owl#EndUser> ;
    rdfs:comment "Anonymity is the guarantee for a user to interact with a system without being tracked or connected to its real-world identity."@en ;
    rdfs:seeAlso "IoT-A Requirement UNI.001",
        "IoT-A Requirement UNI.322",
        "UNI.322"@en ;
    ns4:hasDBpediaResource <http://dbpedia.org/resource/Anonymity>,
        <http://dbpedia.org/resource/Anonymous_web_browsing> ;
    ns5:supports ns4:Privacy .

ns4:ArrowheadProject a owl:NamedIndividual,
        ns8:Organization ;
    rdfs:label "Arrowhead Project" ;
    ns4:seeAlso <http://www.arrowhead.eu/> .

ns4:AssetManagement a owl:NamedIndividual,
        ns4:Concern ;
    rdfs:label "Asset Management"@en ;
    ns2:creator ns4:Priyanka ;
    rdfs:comment "The concern of being able to manage the system onboarding, configuration, policy, software/firmware updates and other lifecycle management operations."@en ;
    ns6:note "Publications referred: 'IIC:PUB:G1:V1.80:20170131' '6.1 THE CONTROL DOMAIN' 'Page 29' " ;
    ns4:hasWikipediaArticle <https://en.wikipedia.org/wiki/Asset_management#Physical_and_Infrastructure_asset_management> ;
    ns5:supports ns4:IoT .

ns4:BDVA a owl:NamedIndividual,
        ns8:Organization ;
    rdfs:label "Big Data Value Association" ;
    ns6:altLabel "BDVA" .

ns4:BdvaCommunicationConnectivity a owl:NamedIndividual,
        ns4:BdvaConcern,
        ns4:StandardClassification ;
    rdfs:label "BDVA Communication and Connectivity"@en ;
    ns2:creator ns4:sebastian ;
    rdfs:comment "Effective communication and connectivity mechanisms are necessary in providing support for Big Data. This area is separately further elaborated, along with various communication communities, such as the 5G community."@en ;
    ns4:isDescribedin ns4:BdvaSira ;
    ns5:frames ns4:Communication,
        ns4:DataAccess,
        ns4:DataAnalytics,
        ns4:Interoperability,
        ns4:QualityOfService,
        ns4:SemanticInteroperability,
        ns4:ServiceDescription .

ns4:BdvaDataSharingPlatforms a owl:NamedIndividual,
        ns4:BdvaConcern,
        ns4:StandardClassification ;
    rdfs:label "BDVA Data Sharing Platforms"@en ;
    ns2:creator ns4:sebastian ;
    ns3:associatedWith ns4:IDSRAMReferenceArchitectureModel,
        ns4:IIRA ;
    rdfs:comment "Data sharing and trading are seen as important ecosystem enablers in the data economy, although closed and personal data present particular challenges for the free flow of data. The following two conceptual solutions – Industrial Data Platforms (IDPs) and Personal Data Platforms (PDPs) – introduce new approaches to addressing this particular need to regulate closed proprietary and personal data."@en ;
    ns4:isDescribedin ns4:BdvaSira ;
    ns5:frames ns4:BusinessContext,
        ns4:DataEconomy,
        ns4:DataPublishing .

ns4:BdvaDataVisualizationAndUserInteraction a owl:NamedIndividual,
        ns4:BdvaConcern,
        ns4:StandardClassification ;
    rdfs:label "Data Visualisation and User Interaction"@en ;
    ns2:creator ns4:sebastian ;
    ns3:associatedWith ns4:IIRAUsageViewpoint,
        ns4:RAMIFunctionalLayer ;
    rdfs:comment "Engineering and DevOps for building Big Data Value systems: This topic will be elaborated in greater detail along with the NESSI Software and Service community."@en ;
    ns4:isDescribedin ns4:BdvaSira ;
    ns5:alignsWith ns4:IIRAUsageViewpoint,
        ns4:RAMIFunctionalLayer ;
    ns5:frames ns4:BigDataApplications .

ns4:BdvaDevelopmentEngineering a owl:NamedIndividual,
        ns4:BdvaConcern,
        ns4:StandardClassification ;
    rdfs:label "BDVA Engineering and DevOps"@en ;
    ns2:creator ns4:sebastian ;
    rdfs:comment "Engineering and DevOps for building Big Data Value systems: This topic will be elaborated in greater detail along with the NESSI Software and Service community."@en ;
    ns4:isDescribedin ns4:BdvaSira .

ns4:BdvaStandards a owl:NamedIndividual,
        ns4:BdvaConcern,
        ns4:StandardClassification ;
    rdfs:label "BDVA Standards"@en ;
    ns2:creator ns4:sebastian ;
    rdfs:comment "Standardisation of Big Data technology areas to facilitate data integration, sharing and interoperability"@en ;
    ns4:isDescribedin ns4:BdvaSira ;
    ns5:frames ns4:BusinessContext,
        ns4:Communication,
        ns4:DataEconomy,
        ns4:Interoperability .

ns4:BdvaThingsAssetsSensorsActuators a owl:NamedIndividual,
        ns4:BdvaConcern,
        ns4:StandardClassification ;
    rdfs:label "BDVA IoT CPS and Edge Computing"@en ;
    ns2:creator ns4:sebastian ;
    rdfs:comment "IoT, CPS, Edge and Fog Computing: A main source of Big Data is sensor data from an IoT context and actuator interaction in Cyber Physical Systems. In order to meet real-time needs it will often be necessary to handle Big Data aspects at the edge of the system. This area is separately elaborated further in collaboration with the IoT (Alliance for Internet of Things Innovation (AIOTI)) and CPS communities"@en ;
    ns4:isDescribedin ns4:BdvaSira ;
    ns5:frames ns4:IoT .

ns4:Billing a owl:NamedIndividual .

ns4:Blockchain a owl:NamedIndividual,
        ns8:Document,
        ns4:Publication,
        ns4:TechnicalSpecification ;
    rdfs:label "Blockchain"@en ;
    rdfs:comment "The term Blockchain refers to a set of technologies for distributed databases."@en ;
    rdfs:seeAlso <https://web.archive.org/web/20140320135003/https://bitcoin.org/bitcoin.pdf> ;
    ns4:hasDBpediaResource <http://dbpedia.org/resource/Blockchain.info> .

ns4:Cloud_Connectivity a owl:NamedIndividual ;
    ns5:supports ns4:CloudComputing .

ns4:ContextAwareness a owl:NamedIndividual,
        ns4:Concern ;
    rdfs:label "Context Awareness"@en ;
    ns7:hasStakeholder "Developer"@en ;
    rdfs:comment "The look-up service of the system shall withold or grant information depending on context. Context includes application involved, requesting entity, and security permissions."@en ;
    rdfs:seeAlso "IoT-A Requirement UNI.407",
        "IoT-A Requirement UNI.420",
        "IoT-A Requirement UNI.421",
        "UNI.407"@en ;
    ns6:note "Publications referred: '<https://doi.org/10.1016/j.jksuci.2016.10.003>' '1.2. Utilities of IoT' 'Page 296'" ;
    ns4:hasDBpediaResource <http://dbpedia.org/resource/Context_awareness> ;
    ns5:supports ns4:AutonomousCommunication .

ns4:ControlDomain a owl:NamedIndividual .

ns4:DDS a owl:NamedIndividual .

ns4:DataConsumer a ns7:StakeholderGroup,
        owl:NamedIndividual .

ns4:DataIntegrity a owl:NamedIndividual,
        ns4:Concern ;
    rdfs:label "Data Integrity"@en ;
    ns2:creator ns4:MuhammadUsman ;
    rdfs:comment "Data integrity is the maintenance of, and the assurance of the accuracy and consistency of, data over its entire life-cycle, and is a critical aspect to the design, implementation and usage of any system which stores, processes, or retrieves data."@en ;
    rdfs:seeAlso <https://ieeexplore.ieee.org/document/6188257>,
        <https://ieeexplore.ieee.org/document/8327600>,
        <https://ieeexplore.ieee.org/document/8487479> ;
    ns4:hasWikipediaArticle <https://en.wikipedia.org/wiki/Data_integrity> ;
    ns5:supports ns4:Privacy .

ns4:DataOwner a ns7:StakeholderGroup,
        owl:NamedIndividual .

ns4:DataProvider a ns7:StakeholderGroup,
        owl:NamedIndividual .

ns4:DataSecurity a owl:NamedIndividual,
        ns4:Concern ;
    rdfs:seeAlso <https://ieeexplore.ieee.org/document/6188257>,
        <https://ieeexplore.ieee.org/document/8249113> ;
    ns4:hasWikipediaArticle <https://en.wikipedia.org/wiki/Data_security> .

ns4:DataSelection a owl:NamedIndividual .

ns4:DataStorage a owl:NamedIndividual,
        ns4:Concern ;
    rdfs:label "Data Storage"@en ;
    ns2:creator ns4:MuhammadUsman,
        ns4:sebastian ;
    rdfs:comment "The IoT data are collected from various data sources in different structures and formats. IoT enables the collected data to be stored both in physical devices and cloud storage."@en ;
    rdfs:seeAlso <https://ieeexplore.ieee.org/document/8102372> ;
    ns4:hasWikipediaArticle <https://en.wikipedia.org/wiki/Data_storage> ;
    ns5:supports ns4:DataProcessing .

ns4:Data_Collection a owl:NamedIndividual,
        ns4:Concern ;
    rdfs:label "Data Collection"@en ;
    ns2:creator ns4:MuhammadUsman ;
    rdfs:comment "The data in IoT are always mass, distributed, and time-related and position related. At the same time, the data sources of the IoT are heterogeneous. There is a vast amount of real-time data collected by the IoT devices."@en ;
    rdfs:seeAlso <https://ieeexplore.ieee.org/document/8102372> ;
    ns4:hasDBpediaResource <http://dbpedia.org/page/Data_collection> ;
    ns4:hasWikipediaArticle <https://en.wikipedia.org/wiki/Data_collection> ;
    ns5:supports ns4:DataAnalytics .

ns4:Data_Transfer_Project_Overview_and_Fundamentals a owl:NamedIndividual,
        ns1:oaSpecificResource ;
    rdfs:label "Data Transfer Project Overview and Fundamentals"@en ;
    ns4:hasOpenResource <https://datatransferproject.dev/dtp-overview.pdf> .

ns4:Developer a ns7:StakeholderGroup,
        owl:NamedIndividual .

ns4:DeviceSecurity a owl:NamedIndividual,
        ns4:Concern ;
    rdfs:label "Device Security"@en ;
    ns2:creator ns4:SebastianBader ;
    rdfs:comment ""@en ;
    rdfs:seeAlso <https://ieeexplore.ieee.org/document/8552311> ;
    ns6:narrower ns4:Security ;
    ns5:supports ns4:Objects_Safety_and_security .

ns4:EdgeAnalytics a owl:NamedIndividual,
        ns4:Concern ;
    rdfs:label "Edge Analytics"@en ;
    ns2:creator ns4:Priyanka ;
    rdfs:comment "The concern of being able to understanding the states, conditions and behaviors of the systems under control and other systems by interpreting and correlating data gathered from sensors and other systems."@en ;
    ns6:narrower ns4:Analytics ;
    ns6:note "Publications referred: 'IIC:PUB:G1:V1.80:20170131' '6.1 THE CONTROL DOMAIN' 'Page 29' " ;
    ns4:hasWikipediaArticle <https://en.wikipedia.org/wiki/Edge_computing> .

ns4:EventDrivenMessaging a owl:NamedIndividual,
        ns4:Concern ;
    rdfs:label "Event-Driven Messaging"@en ;
    ns7:hasStakeholder <https://www.wikidata.org/wiki/Q1548249> ;
    rdfs:seeAlso "IoT-A Requirement UNI.005",
        "IoT-A Requirement UNI.233" ;
    ns4:hasDBpediaResource <http://dbpedia.org/page/Event-Driven_Messaging> ;
    ns5:supports ns4:DataInMotion .

ns4:Fiware a owl:NamedIndividual,
        ns8:Organization ;
    rdfs:label "FIWARE" .

ns4:France a owl:NamedIndividual .

ns4:GeospatialData a owl:NamedIndividual,
        ns4:Concern ;
    rdfs:label "Geospatial data and information"@en ;
    rdfs:comment "Discovery and lookup services of the system shall allow locating physical entities based on geographical parameters."@en ;
    rdfs:seeAlso "IoT-A Requirement UNI.402",
        "IoT-A Requirement UNI.403",
        "IoT-A Requirement UNI.404",
        "IoT-A Requirement UNI.405",
        "IoT-A Requirement UNI.406",
        "IoT-A Requirement UNI.415",
        "IoT-A Requirement UNI.420",
        "IoT-A Requirement UNI.421",
        "UNI.401"@en,
        "UNI.402"@en,
        "UNI.403"@en,
        "UNI.404"@en ;
    ns4:hasDBpediaResource <http://dbpedia.org/resource/Geographic_data_and_information> ;
    ns5:supports ns4:DataAnalytics .

ns4:HTTP2 a owl:NamedIndividual .

ns4:IDSA a owl:NamedIndividual,
        ns8:Organization,
        ns4:IIoTConsortium ;
    rdfs:label "IDSA"@en ;
    ns2:creator ns4:sebastian ;
    ns2:title "International Data Spaces Association"@en ;
    rdfs:comment "IDSA ensures that the special economic interests of business are specifically integrated into the research work of Industrial Date Space."@en ;
    ns4:hasOfficialResource <https://www.internationaldataspaces.org/en/> ;
    ns4:hasWikipediaArticle <https://de.wikipedia.org/wiki/Industrial_Data_Space#Industrial_Data_Space_Association> .

ns4:IDSRAMInteroperability a owl:NamedIndividual,
        ns4:StandardClassification ;
    rdfs:label "IDS Interoperability"@en ;
    ns4:isDescribedin ns4:IDSRAMReferenceArchitectureModel .

ns4:IICF a owl:NamedIndividual,
        ns8:Document,
        ns4:Publication ;
    rdfs:label "IICF"@en ;
    ns2:title "Industrial Internet Connectivity Framework"@en ;
    rdfs:isDefinedBy <https://www.iiconsortium.org/IICF.htm> ;
    rdfs:seeAlso <https://www.iiconsortium.org/pdf/IIC_PUB_G5_V1.01_PB_20180228.pdf> ;
    ns4:hasClassification ns4:IIRAConnectivity .

ns4:IICFLinkLayer a owl:NamedIndividual,
        ns4:IicfConnectivityLayer,
        ns4:StandardClassification ;
    rdfs:label "IICF Link Layer"@en ;
    ns3:associatedWith ns4:IEEE_802,
        ns4:IEEE_802_16-2012,
        ns4:WiFi ;
    ns3:isPartOf ns4:IIRAConnectivity ;
    ns5:frames ns4:Communication .

ns4:IICFNetworkLayer a owl:NamedIndividual,
        ns4:IicfConnectivityLayer,
        ns4:StandardClassification ;
    rdfs:label "IICF Network Layer"@en ;
    ns3:associatedWith ns4:IPv6 ;
    ns3:isPartOf ns4:IIRAConnectivity ;
    ns5:frames ns4:Communication,
        ns4:IPv4Support,
        ns4:IPv6Support,
        ns4:Interoperability,
        ns4:SyntacticInteroperability .

ns4:IICFPhysicalLayer a owl:NamedIndividual,
        ns4:IicfConnectivityLayer,
        ns4:StandardClassification ;
    rdfs:label "IICF Physical Layer" ;
    ns3:associatedWith ns4:IEEE_802,
        ns4:IEEE_802_16-2012 ;
    ns3:isPartOf ns4:IIRAConnectivity ;
    ns5:frames ns4:Communication .

ns4:IICFTansportLayer a owl:NamedIndividual,
        ns4:IicfConnectivityLayer,
        ns4:StandardClassification ;
    rdfs:label "IICF Transport Layer"@en ;
    ns3:associatedWith ns4:HTTP,
        ns4:HTTP2,
        ns4:IEC_61158,
        ns4:ISO_20922,
        ns4:RFC_2616,
        ns4:RFC_793,
        ns4:RFC_8323,
        ns4:UDP ;
    ns3:isPartOf ns4:IIRAConnectivity ;
    ns5:frames ns4:CardinalityOfDataSources,
        ns4:CardinalityOfParticipants,
        ns4:Communication,
        ns4:EndpointInvocation,
        ns4:Interoperability,
        ns4:Multilaterism,
        ns4:SecureCommunication,
        ns4:Security,
        ns4:ServiceComposition,
        ns4:SyntacticInteroperability,
        ns4:TimeSynchronization,
        ns4:Trustworthiness,
        ns4:Unicast .

ns4:IIRAInformationDomain a owl:NamedIndividual,
        ns4:IIRAFunctionalDomain,
        ns4:StandardClassification ;
    rdfs:label "IIRA Information Domain"@en ;
    ns3:associatedWith ns4:BdvaDataAnalytics,
        ns4:BdvaDataProcessingArchitectures,
        ns4:DtpSystemView,
        ns4:EdgecrossEdgeComputingLayer,
        ns4:IDSRAMInformationLayer,
        ns4:IDSRAMProcessLayer,
        ns4:IotaInformationViewpoint,
        ns4:NgsiLdInformationModel,
        ns4:RAMIInformationLayer ;
    ns3:isPartOf ns4:IIRAFunctionalViewpoint ;
    ns6:note "Publications referred: 'IIC:PUB:G1:V1.80:20170131' '6.3 THE INFORMATION DOMAIN' 'Page 32' " ;
    ns4:isDescribedin ns4:IIRA ;
    ns5:alignsWith ns4:BdvaDataAnalytics,
        ns4:BdvaDataProcessingArchitectures,
        ns4:DtpSystemView,
        ns4:EdgecrossEdgeComputingLayer,
        ns4:IDSRAMInformationLayer,
        ns4:IDSRAMProcessLayer,
        ns4:IotaInformationViewpoint,
        ns4:NgsiLdInformationModel,
        ns4:RAMIInformationLayer ;
    ns5:frames ns4:DataAnalytics,
        ns4:DataProcessing,
        ns4:Interoperability,
        ns4:SemanticInteroperability,
        ns4:StreamProcessing,
        ns4:SyntacticInteroperability .

ns4:IIRAReliability a owl:NamedIndividual,
        ns4:IIRASystemCharacteristics,
        ns4:StandardClassification ;
    rdfs:label "IIRA Reliability"@en ;
    ns3:isPartOf ns4:IIRAFunctionalViewpoint ;
    ns6:note "Publications referred: '<https://www.iiconsortium.org/pdf/IIC_PUB_G4_V1.00_PB-3.pdf IIC:PUB:G4:V1.0:PB:20160926>' '3.4 RELIABILITY' 'Page 18'" ;
    ns4:isDescribedin ns4:IIRA ;
    ns5:frames ns4:Reliability,
        ns4:Trustworthiness .

ns4:IIRAResilience a owl:NamedIndividual,
        ns4:IIRASystemCharacteristics,
        ns4:StandardClassification ;
    rdfs:label "IIRA Resilience"@en ;
    ns3:isPartOf ns4:IIRAFunctionalViewpoint ;
    ns4:isDescribedin ns4:IIRA .

ns4:IIRASafety a owl:NamedIndividual,
        ns4:IIRASystemCharacteristics,
        ns4:StandardClassification ;
    rdfs:label "IIRA Safety"@en ;
    ns3:isPartOf ns4:IIRAFunctionalViewpoint ;
    ns4:isDescribedin ns4:IIRA .

ns4:ISO_9594 a owl:NamedIndividual,
        ns4:Standard ;
    rdfs:label "ISO/IEC 9594"@en,
        "X.509"@en ;
    ns4:hasClassification ns4:DataSovereignty,
        ns4:IDSRAMCertification,
        ns4:IDSRAMSecurity .

ns4:InternationalClassificationForStandards a owl:Class ;
    rdfs:label "International Classification For Standards" .

ns4:IoTA a owl:NamedIndividual,
        ns8:Organization,
        ns4:IIoTConsortium ;
    rdfs:label "IoT-A"@en ;
    ns2:title "IoT Architecture"@en ;
    ns3:associatedWith ns4:IotaReferenceArchitecture ;
    rdfs:comment "After much discussion about the core concepts of the IoT for several years, in 2009 a group of researchers from more than 20 large industrial companies and research institutions joined forces to lay the foundation for the much needed common ground or a common “architecture” for the Internet of Things: the IoTArchitecture project (IoT-A) was born. IoT-A has become the European Commission’s flagship project in the European Union’s Seventh Framework Program for Research and Development with respect to establishing an architecture for the Internet of Things."@en ;
    rdfs:seeAlso <http://open-platforms.eu/standard_protocol/iot-a-architectural-reference-model/> .

ns4:IotaPerformanceScalability a owl:NamedIndividual,
        ns4:IotaPerspective,
        ns4:StandardClassification ;
    rdfs:label "IoT-A Performance and Scalability"@en ;
    ns4:isDescribedin ns4:IotaReferenceArchitecture ;
    ns5:frames ns4:Communication,
        ns4:Interoperability,
        ns4:NetworkPerformance,
        ns4:QualityOfService,
        ns4:Scalability,
        ns4:SemanticInteroperability,
        ns4:ServiceDescription .

ns4:Ivi a owl:NamedIndividual,
        ns8:Organization,
        ns4:IIoTConsortium ;
    rdfs:label "IVI"@en ;
    ns2:creator ns4:sebastian ;
    ns2:title "Industrial Value Chain Initiative"@en ;
    rdfs:comment "The Industrial Value Chain Initiative (IVI) is a forum to design a new society by combining manufacturing and information technologies, and for all enterprises to take an initiative collaboratively."@en ;
    ns4:hasOfficialResource <https://iv-i.org/> .

ns4:IviActivityLayer a owl:NamedIndividual,
        ns4:IviLayer,
        ns4:StandardClassification ;
    rdfs:label "IVI Activity Layer"@en ;
    ns2:creator ns4:sebastian ;
    ns3:associatedWith <https://w3id.org/i40/rami#Engineering>,
        ns4:Manufacturing ;
    rdfs:comment "The activity layer has a view point of activities actually conducted at various places in manufacturers. People and machines acting voluntarily, human activity, machine processes, and information as an object og such activities and processes are brought up for discussion. In every production site of every manufacturer, concrete manufacturing activities are conducted in a different way. (source: IVRA-Next)"@en ;
    ns4:isDescribedin ns4:IVRA ;
    ns5:alignsWith <https://w3id.org/i40/rami#Engineering>,
        ns4:Manufacturing ;
    ns5:frames <https://w3id.org/i40/rami#ProcessPlanning> .

ns4:IviSpecificationLayer a owl:NamedIndividual,
        ns4:IviLayer,
        ns4:StandardClassification ;
    rdfs:label "IVI Specification Layer"@en ;
    ns2:creator ns4:sebastian ;
    ns3:associatedWith <https://w3id.org/i40/rami#Engineering>,
        <https://w3id.org/i40/rami#TypeDevelopment> ;
    rdfs:comment "In the specification layer, the following will be considered: Specific operations based on human activities and machine processes and the things and information items that are their subjects, as well as the data and their attributes that are the subject of the processes executed by logic in software. (source: IVRA-Next)"@en ;
    ns4:isDescribedin ns4:IVRA ;
    ns5:alignsWith <https://w3id.org/i40/rami#Engineering>,
        <https://w3id.org/i40/rami#TypeDevelopment> ;
    ns5:frames ns4:DataProcessing .

ns4:LinkLayer a owl:NamedIndividual .

ns4:NetworkLayer a owl:NamedIndividual .

ns4:NonRepudiation a owl:NamedIndividual,
        ns4:Concern ;
    rdfs:label "Non-repudiation"@en ;
    ns2:creator ns4:sebastian ;
    rdfs:comment "In digital security, non-repudiation means:  (a)  A service that provides proof of the integrity and origin of data. (b) An authentication that can be said to be genuine with high confidence. The most common method of verifying the digital origin of data is through digital certificates, a form of public key infrastructure that includes digital signatures."@en ;
    rdfs:seeAlso <https://ieeexplore.ieee.org/document/6188257>,
        "IoT-A Requirement UNI.619" ;
    ns4:hasDBpediaResource <https://dbpedia.org/resource/Non-repudiation> ;
    ns4:hasWikipediaArticle <https://en.wikipedia.org/wiki/Non-repudiation> ;
    ns5:supports ns4:IntegrityProtection .

ns4:OFRAAgilityPillar a owl:NamedIndividual,
        ns4:StandardClassification ;
    rdfs:label "OpenFog Agility Pillar"@en ;
    ns2:creator ns4:sebastian ;
    rdfs:comment """The agility pillar addresses business operational decisions for an OpenFog RA deployment. It is not possible for humans alone to analyze the data generated at the scale predicted by IoT as the basis for rapid, sound business and operational decisions. The agility pillar focuses on transforming this volume of data into actionable insights. Agility also deals with the highly dynamic nature of fog deployments and the need to respond quickly to change.
source: OpenFog Reference Architecture"""@en ;
    ns6:note "Publications referred: '<https://www.openfogconsortium.org/wp-content/uploads/OpenFog_Reference_Architecture_2_09_17-FINAL.pdf> OPFRA001.020817' '4.7 Agility Pillar' 'Page 31' " ;
    ns4:isDescribedin ns4:OpenFogReferenceArchitecture ;
    ns5:frames ns4:Agility .

ns4:OFRAAutonomyPillar a owl:NamedIndividual,
        ns4:StandardClassification ;
    rdfs:label "OpenFog AutonomyPillar"@en ;
    ns2:creator ns4:sebastian ;
    rdfs:comment "The autonomy pillar enables fog nodes to continue to deliver the designed functionality in the face of the external service failures. In this architecture, autonomy is supported throughout the hierarchy. Decision making will be made at all levels of a deployment’s hierarchy including near the device or higher order layers. Centralized decision-making in the cloud is no longer the only option. Autonomy at the network edge means intelligence from local devices and peer data can be used to fulfill the business’ mission at the point where it makes the most business sense."@en ;
    ns6:note "Publications referred: '<https://www.openfogconsortium.org/wp-content/uploads/OpenFog_Reference_Architecture_2_09_17-FINAL.pdf> OPFRA001.020817' '4.4 Autonomy Pillar' 'Page 27' " ;
    ns4:isDescribedin ns4:OpenFogReferenceArchitecture ;
    ns5:frames ns4:AutonomousCommunication,
        ns4:AutonomousConfiguration .

ns4:OFRADataAnalyticsAndControlPerspective a owl:NamedIndividual,
        ns4:StandardClassification ;
    rdfs:label "OpenFog Data Analytics and Control Perspective"@en ;
    ns2:creator ns4:sebastian ;
    ns4:isDescribedin ns4:OpenFogReferenceArchitecture ;
    ns5:alignsWith ns4:IIRAControlDomain,
        ns4:InformationDomain ;
    ns5:frames ns4:DataAnalytics .

ns4:OFRADeploymentViewpoint a owl:NamedIndividual,
        ns4:Viewpoint ;
    rdfs:label "OpenFog Deployment Viewpoint"@en ;
    ns2:creator ns4:sebastian ;
    rdfs:comment "How fog software and fog systems are deployed to address a given scenario is also very important. There are many deployment types ranging from embedded to large clustered systems that are fully interconnected. The deployment type(s) chosen are scenario specific, but key aspects of the architecture remain visible regardless of deployment type. However, some may grow or shrink in importance. source: OpenFog Reference Architecture"@en ;
    ns4:isDescribedin ns4:OpenFogReferenceArchitecture ;
    ns5:alignsWith ns4:IIRAImplementationViewpoint ;
    ns5:frames ns4:ServiceDeployment .

ns4:OFRAFunctionalViewpoint a owl:NamedIndividual,
        ns4:Viewpoint ;
    rdfs:label "OpenFog Functional Viewpoint"@en ;
    ns2:creator ns4:sebastian ;
    rdfs:comment "The functional viewpoint of the architecture shows how we apply the OpenFog architectural elements and views to address the various concerns of the stakeholders to satisfy a given scenario. Each scenario chosen will focus on a different aspects and market opportunities for fog computing. We fully expect that the architectural description, views, and perspective may change over time. This change and refinement should be driven from testbeds and application of the OpenFog RA to multiple different markets we see as important to fog computing. source: OpenFog Reference Architecture"@en ;
    ns4:isDescribedin ns4:OpenFogReferenceArchitecture .

ns4:OFRAHierarchyPillar a owl:NamedIndividual,
        ns4:StandardClassification ;
    rdfs:label "OpenFog Hierarchy Pillar"@en ;
    ns2:creator ns4:sebastian ;
    rdfs:comment "OpenFog RA computing resources can be seen as a logical hierarchy based on the functional requirements of an end-to-end IoT system. Depending on the scale and nature of the scenario being addressed, the hierarchy may be a network of smart and connected partitioned systems arranged in physical or logical layers, or it may collapse into a single physical system (scalability pillar). source: OpenFog Reference Architecture"@en ;
    ns6:note "Publications referred: '<https://www.openfogconsortium.org/wp-content/uploads/OpenFog_Reference_Architecture_2_09_17-FINAL.pdf> OPFRA001.020817' '4.8 Hierarchy Pillar' 'Page 31' " ;
    ns4:isDescribedin ns4:OpenFogReferenceArchitecture ;
    ns5:frames ns4:BusinessValue,
        ns4:DataAnalytics,
        ns4:Sensing .

ns4:OFRAItBusinessAndCrossFogApplicationsPerspective a owl:NamedIndividual,
        ns4:StandardClassification ;
    rdfs:label "OpenFog IT Business and Cross-fog Applications Perspective"@en ;
    ns2:creator ns4:sebastian ;
    rdfs:comment "Fog applications and services should have the flexibility to span and interoperate with various levels in a fog hierarchy. This is a foundational aspect of fog computing that enables a multi-vendor ecosystem. In addition, the data that is collected or generated by one fog node should be shareable with other nodes in the hierarchy. The figure below shows a cross-fog application spanning east to west nodes (it would also be able to span north to south). source: OpenFog Reference Architecture"@en ;
    ns4:isDescribedin ns4:OpenFogReferenceArchitecture ;
    ns5:frames ns4:BusinessContext .

ns4:OFRAManageabilityPerspective a owl:NamedIndividual,
        ns4:StandardClassification ;
    rdfs:label "OpenFog Manageability Perspective"@en ;
    ns2:creator ns4:sebastian ;
    rdfs:comment "Many fog computing deployments involve machine vision, and associated human-like functions. As such, they have the ability to see, respond, remember, move, and make autonomous decisions in order to participate in other fog services. This range of actions requires a higher level of manageability than a traditional static model. In addition, fog nodes may be deployed in a wide range of locations: remote, fixed and non-fixed, and environmentally harsh conditions. source: OpenFog Reference Architecture"@en ;
    ns4:isDescribedin ns4:OpenFogReferenceArchitecture ;
    ns5:frames ns4:AutonomousConfiguration,
        ns4:ServiceLifecycleManagement .

ns4:OFRANodeView a owl:NamedIndividual,
        ns4:Viewpoint ;
    rdfs:label "OpenFog Node View"@en ;
    ns2:creator ns4:sebastian ;
    ns3:associatedWith ns4:WiFi ;
    rdfs:comment "The node view is the lowest level view we currently utilize in the architectural description. The stakeholders involved in formulating the viewpoint (and subsequently this view) are the system on a chip designers, silicon manufacturers, firmware architects, and system architects. source: OpenFog Reference Architecture"@en ;
    ns4:isDescribedin ns4:OpenFogReferenceArchitecture ;
    ns5:alignsWith ns4:IDSRAMSystemLayer,
        ns4:IIRAPhysicalSystems,
        ns4:RAMIAssetlayer ;
    ns5:frames ns4:DataStorage,
        ns4:NetworkPerformance,
        ns4:PhysicalConnectivity,
        ns4:Security .

ns4:OFRAOpennessPillar a owl:NamedIndividual,
        ns4:StandardClassification ;
    rdfs:label "OpenFog Opennes Pillar"@en ;
    ns2:creator ns4:sebastian ;
    rdfs:comment """Openness is essential for the success of a ubiquitous fog computing ecosystem for IoT platforms and applications. Proprietary or single vendor solutions can result in limited supplier diversity, which can have a negative impact on system cost, quality and innovation. The openness pillar importance is highlighted in our desire for fully interoperable systems, supported by a vibrant supplier ecosystem.
source: OpenFog Reference Architecture"""@en ;
    ns6:note "Publications referred: '<https://www.openfogconsortium.org/wp-content/uploads/OpenFog_Reference_Architecture_2_09_17-FINAL.pdf> OPFRA001.020817' '4.3 Openness Pillar' 'Page 26' " ;
    ns4:isDescribedin ns4:OpenFogReferenceArchitecture ;
    ns5:frames ns4:Interoperability,
        ns4:ServiceComposition .

ns4:OFRAPerformancePerspective a owl:NamedIndividual,
        ns4:StandardClassification ;
    rdfs:label "Performance and Scale Perspective"@en ;
    ns2:creator ns4:sebastian ;
    ns4:isDescribedin ns4:OpenFogReferenceArchitecture .

ns4:OFRAProgrammabilityPillar a owl:NamedIndividual,
        ns4:StandardClassification ;
    rdfs:label "OpenFog Programmability Pillar"@en ;
    ns2:creator ns4:sebastian ;
    rdfs:comment """The programmability pillar enables highly adaptive deployments including support for programming at the software and hardware layers. This means that re-tasking a fog node or cluster of fog nodes for accommodating operational dynamics, can be completely automated. The re-tasking can be done with the help of the fog nodes inherent programmability interfaces which we describe using general purpose compute or accelerator interfaces.
source: OpenFog Reference Architecture"""@en ;
    ns6:note "Publications referred: '<https://www.openfogconsortium.org/wp-content/uploads/OpenFog_Reference_Architecture_2_09_17-FINAL.pdf> OPFRA001.020817' '4.5 Programmability Pillar' 'Page 29' " ;
    ns4:isDescribedin ns4:OpenFogReferenceArchitecture ;
    ns5:frames ns4:Programmability .

ns4:OFRAScalabilityPillar a owl:NamedIndividual,
        ns4:StandardClassification ;
    rdfs:label "OpenFog Scalability Pillar"@en ;
    ns2:creator ns4:sebastian ;
    rdfs:comment """The scalability pillar addresses the dynamic technical and business needs behind fog deployments. Elastic scalability cuts across all fog computing applications and verticals. The hierarchical properties of fog and its location at logical edges of networks add additional scaling opportunities.
source: OpenFog Reference Architecture"""@en ;
    ns6:note "Publications referred: '<https://www.openfogconsortium.org/wp-content/uploads/OpenFog_Reference_Architecture_2_09_17-FINAL.pdf> OPFRA001.020817' '4.2 Scalability Pillar' 'Page 24' " ;
    ns4:isDescribedin ns4:OpenFogReferenceArchitecture ;
    ns5:frames ns4:Scalability .

ns4:OFRASecurityPerspective a owl:NamedIndividual,
        ns4:StandardClassification ;
    rdfs:label "OpenFog Security Perspective"@en ;
    ns2:creator ns4:sebastian ;
    ns4:isDescribedin ns4:OpenFogReferenceArchitecture ;
    ns5:alignsWith <https://w3id.org/i40/rami#Security>,
        ns4:BdvaCyberSecurityTrust,
        ns4:FiwareSecurity,
        ns4:IDSRAMSecurity,
        ns4:IIRASecurity,
        ns4:IIRASecurityFramework,
        ns4:IotaTrustSecurityPrivacy,
        ns4:OcfSecurity ;
    ns5:frames ns4:Availability,
        ns4:Identification,
        ns4:IntegrityProtection,
        ns4:Privacy,
        ns4:ServiceAccessControl,
        ns4:Trustworthiness .

ns4:OFRASecurityPillar a owl:NamedIndividual,
        ns4:StandardClassification ;
    rdfs:label "OpenFog Security Pillar"@en ;
    ns2:creator ns4:sebastian ;
    rdfs:comment " Security implementations have many different descriptions and attributes such as privacy, anonymity, integrity, trust, attestation, verification, and measurement. These are key attributes for the OpenFog RA. Achieving the foundational elements for security requires an approach to discover, attest, and verify all smart and connected “things” before trust can be established source: OpenFog Reference Architecture"@en,
        """Security in the OpenFog RA is not a one-size-fits-all architecture. Rather, it describes all of the mechanisms that can be applied to make a fog node secure from silicon to software application. Business case, target market, and vertical use case, as well as the location of the node itself, will all create a set of requirements for that node. However, there are certain foundational parts of the architecture, which must be in place in order to build a secure execution environment.
source: OpenFog Reference Architecture"""@en ;
    ns6:note "Publications referred: ' <https://www.openfogconsortium.org/wp-content/uploads/OpenFog_Reference_Architecture_2_09_17-FINAL.pdf> OPFRA001.020817' '4.1 Security Pillar' 'Page 23' " ;
    ns4:isDescribedin ns4:OpenFogReferenceArchitecture ;
    ns5:alignsWith <https://w3id.org/i40/rami#Security>,
        ns4:BdvaCyberSecurityTrust,
        ns4:FiwareSecurity,
        ns4:IDSRAMSecurity,
        ns4:IIRASecurity,
        ns4:IIRASecurityFramework,
        ns4:IotaTrustSecurityPrivacy,
        ns4:OcfSecurity,
        ns4:OpenFogSecurityPerspective ;
    ns5:frames ns4:Security .

ns4:OFRASoftwareView a owl:NamedIndividual,
        ns4:Viewpoint ;
    ns2:creator ns4:sebastian ;
    rdfs:comment "OpenFog Software Architecture View"@en,
        "The software view of the OpenFog RA is composed of software running on a platform that is comprised of one or more node views coupled with other components to create a system addressing a given scenario. The stakeholders of the software view include the system integrators, software architects, solution designers, and application developers of a fog computing environment. The software running on fog platforms is used to satisfy a given deployment scenario. A robust fog deployment requires that the relationship between a fog node, fog platform, and fog software are seamless. source: OpenFog Reference Architecture"@en ;
    ns5:alignsWith ns4:IIRAApplicationDomain ;
    ns5:frames ns4:ServiceDiscovery .

ns4:OFRASystemView a owl:NamedIndividual,
        ns4:Viewpoint ;
    rdfs:label "OpenFog System Architecture View"@en ;
    ns2:creator ns4:sebastian ;
    rdfs:comment "The system view of the OpenFog RA is composed of one or more node views coupled with other components to create a platform. The stakeholders which typically create these systems to facilitate a fog deployment comprise the concerns of this viewpoint. Subsequently this view is intended to address the concerns of the system architects, hardware OEMs, and platform manufacturers. They also need to understand the Node view such that the systems they create can be deployed to address a given scenario. source: OpenFog Reference Architecture"@en ;
    ns4:isDescribedin ns4:OpenFogReferenceArchitecture ;
    ns5:frames ns4:PhysicalConnectivity .

ns4:OFRA_RASPillar a owl:NamedIndividual,
        ns4:StandardClassification ;
    rdfs:label "OpenFog RAS Pillar"@en ;
    ns2:creator ns4:sebastian ;
    rdfs:comment """Reliability, availability, and serviceability (RAS) is resident throughout successful system architectures and, as such, takes on great importance in the OpenFog RA. Hardware, software, and operations are the three main areas of the RAS pillar.
source: OpenFog Reference Architecture"""@en ;
    ns6:note "Publications referred: '<https://www.openfogconsortium.org/wp-content/uploads/OpenFog_Reference_Architecture_2_09_17-FINAL.pdf> OPFRA001.020817' '4.6 Reliability, Availability, and Serviceability (RAS)Pillar' 'Page 29' " ;
    ns4:isDescribedin ns4:OpenFogReferenceArchitecture ;
    ns5:frames ns4:Availability,
        ns4:MaintenanceCost,
        ns4:Reliability .

ns4:OMG_DDS a owl:NamedIndividual,
        ns8:Document,
        ns4:Publication,
        ns4:Standard ;
    rdfs:label "OMG DDS"@en ;
    ns2:creator ns4:OMG ;
    rdfs:comment "The Data Distribution Service for real-time systems (DDS) is an Object Management Group (OMG) machine-to-machine (sometimes called middleware) standard that aims to enable scalable, real-time, dependable, high-performance and interoperable data exchanges using a publish–subscribe pattern. DDS addresses the needs of applications like financial trading, air-traffic control, smart grid management, and other big data applications. The standard is used in applications such as smartphone operating systems, transportation systems and vehicles, software-defined radio, and by healthcare providers. DDS was promoted for use in the Internet of things."@en ;
    ns8:maker ns4:OMG ;
    ns4:hasClassification ns4:IICFFrameworkLayer,
        ns4:IIRAConnectivity ;
    ns4:hasDBpediaResource <http://dbpedia.org/page/Data_Distribution_Service> ;
    ns4:hasOfficialResource <http://portals.omg.org/dds/> ;
    ns4:hasPublisher ns4:OMG ;
    ns4:hasTag "Data Distribution Service for real-time systems"@en ;
    ns4:hasWikipediaArticle <https://en.wikipedia.org/wiki/Data_Distribution_Service> ;
    ns4:relatedTo ns4:IEC_29182-1,
        ns4:IEC_61158,
        ns4:IEC_61784,
        ns4:OMG_DDS .

ns4:Objects_Safety_and_security a owl:NamedIndividual,
        ns4:Concern ;
    rdfs:label "Objects Safety and Security"@en ;
    ns2:creator ns4:MuhammadUsman ;
    rdfs:comment """The IoT comprises of a huge number of perception objects that spread over a few geographic zone; it is important to keep the intruder's access to the items that
may make physical harm them or may change their operation"""@en ;
    rdfs:seeAlso <https://ieeexplore.ieee.org/document/6188257> ;
    ns5:supports ns4:Safety,
        ns4:Security .

ns4:OcfCoreFramework a owl:NamedIndividual,
        ns4:OcfBlock ;
    rdfs:label "OCF Core Framework"@en ;
    ns2:creator ns4:sebastian ;
    ns4:isDescribedin ns4:OcfFramework ;
    ns5:frames ns4:Communication,
        ns4:EndpointInvocation,
        ns4:Identification,
        ns4:ServiceDiscovery,
        ns4:SyntacticInteroperability .

ns4:OcfDataModels a owl:NamedIndividual,
        ns4:OcfBlock ;
    rdfs:label "OCF Data Models"@en ;
    ns4:isDescribedin ns4:OcfFramework ;
    ns5:frames ns4:SemanticInteroperability .

ns4:OcfL2Connectivity a owl:NamedIndividual,
        ns4:OcfBlock ;
    rdfs:label "OCF L2 Connectivity"@en ;
    ns4:isDescribedin ns4:OcfFramework ;
    ns5:frames ns4:Connectivity,
        ns4:SyntacticInteroperability .

ns4:OcfNetworking a owl:NamedIndividual,
        ns4:OcfBlock ;
    rdfs:label "OCF Networking"@en ;
    ns2:creator ns4:sebastian ;
    ns3:associatedWith ns4:IPv6 ;
    ns4:isDescribedin ns4:OcfFramework ;
    ns5:frames ns4:Connectivity,
        ns4:IPv6Support .

ns4:OpenFogArchitecture a owl:NamedIndividual,
        ns4:Publication ;
    rdfs:label "OpenFog Architecture Whitepaper" ;
    ns12:title "OpenFog Architecture Overview"@en ;
    ns2:creator ns4:sebastian ;
    rdfs:comment "The OpenFog Architecture is a system-level architecture that extends elements of compute, networking and storage across the cloud through to the edge of the network. This approach is particularly suited to IoT systems and accelerates the decision-making velocity. This architecture serves a specific subset of business problems that can’t be successfully implemented using “cloud only” based architectures or relying solely on intelligent edge devices. OpenFog should be thought of as complementary to, and an extension of the traditional cloud based model where implementations of the architecture can reside in multiple layers of a network’s topology. The goal of the OpenFog architecture is to facilitate deployments which highlight interoperability, performance, security, scalability, programmability, reliability, availability, serviceability, and agility. Proprietary or single vendor solutions can result in limited supplier diversity, which can have a negative impact on market adoption, system cost, quality and innovation."@en ;
    ns4:hasDBpediaResource <http://dbpedia.org/resource/OpenFog_Consortium> ;
    ns4:hasOfficialResource <https://www.openfogconsortium.org/white-paper-reference-architecture/white-paper-download-open-fog-reference-architecture/> ;
    ns4:hasPublisher ns4:OpenFogConsortium .

ns4:ProductManager a ns7:StakeholderGroup,
        owl:NamedIndividual,
        ns4:Stakeholder ;
    rdfs:label "Product Manager"@en ;
    rdfs:comment ""@en ;
    ns6:note "Publications referred: '(IIC:PUB:G1:V1.80:20170131' '3.5.1 BUSINESS VIEWPOINT' 'Page 15' 'Priyanka'" .

ns4:Programmability a owl:NamedIndividual,
        ns4:Concern ;
    rdfs:label "Programmability" ;
    ns3:isComponentOf ns4:EdgeComputing ;
    rdfs:comment "In the edge computing, computation is offloaded from the cloud, and the edge nodes are most likely heterogeneous platforms. In this case, the runtime of these nodes differ from each other, and the programmer faces huge difficulties to write an application that may be deployed in the edge computing paradigm." ;
    rdfs:seeAlso <https://dl.acm.org/citation.cfm?doid=3210240.3226062>,
        <https://ieeexplore.ieee.org/document/7488250> ;
    ns6:note "Publications referred: ' <https://www.openfogconsortium.org/wp-content/uploads/OpenFog_Reference_Architecture_2_09_17-FINAL.pdf> OPFRA001.020817' '4.5 Programmability Pillar' 'Page 29' " ;
    ns5:supports ns4:EdgeComputing .

ns4:RAMICommunicationLayer a owl:NamedIndividual .

ns4:RAMIFunctional a owl:NamedIndividual .

ns4:RAMIHeader a owl:NamedIndividual,
        ns4:StandardClassification,
        ns4:StandardizationFramework ;
    rdfs:label "Administration Shell Header"@en ;
    ns3:isPartOf ns4:AdministrationShell ;
    ns6:note "find better class assignment"@en ;
    ns4:hasPublisher ns4:PlatformIndustry40 ;
    ns5:frames <https://w3id.org/i40/rami#Lifecycle_Status>,
        ns4:BusinessContext,
        ns4:DataAccess,
        ns4:EndpointInvocation,
        ns4:Identification,
        ns4:IdentityManagement,
        ns4:Interoperability,
        ns4:Security,
        ns4:SemanticInteroperability,
        ns4:SyntacticInteroperability,
        ns4:ThingDescription,
        ns4:ThingRepresentation,
        ns4:Trustworthiness .

ns4:RAMIProduct a owl:NamedIndividual,
        <https://w3id.org/i40/rami#RAMIHierarchyLevel>,
        ns4:StandardClassification ;
    ns5:frames ns4:Manufacturing .

ns4:RAMIWorkCenter a owl:NamedIndividual .

ns4:RAML a owl:NamedIndividual,
        ns8:Document,
        ns4:Publication,
        ns4:TechnicalSpecification ;
    rdfs:label "RAML"@en ;
    ns2:creator ns4:sebastian ;
    rdfs:comment "RAML (RESTful API Modeling Language) - Makes it easy to manage the whole API lifecycle from design to sharing. It's concise - you only write what you need to define - and reusable.  (source: https://www.postscapes.com/internet-of-things-protocols/)"@en ;
    ns4:hasOfficialResource <http://raml.org/> .

ns4:RDF a owl:NamedIndividual,
        ns8:Document,
        ns4:Publication,
        ns4:TechnicalSpecification .

ns4:RFC_2616 a owl:NamedIndividual,
        ns8:Document,
        ns4:Publication,
        ns4:Standard ;
    rdfs:label "HTTP/1.1"@en,
        "RFC 2616"@en ;
    ns2:creator ns4:IETF ;
    rdfs:comment "The Hypertext Transfer Protocol (HTTP) is an application-level protocol for distributed, collaborative, hypermedia information systems. It is a generic, stateless, protocol which can be used for many tasks beyond its use for hypertext, such as name servers and distributed object management systems, through extension of its request methods, error codes and headers. A feature of HTTP is the typing and negotiation of data representation, allowing systems to be built independently of the data being transferred."@en ;
    ns6:altLabel "HTTP/1.1"@en ;
    ns8:maker ns4:IETF ;
    ns4:hasClassification ns4:IDSRAMSystemLayer,
        ns4:IIRAFunctionalViewpoint,
        ns4:RAMICommunicationlayer,
        ns4:TansportLayer ;
    ns4:hasOfficialResource <https://tools.ietf.org/html/rfc2817>,
        <https://www.ietf.org/rfc/rfc2616> ;
    ns4:hasPublisher ns4:IETF .

ns4:RFC_5246 a owl:NamedIndividual,
        ns8:Document,
        ns4:Publication,
        ns4:Standard ;
    rdfs:label "RFC 5246"@en ;
    ns2:creator ns4:IETF ;
    ns2:description "This document specifies Version 1.2 of the Transport Layer Security (TLS) protocol.  The TLS protocol provides communications security over the Internet.  The protocol allows client/server applications to communicate in a way that is designed to prevent eavesdropping, tampering, or message forgery."@en ;
    rdfs:comment "This document specifies Version 1.2 of the Transport Layer Security (TLS) protocol.  The TLS protocol provides communications security over the Internet.  The protocol allows client/server applications to communicate in a way that is designed to prevent eavesdropping, tampering, or message forgery."@en ;
    ns8:maker ns4:IETF ;
    ns4:hasClassification ns4:DataSovereignty,
        ns4:IDSRAMSecurity ;
    ns4:hasOfficialResource <https://tools.ietf.org/html/rfc5246> ;
    ns4:hasPublisher ns4:IETF .

ns4:RFC_7519 a owl:NamedIndividual,
        ns8:Document,
        ns4:Publication,
        ns4:Standard ;
    rdfs:label "JSON Web Token"@en,
        "RFC 7519"@en ;
    ns2:creator ns4:IETF ;
    ns2:description "JSON Web Token (JWT) is a compact, URL-safe means of representing claims to be transferred between two parties.  The claims in a JWT are encoded as a JSON object that is used as the payload of a JSON Web Signature (JWS) structure or as the plaintext of a JSON Web Encryption (JWE) structure, enabling the claims to be digitally signed or integrity protected with a Message Authentication Code (MAC) and/or encrypted."@en ;
    rdfs:comment "JSON Web Token (JWT) is a compact, URL-safe means of representing claims to be transferred between two parties.  The claims in a JWT are encoded as a JSON object that is used as the payload of a JSON Web Signature (JWS) structure or as the plaintext of a JSON Web Encryption (JWE) structure, enabling the claims to be digitally signed or integrity protected with a Message Authentication Code (MAC) and/or encrypted."@en ;
    ns8:maker ns4:IETF ;
    ns4:hasClassification ns4:DataSovereignty,
        ns4:IDSRAMSecurity ;
    ns4:hasOfficialResource <https://tools.ietf.org/html/rfc7519> ;
    ns4:hasPublisher ns4:IETF .

ns4:RFC_7642 a owl:NamedIndividual,
        ns8:Document,
        ns4:Publication,
        ns4:Standard ;
    rdfs:label "RFC 7642"@en ;
    ns2:creator ns4:IETF,
        ns4:sebastian ;
    ns2:title "SCIM Use Cases"@en ;
    rdfs:comment "This document provides definitions and an overview of the System for Cross-domain Identity Management (SCIM).  It lays out the system's concepts, models and flows, and includes user scenarios, use cases, and requirements."@en ;
    ns8:maker ns4:IETF ;
    ns4:hasClassification ns4:FiwareSecurity ;
    ns4:hasDeveloper ns4:IETF ;
    ns4:hasOfficialResource <https://tools.ietf.org/html/draft-ietf-scim-use-cases-08> ;
    ns4:hasPublisher ns4:IETF ;
    ns5:hasTargetConcern ns4:IdentityManagement .

ns4:RFC_7643 a owl:NamedIndividual,
        ns8:Document,
        ns4:Publication,
        ns4:Standard ;
    rdfs:label "RFC 7643"@en ;
    ns2:creator ns4:IETF,
        ns4:sebastian ;
    ns2:title "SCIM Core Schema"@en ;
    rdfs:comment "This document provides a platform neutral schema and extension model for representing users and groups and other resource types in JSON format.  This schema is intended for exchange and use with cloud service providers."@en ;
    ns8:maker ns4:IETF ;
    ns4:hasClassification ns4:FiwareSecurity ;
    ns4:hasDeveloper ns4:IETF ;
    ns4:hasOfficialResource <https://tools.ietf.org/html/draft-ietf-scim-core-schema-22> ;
    ns4:hasPublisher ns4:IETF ;
    ns5:hasTargetConcern ns4:IdentityManagement .

ns4:RFC_7644 a owl:NamedIndividual,
        ns4:Standard ;
    rdfs:label "RFC 7644"@en ;
    ns2:creator ns4:irlan,
        ns4:sebastian ;
    ns2:title "SCIM API"@en ;
    rdfs:comment "The System for Cross-Domain Identity Management (SCIM) specification is an HTTP based protocol that makes managing identities in multi domain scenarios easier to support through a standardized service. Examples include but are not limited to enterprise to cloud service providers, and inter-cloud based scenarios.  The specification suite seeks to build upon experience with existing schemas and deployments, placing specific emphasis on simplicity of development and integration, while applying existing authentication, authorization, and privacy models.  SCIM's intent is to reduce the cost and complexity of user management operations by providing a common user schema, an extension model, and a service protocol defined by this document."@en ;
    ns8:maker ns4:IETF ;
    ns4:hasClassification ns4:FiwareSecurity ;
    ns4:hasDeveloper ns4:IETF ;
    ns4:hasOfficialResource <https://tools.ietf.org/html/draft-ietf-scim-api-19> ;
    ns4:hasPublisher ns4:IETF ;
    ns5:hasTargetConcern ns4:IdentityManagement .

ns4:RFC_793 a owl:NamedIndividual,
        ns4:Standard ;
    rdfs:label "RFC 793"@en ;
    ns2:creator ns4:irlan,
        ns4:sebastian ;
    ns2:title "TRANSMISSION CONTROL PROTOCOL"@en ;
    rdfs:comment """This document describes the DoD Standard Transmission Control Protocol
(TCP).  There have been nine earlier editions of the ARPA TCP
 specification on which this standard is based, and the present text draws heavily from them.  There have been many contributors to this work both in terms of concepts and in terms of text.  This edition clarifies several details and removes the end-of-letter buffer-size adjustments,
 and redescribes the letter mechanism as a push function."""@en ;
    ns8:maker ns4:IETF ;
    ns4:hasClassification ns4:IDSRAMSystemLayer,
        ns4:TansportLayer ;
    ns4:hasOfficialResource <https://tools.ietf.org/html/rfc793> ;
    ns4:hasPublisher ns4:IETF .

ns4:RFC_8323 a owl:NamedIndividual,
        ns8:Document,
        ns4:Publication,
        ns4:TechnicalSpecification ;
    rdfs:label "CoAP"@en ;
    ns2:creator ns4:IETF,
        ns4:sebastian ;
    rdfs:comment "CoAP (Constrained Application Protocol) is an application layer protocol that is intended for use in resource-constrained internet devices, such as WSN nodes. CoAP is designed to easily translate to HTTP for simplified integration with the web, while also meeting specialized requirements such as multicast support, very low overhead, and simplicity. The CoRE group has proposed the following features for CoAP: RESTful protocol design minimizing the complexity of mapping with HTTP, Low header overhead and parsing complexity, URI and content-type support, Support for the discovery of resources provided by known CoAP services. Simple subscription for a resource, and resulting push notifications, Simple caching based on max-age. (source: https://www.postscapes.com/internet-of-things-protocols/)"@en ;
    ns8:maker ns4:IETF ;
    ns4:hasClassification ns4:IIRAConnectivity,
        ns4:RAMICommunicationlayer ;
    ns4:hasDBpediaResource <http://dbpedia.org/resource/Constrained_Application_Protocol> ;
    ns4:hasDeveloper ns4:IETF ;
    ns4:hasOfficialResource <https://tools.ietf.org/html/rfc8323> ;
    ns4:hasPublisher ns4:IETF ;
    ns4:hasWikipediaArticle <http://en.wikipedia.org/wiki/Constrained_Application_Protocol> .

ns4:ServiceSelection a owl:NamedIndividual,
        ns4:Concern ;
    rdfs:label "Service Selection"@en ;
    ns2:creator ns4:sebastian ;
    rdfs:comment "The ability of a system to invoke or deploy the desired service/Data App."@en ;
    ns5:supports ns4:ServiceComposition .

ns4:SystemEngineer a ns7:StakeholderGroup,
        owl:NamedIndividual,
        ns4:Stakeholder ;
    rdfs:label "System Engineer"@en ;
    rdfs:comment ""@en ;
    ns6:note "Publications referred: '(IIC:PUB:G1:V1.80:20170131' '3.5.1 BUSINESS VIEWPOINT' 'Page 15' 'Priyanka'" .

ns4:SystemOperator a ns7:StakeholderGroup,
        owl:NamedIndividual .

ns4:TechnicalCommittee a owl:Class ;
    rdfs:label "Technical Committee" .

ns4:UDP a owl:NamedIndividual .

ns4:UserExperience a owl:NamedIndividual .

ns4:UserPreferences a owl:NamedIndividual,
        ns4:Concern ;
    rdfs:label "User Preferences"@en ;
    ns2:creator ns4:sebastian ;
    rdfs:comment "Users can have the possibility to prefer one service over another for any reason."@en ;
    rdfs:seeAlso "IoT-A Requirement UNI.253" ;
    ns5:supports ns4:ServiceLevelAgreements .

ns4:communication a owl:NamedIndividual .

ns4:x-road a owl:NamedIndividual,
        ns4:DataSharingInitiative ;
    rdfs:label "x-road" .

ns5:alignsWith a owl:ObjectProperty,
        owl:SymmetricProperty ;
    rdfs:label "alignes With"@en ;
    rdfs:comment "indicates that some Standard Classification entity has a similar scope as another. This property most probably is symmetric but not transitive."@en ;
    rdfs:domain ns4:StandardClassification ;
    rdfs:range ns4:StandardClassification ;
    rdfs:subPropertyOf ns3:associatedWith ;
    owl:inverseOf ns5:alignsWith .

xsd:date a rdfs:Datatype .

ns8:Person a owl:Class ;
    rdfs:label "Person" .

ns8:thing a owl:Class ;
    rdfs:label "thing" .

<https://w3id.org/i40/rami#AdminShellSubmodel> a owl:Class ;
    rdfs:label "Admin Shell Sub Model"@en ;
    rdfs:comment "Describes the Administration Shell concept to organize/classify standards into submodels"@en ;
    rdfs:isDefinedBy <https://www.plattform-i40.de/I40/Redaktion/EN/Downloads/Publikation/structure-of-the-administration-shell.pdf?__blob=publicationFile&v=7> ;
    rdfs:subClassOf ns4:StandardClassification .

ns4:AccessPolicy a owl:NamedIndividual,
        ns4:Concern ;
    rdfs:label "Access Policy"@en ;
    ns2:creator ns4:sebastian ;
    rdfs:comment "Access to the service shall be regulated by access policies. Users entitled in access policies to envoke a given service must be able to actually envoke it."@en ;
    rdfs:seeAlso <https://ieeexplore.ieee.org/document/6188257>,
        <https://ieeexplore.ieee.org/document/8552311>,
        "IoT-A Requirement UNI.604" ;
    ns5:supports ns4:DataAccessControl .

ns4:AutonomousConfiguration a owl:NamedIndividual,
        ns4:Concern ;
    rdfs:label "Autonomous Configuration"@en ;
    ns7:hasStakeholder <https://www.wikidata.org/wiki/Q1548249> ;
    rdfs:comment "A system built using the Reference Architecture shall be able to remotely control and configure devices."@en ;
    rdfs:seeAlso "IoT-A Requirement UNI.015",
        "IoT-A Requirement UNI.031",
        "IoT-A Requirement UNI.032",
        "IoT-A Requirement UNI.060",
        "IoT-A Requirement UNI.247",
        "IoT-A Requirement UNI.509",
        "IoT-A Requirement UNI.704",
        "IoT-A Requirement UNI.706",
        "IoT-A Requirement UNI.717" ;
    ns6:note "Publications referred: '<https://doi.org/10.1016/j.jksuci.2016.10.003>' '1.2. Utilities of IoT' 'Page 295'" ;
    ns5:supports ns4:ServiceChoreography .

ns4:Certification a owl:NamedIndividual,
        ns4:Concern ;
    rdfs:label "Certification"@en ;
    ns2:creator ns4:sebastian ;
    rdfs:comment "Certification refers to the confirmation of certain characteristics of an object, person, or organization. This confirmation is often, but not always, provided by some form of external review, education, assessment, or audit. Accreditation is a specific organization's process of certification. (source: wikipedia)"@en ;
    ns4:hasDBpediaResource <http://dbpedia.org/resource/Certification> ;
    ns5:supports ns4:Security,
        ns4:Trustworthiness .

ns4:Compliance a owl:NamedIndividual,
        ns4:Concern ;
    rdfs:label "Compliance"@en ;
    ns2:creator ns4:sebastian ;
    rdfs:comment "In general, compliance means conforming to a rule, such as a specification, policy, standard or law. Regulatory compliance describes the goal that organisations aspire to achieve in their efforts to ensure that they are aware of and take steps to comply with relevant laws and regulations. Due to the increasing number of regulations and need for operational transparency, organizations are increasingly adopting the use of consolidated and harmonized sets of compliance controls. This approach is used to ensure that all necessary governance requirements can be met without the unnecessary duplication of effort and activity from resources. (source: wikipedia)"@en ;
    ns4:hasDBpediaResource <http://dbpedia.org/resource/Regulatory_compliance> ;
    ns5:supports ns4:Reliability .

ns4:CrossDomainIdentityManagement a owl:NamedIndividual,
        ns4:Concern ;
    rdfs:label "Cross-domain Identity Management"@en ;
    ns2:creator ns4:sebastian ;
    ns7:hasStakeholder "System Architect"@en ;
    rdfs:comment "A system built using the ARM shall support identity-locator split, i.e. making the device's identity independent from its locator."@en ;
    rdfs:seeAlso "IoT-A Requirement UNI.314" ;
    ns4:hasDBpediaResource <http://dbpedia.org/resource/System_for_Cross-domain_Identity_Management> ;
    ns5:supports ns4:IdentityManagement .

ns4:DataLifecycleManagment a owl:NamedIndividual,
        ns4:Concern ;
    rdfs:label "Data lifecycle management"@en ;
    rdfs:comment "Data lifecycle management includes every phase of a \"record\" from its beginning to its end. And while it is generally applied to information that rises to the classic definition of a record (and thus related to records management), it applies to all informational assets. During its existence, information can become a record by being identified as documenting a business transaction or as satisfying a business need. (source: wikipedia)"@en ;
    ns4:hasDBpediaResource <http://dbpedia.org/resource/Information_lifecycle_management> ;
    ns5:supports ns4:DataAnalytics .

ns4:DataPublishing a owl:NamedIndividual,
        ns4:Concern ;
    rdfs:label "Data Publishing"@en ;
    ns2:creator ns4:sebastian ;
    rdfs:comment "Data Publishing is the concern regarding all aspects of getting data (publicly) available."@en ;
    ns5:supports ns4:DataAccessControl .

ns4:DataQuality a owl:NamedIndividual,
        ns4:Concern ;
    rdfs:label "Data Quality"@en ;
    ns2:creator ns4:sebastian ;
    rdfs:comment "Data quality refers to the level of quality of data. There are many definitions of data quality but data are generally considered high quality if \"they are fit for their intended uses in operations, decision making and planning.\" (Tom Redman<Redman, T.C. (2008). Data driven: Profiting from your most important business asset (p. 56). Boston, Mass.: Harvard Business Press.>). Alternatively, data is deemed of high quality if it correctly represents the real-world construct to which it refers. Furthermore, apart from these definitions, as data volume increases, the question of internal consistency within data becomes significant, regardless of fitness for use for any particular external purpose. People's views on data quality can often be in disagreement, even when discussing the same set of data used for the same purpose. (source: wikipedia)"@en ;
    rdfs:seeAlso "IoT-A Requirement UNI.235",
        "IoT-A Requirement UNI.236",
        "IoT-A Requirement UNI.237" ;
    ns4:hasDBpediaResource <http://dbpedia.org/resource/Data_quality> ;
    ns5:supports ns4:QualityOfService .

ns4:Domain a owl:Class ;
    rdfs:label "Domain"@en ;
    rdfs:comment "Represents the Domains in which the Standards can be used"@en .

ns4:EnergyControl a owl:NamedIndividual,
        ns4:Concern ;
    rdfs:label "Energy Control"@en ;
    rdfs:seeAlso <https://ieeexplore.ieee.org/document/7488250>,
        "IoT-A Requirement UNI.100",
        "IoT-A Requirement UNI.101",
        "IoT-A Requirement UNI.309",
        "IoT-A Requirement UNI.310",
        "IoT-A Requirement UNI.505",
        "IoT-A Requirement UNI.512",
        "IoT-A Requirement UNI.714" ;
    ns4:hasWikipediaArticle <https://en.wikipedia.org/wiki/Internet_of_things#Energy_management> ;
    ns5:supports ns4:EnergyEfficiency .

ns4:EnergyEfficiency a owl:NamedIndividual,
        <https://w3id.org/i40/rami#AdminShellSubmodel>,
        ns4:Concern,
        ns4:StandardClassification ;
    rdfs:label "Energy Efficiency"@en ;
    rdfs:comment "Efficient energy use, sometimes simply called energy efficiency, is the goal to reduce the amount of energy required to provide products and services."@en ;
    rdfs:seeAlso <https://dl.acm.org/citation.cfm?doid=2508075.2508082>,
        <https://dl.acm.org/citation.cfm?doid=3266237.3266263> ;
    ns4:hasWikipediaArticle <https://en.wikipedia.org/wiki/Efficient_energy_use> ;
    ns4:isDescribedin ns4:AdministrationShell ;
    ns5:supports ns4:IoT .

ns4:IDSRAMFunctionalLayer a owl:NamedIndividual,
        ns4:IDSRAMLayer,
        ns4:StandardClassification ;
    rdfs:label "IDS RAM Functional Layer"@en ;
    ns3:associatedWith ns4:DataSovereignty,
        ns4:Interoperability ;
    ns4:isDescribedin ns4:IDSRAMReferenceArchitectureModel .

ns4:IEC_62541 a owl:NamedIndividual,
        ns4:Standard ;
    ns4:hasClassification ns4:Communication,
        ns4:DataSovereignty,
        ns4:IDSRAMSystemLayer,
        ns4:IICFFrameworkLayer,
        ns4:IIRAApplicationDomain,
        ns4:IIRAOperationsDomain,
        ns4:InformationDomain,
        ns4:RAMICommunicationlayer,
        ns4:RAMIConnectedWorld,
        ns4:RAMIControlDevice,
        ns4:RAMIEnterprise,
        ns4:RAMIFieldDevice,
        ns4:RAMIStation,
        ns4:RAMIWorkCenter,
        ns4:SCADALevel ;
    ns5:hasTargetConcern ns4:AutonomousCommunication .

ns4:IEEE_802 a owl:NamedIndividual .

ns4:IEEE_802_16-2012 a owl:NamedIndividual .

ns4:IIC_PUB_G1_V1_80_20170131 a owl:NamedIndividual,
        ns1:oaSpecificResource ;
    rdfs:label "The Industrial Internet of Things Volume G1: Reference Architecture IIC:PUB:G1:V1.80:20170131"@en ;
    ns4:hasOpenResource <https://www.iiconsortium.org/IIC_PUB_G1_V1.80_2017-01-31.pdf> .

ns4:IIRAPrivacy a owl:NamedIndividual,
        ns4:IIRASystemCharacteristics,
        ns4:StandardClassification ;
    rdfs:label "IIRA Privacy"@en ;
    ns3:associatedWith ns4:DtpSecurityPrivacy ;
    ns3:isPartOf ns4:IIRAFunctionalViewpoint ;
    ns4:isDescribedin ns4:IIRA ;
    ns5:alignsWith ns4:DtpSecurityPrivacy ;
    ns5:frames ns4:DataSovereignty,
        ns4:Privacy,
        ns4:Trustworthiness .

ns4:IIRAScalability a owl:NamedIndividual,
        ns4:IIRASystemCharacteristics,
        ns4:StandardClassification ;
    rdfs:label "IIRA Scalability"@en ;
    ns3:associatedWith ns4:FiwareCloudHosting ;
    ns3:isPartOf ns4:IIRAFunctionalViewpoint ;
    ns4:isDescribedin ns4:IIRA ;
    ns5:alignsWith ns4:FiwareCloudHosting ;
    ns5:frames ns4:Scalability .

ns4:IPv6 a owl:NamedIndividual,
        ns8:Document,
        ns4:Publication,
        ns4:TechnicalSpecification ;
    rdfs:label "IPv6"@en ;
    ns2:creator ns4:sebastian ;
    rdfs:comment "IPv6, is an Internet Layer protocol for packet-switched internetworking and provides end-to-end datagram transmission across multiple IP networks. (source: https://www.postscapes.com/internet-of-things-protocols/)"@en ;
    ns4:hasWikipediaArticle <https://en.wikipedia.org/wiki/IPv6> ;
    ns5:hasTargetConcern ns4:SyntacticInteroperability .

ns4:ISA95Level a owl:Class ;
    rdfs:label "ISA 95 Level"@en ;
    rdfs:comment "Describes the ISA95 levels to classify the industry Standards according to those levels. Eg., Device, SCADA, etc. It has strong relation to the RAMI Hierarchy levels"@en ;
    rdfs:subClassOf ns4:StandardClassification .

ns4:MachineLearning a owl:NamedIndividual,
        ns4:Concern ;
    rdfs:label "Machine Learning"@en ;
    ns2:creator ns4:sebastian ;
    rdfs:comment "Machine learning is the subfield of computer science that \"gives computers the ability to learn without being explicitly programmed\" (Arthur Samuel, 1959). Evolved from the study of pattern recognition and computational learning theory in artificial intelligence, machine learning explores the study and construction of algorithms that can learn from and make predictions on data – such algorithms overcome following strictly static program instructions by making data-driven predictions or decisions, through building a model from sample inputs. (source: wikipedia)"@en ;
    ns4:hasDBpediaResource <http://dbpedia.org/resource/Machine_learning> ;
    ns5:supports ns4:AI .

ns4:Ocean_Protocol_Business_Strategy_Oct_2017 a owl:NamedIndividual,
        ns1:oaSpecificResource ;
    rdfs:label "Ocean Protocol: A Decentralized Data Exchange Protocol,powered by blockchain technology and a cryptotoken. Business Strategy. Oct 2017"@en ;
    ns4:hasOpenResource <https://oceanprotocol.com/business-strategy.pdf> .

ns4:Ocean_Protocol_Reference_Marketplace_Framework_Feb_2019 a owl:NamedIndividual,
        ns1:oaSpecificResource ;
    rdfs:label "Ocean Protocol: A Decentralized Data Exchange Protocol to Unlock Data for Artificial Intelligence. Reference Marketplace Framework. Feb 2019"@en ;
    ns4:hasOpenResource <https://oceanprotocol.com/marketplace-framework.pdf> .

ns4:Ocean_Protocol_Technical_Whitepaper_Apr_2019 a owl:NamedIndividual,
        ns1:oaSpecificResource ;
    rdfs:label "Ocean Protocol: A Decentralized Substrate for AI Data & Services . Technical Whitepaper. Apr 2019"@en ;
    ns4:hasOpenResource <https://oceanprotocol.com/tech-whitepaper.pdf> .

ns4:OpenConnectivityFoundation a owl:NamedIndividual,
        ns4:StandardOrganization ;
    rdfs:label "Open Connectivity Foundation" ;
    rdfs:comment "The Open Connectivity Foundation (OCF) is an industry group whose stated mission is to develop specification standards, promote a set of interoperability guidelines, and provide a certification program for devices involved in the Internet of Things (IoT). It has become one of the biggest industrial connectivity standards organizations for IoT, including in its membership Samsung Electronics, Intel, Microsoft, Qualcomm and Electrolux. Currently, there are more than 300 member companies. source: wikipedia"@en ;
    rdfs:seeAlso <https://openconnectivity.org/> ;
    ns4:hasDBpediaResource <https://dbpedia.org/resource/Open_Connectivity_Foundation> .

ns4:OpenFogConsortium a owl:NamedIndividual,
        ns4:IIoTConsortium ;
    rdfs:label "OpenFog Consortium",
        "OpenFog Consortium"@en ;
    rdfs:comment "The OpenFog Consortium work is done by committees and workgroups focused on specific tasks aligned to our mission. This work includes technical work; influencing standards development through liaisons with other organizations; testbed; promoting innovation and industry interest in fog computing; and industry education."@en ;
    ns4:hasOfficialResource <https://www.openfogconsortium.org/> ;
    ns4:seeAlso <https://www.openfogconsortium.org/> .

ns4:OpenFogSecurityPerspective a owl:NamedIndividual .

ns4:PhysicalConnectivity a owl:NamedIndividual,
        ns4:Concern ;
    rdfs:label "Physical Connectivity"@en ;
    ns2:creator ns4:sebastian ;
    rdfs:comment "Physical Connectivity is the concern including all aspects of low-level connectivity and transporting a physical (electrical) signal from A to B. This might be achieved through wired connections (e.g. ethernet) but also wireless (e.g. WIFI)."@en ;
    ns5:supports ns4:Interoperability .

ns4:PlatformIndustry40 a owl:NamedIndividual,
        ns8:Organization,
        ns4:IIoTConsortium ;
    rdfs:label "Plattform Industrie 4.0"@de,
        "Platform Industry 4.0"@en ;
    ns2:creator ns4:sebastian ;
    ns3:associatedWith ns4:RAMI .

ns4:ProductLiability a owl:NamedIndividual,
        ns4:Concern ;
    rdfs:label "Product Liability"@en ;
    ns6:note "Publications referred: '(IIC:PUB:G1:V1.80:20170131' '4 BUSINESS VIEWPOINT' 'Page 20' " ;
    ns5:supports ns4:BusinessContext .

ns4:RAMIConnectedWorld a owl:NamedIndividual,
        <https://w3id.org/i40/rami#RAMIHierarchyLevel> ;
    ns5:frames ns4:Interoperability,
        ns4:SemanticInteroperability,
        ns4:ThingDescription .

ns4:RAMIControlDevice a owl:NamedIndividual .

ns4:RAMIEnterprise a owl:NamedIndividual .

ns4:RAMIFieldDevice a owl:NamedIndividual,
        <https://w3id.org/i40/rami#RAMIHierarchyLevel>,
        ns4:StandardClassification ;
    ns5:frames ns4:Manufacturing .

ns4:RAMIStation a owl:NamedIndividual .

ns4:RFC_6750 a owl:NamedIndividual,
        ns8:Document,
        ns4:Publication,
        ns4:Standard ;
    rdfs:label "RFC 6750"@en ;
    ns2:creator ns4:IETF ;
    ns2:description "This specification describes how to use bearer tokens in HTTP requests to access OAuth 2.0 protected resources.  Any party in possession of a bearer token (a \"bearer\") can use it to get access to the associated resources (without demonstrating possession of a cryptographic key).  To prevent misuse, bearer tokens need to be protected from disclosure in storage and in transport."@en ;
    ns3:associatedWith ns4:DtpArchitecture ;
    rdfs:comment "This specification describes how to use bearer tokens in HTTP requests to access OAuth 2.0 protected resources.  Any party in possession of a bearer token (a \"bearer\") can use it to get access to the associated resources (without demonstrating possession of a cryptographic key).  To prevent misuse, bearer tokens need to be protected from disclosure in storage and in transport."@en ;
    ns6:altLabel "OAuth2.0"@en ;
    ns8:maker ns4:IETF ;
    ns4:hasClassification ns4:IDSRAMSecurity ;
    ns4:hasDBpediaResource <http://dbpedia.org/resource/OAuth> ;
    ns4:hasOfficialResource <https://tools.ietf.org/html/rfc6750> ;
    ns4:hasPublisher ns4:IETF .

ns4:RealTimeAnalytics a owl:NamedIndividual,
        ns4:Concern ;
    rdfs:label "Real Time Analytics"@en ;
    ns7:hasStakeholder <http://purl.oclc.org/NET/mvco.owl#EndUser> ;
    rdfs:comment "In computer science, real-time computing (RTC), or reactive computing describes hardware and software systems subject to a \"real-time constraint\", for example from event to system response. Real-time programs must guarantee response within specified time constraints, often referred to as \"deadlines\". Systems of this type whose correctness depends on their temporal aspects as well as their functional aspects. Real-time responses are often understood to be in the order of milliseconds, and sometimes microseconds."@en ;
    rdfs:seeAlso "IoT-A Requirement UNI.020" ;
    ns4:hasDBpediaResource <http://dbpedia.org/resource/Real-time_computing> ;
    ns5:supports ns4:DataAnalytics .

ns4:ReturnOnInvestment a owl:NamedIndividual,
        ns4:Concern ;
    rdfs:label "Return On Investment"@en ;
    ns6:note "Publications referred: '(IIC:PUB:G1:V1.80:20170131' '4 BUSINESS VIEWPOINT' 'Page 20' " ;
    ns5:supports ns4:BusinessContext .

ns4:StandardPart a owl:Class ;
    rdfs:label "StandardPart" ;
    rdfs:comment "Typically Standards are divided into parts. E.g., ISA 95 has part Part 1: Models and Terminology, Part 2: Object Model Attributes, etc."@en ;
    rdfs:subClassOf ns4:Publication .

ns4:TechnicalReport a owl:Class,
        owl:namedIndividial ;
    rdfs:label "Technical Report"@en ;
    ns9:attributionURL "http://www.iec.ch" ;
    rdfs:comment "Specifies that a given Publication is a Technical Report"@en,
        "Technical Reports contain collected data of a kind different from that normally published as an International Standard, for example data obtained from a survey carried out among national committees, data of work in other international organizations or data on \"the state of the art\" in relation to standards of national committees on a particular subject.Technical Reports are entirely informative in nature and shall not contain matter implying that they are normative"@en ;
    rdfs:isDefinedBy ns4:IEC ;
    rdfs:seeAlso <http://www.iec.ch/standardsdev/publications/tr.htm> ;
    rdfs:subClassOf ns4:Publication ;
    ns4:abbreviation "TR" .

ns4:Technology a owl:Class ;
    rdfs:label "Technology"@en ;
    ns2:creator ns4:sebastian,
        "sebastian"@en ;
    rdfs:comment "A Technology is an implementation of one or many standards in order to achieve a goal."@en .

ns4:Vocabulary a owl:NamedIndividual .

ns4:WiFi a owl:NamedIndividual .

ns4:XACML a owl:NamedIndividual,
        ns8:Document,
        ns4:Publication,
        ns4:TechnicalSpecification ;
    ns3:associatedWith ns4:FiwareSecurity ;
    ns5:hasTargetConcern ns4:Authorization,
        ns4:DataAccessControl .

ns4:xRoadTechnologyMatrix a owl:NamedIndividual,
        ns4:StandardClassification,
        ns4:xRoadSection ;
    rdfs:label "x-road Technology Matrix"@en ;
    ns4:isDescribedin ns4:xTee .

<https://w3id.org/ids/core/TrustedConnector> a owl:NamedIndividual,
        ns4:Technology ;
    rdfs:label "Trusted Connector"@en ;
    ns2:creator ns4:IDSRAMReferenceArchitectureModel ;
    ns3:associatedWith ns4:AdministrationShell,
        ns4:IDSRAMReferenceArchitectureModel ;
    rdfs:comment "TODO: model IDS concepts correctly"@en ;
    ns8:maker ns4:IDSRAMReferenceArchitectureModel ;
    ns5:alignsWith ns4:AdministrationShell .

rdf:PlainLiteral a owl:Class ;
    rdfs:label "Plain Literal" .

rdfs:Datatype a owl:Class ;
    rdfs:label "Datatype" .

ns8:maker a owl:ObjectProperty .

<https://w3id.org/i40/rami#RAMIHierarchyLevel> a owl:Class ;
    rdfs:label "RAMI Hierarchy Level"@en ;
    rdfs:subClassOf ns4:StandardClassification ;
    owl:equivalentClass [ a owl:Class ;
            owl:oneOf ( <https://w3id.org/i40/rami#ConnectedWorld> <https://w3id.org/i40/rami#ControlDevice> <https://w3id.org/i40/rami#Enterprise> <https://w3id.org/i40/rami#FieldDevice> <https://w3id.org/i40/rami#Product> <https://w3id.org/i40/rami#Station> <https://w3id.org/i40/rami#WorkCenter> ) ] .

ns4:Actuation a owl:NamedIndividual,
        ns4:Concern ;
    rdfs:label "Actuation"@en ;
    ns2:creator ns4:sebastian ;
    rdfs:comment "Sending data or a signal to a kind of actuating device, which leads to a change in a defined environment."@en ;
    ns6:note "Publications referred: 'IIC:PUB:G1:V1.80:20170131' '6.1 THE CONTROL DOMAIN' 'Page 28' " ;
    ns4:hasDBpediaResource <http://dbpedia.org/resource/Actuator> ;
    ns5:supports ns4:IoT .

ns4:AutonomousCommunication a owl:NamedIndividual,
        ns4:Concern ;
    rdfs:label "Autonomous Communication"@en ;
    ns7:hasStakeholder <https://www.wikidata.org/wiki/Q1548249> ;
    rdfs:comment "Authonomous Communication frames all requirements in order to autonomously establish communication channels between participants of a network. In most cases, this will be a machine-to-machine communication channel. Main challenges are related to interoperability."@en ;
    rdfs:seeAlso "IoT-A Requirement UNI.005",
        "IoT-A Requirement UNI.012",
        "IoT-A Requirement UNI.708" ;
    ns5:supports ns4:Communication,
        ns4:ServiceChoreography .

ns4:BdvaCloudAndHighPerformanceComputing a owl:NamedIndividual,
        ns4:BdvaConcern,
        ns4:StandardClassification ;
    rdfs:label "BDVA Cloud and High Performance Computing"@en ;
    ns2:creator ns4:sebastian ;
    ns3:associatedWith ns4:IIRAApplicationDomain ;
    rdfs:comment "The Cloud and High Performance Computing (HPC): Effective Big Data processing and data management might imply the effective usage of Cloud and High Performance Computing infrastructures. This area is separately elaborated further in collaboration with the Cloud and High Performance Computing (ETP4HPC) communities."@en ;
    ns4:isDescribedin ns4:BdvaSira ;
    ns5:alignsWith ns4:IIRAApplicationDomain ;
    ns5:frames ns4:AI,
        ns4:BigDataApplications,
        ns4:CloudComputing,
        ns4:DataAnalytics,
        ns4:DataProcessing,
        ns4:DataPublishing,
        ns4:MachineLearning .

ns4:BusinessValue a owl:NamedIndividual,
        ns4:Concern ;
    rdfs:label "Business Value"@en ;
    ns2:creator ns4:sebastian ;
    ns6:note "Publications referred: '(IIC:PUB:G1:V1.80:20170131' '4 BUSINESS VIEWPOINT' 'Page 20' " ;
    ns5:supports ns4:BusinessContext .

ns4:CardinalityOfParticipants a owl:NamedIndividual,
        ns4:Concern ;
    rdfs:label "Cardinality of Participants"@en ;
    ns2:creator ns4:sebastian ;
    rdfs:comment "Data Artefacts from different Data Providers are delivered in order to provide additional insights (e.g. Collaborative Predictive Maintenance)."@en ;
    ns4:hasDBpediaResource <http://dbpedia.org/resource/Cardinality_(computer_engineering)> ;
    ns5:supports ns4:interoperability .

ns4:DataEconomy a owl:NamedIndividual,
        ns4:Concern ;
    rdfs:label "Data Economy"@en ;
    ns2:creator ns4:sebastian ;
    rdfs:comment "Business aspects of data exchange"@en,
        "Digital economy refers to an economy that is based on digital computing technologies. The digital economy is also sometimes called the Internet Economy, the New Economy, or Web Economy. Increasingly, the \"digital economy\" is intertwined with the traditional economy making a clear delineation harder. (source: wikipedia)"@en ;
    ns4:hasDBpediaResource <http://dbpedia.org/resource/Digital_economy> ;
    ns5:supports ns4:BusinessContext .

ns4:DataProtection a owl:NamedIndividual,
        ns4:Concern ;
    rdfs:label "Data Protection"@en ;
    ns2:creator ns4:sebastian ;
    rdfs:comment "Data protection is the relationship between collection and dissemination of data, technology, the public expectation of privacy, and the legal and political issues surrounding them. Privacy concerns exist wherever personally identifiable information or other sensitive information is collected, stored, used, and finally destroyed or deleted – in digital form or otherwise. Improper or non-existent disclosure control can be the root cause for privacy issues. (source: wikipedia)"@en ;
    owl:sameAs ns4:DataSecurity ;
    ns6:altLabel "Datenschutz"@de,
        "Information privacy"@en ;
    ns4:hasDBpediaResource <http://dbpedia.org/resource/Information_privacy> ;
    ns5:supports ns4:Privacy .

ns4:DataSharingInitiative a owl:Class,
        owl:NamedIndividual ;
    rdfs:label "Data Sharing Initiative"@en ;
    ns2:creator ns4:sebastian ;
    rdfs:comment "This class frames all organizations with the main intend to create, specify and implement a data sharing concept with according interfaces, components, data descriptions, and retrieval algorithms."@en ;
    rdfs:subClassOf ns8:Organization .

ns4:DataUsageControl a owl:NamedIndividual,
        ns4:Concern ;
    rdfs:label "Data Usage Control"@en ;
    ns2:creator ns4:sebastian ;
    rdfs:comment "Data usage control can be seen as an extension of data access control. It is about the specification and enforcement of restrictions regulating what is allowed to happen with data, and what is not. Data usage control thus is concerned with requirements that pertain to data processing (obligations) rather than data access (provisions). It is primarily relevant in the context of intellectual property protection, privacy protection, compliance with regulations, and digital rights management."@en ;
    ns5:supports ns4:Authorization .

ns4:DecisionMaker a owl:NamedIndividual,
        ns4:Stakeholder ;
    rdfs:label "Decision maker"@en ;
    rdfs:comment "These are business Decision makers"@en ;
    ns6:note "Publications referred: '(IIC:PUB:G1:V1.80:20170131' '3.5.1 BUSINESS VIEWPOINT' 'Page 15' 'Priyanka'" .

ns4:EndpointDescription a owl:NamedIndividual,
        ns4:Concern ;
    rdfs:label "Endpoint Description"@en ;
    ns2:creator ns4:sebastian ;
    rdfs:comment "Methods to unambiguously describe client and server endpoints."@en ;
    ns5:supports ns4:SemanticInteroperability .

ns4:EstonianInformationSystemAuthority a owl:NamedIndividual .

ns4:IPv4Support a owl:NamedIndividual,
        ns4:Concern ;
    rdfs:label "IPv4 Support"@en ;
    ns2:creator ns4:sebastian ;
    ns7:hasStakeholder "System Architect"@en ;
    rdfs:comment "Communication with non-IPv6 networks must be possible (IPv4, others)."@en ;
    rdfs:seeAlso "IoT-A Requirement UNI.313" ;
    ns4:hasDBpediaResource <http://dbpedia.org/resource/Internet_Protocol> ;
    ns5:supports ns4:SyntacticInteroperability .

ns4:IdsPerspective a owl:Class,
        owl:NamedIndividual ;
    rdfs:label "IDS RAM Perspective"@en ;
    ns2:creator ns4:sebastian ;
    rdfs:subClassOf ns4:StandardClassification ;
    owl:equivalentClass [ a owl:Class ;
            owl:oneOf ( ns4:IDSRAMCertification ns4:IDSRAMGovernance ns4:IDSRAMSecurity ) ] .

ns4:IndustrialInternetArchitecture a owl:NamedIndividual,
        ns4:ArchitectureDescription ;
    rdfs:label "AII Industrial Internet Architecture"@en ;
    ns4:hasOfficialResource <http://en.aii-alliance.org/uploadfile/2017/0307/Industrial.pdf> ;
    ns4:hasPublisher ns4:AllianceOfIndustrialInternet .

ns4:IotaAvailabilityResilience a owl:NamedIndividual,
        ns4:IotaPerspective,
        ns4:StandardClassification ;
    rdfs:label "IoT-A Availability and Resilience"@en ;
    ns3:associatedWith ns4:Security ;
    ns4:isDescribedin ns4:IotaReferenceArchitecture ;
    ns5:alignsWith ns4:Security ;
    ns5:frames ns4:Availability,
        ns4:Resilience,
        ns4:Security,
        ns4:Trustworthiness .

ns4:IviActivityView a owl:NamedIndividual,
        ns4:StandardClassification,
        ns4:Viewpoint ;
    rdfs:label "IVI Activity View"@en ;
    ns2:creator ns4:sebastian ;
    ns3:associatedWith <https://w3id.org/i40/rami#Engineering>,
        ns4:IIRAOperationsDomain ;
    ns4:isDescribedin ns4:IVRA ;
    ns5:alignsWith <https://w3id.org/i40/rami#Engineering>,
        ns4:IIRAOperationsDomain ;
    ns5:frames ns4:Manufacturing .

ns4:IviLayer a owl:Class ;
    rdfs:label "IVI Layer"@en ;
    ns2:creator ns4:sebastian ;
    rdfs:comment "A IVI Layer describes one of three layers of smart manufactoring as proposed by the Industrial Value Chain Initiative (IVI)."@en ;
    rdfs:isDefinedBy <https://iv-i.org/wp/wp-content/uploads/2018/04/IVRA-Next_en.pdf> ;
    rdfs:subClassOf ns4:StandardClassification .

ns4:Multilaterism a owl:NamedIndividual,
        ns4:Concern ;
    rdfs:label "Multilateralism"@en ;
    ns2:creator ns4:sebastian ;
    rdfs:comment "Data Artefacts are received by 1 to m Data Consumer."@en ;
    ns6:altLabel "Cardinality of Participants"@en,
        "Multicast"@en ;
    ns5:supports ns4:CardinalityOfDataSources .

ns4:OceanBusinessViewpoint a owl:NamedIndividual,
        ns4:StandardClassification,
        ns4:Viewpoint ;
    rdfs:label "Ocean Protocol Business Viewpoint"@en ;
    ns3:associatedWith ns4:IIRABusinessViewpoint ;
    ns4:isDescribedin ns4:OceanProtocol ;
    ns5:alignsWith ns4:IIRABusinessViewpoint ;
    ns5:frames ns4:BusinessContext,
        ns4:BusinessTransactions,
        ns4:RoleCategorization,
        ns4:Trustworthiness .

ns4:OceanMarketplaceViewpoint a owl:NamedIndividual,
        ns4:StandardClassification,
        ns4:Viewpoint ;
    rdfs:label "Ocean Protocol Marketplace Viewpoint"@en ;
    ns3:associatedWith ns4:IIRABusinessViewpoint ;
    ns4:isDescribedin ns4:OceanProtocol ;
    ns5:alignsWith ns4:IIRABusinessViewpoint ;
    ns5:frames ns4:BusinessContext .

ns4:OceanProtocol a owl:NamedIndividual,
        ns8:Document,
        ns4:Publication,
        ns4:StandardizationFramework,
        ns4:TechnicalSpecification ;
    rdfs:label "Ocean Protocol"@en ;
    ns2:creator ns4:OceanProtocolFoundation ;
    rdfs:comment "Ocean is a decentralized protocol and network of artificial intelligence (AI) data/services. It incentivizes for a vast supply of relevant AI data/services. This network helps to power AI data/service marketplaces, as well as public commons data. The heart of Ocean’s network is a new construction: a Curated Proofs Market. CPMs bridge predicted relevance with actual relevance of each AI service, by having curation markets for cryptographic proofs (e.g. proof of data availability). (source: https://oceanprotocol.com/tech-whitepaper.pdf)"@en ;
    rdfs:seeAlso <https://oceanprotocol.com/tech-whitepaper.pdf> ;
    ns8:maker ns4:OceanProtocolFoundation ;
    ns4:hasDeveloper ns4:OceanProtocolFoundation ;
    ns4:hasOfficialResource <https://oceanprotocol.com/> ;
    ns4:hasPublisher ns4:OceanProtocolFoundation .

ns4:ProvenanceTracking a owl:NamedIndividual,
        ns4:Concern ;
    rdfs:label "Provenance Tracking"@en ;
    ns2:creator ns4:sebastian ;
    ns7:hasStakeholder <http://purl.oclc.org/NET/mvco.owl#EndUser> ;
    rdfs:comment "Data provenance includes the data's origins, what happens to it and where it moves/moved over time."@en ;
    rdfs:seeAlso "IoT-A Requirement UNI.041",
        "IoT-A Requirement UNI.606" ;
    ns4:hasDBpediaResource <http://dbpedia.org/resource/Data_lineage> ;
    ns5:supports ns4:Security .

ns4:REST a owl:NamedIndividual,
        ns8:Document,
        ns4:Publication,
        ns4:TechnicalSpecification ;
    rdfs:label "REST"@en ;
    ns2:creator ns4:sebastian ;
    ns3:associatedWith ns4:DtpDeploymentView ;
    rdfs:comment "REST (Representational state transfer) - RESTful HTTP (source: https://www.postscapes.com/internet-of-things-protocols/)"@en ;
    ns4:hasWikipediaArticle <https://en.wikipedia.org/wiki/Representational_state_transfer> .

ns4:SecurityConfiguration a owl:NamedIndividual,
        ns4:Concern ;
    rdfs:label "Security Configuration"@en ;
    rdfs:comment "Users should be able to monitor and control the security and privacy settings of all the devices that they own."@en ;
    rdfs:seeAlso "IoT-A Requirement UNI.625" ;
    ns4:hasDBpediaResource <http://dbpedia.org/resource/Hardening_(computing)> ;
    ns5:supports ns4:Security .

ns4:Sensing a owl:NamedIndividual,
        ns4:Concern ;
    rdfs:label "Sensing"@en ;
    ns2:creator ns4:sebastian ;
    rdfs:comment "The concern of being able to measure values from a defined environment."@en ;
    ns6:note "Publications referred: 'IIC:PUB:G1:V1.80:20170131' '6.1 THE CONTROL DOMAIN' 'Page 28' " ;
    ns4:hasDBpediaResource <http://dbpedia.org/resource/Sensor> ;
    ns5:supports ns4:IoT .

ns4:ServiceIsolation a owl:NamedIndividual,
        ns4:Concern ;
    rdfs:label "Service Isolation"@en ;
    ns2:creator ns4:sebastian ;
    rdfs:comment "Service isolation via a process group (as done with Docker) or by least privilege with clear separation and support for additional security modules (as done by trustme)."@en ;
    ns6:narrower ns4:Isolation ;
    ns4:hasDBpediaResource <http://dbpedia.org/resource/Process_isolation> .

ns4:Stakeholder a owl:Class ;
    rdfs:label "Layer"@en,
        "Stakeholder"@en ;
    rdfs:comment " A stakeholder is an individual, team, organization or classes thereof,having an interest in a concern and by extension an interest in the viewpoint and system.",
        "Describes the layers of the standardization frameworks. In some cases, the layers are connected to dimensions of the frameworks. "@en ;
    rdfs:seeAlso "IIC:PUB:G1:V1.80:20170131" ;
    rdfs:subClassOf ns8:Person ;
    ns6:note "Publications referred: 'IIC:PUB:G1:V1.80:20170131' '4.1 STAKEHOLDERS' 'Page 20' " ;
    ns4:hasWikipediaArticle <https://en.wikipedia.org/wiki/Stakeholder> .

ns4:TimeSynchronization a owl:NamedIndividual,
        ns4:Concern ;
    rdfs:label "Time Synchronization"@en ;
    ns2:creator ns4:sebastian ;
    ns7:hasStakeholder <https://w3id.org/i40/Developer> ;
    rdfs:seeAlso "IoT-A Requirement UNI.089" ;
    ns4:hasDBpediaResource <http://dbpedia.org/resource/Synchronization_(computer_science)>,
        "Synchronization refers to one of two distinct but related concepts: synchronization of processes, and synchronization of data. Process synchronization refers to the idea that multiple processes are to join up or handshake at a certain point, in order to reach an agreement or commit to a certain sequence of action. Data synchronization refers to the idea of keeping multiple copies of a dataset in coherence with one another, or to maintain data integrity. Process synchronization primitives are commonly used to implement data synchronization. (sourc: wikipedia)"@en ;
    ns5:supports ns4:ServiceComposition .

ns4:Unicast a owl:NamedIndividual,
        ns4:Concern ;
    rdfs:label "Unicast"@en ;
    ns2:creator ns4:sebastian ;
    rdfs:comment "one-to-one connectivity"@en ;
    rdfs:seeAlso "IoT-A Requirement UNI.301",
        "IoT-A Requirement UNI.304" ;
    ns5:supports ns4:CardinalityOfDataSources .

ns4:UserInteraction a owl:NamedIndividual,
        ns4:Concern ;
    rdfs:label "User Interaction"@en ;
    ns2:creator ns4:sebastian ;
    ns7:hasStakeholder <http://purl.oclc.org/NET/mvco.owl#EndUser> ;
    rdfs:comment "Interaction design, often abbreviated as IxD, is defined as \"the practice of designing interactive digital products, environments, systems, and services.\" While the digital side of this statement is true, Interaction design is also valid when creating physical (non-digital) products, covering the ideology of how a user may interact with it. (source: wikipedia)"@en ;
    rdfs:seeAlso "IoT-A Requirement UNI.019",
        "IoT-A Requirement UNI.092",
        "IoT-A Requirement UNI.214",
        "IoT-A Requirement UNI.252" ;
    ns4:hasDBpediaResource <http://dbpedia.org/resource/Interaction_design> ;
    ns5:supports ns4:UserExperience .

ns4:interoperability a owl:NamedIndividual .

ns4:AI a owl:NamedIndividual,
        ns4:Concern ;
    rdfs:label "Artificial Intelligence"@en ;
    ns2:creator ns4:sebastian ;
    rdfs:comment "Artificial intelligence (AI) is intelligence exhibited by machines. In computer science, an ideal \"intelligent\" machine is a flexible rational agent that perceives its environment and takes actions that maximize its chance of success at some goal. Colloquially, the term \"artificial intelligence\" is applied when a machine mimics \"cognitive\" functions that humans associate with other human minds, such as \"learning\" and \"problem solving\". (source: wikipedia)"@en ;
    ns4:hasDBpediaResource <http://dbpedia.org/resource/Artificial_intelligence>,
        ""@en ;
    ns5:supports ns4:DataAnalytics .

ns4:AiiClassification a owl:Class ;
    rdfs:label "Alliance of Industrial Internet Architecture Classification"@en ;
    ns2:creator ns4:sebastian ;
    rdfs:subClassOf ns4:StandardClassification .

ns4:BusinessTransactions a owl:NamedIndividual,
        ns4:Concern ;
    rdfs:label "Business Transactions"@en ;
    ns2:creator ns4:sebastian ;
    rdfs:comment "A financial transaction is an agreement, communication, or movement carried out between a buyer and a seller to exchange an asset for payment. It involves a change in the status of the finances of two or more businesses or individuals. The buyer and seller are separate entities or objects, often involving the exchange of items of value, such as information, goods, services, and money. It is still a transaction if the goods are exchanged at one time, and the money at another. This is known as a two-part transaction: part one is giving the money, part two is receiving the goods. (source: wikipedia)"@en ;
    ns4:hasDBpediaResource <http://dbpedia.org/resource/Financial_transaction> ;
    ns5:supports ns4:BusinessContext .

ns4:Connectivity a owl:NamedIndividual,
        ns4:Concern ;
    rdfs:label "Connectivity"@en ;
    ns2:creator ns4:MuhammadUsman ;
    rdfs:comment """Internet of Things associates various smart devices through the Internet, and it gives a facility to concentrated checking and control of associated
equipment."""@en ;
    rdfs:seeAlso <https://ieeexplore.ieee.org/document/6188257> ;
    ns4:hasDBpediaResource <http://dbpedia.org/property/connectivity> ;
    ns4:hasWikipediaArticle <https://en.wikipedia.org/wiki/Connectivity> ;
    ns5:supports ns4:SyntacticInteroperability .

ns4:DataAtRest a owl:NamedIndividual,
        ns4:Concern ;
    rdfs:label "Data at rest"@en ;
    ns2:creator ns4:sebastian ;
    rdfs:comment "Data at rest in information technology means inactive data that is stored physically in any digital form (e.g. databases, data warehouses, spreadsheets, archives, tapes, off-site backups, mobile devices etc.). Data at rest is used as a complement to the terms data in use and data in transit which together define the three states of digital Data. (source: wikipedia)"@en ;
    ns4:hasDBpediaResource <http://dbpedia.org/resource/Data_at_rest> ;
    ns5:supports ns4:Communication .

ns4:DataMarketAustria a owl:NamedIndividual,
        ns8:Organization,
        ns4:DataSharingInitiative,
        ns4:StandardOrganization ;
    rdfs:label "DMA"@en ;
    ns2:creator ns4:sebastian ;
    ns2:title "Data Market Austria"@en ;
    ns4:hasOfficialResource <http://www.datamarket.at/> .

ns4:EdgecrossArchitecture a owl:NamedIndividual,
        ns4:ArchitectureDescription,
        ns4:StandardizationFramework ;
    rdfs:label "Edgecross Architecture"@en ;
    ns4:hasPublisher ns4:EdgecrossConsortium .

ns4:EdgecrossConsortium a owl:NamedIndividual,
        ns8:Organization,
        ns4:IIoTConsortium,
        ns4:StandardOrganization ;
    rdfs:label "Edgecross Consortium"@en ;
    ns4:hasOfficialResource <https://www.edgecross.org/en/> .

ns4:EdgecrossLayer a owl:Class ;
    rdfs:label "Edgecross Layer"@en ;
    rdfs:subClassOf [ a owl:Restriction ;
            owl:hasValue ns4:EdgecrossArchitecture ;
            owl:onProperty ns4:isDescribedin ],
        ns4:StandardClassification .

ns4:Governance a owl:NamedIndividual,
        ns4:Concern ;
    ns5:supports ns4:BusinessContext .

ns4:IIC a owl:NamedIndividual,
        ns8:Organization,
        ns4:IIoTConsortium,
        ns4:StandardOrganization ;
    rdfs:label "IIC"@en,
        "Industrial Internet Consortium"@en ;
    ns2:creator ns4:sebastian ;
    ns3:associatedWith ns4:IIRA ;
    rdfs:comment "Founded in 2014 to further development, adoption and wide-spread use of interconnected machines, intelligent analytics and people at work. (source: https://www.postscapes.com/internet-of-things-protocols/)"@en ;
    ns4:hasOfficialResource <http://www.iiconsortium.org/> .

ns4:IIRADistributedDataManagement a owl:NamedIndividual,
        ns4:IIRACrosscuttingFunction,
        ns4:StandardClassification ;
    rdfs:label "IIRA Distributed Data Management"@en ;
    ns2:creator ns4:sebastian ;
    ns3:associatedWith ns4:FiwareCloudHosting,
        ns4:RAMICommunicationlayer ;
    ns3:isPartOf ns4:IIRAFunctionalViewpoint ;
    ns4:isDescribedin ns4:IIRA ;
    ns5:alignsWith ns4:FiwareCloudHosting,
        ns4:RAMICommunicationlayer ;
    ns5:frames ns4:Interoperability,
        ns4:SemanticInteroperability .

ns4:IPv6Support a owl:NamedIndividual,
        ns4:Concern ;
    rdfs:label "IPv6 Support"@en ;
    ns2:creator ns4:sebastian ;
    ns7:hasStakeholder "System Architect"@en ;
    rdfs:comment "A system built using the ARM shall use/support common-addressing-schemes such as IPv6."@en ;
    rdfs:seeAlso "IoT-A Requirement UNI.312" ;
    ns4:hasDBpediaResource <http://dbpedia.org/resource/Internet_Protocol> ;
    ns5:supports ns4:SyntacticInteroperability .

ns4:MaintenanceCost a owl:NamedIndividual,
        ns4:Concern ;
    rdfs:label "Maintenance Cost"@en ;
    rdfs:comment "The ability of a system to be maintained."@en ;
    ns6:note "Publications referred: '<https://www.openfogconsortium.org/wp-content/uploads/OpenFog_Reference_Architecture_2_09_17-FINAL.pdf> OPFRA001.020817' '3 Use Cases for Fog' 'Page 13' ",
        "Publications referred: 'IIC:PUB:G1:V1.80:20170131' '4 BUSINESS VIEWPOINT' 'Page 20' " ;
    ns5:supports ns4:BusinessContext .

ns4:NGSI_Context_Information_Management_API a owl:Class ;
    rdfs:label "NGSI Context Information Management API"@en ;
    ns2:creator ns4:sebastian ;
    ns2:title "NGSI-LD" ;
    rdfs:subClassOf [ a owl:Restriction ;
            owl:hasValue ns4:FIWARE ;
            owl:onProperty ns4:isDescribedin ],
        ns4:StandardClassification .

ns4:NetworkPerformance a owl:NamedIndividual,
        ns4:Concern ;
    rdfs:label "Network performance"@en ;
    rdfs:comment "Network performance refers to measures of service quality of a network as seen by the customer. There are many different ways to measure the performance of a network, as each network is different in nature and design. (source: wikidata)"@en ;
    rdfs:seeAlso "IoT-A Requirement UNI.252" ;
    ns4:hasDBpediaResource <http://dbpedia.org/resource/Network_performance> ;
    ns5:supports ns4:Communication,
        ns4:QualityOfService .

ns4:OceanProtocolFoundation a owl:NamedIndividual,
        ns8:Organization,
        ns4:StandardOrganization ;
    rdfs:label "Ocean Protocol Foundation"@en ;
    ns2:creator ns4:sebastian ;
    rdfs:comment "Ocean Protocol is supported by a Singapore based non-profit foundation, whose mandate is to ensure open access to the protocol and platform, provide data governance, encourage the network ecosystem growth and take measures to ensure that the platform becomes ever more decentralized with time."@en ;
    ns4:hasOfficialResource <https://oceanprotocol.com/> .

ns4:OcfSecurity a owl:NamedIndividual,
        ns4:OcfBlock ;
    rdfs:label "OCF Security"@en ;
    ns2:creator ns4:sebastian ;
    ns3:associatedWith ns4:RAML ;
    rdfs:seeAlso <https://openconnectivity.org/industries/ocf-security> ;
    ns4:hasPublisher ns4:OpenConnectivityFoundation ;
    ns4:isDescribedin ns4:OcfFramework ;
    ns5:alignsWith <https://w3id.org/i40/rami#Security>,
        ns4:BdvaCyberSecurityTrust,
        ns4:FiwareSecurity,
        ns4:IDSRAMSecurity,
        ns4:IIRASecurity,
        ns4:IIRASecurityFramework,
        ns4:IotaTrustSecurityPrivacy,
        ns4:OpenFogSecurityPerspective ;
    ns5:frames ns4:Certification,
        ns4:Connectivity,
        ns4:SecureCommunication .

ns4:RoleCategorization a owl:NamedIndividual,
        ns4:Concern ;
    rdfs:label "Role Categorization"@en ;
    ns2:creator ns4:sebastian ;
    rdfs:comment "The necessity to categorize participants of a network (users or components) by roles according to the contributions they provide and the demands they have. Examples are identity provider, analytics service, data provider etc. Not to be confused with 'role-based access control', which distinguishes users according to their organizational group, e.g. adimistrators, managers, data analysts etc."@en ;
    ns5:supports ns4:IdentityManagement .

ns4:ServiceAccessControl a owl:NamedIndividual,
        ns4:Concern ;
    rdfs:label "Service Access Control"@en ;
    ns2:creator ns4:sebastian ;
    ns3:associatedWith ns4:DataAccessControl ;
    rdfs:comment "Service access control is the selective restriction of access to a specific (web) service or process. The act of accessing may mean consuming, entering, or using. Permission to access a service is called service authorization. Locks and login credentials are two analogous mechanisms of access control. (source: wikipedia)"@en ;
    rdfs:seeAlso "IoT-A Requirement UNI.611" ;
    ns4:hasDBpediaResource <http://dbpedia.org/resource/Network_Access_Control> ;
    ns5:supports ns4:Authorization .

ns4:VirtualEntity a owl:NamedIndividual,
        ns4:Concern ;
    rdfs:label "Virtual Entity"@en ;
    ns2:creator ns4:sebastian ;
    rdfs:comment "Entities are provided through a virtual form."@en ;
    rdfs:seeAlso "UNI.030"@en,
        "UNI.066"@en,
        "UNI.402"@en ;
    ns6:note "Publications referred: 'IIC:PUB:G1:V1.80:20170131' '6.1 THE CONTROL DOMAIN' 'Page 28' " ;
    ns4:hasDBpediaResource <http://dbpedia.org/resource/Digital_twin> ;
    ns5:supports ns4:ThingRepresentation .

ns4:X_Road_Architecture_Technical_Specification a owl:NamedIndividual,
        ns1:oaSpecificResource ;
    rdfs:label "X-Road Architecture Technical Specification Version: 1.0 18.09.2015 15 pages Doc. ID: ARC-G"@en ;
    ns4:hasOpenResource <https://www.riha.ee/api/v1/systems/70006317-xroad-center/files/257bc950-9149-25be-496b-f54b6a608791> .

ns4:xRoadSection a owl:Class ;
    rdfs:label "x-road Section"@en ;
    ns2:creator ns4:sebastian ;
    rdfs:subClassOf [ a owl:Restriction ;
            owl:hasValue ns4:xTee ;
            owl:onProperty ns4:isDescribedin ],
        ns4:StandardClassification .

ns4:AdministrationShell a owl:NamedIndividual,
        ns4:StandardClassification,
        ns4:StandardizationFramework ;
    rdfs:label "Administration Shell"@en ;
    ns3:associatedWith <https://w3id.org/ids/core/TrustedConnector> ;
    rdfs:comment "Represents the classifications of the standards according to the submodels of the administration shell."@en ;
    ns4:hasPublisher ns4:PlatformIndustry40 ;
    ns5:alignsWith <https://w3id.org/ids/core/TrustedConnector> ;
    ns5:frames <https://w3id.org/i40/rami#Lifecycle_Status>,
        ns4:Availability,
        ns4:BusinessContext,
        ns4:Communication,
        ns4:DataAccess,
        ns4:DynamicAdjustability,
        ns4:EndpointInvocation,
        ns4:Identification,
        ns4:IdentityManagement,
        ns4:IntegrityProtection,
        ns4:Interoperability,
        ns4:SecureCommunication,
        ns4:Security,
        ns4:SemanticInteroperability,
        ns4:ServiceChoreography,
        ns4:ServiceComposition,
        ns4:ServiceOrchestration,
        ns4:SyntacticInteroperability,
        ns4:ThingDescription,
        ns4:ThingRepresentation,
        ns4:Trustworthiness .

ns4:BdvaDataProtection a owl:NamedIndividual,
        ns4:BdvaConcern,
        ns4:StandardClassification ;
    rdfs:label "BDVA Data Protection"@en ;
    ns2:creator ns4:sebastian ;
    ns3:associatedWith ns4:IDSRAMSecurity,
        ns4:IIRASecurityFramework ;
    rdfs:comment "Privacy and anonymisation mechanisms to facilitate data protection. This is shown related to data management and processing as there is a strong link here, but it can also be associated with the area of cybersecurity."@en ;
    ns4:isDescribedin ns4:BdvaSira ;
    ns5:alignsWith ns4:IDSRAMSecurity,
        ns4:IIRASecurityFramework ;
    ns5:frames ns4:DataProtection,
        ns4:DataSovereignty,
        ns4:Privacy,
        ns4:Trustworthiness .

ns4:CardinalityOfDataSources a owl:NamedIndividual,
        ns4:Concern ;
    ns5:supports ns4:Interoperability .

ns4:DataDescription a owl:NamedIndividual,
        ns4:Concern ;
    rdfs:label "Data Description"@en ;
    ns2:creator ns4:sebastian ;
    ns7:hasStakeholder <http://dbpedia.org/ontology/developer> ;
    rdfs:comment <http://dbpedia.org/resource/Data_model>,
        "Methods to unambiguously describe data resources."@en ;
    rdfs:seeAlso "IoT-A Requirement UNI.004",
        "IoT-A Requirement UNI.240" ;
    ns5:supports ns4:SemanticInteroperability .

ns4:DtpEcosystemView a owl:NamedIndividual,
        ns4:StandardClassification,
        ns4:Viewpoint ;
    rdfs:label "DTP Ecosystem"@en ;
    ns3:associatedWith ns4:IDSRAMGovernance,
        ns4:IIRAUsageViewpoint ;
    ns4:isDescribedin ns4:DtpArchitecture ;
    ns5:alignsWith ns4:IDSRAMGovernance,
        ns4:IIRAUsageViewpoint .

ns4:FiwareAdvancedUi a owl:NamedIndividual,
        ns4:FiwareChapter,
        ns4:StandardClassification ;
    rdfs:label "FIWARE Advanced Web-based User Interface"@en ;
    ns2:creator ns4:sebastian ;
    ns3:associatedWith <http://purl.oclc.org/NET/mvco.owl#EndUser>,
        ns4:IIRAApplicationDomain,
        ns4:IIRAUsageViewpoint ;
    rdfs:comment """The Generic Enablers (GEs) from the Advanced Web-based User Interface (WebUI) chapter cover a set of GEs that provide an advanced user experience using HTML-5 and a Web-based UI approach.

The objective of the Advanced Web-based UI GE is to significantly improve the user experience for the Future Internet by adding new user input and interaction capabilities, such as interactive 3D graphics, immersive interaction with the real and virtual world via Augmented Reality, virtualizing the display and driving them over the network, and many more."""@en ;
    ns4:isDescribedin ns4:FIWARE ;
    ns5:alignsWith ns4:IIRAApplicationDomain,
        ns4:IIRAUsageViewpoint ;
    ns5:frames ns4:UserInteraction .

ns4:IIRACrosscuttingFunction a owl:Class,
        owl:NamedIndividual ;
    rdfs:label "IIRA Crosscutting Function"@en ;
    ns2:creator ns4:sebastian ;
    rdfs:comment "Often these enabling functions, the so-called crosscutting functions, need to be made available across many of the system functional components. For Reference Architecture 6: Functional Viewpoint example, system functions need to be connected so they can interact with each other to complete functionality at the system level."@en ;
    rdfs:subClassOf [ a owl:Restriction ;
            owl:hasValue ns4:IIRAFunctionalViewpoint ;
            owl:onProperty ns3:isPartOf ],
        ns4:StandardClassification ;
    ns6:note "Publications referred: 'IIC:PUB:G1:V1.80:20170131' '6.6 CROSSCUTTING FUNCTIONS AND SYSTEM CHARACTERISTICS' 'Page 34' " .

ns4:IIRAFunctionalDomain a owl:Class,
        owl:NamedIndividual ;
    rdfs:label "IIRA Functional Domain"@en ;
    ns2:creator ns4:sebastian ;
    rdfs:subClassOf [ a owl:Restriction ;
            owl:hasValue ns4:IIRAFunctionalViewpoint ;
            owl:onProperty ns3:isPartOf ],
        [ a owl:Restriction ;
            owl:hasValue ns4:IIRA ;
            owl:onProperty ns4:isDescribedin ],
        ns4:StandardClassification .

ns4:Industrial_Internet_Architecture_Version_1 a owl:NamedIndividual,
        ns1:oaSpecificResource ;
    rdfs:label "Industrial Internet Architecture Version 1"@en ;
    ns4:hasOpenResource <http://en.aii-alliance.org/uploadfile/2017/0307/Industrial.pdf> .

ns4:IotaDeploymentOperationViewpoint a owl:NamedIndividual,
        ns4:StandardClassification,
        ns4:Viewpoint ;
    rdfs:label "IoT-A Deployment and Operation"@en ;
    ns2:creator ns4:sebastian ;
    ns3:associatedWith ns4:IDSRAMSystemLayer,
        ns4:IIRAImplementationViewpoint ;
    ns4:isDescribedin ns4:IotaReferenceArchitecture ;
    ns5:alignsWith ns4:IDSRAMSystemLayer,
        ns4:IIRAImplementationViewpoint ;
    ns5:frames <https://w3id.org/i40/rami#EnergyEfficiency>,
        ns4:DynamicAdjustability,
        ns4:Evolvability,
        ns4:ServiceChoreography,
        ns4:ServiceComposition,
        ns4:ServiceDeployment,
        ns4:ServiceLifecycleManagement,
        ns4:ServiceOrchestration .

ns4:IotaEvolutionInteroperability a owl:NamedIndividual,
        ns4:IotaPerspective,
        ns4:StandardClassification ;
    rdfs:label "IoT-A Evolution and Interoperability"@en ;
    ns3:associatedWith ns4:IIRAConnectivity,
        ns4:RAMIIntegrationLayer ;
    ns4:isDescribedin ns4:IotaReferenceArchitecture ;
    ns5:alignsWith ns4:IIRAConnectivity,
        ns4:RAMIIntegrationLayer ;
    ns5:frames ns4:DynamicAdjustability,
        ns4:Evolvability,
        ns4:Interoperability,
        ns4:ServiceChoreography,
        ns4:ServiceComposition,
        ns4:ServiceOrchestration .

ns4:IotaPerspective a owl:Class,
        owl:NamedIndividual ;
    rdfs:label "IoT-A Perspective"@en ;
    ns2:creator ns4:sebastian ;
    rdfs:subClassOf ns4:StandardClassification .

ns4:IviAssetView a owl:NamedIndividual,
        ns4:StandardClassification,
        ns4:Viewpoint ;
    rdfs:label "IVI Asset View"@en ;
    ns2:creator ns4:sebastian ;
    ns3:associatedWith ns4:IIRAPhysicalSystems,
        ns4:RAMIAssetlayer ;
    ns4:isDescribedin ns4:IVRA ;
    ns5:alignsWith ns4:IIRAPhysicalSystems,
        ns4:RAMIAssetlayer ;
    ns5:frames ns4:ThingRepresentation .

ns4:IviBusinessLayer a owl:NamedIndividual,
        ns4:IviLayer,
        ns4:StandardClassification ;
    rdfs:label "IVI Business Layer"@en ;
    ns2:creator ns4:sebastian ;
    ns3:associatedWith ns4:IIRABusinessViewpoint,
        ns4:RAMIBusinessLayer ;
    rdfs:comment "In the business layer, from a perspective of enterprise management, the focus of discussions is placed on the fundamentel structure of manufacturing, organization forms for manufacturing, presence of essential perspectives and axes as well as a philosophy and concept of values underpinning the big picture. (source: IVRA-Next)"@en ;
    ns4:isDescribedin ns4:IVRA ;
    ns5:alignsWith ns4:IIRABusinessViewpoint,
        ns4:RAMIBusinessLayer ;
    ns5:frames ns4:BusinessContext,
        ns4:BusinessTransactions .

ns4:IviManagementView a owl:NamedIndividual,
        ns4:StandardClassification,
        ns4:Viewpoint ;
    rdfs:label "IVI Management View"@en ;
    ns2:creator ns4:sebastian ;
    ns3:associatedWith ns4:IIRAUsageViewpoint,
        ns4:RAMIFunctionalLayer ;
    ns4:isDescribedin ns4:IVRA ;
    ns5:alignsWith ns4:IIRAUsageViewpoint,
        ns4:RAMIFunctionalLayer ;
    ns5:frames ns4:BusinessContext,
        ns4:BusinessTransactions,
        ns4:MaintenanceCost,
        ns4:QualityOfService,
        ns4:ServiceLevelAgreements,
        ns4:ServiceLifecycleManagement .

ns4:Manufacturing a owl:NamedIndividual .

ns4:OcfBlock a owl:Class ;
    rdfs:label "OCF Framework Block" ;
    ns2:creator ns4:sebastian ;
    rdfs:subClassOf ns4:StandardClassification .

ns4:Resilience a owl:NamedIndividual,
        ns4:Concern ;
    rdfs:label "Resilience"@en ;
    ns2:creator ns4:sebastian ;
    ns7:hasStakeholder <http://dbpedia.org/ontology/generalManager>,
        <https://www.wikidata.org/wiki/Q1548249> ;
    rdfs:comment "Resilience is the ability to provide and maintain an acceptable level of service in the face of faults and challenges to normal operation.” Threats and challenges for services can range from simple misconfiguration over large scale natural disasters to targeted attacks. As such, network resilience touches a very wide range of topics. In order to increase the resilience of a given communication network, the probable challenges and risks have to be identified and appropriate resilience metrics have to be defined for the service to be protected. (source: wikipedia)"@en ;
    rdfs:seeAlso <https://ieeexplore.ieee.org/document/7919553>,
        "IoT-A Requirement UNI.012",
        "IoT-A Requirement UNI.040",
        "IoT-A Requirement UNI.058",
        "IoT-A Requirement UNI.064",
        "IoT-A Requirement UNI.718" ;
    ns4:hasDBpediaResource <http://dbpedia.org/resource/Resilience_(network)> ;
    ns5:supports ns4:Trustworthiness .

ns4:ServiceLevelAgreements a owl:NamedIndividual,
        ns4:Concern ;
    rdfs:label "Service level agreement"@en ;
    ns2:creator ns4:sebastian ;
    rdfs:comment "A service-level agreement (SLA) is defined as an official commitment that prevails between a service provider and the customer. Particular aspects of the service – quality, availability, responsibilities – are agreed between the service provider and the service user. The most common component of SLA is that the services should be provided to the customer as agreed upon in the contract. As an example, Internet service providers and telcos will commonly include service level agreements within the terms of their contracts with customers to define the level(s) of service being sold in plain language terms. In this case the SLA will typically have a technical definition in terms of mean time between failures (MTBF), mean time to repair or mean time to recovery (MTTR); identifying which party is responsible for reporting faults or paying fees; responsibility for various data rates; throughput; jitter; or similar measurable details. (source: wikipedia)"@en ;
    rdfs:seeAlso "IoT-A Requirement UNI.060" ;
    ns4:hasDBpediaResource <http://dbpedia.org/resource/Service-level_agreement> ;
    ns5:supports ns4:ServiceLifecycleManagement .

ns4:TansportLayer a owl:NamedIndividual .

ns4:xTee a owl:NamedIndividual,
        ns4:ArchitectureDescription,
        ns4:StandardizationFramework ;
    rdfs:label "x-Tee"@en ;
    ns4:hasPublisher ns4:x-road .

rdfs:Literal a owl:Class ;
    rdfs:label "Literal" .

<https://w3id.org/i40/rami#RAMIITLayer> a owl:Class ;
    rdfs:label "RAMI IT Layer"@en ;
    rdfs:subClassOf ns4:StandardClassification ;
    owl:equivalentClass [ a owl:Class ;
            owl:oneOf ( <https://w3id.org/i40/rami#Asset> <https://w3id.org/i40/rami#Business> <https://w3id.org/i40/rami#Communication> <https://w3id.org/i40/rami#Functional> <https://w3id.org/i40/rami#Information> <https://w3id.org/i40/rami#Integration> ) ] .

ns4:BdvaDataViualisationAndUserInteraction a owl:NamedIndividual .

ns4:BigDataApplications a owl:NamedIndividual,
        ns4:Concern ;
    rdfs:label "Big Data Applications"@en ;
    rdfs:comment "Big data is a term for data sets that are so large or complex that traditional data processing applications are inadequate to deal with them. Challenges include analysis, capture, data curation, search, sharing, storage, transfer, visualization, querying, updating and information privacy. The term \"big data\" often refers simply to the use of predictive analytics, user behavior analytics, or certain other advanced data analytics methods that extract value from data, and seldom to a particular size of data set. (source: wikipedia)"@en ;
    ns4:hasDBpediaResource <http://dbpedia.org/resource/Big_data> ;
    ns5:supports ns4:DataAnalytics .

ns4:DataInMotion a owl:NamedIndividual .

ns4:DataTransferProject a owl:NamedIndividual,
        ns8:Organization,
        ns4:DataSharingInitiative ;
    rdfs:label "Data Transfer Project"@en ;
    ns2:creator ns4:sebastian ;
    ns3:associatedWith ns4:DtpArchitecture ;
    rdfs:comment "The Data Transfer Project (DTP) extends data portability beyond a user’s ability to download a copy of their data from their service provider (“provider”), to providing the user the ability 1 to initiate a direct transfer of their data into and out of any participating provider. The Data Transfer Project is an open source initiative to encourage participation of as many providers as possible. The DTP will enhance the data portability ecosystem by reducing the infrastructure burden on both providers and users, which should in turn increase the number of services offering portability. The protocols and methodology of the DTP enable direct, service-to-service data transfer with streamlined engineering work."@en ;
    ns4:hasOfficialResource <https://github.com/google/data-transfer-project> .

ns4:DtpArchitecture a owl:NamedIndividual,
        ns4:ArchitectureDescription,
        ns4:StandardizationFramework ;
    rdfs:label "Data Transfer Project Architecture"@en ;
    ns2:creator ns4:sebastian ;
    rdfs:comment "The architecture description of the Data Transfer Project has not yet been published in a sufficient manner."@en ;
    ns4:hasPublisher ns4:DataTransferProject .

ns4:DtpDeploymentView a owl:NamedIndividual,
        ns4:StandardClassification,
        ns4:Viewpoint ;
    rdfs:label "DTP Deployment"@en ;
    ns3:associatedWith ns4:IDSRAMProcessLayer,
        ns4:IIRAImplementationViewpoint ;
    ns4:isDescribedin ns4:DtpArchitecture ;
    ns5:alignsWith ns4:IDSRAMProcessLayer,
        ns4:IIRAImplementationViewpoint ;
    ns5:frames ns4:Identification,
        ns4:IdentityManagement,
        ns4:Security,
        ns4:ServiceDeployment,
        ns4:ServiceLifecycleManagement,
        ns4:Trustworthiness,
        ns4:UserInteraction .

ns4:EdgecrossFacilityLayer a owl:NamedIndividual,
        ns4:EdgecrossLayer,
        ns4:StandardClassification ;
    rdfs:label "Edgecross FA"@en ;
    ns3:associatedWith ns4:IIRAPhysicalSystems,
        ns4:RAMIAssetlayer ;
    ns4:isDescribedin ns4:EdgecrossArchitecture ;
    ns5:alignsWith ns4:IIRAPhysicalSystems,
        ns4:RAMIAssetlayer .

ns4:IDSRAMLayer a owl:Class ;
    rdfs:label "IDS RAM Layer"@en ;
    ns2:creator ns4:sebastian ;
    rdfs:subClassOf ns4:StandardClassification ;
    owl:equivalentClass [ a owl:Class ;
            owl:oneOf ( ns4:IDSRAMBusinessLayer ns4:IDSRAMFunctionalLayer ns4:IDSRAMInformationLayer ns4:IDSRAMProcessLayer ns4:IDSRAMSystemLayer ) ] .

ns4:IIRASystemCharacteristics a owl:Class,
        owl:NamedIndividual ;
    rdfs:label "IIRA System Characteristic"@en ;
    ns2:creator ns4:sebastian ;
    rdfs:subClassOf [ a owl:Restriction ;
            owl:hasValue ns4:IIRAFunctionalViewpoint ;
            owl:onProperty ns3:isPartOf ],
        [ a owl:Restriction ;
            owl:hasValue ns4:IIRA ;
            owl:onProperty ns4:isDescribedin ],
        ns4:StandardClassification .

ns4:IVRA a owl:NamedIndividual,
        ns4:ArchitectureDescription,
        ns4:StandardizationFramework ;
    rdfs:label "Industrial Value Chain Reference Architecture"@en ;
    ns3:associatedWith ns4:Ivi ;
    rdfs:comment "The Reference Architecture (IVRA) of the Industrial Value Chain Initive (IVI) proposes a system architecture for the manufactoring domain targeting interoperability and communicational aspects."@en ;
    ns6:altLabel "IVRA"@en ;
    ns4:hasOfficialResource <https://iv-i.org/wp-test/wp-content/uploads/2017/09/doc_161208_Industrial_Value_Chain_Reference_Architecture.pdf> .

ns4:IicfConnectivityLayer a owl:Class,
        owl:NamedIndividual ;
    rdfs:label "Connectivity Layer"@en,
        "IICF Connectivity Layer"@en ;
    ns2:creator ns4:sebastian ;
    rdfs:comment "Connectivity Layer of the Internet Connectivity Framework"@en ;
    rdfs:isDefinedBy <https://www.iiconsortium.org/pdf/IIC_PUB_G5_V1.01_PB_20180228.pdf> ;
    rdfs:subClassOf [ a owl:Restriction ;
            owl:hasValue ns4:IIRAConnectivity ;
            owl:onProperty ns3:isPartOf ],
        ns4:StandardClassification .

ns4:Industrial_Value_Chain_Reference_Architecture_IVRA a owl:NamedIndividual,
        ns1:oaSpecificResource ;
    rdfs:label "Industrial Value Chain Reference Architecture (IVRA)"@en ;
    rdfs:comment "Industrial Value Chain Reference Architecture (IVRA) Industrial Value Chain Initiative " ;
    ns4:hasOpenResource <https://iv-i.org/docs/doc_161208_Industrial_Value_Chain_Reference_Architecture.pdf> .

ns4:Industrial_Value_Chain_Reference_Architecture_IVRA_Next a owl:NamedIndividual,
        ns1:oaSpecificResource ;
    rdfs:label "Industrial Value Chain Reference Architecture (IVRA)- Next"@en ;
    ns6:note "Industrial Value Chain Reference Architecture (IVRA) Industrial Value Chain Initiative Next" ;
    ns4:hasOpenResource <https://www.innovation4.cn/library/r26680> .

ns4:NgsiLdDataRepresentation a owl:NamedIndividual,
        ns4:NGSI_Context_Information_Management_API,
        ns4:StandardClassification ;
    rdfs:label "NGSI-LD Data Representation"@en ;
    ns3:associatedWith ns4:FiwareDataContextManagement,
        ns4:IDSRAMInformationLayer,
        ns4:RAMIFunctionalLayer,
        ns4:RDF ;
    ns4:isDescribedin ns4:FIWARE ;
    ns5:alignsWith ns4:FiwareDataContextManagement,
        ns4:IDSRAMInformationLayer,
        ns4:RAMIFunctionalLayer ;
    ns5:frames ns4:DataDescription,
        ns4:Interoperability,
        ns4:SemanticInteroperability .

ns4:OcfFramework a owl:NamedIndividual,
        ns4:StandardizationFramework ;
    rdfs:label "OCF Framework"@en ;
    ns2:creator ns4:sebastian ;
    ns4:hasPublisher ns4:OpenConnectivityFoundation .

ns4:ServiceDiscovery a owl:NamedIndividual,
        ns4:Concern ;
    rdfs:label "Service Discovery"@en ;
    ns2:creator ns4:sebastian ;
    rdfs:comment "How to find desired (Web) services, Data Apps, functionalities."@en ;
    rdfs:seeAlso "IoT-A Requirement UNI.406",
        "IoT-A Requirement UNI.408",
        "IoT-A Requirement UNI.414",
        "IoT-A Requirement UNI.415",
        "IoT-A Requirement UNI.416",
        "IoT-A Requirement UNI.422",
        "IoT-A Requirement UNI.427" ;
    ns6:note "Publications referred: '<https://doi.org/10.1016/j.jksuci.2016.10.003>' '2.8.2. Societal data service' 'Page 309'" ;
    ns4:hasDBpediaResource <http://dbpedia.org/resource/Service_discovery> .

ns4:isDescribedin a owl:ObjectProperty ;
    rdfs:label "is Described in"@en ;
    rdfs:comment "Links the Standarization Frameworks with the Classification of Standards"@en ;
    rdfs:domain ns4:StandardClassification ;
    rdfs:range ns4:StandardizationFramework .

ns4:relatedTo a owl:ObjectProperty,
        owl:SymmetricProperty,
        owl:TransitiveProperty ;
    rdfs:label "related To"@en ;
    ns2:creator ns4:irlan ;
    rdfs:comment "Represent any type of relation that connects two standards."@en ;
    rdfs:domain ns4:Standard ;
    rdfs:range ns4:Standard ;
    ns6:altLabel "has Associated Standard"@en .

ns3:associatedWith a owl:ObjectProperty .

ns4:BdvaDataManagement a owl:NamedIndividual,
        ns4:BdvaConcern,
        ns4:StandardClassification ;
    rdfs:label "BDVA Data Management"@en ;
    ns2:creator ns4:sebastian ;
    ns3:associatedWith ns4:IDSRAMInformationLayer,
        ns4:IDSRAMProcessLayer,
        ns4:RAMIInformationLayer ;
    rdfs:comment "Principles and techniques for data management"@en ;
    ns4:isDescribedin ns4:BdvaSira ;
    ns5:alignsWith ns4:IDSRAMInformationLayer,
        ns4:IDSRAMProcessLayer,
        ns4:RAMIInformationLayer ;
    ns5:frames ns4:BigDataApplications,
        ns4:DataQuality,
        ns4:Interoperability,
        ns4:ProvenanceTracking,
        ns4:Security,
        ns4:SemanticInteroperability,
        ns4:SyntacticInteroperability,
        ns4:Trustworthiness .

ns4:BdvaDataProcessingArchitectures a owl:NamedIndividual,
        ns4:BdvaConcern,
        ns4:StandardClassification ;
    rdfs:label "BDVA Data Processing Architectures"@en ;
    ns2:creator ns4:sebastian ;
    ns3:associatedWith ns4:IDSRAMProcessLayer,
        ns4:IIRAConnectivity,
        ns4:InformationDomain ;
    rdfs:comment "Optimised and scalable architectures for analytics of both data-at-rest and data-in-motion, with low latency delivering real-time analytics."@en ;
    ns4:isDescribedin ns4:BdvaSira ;
    ns5:alignsWith ns4:IDSRAMProcessLayer,
        ns4:IIRAConnectivity,
        ns4:InformationDomain ;
    ns5:frames ns4:BigDataApplications,
        ns4:Communication,
        ns4:DataAtRest,
        ns4:DataInMotion,
        ns4:DataProcessing,
        ns4:Scalability,
        ns4:StreamProcessing .

ns4:DataDiscovery a owl:NamedIndividual,
        ns4:Concern ;
    rdfs:label "Data Discovery"@en ;
    ns2:creator ns4:sebastian ;
    rdfs:comment "How to find desired resources, Data Assets, Data Artifacts in a defined environment."@en ;
    rdfs:seeAlso "IoT-A Requirement UNI.236",
        "IoT-A Requirement UNI.408",
        "IoT-A Requirement UNI.422" ;
    ns5:supports ns4:Interoperability .

ns4:DtpSecurityPrivacy a owl:NamedIndividual,
        ns4:StandardClassification,
        ns4:Viewpoint ;
    rdfs:label "DTP Security & Privacy"@en ;
    ns3:associatedWith <https://w3id.org/i40/rami#Security>,
        ns4:IDSRAMGovernance,
        ns4:IIRAPrivacy,
        ns4:IIRASecurity ;
    ns4:isDescribedin ns4:DtpArchitecture ;
    ns5:alignsWith <https://w3id.org/i40/rami#Security>,
        ns4:IDSRAMGovernance,
        ns4:IIRAPrivacy,
        ns4:Security .

ns4:DynamicAdjustability a owl:NamedIndividual,
        ns4:Concern ;
    rdfs:label "Dynamic Adjustability"@en ;
    rdfs:comment "A systems ability to adjust its behaviour on dynamic changes in its environment."@en ;
    rdfs:seeAlso "IoT-A Requirement UNI.713" ;
    ns5:supports ns4:ServiceChoreography,
        ns4:ServiceComposition,
        ns4:ServiceOrchestration .

ns4:FiwareApplicationsServicesAndDataDelivery a owl:NamedIndividual,
        ns4:FiwareChapter,
        ns4:StandardClassification ;
    rdfs:label "FIWARE Applications Services and Data Delivery"@en ;
    ns2:creator ns4:sebastian ;
    ns3:associatedWith ns4:IDSRAMProcessLayer,
        ns4:IIRAConnectivity,
        ns4:NgsiLdArchitecture ;
    rdfs:comment """The Generic Enablers (GE) for the Apps Chapter together build an ecosystem of applications, services and data that is sustainable and fosters innovation as well as cross-fertilization. In particular the Apps Generic Enablers supports managing applications, services and data in a business framework across the whole service life cycle from creation through composition of applications and data to monetization and revenue sharing.

A couple of basic GEs are important to realize the vision of such an applications, services and data business framework, which enables new business models in an agile and flexible way. Among them: a store, a marketplace, a revenue sharing engine, an application composer through mashup and a data visualization and analysis component.

The Business Framework is heavily relying on USDL as common uniform description format for services which does not only focus on technical aspects of service, but also on business aspects as well as functional and non-functional service attributes.

The Application Mashup GE aims at allowing end users without programming skills to quickly compose beautiful web applications and dashboards/cockpits mashing up widgets, operators and data sources from a shared catalogue.

The Data Visualisation GE aims at creating agile, beautiful visualizations and meaningful reports useful to present the large variety of datasets. Data stakeholders will bring in the play as well as providing customisable data analytics."""@en ;
    ns4:isDescribedin ns4:FIWARE ;
    ns5:alignsWith ns4:IDSRAMProcessLayer,
        ns4:IIRAConnectivity,
        ns4:NgsiLdArchitecture ;
    ns5:frames ns4:DataAnalytics,
        ns4:DataSelection,
        ns4:ServiceComposition,
        ns4:ServiceSelection .

ns4:IICFFrameworkLayer a owl:NamedIndividual,
        ns4:IicfConnectivityLayer,
        ns4:StandardClassification ;
    rdfs:label "IICF Framework Layer"@en ;
    ns3:associatedWith ns4:DDS,
        ns4:IDSRAMGovernance,
        ns4:IDSRAMSystemLayer,
        ns4:IEC_62541,
        ns4:oneM2M,
        <https://www.wikidata.org/wiki/Q1548249> ;
    ns3:isPartOf ns4:IIRAConnectivity ;
    rdfs:comment "IICF Framework Layer"@en,
        "IICF Framework Layer an instance of the IICF Connectivity Layer"@en ;
    rdfs:isDefinedBy <https://www.iiconsortium.org/pdf/IIC_PUB_G5_V1.01_PB_20180228.pdf> ;
    ns5:alignsWith ns4:IDSRAMGovernance,
        ns4:IDSRAMSystemLayer ;
    ns5:frames ns4:Authentication,
        ns4:Communication,
        ns4:DataAccess,
        ns4:DataDiscovery,
        ns4:Governance,
        ns4:Identification,
        ns4:IdentityManagement,
        ns4:IntegrityProtection,
        ns4:Interoperability,
        ns4:QualityOfService,
        ns4:SecureCommunication,
        ns4:Security,
        ns4:SemanticInteroperability,
        ns4:ServiceDescription,
        ns4:ServiceDiscovery,
        ns4:SyntacticInteroperability,
        ns4:Trustworthiness .

ns4:IIRABusinessViewpoint a owl:NamedIndividual,
        ns4:StandardClassification,
        ns4:Viewpoint ;
    rdfs:label "IIRA Business Viewpoint"@en ;
    ns2:creator ns4:sebastian ;
    ns3:associatedWith ns4:IviBusinessLayer,
        ns4:OceanBusinessViewpoint,
        ns4:OceanMarketplaceViewpoint ;
    rdfs:comment "The business viewpoint frames economic aspects and business relations regarded by the IIC Reference Architecture."@en ;
    ns6:note "Publications referred: '(IIC:PUB:G1:V1.80:20170131' '3.5.1 BUSINESS VIEWPOINT' 'Page 15' " ;
    ns4:isDescribedin ns4:IIRA ;
    ns5:alignsWith ns4:IviBusinessLayer,
        ns4:OceanBusinessViewpoint,
        ns4:OceanMarketplaceViewpoint ;
    ns5:frames ns4:BusinessContext,
        ns4:BusinessValue,
        ns4:MaintenanceCost,
        ns4:ProductLiability,
        ns4:Resilience,
        ns4:ReturnOnInvestment,
        ns4:Safety,
        ns4:Security,
        ns4:Trustworthiness .

ns4:InterfaceNetworksDevices a owl:NamedIndividual,
        ns4:FiwareChapter,
        ns4:StandardClassification ;
    rdfs:label "FIWARE Interface to Networks and Devices"@en ;
    ns2:creator ns4:sebastian ;
    ns3:associatedWith ns4:IDSRAMProcessLayer,
        ns4:IDSRAMSystemLayer,
        ns4:NgsiLdArchitecture,
        ns4:OpenDaylight ;
    rdfs:comment """The GEs in the I2ND chapter provide three sets of functionalities.

The first is an advanced integration middleware to be used by all FIWARE GEs with high performance communication needs

Open networking elements enable cloud network application developers to build value-added services in private, enterprise and public settings.

The third set of functionalities enables the management of robots by means of platform components and interfaces towards other FIWARE GEs, allowing users to develop smarter and faster robotic applications."""@en ;
    ns4:isDescribedin ns4:FIWARE ;
    ns5:alignsWith ns4:IDSRAMProcessLayer,
        ns4:IDSRAMSystemLayer,
        ns4:NgsiLdArchitecture ;
    ns5:frames ns4:CloudComputing,
        ns4:DataDescription,
        ns4:DataProcessing,
        ns4:DataSovereignty,
        ns4:EndpointDescription,
        ns4:EndpointInvocation,
        ns4:Interoperability,
        ns4:IoT,
        ns4:Privacy,
        ns4:QualityOfService,
        ns4:Scalability,
        ns4:Security,
        ns4:SemanticInteroperability,
        ns4:ServiceComposition,
        ns4:ServiceDescription,
        ns4:ServiceOrchestration,
        ns4:SyntacticInteroperability,
        ns4:Trustworthiness .

ns4:StreamProcessing a owl:NamedIndividual,
        ns4:Concern ;
    rdfs:label "Stream processing"@en ;
    ns2:creator ns4:sebastian ;
    rdfs:comment "Stream processing is a computer programming paradigm, equivalent to dataflow programming, event stream processing, and reactive programming, that allows some applications to more easily exploit a limited form of parallel processing. (source: wikipedia)"@en ;
    ns4:hasDBpediaResource <http://dbpedia.org/resource/Stream_processing> ;
    ns5:supports ns4:DataProcessing .

ns4:BdvaCyberSecurityTrust a owl:NamedIndividual,
        ns4:BdvaConcern,
        ns4:StandardClassification ;
    rdfs:label "BDVA Cybersecurity and Trust"@en ;
    ns2:creator ns4:sebastian ;
    ns3:associatedWith <https://w3id.org/i40/rami#Security>,
        ns4:IDSRAMSecurity,
        ns4:IIRASecurityFramework ;
    rdfs:comment """Big Data often need support to maintain security and trust beyond privacy and anonymisation. The aspect of trust frequently has links to trust 
mechanisms such as blockchain technologies, smart contracts and various forms of encryption."""@en ;
    ns4:isDescribedin ns4:BdvaSira ;
    ns5:alignsWith <https://w3id.org/i40/rami#Security>,
        ns4:IDSRAMSecurity,
        ns4:IIRASecurityFramework ;
    ns5:frames ns4:Communication,
        ns4:DataSovereignty,
        ns4:IntegrityProtection,
        ns4:Privacy,
        ns4:SecureCommunication,
        ns4:Security,
        ns4:Trustworthiness .

ns4:EdgeComputing a owl:NamedIndividual,
        ns4:Concern ;
    rdfs:label "Edge computing"@en ;
    rdfs:comment "Edge Computing is pushing the frontier of computing applications, data, and services away from centralized nodes to the logical extremes of a network. It enables analytics and knowledge generation to occur at the source of the data. This approach requires leveraging resources that may not be continuously connected to a network such as laptops, smartphones, tablets and sensors. Edge Computing covers a wide range of technologies including wireless sensor networks, mobile data acquisition, mobile signature analysis, cooperative distributed peer-to-peer ad hoc networking and processing also classifiable as Local Cloud/Fog computing and Grid/Mesh Computing, dew computing, mobile edge computing, cloudlet, distributed data storage and retrieval, autonomic self-healing networks, remote cloud services, augmented reality, and more. (source: wikipedia)"@en ;
    ns4:hasDBpediaResource <http://dbpedia.org/resource/Edge_computing> ;
    ns5:supports ns4:CloudComputing,
        ns4:DataProcessing .

ns4:EdgecrossItSystemsLayer a owl:NamedIndividual,
        ns4:EdgecrossLayer,
        ns4:StandardClassification ;
    rdfs:label "Edgecross IT Systems Layer"@en ;
    ns3:associatedWith ns4:IDSRAMSystemLayer,
        ns4:IIRAApplicationDomain,
        ns4:RAMIIntegrationLayer ;
    ns4:isDescribedin ns4:EdgecrossArchitecture ;
    ns5:alignsWith ns4:IDSRAMSystemLayer,
        ns4:IIRAApplicationDomain,
        ns4:RAMIIntegrationLayer ;
    ns5:frames ns4:Communication,
        ns4:DataAnalytics,
        ns4:DataInMotion .

ns4:Edgecross_Consortium_to_Address_Edge_Integration_in_IIoT_enabled_Architectures a owl:NamedIndividual,
        ns1:oaSpecificResource ;
    rdfs:label "Edgecross Consortium to Address Edge Integration in IIoT-enabled Architectures"@en ;
    ns4:hasOpenResource <https://www.edgecross.org/ja/data-download/pdf/Edgecross_Consortium_WP(E).pdf> .

ns4:Evolvability a owl:NamedIndividual,
        ns4:Concern ;
    rdfs:label "Evolvability"@en ;
    ns2:creator ns4:sebastian ;
    rdfs:comment "A system shall accomodate fast developmental changes in applications and network."@en ;
    rdfs:seeAlso "IoT-A Requirement UNI.701",
        "IoT-A Requirement UNI.702" ;
    ns4:hasDBpediaResource <http://dbpedia.org/resource/Evolving_intelligent_system>,
        <http://dbpedia.org/resource/Software_evolution> ;
    ns5:supports ns4:DynamicAdjustability .

ns4:FiwareChapter a owl:Class,
        owl:NamedIndividual ;
    rdfs:label "Fiware Chapter"@en ;
    ns2:creator ns4:sebastian,
        "sebastian"@en ;
    rdfs:comment "Following is a description of the Reference Architecture linked to the different chapters of FIWARE. A description of FIWARE Generic Enablers (GEs) being supported in each chapter is provided, including the high-level description of the APIs that each FIWARE Generic Enabler (GE) exposes to application developers or it uses to connect to another FIWARE GEs."@en ;
    rdfs:subClassOf ns4:StandardClassification .

ns4:FiwareDataContextManagement a owl:NamedIndividual,
        ns4:FiwareChapter,
        ns4:StandardClassification ;
    rdfs:label "FIWARE Data/Context Management"@en ;
    ns2:creator ns4:sebastian ;
    ns3:associatedWith ns4:NgsiLdApiOperation,
        ns4:NgsiLdDataRepresentation,
        ns4:NgsiLdInformationModel ;
    rdfs:comment """The Data/Context Management FIWARE chapter aims at providing outperforming and platform-like GEs that will ease development and provision of innovative Applications that require gathering, publication, processing and exploitation of information and data streams in real-time and at massive scale. Combined with GEs coming from the Apps Chapters, Application Providers will be able to build innovative business models based on exploitation of massive data provided by end users.

FIWARE Data/Context Management GEs allow to gather information from context and other sources (Context Broker), mediate metadata among GEs and applications (Metadata pre-processor) query stored information through an homogeneous layer (Query Broker), , annotate existing information (Semantic Annotation), store and manage semantic information (Semantic Application Support), generate new knowledge from big data stores using a Map & Reduce paradigm (Big Data analysis) and react to different types of scenarios (Complex Event Processing). It also provides GEs for media management, as easy creation of advanced video applications (Stream Oriented GE) and specifically, video analysis in the compressed domain (CDVA)."""@en ;
    ns4:isDescribedin ns4:FIWARE ;
    ns5:alignsWith ns4:NgsiLdApiOperation,
        ns4:NgsiLdDataRepresentation,
        ns4:NgsiLdInformationModel ;
    ns5:frames ns4:BigDataApplications,
        ns4:DataDiscovery,
        ns4:DataProcessing,
        ns4:Interoperability,
        ns4:StreamProcessing .

ns4:IIRABusinessDomain a owl:NamedIndividual,
        ns4:IIRAFunctionalDomain,
        ns4:StandardClassification ;
    rdfs:label "IIRA Business Domain"@en ;
    ns2:creator ns4:sebastian ;
    ns3:associatedWith ns4:IDSRAMBusinessLayer,
        ns4:OceanSystemViewpoint,
        ns4:RAMIBusinessLayer ;
    ns3:isPartOf ns4:IIRAFunctionalViewpoint ;
    ns6:note "Publications referred: 'IIC:PUB:G1:V1.80:20170131' '6.5 THE BUSINESS DOMAIN' 'Page 34' " ;
    ns4:isDescribedin ns4:IIRA ;
    ns5:alignsWith ns4:IDSRAMBusinessLayer,
        ns4:OceanSystemViewpoint,
        ns4:RAMIBusinessLayer ;
    ns5:frames <https://w3id.org/i40/rami#ProcessPlanning> .

ns4:IotaTrustSecurityPrivacy a owl:NamedIndividual,
        ns4:IotaPerspective,
        ns4:StandardClassification ;
    rdfs:label "IoT-A Trust Security and Privacy"@en ;
    ns3:associatedWith ns4:IDSRAMSecurity,
        ns4:IIRASecurity ;
    ns4:isDescribedin ns4:IotaReferenceArchitecture ;
    ns5:alignsWith ns4:IDSRAMSecurity,
        ns4:Security ;
    ns5:frames ns4:DataSovereignty,
        ns4:Privacy,
        ns4:Security,
        ns4:Trustworthiness .

ns4:NgsiLdInformationModel a owl:NamedIndividual,
        ns4:NGSI_Context_Information_Management_API,
        ns4:StandardClassification ;
    rdfs:label "NGSI-LD Information Model"@en ;
    ns2:creator ns4:sebastian ;
    ns3:associatedWith ns4:FiwareDataContextManagement,
        ns4:IDSRAMInformationLayer,
        ns4:InformationDomain,
        ns4:RAMIInformationLayer ;
    rdfs:comment "The FIWARE data models have been harmonized to enable data portability for different applications including, but not limited, to Smart Cities. They are intended to be used together with FIWARE NGSI version 2. If you want to contribute and create additional data models, please have a look at our repository of data models and the data model development guidelines. (source: https://www.fiware.org/developers/data-models/)"@en ;
    ns4:isDescribedin ns4:FIWARE ;
    ns5:alignsWith ns4:FiwareDataContextManagement,
        ns4:IDSRAMInformationLayer,
        ns4:InformationDomain,
        ns4:RAMIInformationLayer ;
    ns5:frames ns4:DataAnalytics,
        ns4:DataDescription,
        ns4:GeospatialData,
        ns4:Interoperability,
        ns4:SemanticInteroperability .

ns4:ThingRepresentation a owl:NamedIndividual,
        ns4:Concern ;
    rdfs:label "Thing representation"@en ;
    ns2:creator ns4:sebastian ;
    rdfs:comment "Physical objects need to be represented."@en ;
    rdfs:seeAlso "IoT-A Requirement UNI.239" ;
    ns5:supports ns4:IoT .

ns4:xRoadDeploymentView a owl:NamedIndividual,
        ns4:StandardClassification,
        ns4:xRoadSection ;
    rdfs:label "x-road Deplyoment View"@en ;
    ns3:associatedWith ns4:IDSRAMSystemLayer,
        ns4:IIRAImplementationViewpoint,
        ns4:RAMIIntegrationLayer ;
    ns4:isDescribedin ns4:xTee ;
    ns5:alignsWith ns4:IDSRAMSystemLayer,
        ns4:IIRAImplementationViewpoint,
        ns4:RAMIIntegrationLayer ;
    ns5:frames ns4:Communication,
        ns4:DataAccess,
        ns4:Security,
        ns4:ServiceDeployment,
        ns4:ServiceLifecycleManagement,
        ns4:Trustworthiness .

ns4:xRoadProtocolsInterfaces a owl:NamedIndividual,
        ns4:StandardClassification,
        ns4:xRoadSection ;
    rdfs:label "x-road Protocols and Interfaces"@en ;
    ns3:associatedWith ns4:IDSRAMProcessLayer,
        ns4:IIRAControlDomain,
        ns4:RAMIIntegrationLayer ;
    ns4:isDescribedin ns4:xTee ;
    ns5:alignsWith ns4:IDSRAMProcessLayer,
        ns4:IIRAControlDomain,
        ns4:RAMIIntegrationLayer ;
    ns5:frames ns4:Communication,
        ns4:Interoperability,
        ns4:SyntacticInteroperability .

<http://purl.oclc.org/NET/mvco.owl#EndUser> a ns7:StakeholderGroup,
        owl:NamedIndividual .

ns4:Availability a owl:NamedIndividual,
        ns4:Concern ;
    rdfs:label "Availability"@en ;
    ns2:creator ns4:sebastian ;
    rdfs:comment "In reliability theory and reliability engineering, the term availability has the following meanings: * The degree to which a system, subsystem or equipment is in a specified operable and committable state at the start of a mission, when the mission is called for at an unknown, i.e. a random, time. Simply put, availability is the proportion of time a system is in a functioning condition. This is often described as a mission capable rate. Mathematically, this is expressed as 100% minus unavailability. * The ratio of (a) the total time a functional unit is capable of being used during a given interval to (b) the length of the interval. For example, a unit that is capable of being used 100 hours per week (168 hours) would have an availability of 100/168. However, typical availability values are specified in decimal (such as 0.9998). In high availability applications, a metric known as nines, corresponding to the number of nines following the decimal point, is used. With this convention, \"five nines\" equals 0.99999 (or 99.999%) availability. (source: wikipedia)"@en ;
    rdfs:seeAlso <https://dl.acm.org/citation.cfm?doid=3108421.3108426>,
        <https://ieeexplore.ieee.org/document/7919553>,
        <https://ieeexplore.ieee.org/document/8327600>,
        <https://ieeexplore.ieee.org/document/8463303>,
        <https://ieeexplore.ieee.org/document/8474855>,
        ns4:OpenFogArchitecture,
        "IoT-A Requirement UNI.058",
        "IoT-A Requirement UNI.064",
        "IoT-A Requirement UNI.239",
        "IoT-A Requirement UNI.321",
        "IoT-A Requirement UNI.601",
        "IoT-A Requirement UNI.610",
        "IoT-A Requirement UNI.616" ;
    ns6:note "Publications referred: '<https://www.openfogconsortium.org/wp-content/uploads/OpenFog_Reference_Architecture_2_09_17-FINAL.pdf> OPFRA001.020817' '4.6 Reliability, Availability, and Serviceability (RAS)Pillar' 'Page 29' " ;
    ns4:hasDBpediaResource <http://dbpedia.org/resource/Availability> ;
    ns5:supports ns4:Reliability .

ns4:BdvaDataAnalytics a owl:NamedIndividual,
        ns4:BdvaConcern,
        ns4:StandardClassification ;
    rdfs:label "BDVA Data Analytics"@en ;
    ns2:creator ns4:sebastian ;
    ns3:associatedWith ns4:IDSRAMProcessLayer,
        ns4:InformationDomain,
        ns4:RAMIFunctionalLayer,
        ns4:RAMIInformationLayer ;
    rdfs:comment "Data analytics to improve data understanding, deep learning and the meaningfulness of data."@en ;
    ns4:isDescribedin ns4:BdvaSira ;
    ns5:alignsWith ns4:IDSRAMProcessLayer,
        ns4:InformationDomain,
        ns4:RAMIFunctionalLayer,
        ns4:RAMIInformationLayer ;
    ns5:frames ns4:AI,
        ns4:DataAnalytics,
        ns4:DataProcessing,
        ns4:MachineLearning,
        ns4:StreamProcessing,
        ns4:Trustworthiness .

ns4:DataAccessControl a owl:NamedIndividual,
        ns4:Concern ;
    rdfs:label "Data Access Control"@en ;
    ns2:creator ns4:sebastian ;
    ns7:hasStakeholder <http://purl.oclc.org/NET/mvco.owl#EndUser>,
        <https://w3id.org/i40/DataOwner> ;
    rdfs:comment "Automated access control based on formalized descriptions."@en,
        "In the fields of physical security and information security, access control (AC) is the selective restriction of access to a place or other resource. The act of accessing may mean consuming, entering, or using. Permission to access a resource is called authorization. Locks and login credentials are two analogous mechanisms of access control. (source: wikipedia)"@en ;
    rdfs:seeAlso "IoT-A Requirement UNI.002",
        "IoT-A Requirement UNI.067",
        "IoT-A Requirement UNI.410",
        "IoT-A Requirement UNI.411",
        "IoT-A Requirement UNI.412",
        "IoT-A Requirement UNI.413",
        "IoT-A Requirement UNI.504" ;
    ns4:hasDBpediaResource <http://dbpedia.org/resource/Access_control> ;
    ns5:supports ns4:Authorization .

ns4:FiwareIotServicesEnablement a owl:NamedIndividual,
        ns4:FiwareChapter,
        ns4:StandardClassification ;
    rdfs:label "FIWARE IoT Services Enablement"@en ;
    ns2:creator ns4:sebastian ;
    ns3:associatedWith ns4:IDSRAMSystemLayer,
        ns4:IIRAControlDomain,
        ns4:RAMICommunicationlayer,
        ns4:RAMIIntegrationLayer ;
    rdfs:comment """The deployment of the architecture of the IoT Service Enablement chapter is typically distributed across a large number of Devices, several Gateways and the Backend.

A device is a hardware entity, component or system that either measures properties of a thing/group of things or influences the properties of a thing/group of things or both measures/influences. Sensors and actuators are devices.

IoT Resources are computational elements (software) that provide the technical means to perform sensing and/or actuation on the device. The resource is usually hosted on the device.

IoT GEs have been spread in two different domains: Gateway and Backend. While IoT Gateway GEs provide inter-networking and protocol conversion functionalities between devices and the IoT Backend GEs, the IoT Backend GEs provide management functionalities for the devices and IoT domain-specific support for the applications."""@en ;
    ns4:isDescribedin ns4:FIWARE ;
    ns5:alignsWith ns4:IDSRAMSystemLayer,
        ns4:IIRAControlDomain,
        ns4:RAMICommunicationlayer,
        ns4:RAMIIntegrationLayer ;
    ns5:frames ns4:CloudComputing,
        ns4:DataDiscovery,
        ns4:DataProcessing,
        ns4:EdgeComputing,
        ns4:EndpointInvocation,
        ns4:Interoperability,
        ns4:IoT,
        ns4:SyntacticInteroperability .

ns4:IIRAPhysicalSystems a owl:NamedIndividual,
        ns4:StandardClassification ;
    rdfs:label "IIRA Physical Systems"@en ;
    ns2:creator ns4:sebastian ;
    ns3:associatedWith ns4:EdgecrossFacilityLayer,
        ns4:IDSRAMSystemLayer,
        ns4:IviAssetView,
        ns4:RAMIAssetlayer ;
    ns3:isPartOf ns4:IIRAFunctionalViewpoint ;
    rdfs:comment "Computational capabilities ranging from very limited (e.g. in a smart sensor) to reasonably rich (e.g. a cluster of servers) are placed in, attached to or collocated with physical systems (e.g. in smart sensors, devices or machines). These capabilities are connected through a variety of connectivity technologies including wireless."@en ;
    ns4:hasOfficialResource <https://www.iiconsortium.org/IIRA.htm> ;
    ns4:isDescribedin ns4:IIRA ;
    ns5:alignsWith ns4:EdgecrossFacilityLayer,
        ns4:IDSRAMSystemLayer,
        ns4:IviAssetView,
        ns4:RAMIAssetlayer .

ns4:IIRAUsageViewpoint a owl:NamedIndividual,
        ns4:StandardClassification,
        ns4:Viewpoint ;
    rdfs:label "IIRA Usage Viewpoint"@en ;
    ns3:associatedWith ns4:BdvaDataViualisationAndUserInteraction,
        ns4:DtpEcosystemView,
        ns4:FiwareAdvancedUi,
        ns4:IviManagementView ;
    ns6:note "Publications referred: '(IIC:PUB:G1:V1.80:20170131' '3.5.2 USAGE VIEWPOINT' 'Page 16' " ;
    ns4:isDescribedin ns4:IIRA ;
    ns5:alignsWith ns4:BdvaDataViualisationAndUserInteraction,
        ns4:DtpEcosystemView,
        ns4:FiwareAdvancedUi,
        ns4:IviManagementView ;
    ns5:frames <https://w3id.org/i40/rami#ProcessPlanning>,
        ns4:DynamicAdjustability,
        ns4:Evolvability,
        ns4:RoleCategorization,
        ns4:ServiceChoreography,
        ns4:ServiceComposition,
        ns4:ServiceDeployment,
        ns4:ServiceLifecycleManagement,
        ns4:ServiceOrchestration .

ns4:IotaReferenceArchitecture a owl:NamedIndividual,
        ns4:ArchitectureDescription,
        ns4:StandardizationFramework ;
    rdfs:label "IoT-A Reference Architecture"@en ;
    ns2:creator ns4:sebastian ;
    ns4:hasPublisher ns4:IoTA .

ns4:RAMIBusinessLayer a owl:NamedIndividual,
        <https://w3id.org/i40/rami#RAMIITLayer>,
        ns4:StandardClassification ;
    rdfs:label "RAMI Business Layer"@en ;
    ns3:associatedWith ns4:IDSRAMBusinessLayer,
        ns4:IDSRAMGovernance,
        ns4:IIRABusinessDomain,
        ns4:IviBusinessLayer ;
    ns4:isDescribedin ns4:RAMI ;
    ns5:alignsWith ns4:IDSRAMBusinessLayer,
        ns4:IDSRAMGovernance,
        ns4:IIRABusinessDomain,
        ns4:IviBusinessLayer ;
    ns5:frames <https://w3id.org/i40/rami#ProcessPlanning>,
        ns4:BusinessContext,
        ns4:ServiceComposition,
        ns4:ServiceOrchestration .

ns4:Scalability a owl:NamedIndividual,
        ns4:Concern ;
    rdfs:label "Scalability"@en ;
    ns2:creator ns4:sebastian ;
    rdfs:comment "Scalability is the capability of a system, network, or process to handle a growing amount of work, or its potential to be enlarged in order to accommodate that growth. For example, it can refer to the capability of a system to increase its total output under an increased load when resources (typically hardware) are added. An analogous meaning is implied when the word is used in an economic context, where scalability of a company implies that the underlying business model offers the potential for economic growth within the company. Scalability, as a property of systems, is generally difficult to define and in any particular case it is necessary to define the specific requirements for scalability on those dimensions that are deemed important. It is a highly significant issue in electronics systems, databases, routers, and networking. (source: wikipedia)"@en ;
    rdfs:seeAlso <https://dl.acm.org/citation.cfm?doid=3266237.3266263>,
        <https://ieeexplore.ieee.org/document/6188257>,
        <https://ieeexplore.ieee.org/document/8327600>,
        "IoT-A Requirement UNI.026",
        "IoT-A Requirement UNI.234",
        "IoT-A Requirement UNI.511",
        "IoT-A Requirement UNI.711" ;
    ns4:hasDBpediaResource <http://dbpedia.org/resource/Scalability> .

ns7:StakeholderGroup a owl:Class,
        owl:NamedIndividual ;
    rdfs:label "Stakeholder Group"@en ;
    ns2:creator ns4:sebastian ;
    rdfs:comment "A Stakeholder Group is a party of people who have common interests and concerns."@en,
        "A stakeholder is everyone with an interest in a system."@en ;
    ns6:note "Stakeholders are interpreted in the same manner as outlined by ISO 42010: '<system> individual, team, organization, or classes thereof, having an interest in a system'"@en .

ns4:IDSRAMBusinessLayer a owl:NamedIndividual,
        ns4:IDSRAMLayer,
        ns4:StandardClassification ;
    rdfs:label "IDS RAM Business Layer"@en ;
    ns3:associatedWith ns4:IIRABusinessDomain,
        ns4:OceanSystemViewpoint,
        ns4:RAMIBusinessLayer,
        ns4:xRoadSystemComponents ;
    ns4:isDescribedin ns4:IDSRAMReferenceArchitectureModel ;
    ns5:alignsWith ns4:IIRABusinessDomain,
        ns4:OceanSystemViewpoint,
        ns4:RAMIBusinessLayer,
        ns4:xRoadSystemComponents ;
    ns5:frames ns4:RoleCategorization .

ns4:IDSRAMGovernance a owl:NamedIndividual,
        ns4:IdsPerspective,
        ns4:StandardClassification ;
    rdfs:label "IDS RAM Governance Perspective"@en ;
    ns3:associatedWith ns4:DtpEcosystemView,
        ns4:DtpSecurityPrivacy,
        ns4:IICFFrameworkLayer,
        ns4:RAMIBusinessLayer ;
    ns4:isDescribedin ns4:IDSRAMReferenceArchitectureModel ;
    ns5:alignsWith ns4:DtpEcosystemView,
        ns4:DtpSecurityPrivacy,
        ns4:IICFFrameworkLayer,
        ns4:RAMIBusinessLayer ;
    ns5:frames ns4:Compliance,
        ns4:Trustworthiness .

ns4:IDS_REFERENCE_ARCHITECTURE_MODEL_INDUSTRIAL_DATA_SPACE_VERSION_2_0 a owl:NamedIndividual,
        ns1:oaSpecificResource ;
    rdfs:label "IDS REFERENCE ARCHITECTURE MODEL INDUSTRIAL DATA SPACE VERSION 2.0"@en ;
    ns4:hasOpenResource <https://www.fraunhofer.de/content/dam/zv/de/Forschungsfelder/industrial-data-space/IDS_Referenz_Architecture.pdf> .

ns4:NgsiLdApiOperation a owl:NamedIndividual,
        ns4:NGSI_Context_Information_Management_API,
        ns4:StandardClassification ;
    rdfs:label "NGSI-LD API Operation"@en ;
    ns3:associatedWith ns4:FiwareDataContextManagement,
        ns4:IDSRAMProcessLayer,
        ns4:IDSRAMSystemLayer,
        ns4:IIRAConnectivity,
        ns4:IIRAControlDomain ;
    ns4:isDescribedin ns4:FIWARE ;
    ns5:alignsWith ns4:FiwareDataContextManagement,
        ns4:IDSRAMProcessLayer,
        ns4:IDSRAMSystemLayer,
        ns4:IIRAConnectivity,
        ns4:IIRAControlDomain ;
    ns5:frames ns4:Communication,
        ns4:EndpointInvocation,
        ns4:Interoperability,
        ns4:SyntacticInteroperability .

ns4:RAMIAssetlayer a owl:NamedIndividual,
        <https://w3id.org/i40/rami#RAMIITLayer>,
        ns4:StandardClassification ;
    rdfs:label "RAMI Asset Layer"@en ;
    ns3:associatedWith <https://w3id.org/i40/rami#Lifecycle_Status>,
        ns4:EdgecrossFacilityLayer,
        ns4:IIRAPhysicalSystems,
        ns4:IotaFunctionalViewpoint,
        ns4:IviAssetView ;
    ns4:isDescribedin ns4:RAMI ;
    ns5:alignsWith ns4:EdgecrossFacilityLayer,
        ns4:IIRAPhysicalSystems,
        ns4:IotaFunctionalViewpoint,
        ns4:IviAssetView ;
    ns5:frames ns4:Communication,
        ns4:Identification,
        ns4:IdentityManagement,
        ns4:Interoperability,
        ns4:Security,
        ns4:SemanticInteroperability,
        ns4:ThingDescription,
        ns4:ThingRepresentation,
        ns4:Trustworthiness,
        ns4:VirtualEntity .

ns4:ServiceDeployment a owl:NamedIndividual,
        ns4:Concern ;
    rdfs:label "Service Deployment"@en ;
    rdfs:comment "Software deployment is all of the activities that make a software system available for use. The general deployment process consists of several interrelated activities with possible transitions between them. These activities can occur at the producer side or at the consumer side or both. Because every software system is unique, the precise processes or procedures within each activity can hardly be defined. Therefore, \"deployment\" should be interpreted as a general process that has to be customized according to specific requirements or characteristics. (source: wikipedia)"@en ;
    rdfs:seeAlso "IoT-A Requirement UNI.429" ;
    ns4:hasDBpediaResource <http://dbpedia.org/resource/Software_deployment> ;
    ns5:supports ns4:ServiceLifecycleManagement .

ns4:ServiceDescription a owl:NamedIndividual,
        ns4:Concern ;
    rdfs:label "Service Description"@en ;
    ns2:creator ns4:sebastian ;
    ns7:hasStakeholder <http://dbpedia.org/ontology/developer> ;
    rdfs:comment "A Service Description plays an important role in enabling access to a service. Most service description languages are designed for machine consumption, allowing for the automatic creation of code skeletons, easier search, and classification of services. However, people may also find descriptions useful to learn about the use of parameters or the precise semantics of some operation.  (https://www.w3.org/standards/webofservices/description)"@en ;
    rdfs:seeAlso "IoT-A Requirement UNI.004",
        "IoT-A Requirement UNI.036",
        "IoT-A Requirement UNI.042",
        "IoT-A Requirement UNI.240",
        "IoT-A Requirement UNI.715" ;
    ns5:supports ns4:SemanticInteroperability .

ns4:ThingDescription a owl:NamedIndividual,
        ns4:Concern ;
    rdfs:label "Thing description"@en ;
    ns2:creator ns4:sebastian ;
    ns7:hasStakeholder <https://www.wikidata.org/wiki/Q1548249>,
        <owl:Developer> ;
    rdfs:comment "'Things' in terms of physical objects in the IoT need to be described in order to identify them and to provide further information."@en ;
    rdfs:seeAlso "IoT-A Requirement UNI.036",
        "IoT-A Requirement UNI.042",
        "IoT-A Requirement UNI.213",
        "IoT-A Requirement UNI.237",
        "IoT-A Requirement UNI.240",
        "IoT-A Requirement UNI.404",
        "IoT-A Requirement UNI.509",
        "IoT-A Requirement UNI.512" ;
    ns5:supports ns4:SemanticInteroperability .

ns4:xRoadSystemComponents a owl:NamedIndividual,
        ns4:StandardClassification,
        ns4:xRoadSection ;
    rdfs:label "x-road System Components"@en ;
    ns3:associatedWith ns4:IDSRAMBusinessLayer,
        ns4:IDSRAMProcessLayer,
        ns4:IIRASecurityFramework,
        ns4:RAMIFunctionalLayer ;
    ns4:isDescribedin ns4:xTee ;
    ns5:alignsWith ns4:IDSRAMBusinessLayer,
        ns4:IDSRAMProcessLayer,
        ns4:IIRASecurityFramework,
        ns4:RAMIFunctionalLayer ;
    ns5:frames ns4:Authentication,
        ns4:Communication,
        ns4:IdentityManagement,
        ns4:SecureCommunication,
        ns4:Security,
        ns4:SecurityConfiguration,
        ns4:Trustworthiness .

ns4:ArchitectureDescription a owl:Class ;
    rdfs:label "Architecture Description" ;
    rdfs:comment """A Reference Architecture describes the structure of a system with its element types and their structures, as well as their interaction types, among each other and with their environment. Describing this, a Reference Architecture defines restrictions for an instantiation (concrete architecture). Through abstraction from individual details, a Reference Architecture is universally valid within a specific domain. Further architectures with the same functional requirements can be constructed based on the reference architecture. Along with reference architectures comes a recommendation, based on experiences from existing developments as well as from a wide acceptance and recognition by its users or per definition. [ISO/IEC42010]

Note: It is important to distinguish the Reference Architecture from a Reference Architecture Description. While the first refers to a mental model or shared concept, the second is potentially only one of several different documents describing this model."""@en,
        """A Reference Architecture describes the structure of a system with its element types and their structures, as well as their interaction types, among each other and with their environment. Describing this, a Reference Architecture defines restrictions for an instantiation (concrete architecture). Through abstraction from individual details, a Reference Architecture is universally valid within a specific domain. Further architectures with the same functional requirements can be constructed based on the reference architecture. Along with reference architectures comes a recommendation, based on experiences from existing developments as well as from a wide acceptance and recognition by its users or per definition. [ISO/IEC42010]
Note: It is important to distinguish the Reference Architecture from a Reference Architecture Description. While the first refers to a mental model or shared concept, the second is potentially only one of several different documents describing this model."""@en,
        "ISO 42010 definition of an Architecture Description"@en ;
    rdfs:seeAlso <https://www.iso.org/standard/50508.html>,
        "https://www.iso.org/standard/50508.html" ;
    rdfs:subClassOf ns4:StandardizationFramework .

ns4:Authorization a owl:NamedIndividual,
        ns4:Concern ;
    rdfs:seeAlso <https://ieeexplore.ieee.org/document/7919553>,
        <https://ieeexplore.ieee.org/document/8552311>,
        "IoT-A Requirement UNI.319",
        "IoT-A Requirement UNI.502",
        "IoT-A Requirement UNI.503" ;
    ns5:supports ns4:Privacy .

ns4:FiwareCloudHosting a owl:NamedIndividual,
        ns4:FiwareChapter,
        ns4:StandardClassification ;
    rdfs:label "FIWARE Cloud Hosting"@en ;
    ns2:creator ns4:sebastian ;
    ns3:associatedWith ns4:IDSRAMSystemLayer,
        ns4:IIRAApplicationDomain,
        ns4:IIRADistributedDataManagement,
        ns4:IIRAScalability,
        ns4:NgsiLdArchitecture ;
    rdfs:comment """The Cloud Chapter offers Generic Enablers (GEs) that comprise the foundation for designing a modern cloud hosting infrastructure that can be used to develop, deploy and manage Future Internet applications and services. Provided hosting capabilities are of several kinds and at several levels of resource abstraction -- aiming at the needs of different applications hosted on the cloud.

The IaaS Data Center Resource Management (DCRM) GE is offering provisioning and life cycle management of virtualized resources (compute, storage, network) associated with virtual machines. The Object Storage GE offers provisioning and life cycle management of object-based storage containers and elements. The Job Scheduler GE offers the application to submit and manage computational jobs in a unified and scalable manner. The Edgelet Management GE offers the capability to host lightweight application components, called edgelets. Moreover, the IaaS Service Management (SM) GE provides the means to host complex applications. Lastly, the PaaS Management GE uses the above capabilities to offer provisioning and management of complete PaaS environments, leveraging also the Software Deployment and Configuration (SDC) GE which offers a flexible framework for installation and customization of software products (via Chef recipes) within individual virtual machines."""@en ;
    ns4:isDescribedin ns4:FIWARE ;
    ns5:alignsWith ns4:IDSRAMSystemLayer,
        ns4:IIRAApplicationDomain,
        ns4:IIRADistributedDataManagement,
        ns4:IIRAScalability,
        ns4:NgsiLdArchitecture ;
    ns5:frames ns4:Availability,
        ns4:CloudComputing,
        ns4:DataProcessing,
        ns4:DataSovereignty,
        ns4:IntegrityProtection,
        ns4:Privacy,
        ns4:Reliability,
        ns4:Safety,
        ns4:Security,
        ns4:ServiceComposition,
        ns4:ServiceDeployment,
        ns4:ServiceLifecycleManagement,
        ns4:ServiceOrchestration,
        ns4:Trustworthiness .

ns4:IotaFunctionalViewpoint a owl:NamedIndividual,
        ns4:StandardClassification,
        ns4:Viewpoint ;
    rdfs:label "IoT-A Functional Viewpoint"@en ;
    ns2:creator ns4:sebastian ;
    ns3:associatedWith ns4:IDSRAMProcessLayer,
        ns4:IDSRAMSecurity,
        ns4:IIRAFunctionalViewpoint,
        ns4:RAMIAssetlayer,
        ns4:RAMIFunctional ;
    ns4:isDescribedin ns4:IotaReferenceArchitecture ;
    ns5:alignsWith ns4:IDSRAMProcessLayer,
        ns4:IDSRAMSecurity,
        ns4:IIRAFunctionalViewpoint,
        ns4:RAMIAssetlayer,
        ns4:RAMIFunctionalLayer ;
    ns5:frames <https://w3id.org/i40/rami#Configuration>,
        <https://w3id.org/i40/rami#ProcessPlanning>,
        ns4:Authentication,
        ns4:Authorization,
        ns4:Communication,
        ns4:DataSovereignty,
        ns4:IdentityManagement,
        ns4:Privacy,
        ns4:Security,
        ns4:ServiceChoreography,
        ns4:ServiceComposition,
        ns4:ServiceOrchestration,
        ns4:ThingRepresentation,
        ns4:Trustworthiness,
        ns4:VirtualEntity .

ns4:OceanSystemViewpoint a owl:NamedIndividual,
        ns4:StandardClassification,
        ns4:Viewpoint ;
    rdfs:label "Ocean Protocol System Viewpoint"@en ;
    ns3:associatedWith ns4:DataConsumer,
        ns4:DataProvider,
        ns4:IDSRAMBusinessLayer,
        ns4:IDSRAMProcessLayer,
        ns4:IIRABusinessDomain,
        ns4:IIRAFunctionalViewpoint,
        ns4:RAMIFunctionalLayer ;
    ns4:isDescribedin ns4:OceanProtocol ;
    ns5:alignsWith ns4:IDSRAMBusinessLayer,
        ns4:IDSRAMProcessLayer,
        ns4:IIRABusinessDomain,
        ns4:IIRAFunctionalViewpoint,
        ns4:RAMIFunctionalLayer ;
    ns5:frames ns4:AI,
        ns4:Authorization,
        ns4:Availability,
        ns4:BusinessContext,
        ns4:BusinessTransactions,
        ns4:DataAccess,
        ns4:DataAccessControl,
        ns4:DataAnalytics,
        ns4:DataDiscovery,
        ns4:DataSovereignty,
        ns4:Governance,
        ns4:Identification,
        ns4:IdentityManagement,
        ns4:IntegrityProtection,
        ns4:Interoperability,
        ns4:Privacy,
        ns4:ProvenanceTracking,
        ns4:Security,
        ns4:ServiceLevelAgreements,
        ns4:ServiceLifecycleManagement,
        ns4:SyntacticInteroperability,
        ns4:Trustworthiness .

ns4:QualityOfService a owl:NamedIndividual,
        ns4:Concern ;
    rdfs:label "Quality of Service"@en ;
    rdfs:comment "Quality of service (QoS) is the overall performance of a telephony or computer network, particularly the performance seen by the users of the network. To quantitatively measure quality of service, several related aspects of the network service are often considered, such as error rates, bit rate, throughput, transmission delay, availability, jitter, etc. In the field of computer networking and other packet-switched telecommunication networks, quality of service refers to traffic prioritization and resource reservation control mechanisms rather than the achieved service quality. (source: wikipedia)"@en ;
    rdfs:seeAlso <https://dl.acm.org/citation.cfm?doid=3098208.3098210>,
        <https://dl.acm.org/citation.cfm?doid=3266237.3266263>,
        <https://ieeexplore.ieee.org/document/7919553>,
        "IoT-A Requirement UNI.613",
        "IoT-A Requirement UNI.614",
        "IoT-A Requirement UNI.717" ;
    ns4:hasDBpediaResource <http://dbpedia.org/resource/Quality_of_service> ;
    ns5:supports ns4:ServiceDescription .

ns4:Reliability a owl:NamedIndividual,
        ns4:Concern ;
    rdfs:label "Reliability"@en ;
    ns2:creator ns4:sebastian ;
    rdfs:comment "In computer networking, a reliable protocol provides reliability properties with respect to the delivery of data to the intended recipient(s), as opposed to an unreliable protocol, which does not provide notifications to the sender as to the delivery of transmitted data. (source: wikipedia)"@en ;
    rdfs:seeAlso <https://dl.acm.org/citation.cfm?doid=3266237.3266263>,
        <https://ieeexplore.ieee.org/document/7488250>,
        <https://ieeexplore.ieee.org/document/8463303>,
        "IoT-A Requirement UNI.065" ;
    ns6:note "Publications referred: '<https://www.iiconsortium.org/pdf/IIC_PUB_G4_V1.00_PB-3.pdf IIC:PUB:G4:V1.0:PB:20160926>'",
        "Publications referred: '<https://www.openfogconsortium.org/wp-content/uploads/OpenFog_Reference_Architecture_2_09_17-FINAL.pdf> OPFRA001.020817' '4.6 Reliability, Availability, and Serviceability (RAS)Pillar' 'Page 29' " ;
    ns4:hasDBpediaResource <http://dbpedia.org/resource/Reliability_(computer_networking)> ;
    ns5:supports ns4:Trustworthiness .

ns4:ServiceChoreography a owl:NamedIndividual,
        ns4:Concern ;
    rdfs:label "Service Choreography"@en ;
    ns2:creator ns4:sebastian ;
    rdfs:comment "2 to n Data Apps/Services/Data Provider are connected (without a central coordinator)"@en,
        "Service choreography is a form of service composition in which the interaction protocol between several partner services is defined from a global perspective.The intuition underlying the notion of service choreography can be summarised as follows: “Dancers dance following a global scenario without a single point of control\" That is, at run-time each participant in a service choreography executes its part of it (i.e. its role) according to the behavior of the other participants.A choreography's role specifies the expected messaging behavior of the participants that will play it in terms of the sequencing and timing of the messages that they can consume and produce. (source: wikipedia)"@en ;
    rdfs:seeAlso "IoT-A Requirement UNI.096",
        "IoT-A Requirement UNI.704" ;
    ns4:hasDBpediaResource <http://dbpedia.org/resource/Service_choreography> ;
    ns5:supports ns4:ServiceComposition .

ns4:StandardOrganization a owl:Class ;
    rdfs:label "StandardOrganization"@en ;
    ns2:creator ns4:irlan ;
    rdfs:comment "Define the standards organizations that develop and publish industry standards"@en ;
    rdfs:subClassOf ns8:Organization .

ns4:Authentication a owl:NamedIndividual,
        ns4:Concern ;
    rdfs:label "Authentication"@en ;
    ns2:creator ns4:sebastian ;
    rdfs:comment "Authentication before opening a valid connection; this can be done by just verifying the server identity or doing mutual authentication."@en ;
    rdfs:seeAlso <https://ieeexplore.ieee.org/document/6188257>,
        <https://ieeexplore.ieee.org/document/7919553Y>,
        <https://ieeexplore.ieee.org/document/8327600>,
        <https://ieeexplore.ieee.org/document/8552311>,
        "IoT-A Requirement UNI.612",
        "IoT-A Requirement UNI.618" ;
    ns5:supports ns4:IdentityManagement .

ns4:EndpointInvocation a owl:NamedIndividual,
        ns4:Concern ;
    rdfs:label "Endpoint Invocation"@en ;
    ns2:creator ns4:sebastian ;
    rdfs:comment "Mechanisms to interact with a service and to access it through the network."@en ;
    rdfs:seeAlso "IoT-A Requirement UNI.100",
        "IoT-A Requirement UNI.417" ;
    ns5:supports ns4:SyntacticInteroperability .

ns4:IIRASecurityFramework a owl:NamedIndividual,
        ns4:StandardClassification ;
    rdfs:label "IIC Security Framework"@en ;
    ns2:creator ns4:sebastian ;
    ns3:associatedWith ns4:BdvaCyberSecurityTrust,
        ns4:BdvaDataProtection,
        ns4:IDSRAMSecurity,
        ns4:xRoadSystemComponents ;
    ns6:note "Publications referred: '<https://www.iiconsortium.org/pdf/IIC_PUB_G4_V1.00_PB-3.pdf IIC:PUB:G4:V1.0:PB:20160926>'" ;
    ns4:hasOfficialResource <https://www.iiconsortium.org/IISF.htm> ;
    ns5:alignsWith ns4:BdvaCyberSecurityTrust,
        ns4:BdvaDataProtection,
        ns4:IDSRAMSecurity,
        ns4:xRoadSystemComponents .

ns4:NgsiLdArchitecture a owl:NamedIndividual,
        ns4:NGSI_Context_Information_Management_API,
        ns4:StandardClassification ;
    rdfs:label "NGSI-LD Architecture"@en ;
    ns3:associatedWith ns4:FiwareApplicationsServicesAndDataDelivery,
        ns4:FiwareCloudHosting,
        ns4:IDSRAMSystemLayer,
        ns4:IIRAImplementationViewpoint,
        ns4:InterfaceNetworksDevices,
        ns4:RAMIIntegrationLayer ;
    ns4:isDescribedin ns4:FIWARE ;
    ns5:alignsWith ns4:FiwareApplicationsServicesAndDataDelivery,
        ns4:FiwareCloudHosting,
        ns4:IDSRAMSystemLayer,
        ns4:IIRAImplementationViewpoint,
        ns4:InterfaceNetworksDevices,
        ns4:RAMIIntegrationLayer ;
    ns5:frames <https://w3id.org/i40/rami#ProcessPlanning>,
        ns4:Interoperability,
        ns4:SyntacticInteroperability .

ns4:ServiceOrchestration a owl:NamedIndividual,
        ns4:Concern ;
    rdfs:label "Service Orchestration"@en ;
    ns2:creator ns4:sebastian ;
    ns7:hasStakeholder <https://www.wikidata.org/wiki/Q1548249> ;
    rdfs:comment "A Service/Data App are connected with Data Provider, other Services/Data Apps in order to fulfill a certain task, orchestrates by a central entity."@en ;
    rdfs:seeAlso <https://dl.acm.org/citation.cfm?doid=3098208.3098210>,
        "IoT-A Requirement UNI.010" ;
    ns6:note "Publications referred: '<https://doi.org/10.1016/j.jksuci.2016.10.003>' '2.2.2. Middleware enablement' 'Page 300'" ;
    ns4:hasDBpediaResource <http://dbpedia.org/resource/Orchestration_(computing)> ;
    ns4:hasWikipediaArticle <https://en.wikipedia.org/wiki/Deployment>,
        <https://en.wikipedia.org/wiki/Orchestration_(computing)> ;
    ns5:supports ns4:ServiceComposition .

ns4:BdvaConcern a owl:Class,
        owl:NamedIndividual,
        owl:class ;
    rdfs:label "BDVA Concern"@en ;
    ns2:creator ns4:sebastian,
        "sebastian"@en ;
    rdfs:comment """The BDV Reference Model distinguishes between two different elements. On the one hand, it describes the elements that are at the core of the BDVA; on the other, it outlines the features that are developed in strong collaboration with related European activities. The BDV Reference Model is structured into horizontal and vertical concerns.
Horizontal concerns cover specific aspects along the data processing
Vertical concerns address cross-cutting issues, which may affect all the horizontal concerns. In addition, vertical concerns may also involve non-technical aspects."""@en,
        """The BDV Reference Model distinguishes between two different elements. On the one hand, it describes the elements that are at the core of the BDVA; on the other, it outlines the features that are developed in strong collaboration with related European activities. The BDV Reference Model is structured into horizontal and vertical concerns.
Horizontal concerns cover specific aspects along the data processing Vertical concerns address cross-cutting issues, which may affect all the horizontal concerns. In addition, vertical concerns may also involve non-technical aspects."""@en,
        "The BDV Reference Model distinguishes between two different elements. On the one hand, it describes the elements that are at the core of the BDVA; on the other, it outlines the features that are developed in strong collaboration with related European activities. The BDV Reference Model is structured into horizontal and vertical concerns. Horizontal concerns cover specific aspects along the data processing Vertical concerns address cross-cutting issues, which may affect all the horizontal concerns. In addition, vertical concerns may also involve non-technical aspects."@en ;
    rdfs:subClassOf ns4:StandardClassification ;
    ns4:hasOfficialResource <http://www.bdva.eu/sites/default/files/BDVA_SRIA_v4_Ed1.1.pdf> .

ns4:BdvaSira a owl:NamedIndividual,
        ns4:StandardizationFramework ;
    rdfs:label "BDVA SIRA"@en ;
    ns2:creator ns4:sebastian ;
    ns2:title "BDVA Strategic Research and Innovation Agenda"@en ;
    rdfs:comment "This Strategic Research and Innovation Agenda (SRIA) defines the overall goals, main technical and non-technical priorities, and a research and innovation roadmap for the European Public Private Partnership (PPP) on Big Data Value. The SRIA has been developed by the Big Data Value Association (BDVA), an industry-led organisation representing large businesses, small and medium-sized enterprises (SMEs), and research organisations in Europe."@en ;
    ns4:hasPublisher ns4:BDVA .

ns4:DataAccess a owl:NamedIndividual,
        ns4:Concern ;
    rdfs:label "Data Access"@en ;
    ns2:creator ns4:sebastian ;
    rdfs:comment "Data access typically refers to software and activities related to storing, retrieving, or acting on data housed in a database or other repository. [...] Data access crucially involves authorization to access different data repositories. (source: wikipedia)"@en ;
    rdfs:seeAlso "IoT-A Requirement UNI.022" ;
    ns4:hasDBpediaResource <http://dbpedia.org/resource/Data_access> .

ns4:DtpSystemView a owl:NamedIndividual,
        ns4:StandardClassification,
        ns4:Viewpoint ;
    rdfs:label "DTP System"@en ;
    ns3:associatedWith ns4:IDSRAMSystemLayer,
        ns4:IIRAConnectivity,
        ns4:IIRAOperationsDomain,
        ns4:InformationDomain,
        ns4:RAMIFunctionalLayer,
        ns4:RAMIIntegrationLayer,
        ns4:RFC_6750 ;
    ns4:isDescribedin ns4:DtpArchitecture ;
    ns5:alignsWith ns4:IDSRAMSystemLayer,
        ns4:IIRAConnectivity,
        ns4:IIRAOperationsDomain,
        ns4:InformationDomain,
        ns4:RAMIFunctionalLayer,
        ns4:RAMIIntegrationLayer ;
    ns5:frames ns4:Authentication,
        ns4:Communication,
        ns4:DataAccess,
        ns4:Interoperability,
        ns4:SecureCommunication,
        ns4:Security,
        ns4:SemanticInteroperability,
        ns4:SyntacticInteroperability,
        ns4:Trustworthiness .

ns4:IIRAImplementationViewpoint a owl:NamedIndividual,
        ns4:StandardClassification,
        ns4:Viewpoint ;
    rdfs:label "IIRA Implementation Viewpoint"@en ;
    ns3:associatedWith ns4:ControlDomain,
        ns4:DtpDeploymentView,
        ns4:FIWARE,
        ns4:IDSRAMSystemLayer,
        ns4:IIRAApplicationDomain,
        ns4:IIRABusinessDomain,
        ns4:IIRAOperationsDomain,
        ns4:InformationDomain,
        ns4:IotaDeploymentOperationViewpoint,
        ns4:NgsiLdArchitecture,
        ns4:xRoadDeploymentView ;
    ns6:note "Publications referred: '(IIC:PUB:G1:V1.80:20170131' '3.5.4 IMPLEMENTATION VIEWPOINT' 'Page 16' " ;
    ns4:isDescribedin ns4:IIRA ;
    ns5:alignsWith ns4:DtpDeploymentView,
        ns4:FIWARE,
        ns4:IotaDeploymentOperationViewpoint,
        ns4:NgsiLdArchitecture,
        ns4:xRoadDeploymentView ;
    ns5:frames ns4:CloudComputing,
        ns4:Communication,
        ns4:DataProcessing,
        ns4:EdgeComputing,
        ns4:EndpointDescription,
        ns4:Interoperability,
        ns4:SemanticInteroperability .

ns4:IIRASecurity a owl:NamedIndividual,
        ns4:IIRASystemCharacteristics,
        ns4:StandardClassification ;
    rdfs:label "IIRA Security"@en ;
    ns2:creator ns4:sebastian ;
    ns3:associatedWith ns4:DataOwner,
        ns4:DecisionMaker,
        ns4:DtpSecurityPrivacy,
        ns4:FiwareSecurity,
        ns4:IDSRAMSecurity,
        ns4:IotaAvailabilityResilience,
        ns4:IotaTrustSecurityPrivacy,
        <https://www.wikidata.org/wiki/Q1548249> ;
    ns3:isPartOf ns4:IIRAFunctionalViewpoint ;
    ns4:isDescribedin ns4:IIRA ;
    ns5:alignsWith ns4:DtpSecurityPrivacy,
        ns4:FiwareSecurity,
        ns4:IDSRAMSecurity,
        ns4:IotaAvailabilityResilience,
        ns4:IotaTrustSecurityPrivacy ;
    ns5:frames ns4:AccessPolicy,
        ns4:Authorization,
        ns4:Availability,
        ns4:CloudComputing,
        ns4:Communication,
        ns4:DataAccessControl,
        ns4:DataAtRest,
        ns4:DataInMotion,
        ns4:DataProcessing,
        ns4:DataProtection,
        ns4:DataSovereignty,
        ns4:Identification,
        ns4:IdentityManagement,
        ns4:IntegrityProtection,
        ns4:Privacy,
        ns4:Reliability,
        ns4:Resilience,
        ns4:Safety,
        ns4:SecureCommunication,
        ns4:Security,
        ns4:SecurityConfiguration,
        ns4:ServiceAccessControl,
        ns4:ServiceIsolation,
        ns4:ServiceLevelAgreements,
        ns4:ServiceLifecycleManagement,
        ns4:Trustworthiness .

ns4:IIoTConsortium a owl:Class ;
    rdfs:label "I Io T Consortium" ;
    ns2:creator ns4:sebastian,
        "sebastian" ;
    rdfs:subClassOf ns8:Organization .

ns4:IntegrityProtection a owl:NamedIndividual,
        ns4:Concern ;
    rdfs:label "Integrity Protection and Verification"@en ;
    ns2:creator ns4:sebastian ;
    ns7:hasStakeholder "Device/Service Owner" ;
    rdfs:comment "In telecommunications, the term system integrity has the following meanings: 1. * That condition of a system wherein its mandated operational and technical parameters are within the prescribed limits. 2. * The quality of an AIS when it performs its intended function in an unimpaired manner, free from deliberate or inadvertent unauthorized manipulation of the system. 3. * The state that exists when there is complete assurance that under all conditions an IT system is based on the logical correctness and reliability of the operating system, the logical completeness of the hardware and software that implement the protection mechanisms, and data integrity. (source: wikipedia)"@en,
        "Integrity protection and verification of the software stack installed; local integrity protection would be something like trusted boot; remote integrity verification means support for remote attestation."@en ;
    rdfs:seeAlso "IoT-A Requirement UNI.066",
        "IoT-A Requirement UNI.603",
        "IoT-A Requirement UNI.620" ;
    ns6:altLabel "Attestation"@en ;
    ns4:hasDBpediaResource <http://dbpedia.org/resource/System_integrity> ;
    ns5:supports ns4:DeviceSecurity .

ns4:IotaInformationViewpoint a owl:NamedIndividual,
        ns4:StandardClassification,
        ns4:Viewpoint ;
    rdfs:label "IoT-A Information Viewpoint"@en ;
    ns2:creator ns4:sebastian ;
    ns3:associatedWith ns4:IDSRAMInformationLayer,
        ns4:IDSRAMProcessLayer,
        ns4:IIRAControlDomain,
        ns4:IIRAOperationsDomain,
        ns4:InformationDomain,
        ns4:RAMICommunicationlayer ;
    rdfs:comment "One of the main purposes of connected and smart objects in the IoT is the exchange of information between each other and also with external systems. Therefore the way how to define, structure, store, process, manage and exchange information is very important. The information view helps to generate an overview about static information structure and dynamic information flow. (source: Bassi et al.: Enabling Things to Talk)"@en ;
    ns4:hasOfficialResource <http://doi.org/10.1007/978-3-642-40403-0> ;
    ns4:isDescribedin ns4:IotaReferenceArchitecture ;
    ns5:alignsWith ns4:IDSRAMInformationLayer,
        ns4:IDSRAMProcessLayer,
        ns4:IIRAControlDomain,
        ns4:IIRAOperationsDomain,
        ns4:InformationDomain,
        ns4:RAMICommunicationlayer ;
    ns5:frames ns4:Communication,
        ns4:DataAnalytics,
        ns4:DataAtRest,
        ns4:DataInMotion,
        ns4:DataLifecycleManagment,
        ns4:EndpointInvocation,
        ns4:Interoperability,
        ns4:SemanticInteroperability,
        ns4:ServiceDescription,
        ns4:SyntacticInteroperability,
        ns4:ThingRepresentation,
        ns4:VirtualEntity .

ns4:EdgecrossEdgeComputingLayer a owl:NamedIndividual,
        ns4:EdgecrossLayer,
        ns4:StandardClassification ;
    rdfs:label "Edgecross Edgecomputing Layer"@en ;
    ns3:associatedWith ns4:IDSRAMSystemLayer,
        ns4:IIRAControlDomain,
        ns4:IIRAOperationsDomain,
        ns4:InformationDomain,
        ns4:RAMIInformationLayer,
        ns4:RAMIIntegrationLayer ;
    ns4:isDescribedin ns4:EdgecrossArchitecture ;
    ns5:alignsWith ns4:IDSRAMSystemLayer,
        ns4:IIRAControlDomain,
        ns4:IIRAOperationsDomain,
        ns4:InformationDomain,
        ns4:RAMIInformationLayer,
        ns4:RAMIIntegrationLayer ;
    ns5:frames ns4:CloudComputing,
        ns4:DataProcessing,
        ns4:EdgeComputing,
        ns4:Interoperability,
        ns4:SemanticInteroperability .

ns4:FiwareSecurity a owl:NamedIndividual,
        ns4:FiwareChapter,
        ns4:StandardClassification ;
    rdfs:label "FIWARE Security"@en ;
    ns2:creator ns4:sebastian ;
    ns3:associatedWith <https://w3id.org/i40/rami#Security>,
        ns4:IDSRAMSecurity,
        ns4:IIRASecurity,
        ns4:XACML ;
    rdfs:comment """The Future Internet services will always be exposed to different types of threats that can lead to severe misuse and damage. Creating secured and trusted services without sacrificing much of the desired functionality, usability, performance and cost efficiency is a great challenge, especially in a dynamic environment where new threats and attack methods emerge on a daily basis.

The overall ambition of the Security Architecture of FIWARE is to demonstrate that the Vision of an Internet that is "secure by design" is becoming reality. Based on achievements to date and/or to come in the short-term (both from a technological but also a standardization perspective) we will show that "secure by design" is possible.

Security, Privacy and Trust in FIWARE is mainly focusing on delivering tools and techniques to have the above-mentioned security needs properly met. Furthermore a decision making support and the automation of countermeasures allow alleviating the workload of users and administrators while raising their security awareness.

The high-level Reference Architecture is formed by four main blocks of GEs: Cybersecurity, Identity and Access Management (and Enforcement), Privacy, Trust and Trustworthiness."""@en ;
    ns4:isDescribedin ns4:FIWARE ;
    ns5:alignsWith <https://w3id.org/i40/rami#Security>,
        ns4:IDSRAMSecurity,
        ns4:IIRASecurity ;
    ns5:frames ns4:Authentication,
        ns4:Authorization,
        ns4:DataAccessControl,
        ns4:DataSovereignty,
        ns4:IdentityManagement,
        ns4:Privacy,
        ns4:Security,
        ns4:Trustworthiness .

ns4:IDSRAMCertification a owl:NamedIndividual,
        ns4:IdsPerspective,
        ns4:StandardClassification ;
    rdfs:label "IDS RAM Certification Perspective"@en ;
    ns4:isDescribedin ns4:IDSRAMReferenceArchitectureModel ;
    ns5:frames ns4:Certification,
        ns4:Safety,
        ns4:Security .

ns4:Industrial_Internet_of_Things_Volume_G4_Security_Framework a owl:NamedIndividual,
        ns1:oaSpecificResource ;
    rdfs:label "Industrial Internet of Things Volume G4: Security Framework"@en ;
    ns6:note "Industrial Internet of Things Volume G4: Security Framework IIC:PUB:G4:V1.0:PB:20160926" ;
    ns4:hasOpenResource <https://www.iiconsortium.org/pdf/IIC_PUB_G4_V1.00_PB-3.pdf> .

ns4:IoT a owl:NamedIndividual,
        ns4:Concern ;
    rdfs:label "IoT"@en ;
    ns2:title "Internet of Things"@en ;
    rdfs:comment "The internet of things (IoT) is the internetworking of physical devices, vehicles (also referred to as \"connected devices\" and \"smart devices\"), buildings and other items—embedded with electronics, software, sensors, actuators, and network connectivity that enable these objects to collect and exchange data. (source: wikipedia)"@en ;
    rdfs:seeAlso "IoT-A Requirement UNI.213" ;
    ns4:hasDBpediaResource <http://dbpedia.org/resource/Internet_of_things> .

ns4:SecureCommunication a owl:NamedIndividual,
        ns4:Concern ;
    rdfs:label "Secure Communication"@en ;
    ns2:creator ns4:sebastian ;
    ns7:hasStakeholder <http://dbpedia.org/ontology/developer>,
        <http://purl.oclc.org/NET/mvco.owl#EndUser>,
        <https://w3id.org/i40/SystemArchitect> ;
    rdfs:comment <http://dbpedia.org/resource/Secure_communication>,
        "This concern frames everything necessary to establish and conduct a secure communication channel, which cannot be read, intercepted or altered by a third party. Especially relevant are encrypting techniques."@en ;
    rdfs:seeAlso <https://ieeexplore.ieee.org/document/7919553>,
        "IoT-A Requirement UNI.022",
        "IoT-A Requirement UNI.062",
        "IoT-A Requirement UNI.501",
        "IoT-A Requirement UNI.607",
        "IoT-A Requirement UNI.608",
        "IoT-A Requirement UNI.609" ;
    ns5:supports ns4:Communication,
        ns4:IntegrityProtection .

ns4:ServiceLifecycleManagement a owl:NamedIndividual,
        ns4:Concern ;
    rdfs:label "Service life-cycle management"@en ;
    ns7:hasStakeholder <https://w3id.org/i40/SystemArchitect> ;
    rdfs:comment "Information lifecycle management (ILM) refers to strategies for administering storage systems on computing devices. ILM is the practice of applying certain policies to effective information management. This practice had its basis in the management of information in paper or other physical forms (microfilm, negatives, photographs, audio or video recordings and other assets). ILM includes every phase of a \"record\" from its beginning to its end. And while it is generally applied to information that rises to the classic definition of a record (and thus related to records management), it applies to all informational assets. (source: wikipedia)"@en ;
    rdfs:seeAlso "IoT-A Requirement UNI.087" ;
    ns4:hasDBpediaResource <http://dbpedia.org/resource/Information_lifecycle_management> .

ns4:The_Industrial_Internet_of_Things_Volume_G5_Connectivity_Framework a owl:NamedIndividual,
        ns1:oaSpecificResource ;
    rdfs:label "The Industrial Internet of Things Volume G5: Connectivity Framework "@en ;
    ns6:note "The Industrial Internet of Things Volume G5: Connectivity Framework IIC:PUB:G5:V1.0:PB:20170228" ;
    ns4:hasOpenResource <https://www.iiconsortium.org/pdf/IIC_PUB_G5_V1.0_PB_20170228.pdf> .

ns4:RAMIInformationLayer a owl:NamedIndividual,
        <https://w3id.org/i40/rami#RAMIITLayer>,
        ns4:StandardClassification ;
    rdfs:label "RAMI Information Layer"@en ;
    ns3:associatedWith ns4:BdvaDataAnalytics,
        ns4:BdvaDataManagement,
        ns4:EdgecrossEdgeComputingLayer,
        ns4:IDSRAMInformationLayer,
        ns4:IIRAApplicationDomain,
        ns4:InformationDomain,
        ns4:NgsiLdInformationModel ;
    ns4:isDescribedin ns4:RAMI ;
    ns5:alignsWith ns4:BdvaDataAnalytics,
        ns4:BdvaDataManagement,
        ns4:EdgecrossEdgeComputingLayer,
        ns4:IDSRAMInformationLayer,
        ns4:IIRAApplicationDomain,
        ns4:InformationDomain,
        ns4:NgsiLdInformationModel ;
    ns5:frames ns4:DataAnalytics,
        ns4:DataDescription,
        ns4:DataProcessing,
        ns4:IntegrityProtection,
        ns4:Interoperability,
        ns4:Security,
        ns4:SemanticInteroperability,
        ns4:StreamProcessing,
        ns4:Trustworthiness .

ns4:IIRAControlDomain a owl:NamedIndividual,
        ns4:IIRAFunctionalDomain,
        ns4:StandardClassification ;
    rdfs:label "IIRA Control Domain"@en ;
    ns2:creator ns4:sebastian ;
    ns3:associatedWith ns4:EdgecrossEdgeComputingLayer,
        ns4:FiwareIotServicesEnablement,
        ns4:IDSRAMSystemLayer,
        ns4:IotaInformationViewpoint,
        ns4:NgsiLdApiOperation,
        ns4:RAMIIntegrationLayer,
        ns4:xRoadProtocolsInterfaces ;
    ns3:isPartOf ns4:IIRAFunctionalViewpoint ;
    ns6:note "Publications referred: 'IIC:PUB:G1:V1.80:20170131' '6.1 THE CONTROL DOMAIN' 'Page 27' " ;
    ns4:isDescribedin ns4:IIRA ;
    ns5:alignsWith ns4:EdgecrossEdgeComputingLayer,
        ns4:FiwareIotServicesEnablement,
        ns4:IDSRAMSystemLayer,
        ns4:IotaInformationViewpoint,
        ns4:NgsiLdApiOperation,
        ns4:RAMIIntegrationLayer,
        ns4:xRoadProtocolsInterfaces ;
    ns5:frames ns4:Actuation,
        ns4:AssetManagement,
        ns4:Communication,
        ns4:EdgeAnalytics,
        ns4:IoT,
        ns4:Sensing,
        ns4:VirtualEntity .

ns4:IIRAOperationsDomain a owl:NamedIndividual,
        ns4:IIRAFunctionalDomain,
        ns4:StandardClassification ;
    rdfs:label "IIRA Operation Domain"@en ;
    ns3:associatedWith ns4:DtpSystemView,
        ns4:EdgecrossEdgeComputingLayer,
        ns4:IDSRAMProcessLayer,
        ns4:IotaInformationViewpoint,
        ns4:IviActivityView,
        ns4:RAMIFunctionalLayer ;
    ns3:isPartOf ns4:IIRAFunctionalViewpoint ;
    ns6:note "Publications referred: 'IIC:PUB:G1:V1.80:20170131' '6.2 THE OPERATIONS DOMAIN' 'Page 30' " ;
    ns4:isDescribedin ns4:IIRA ;
    ns5:alignsWith ns4:DtpSystemView,
        ns4:EdgecrossEdgeComputingLayer,
        ns4:IDSRAMProcessLayer,
        ns4:IotaInformationViewpoint,
        ns4:IviActivityView,
        ns4:RAMIFunctionalLayer ;
    ns5:frames ns4:DataAnalytics,
        ns4:RealTimeAnalytics,
        ns4:ServiceDeployment,
        ns4:ServiceLifecycleManagement .

<https://www.wikidata.org/wiki/Q1548249> a owl:NamedIndividual .

ns4:CloudComputing a owl:NamedIndividual,
        ns4:Concern ;
    rdfs:label "Cloud Computing Capability"@en ;
    ns2:creator ns4:sebastian ;
    ns3:isPartOf ns4:DataProcessing ;
    rdfs:comment "Cloud computing is a type of Internet-based computing that provides shared computer processing resources and data to computers and other devices on demand. It is a model for enabling ubiquitous, on-demand access to a shared pool of configurable computing resources (e.g., computer networks, servers, storage, applications and services), which can be rapidly provisioned and released with minimal management effort. Cloud computing and storage solutions provide users and enterprises with various capabilities to store and process their data in third-party data centers that may be located far from the user–ranging in distance from across a city to across the world. Cloud computing relies on sharing of resources to achieve coherence and economy of scale, similar to a utility (like the electricity grid) over an electricity network. (source: wikipedia)"@en ;
    rdfs:seeAlso "IoT-A Requirement UNI.102",
        "IoT-A Requirement UNI.234" ;
    ns4:hasDBpediaResource <http://dbpedia.org/resource/Cloud_computing> .

ns4:IDSRAMReferenceArchitectureModel a owl:NamedIndividual,
        ns4:ArchitectureDescription,
        ns4:StandardizationFramework ;
    rdfs:label "IDS RAM"@en ;
    ns2:title "Industrial Data Space Reference Architecture Model"@en ;
    ns3:associatedWith ns4:IIRAFunctionalViewpoint ;
    ns4:hasPublisher ns4:IDSA ;
    ns5:alignsWith ns4:IIRAFunctionalViewpoint .

ns4:Identification a owl:NamedIndividual,
        ns4:Concern,
        ns4:StandardClassification ;
    rdfs:label "Identification"@en ;
    ns3:associatedWith <https://w3id.org/i40/rami#Identification>,
        ns4:IEC_24760,
        ns4:IEC_62443,
        ns4:ISO_24760 ;
    rdfs:comment "The concern how to identify a participant (client, endpoint etc.) in the internet."@en ;
    rdfs:seeAlso "IoT-A Requirement UNI.030",
        "IoT-A Requirement UNI.425",
        "IoT-A Requirement UNI.428",
        "IoT-A Requirement UNI.622" ;
    ns6:note "Publications referred: '<https://doi.org/10.1016/j.jksuci.2016.10.003>' 'Survey on domain specific IoT architectures' 'Page 299'" ;
    ns4:hasDBpediaResource <http://dbpedia.org/resource/Identification_(information)> ;
    ns5:alignsWith <https://w3id.org/i40/rami#Identification>,
        ns4:IEC_24760,
        ns4:IEC_62443,
        ns4:ISO_24760 ;
    ns5:supports ns4:IdentityManagement .

ns4:OpenFogReferenceArchitecture a owl:NamedIndividual,
        ns4:ArchitectureDescription,
        ns4:StandardizationFramework ;
    rdfs:label "OpenFog Reference Architecture"@en ;
    ns2:creator ns4:sebastian ;
    rdfs:comment "The OpenFog Reference Architecture (OpenFog RA) is intended to help business leaders, software developers, silicon architects, and system designers create and maintain the hardware, software and system elements necessary for fog computing."@en ;
    ns4:hasOfficialResource <https://www.openfogconsortium.org/ra/> ;
    ns4:hasPublisher ns4:OpenFogConsortium .

ns4:RAMICommunicationlayer a owl:NamedIndividual,
        <https://w3id.org/i40/rami#RAMIITLayer>,
        ns4:StandardClassification ;
    rdfs:label "RAMI Communication Layer"@en ;
    ns3:associatedWith ns4:FiwareIotServicesEnablement,
        ns4:IDSRAMSystemLayer,
        ns4:IIRAConnectivity,
        ns4:IIRADistributedDataManagement,
        ns4:IotaInformationViewpoint ;
    ns4:isDescribedin ns4:RAMI ;
    ns5:alignsWith ns4:FiwareIotServicesEnablement,
        ns4:IDSRAMSystemLayer,
        ns4:IIRAConnectivity,
        ns4:IIRADistributedDataManagement,
        ns4:IotaInformationViewpoint ;
    ns5:frames ns4:DataAccess,
        ns4:EndpointInvocation,
        ns4:Interoperability,
        ns4:ProvenanceTracking,
        ns4:Security,
        ns4:SyntacticInteroperability,
        ns4:Trustworthiness .

ns4:Safety a owl:NamedIndividual,
        ns4:Concern ;
    rdfs:label "Safety"@en ;
    ns2:creator ns4:sebastian ;
    rdfs:comment "Functional safety (as defined by the IDS) is the ability of a system to prevent physical damage."@en,
        "Safety is the state of being \"safe\" (from French sauf), the condition of being protected from harm or other non-desirable outcomes. Safety can also refer to the control of recognized hazards in order to achieve an acceptable level of risk. (source: wikipedia)"@en ;
    ns4:hasDBpediaResource <http://dbpedia.org/resource/Safety> ;
    ns5:supports ns4:Trustworthiness .

ns4:IDSRAMInformationLayer a owl:NamedIndividual,
        ns4:IDSRAMLayer,
        ns4:StandardClassification ;
    rdfs:label "IDS RAM Information Layer"@en ;
    ns3:associatedWith ns4:BdvaDataManagement,
        ns4:InformationDomain,
        ns4:IotaInformationViewpoint,
        ns4:NgsiLdDataRepresentation,
        ns4:NgsiLdInformationModel,
        ns4:RAMIInformationLayer,
        ns4:Vocabulary ;
    ns4:isDescribedin ns4:IDSRAMReferenceArchitectureModel ;
    ns5:alignsWith ns4:BdvaDataManagement,
        ns4:InformationDomain,
        ns4:IotaInformationViewpoint,
        ns4:NgsiLdDataRepresentation,
        ns4:NgsiLdInformationModel,
        ns4:RAMIInformationLayer,
        ns4:Vocabulary .

ns4:IIRAApplicationDomain a owl:NamedIndividual,
        ns4:IIRAFunctionalDomain,
        ns4:StandardClassification ;
    rdfs:label "IIRA Application Domain"@en ;
    ns2:creator ns4:sebastian ;
    ns3:associatedWith ns4:BdvaCloudAndHighPerformanceComputing,
        ns4:EdgecrossItSystemsLayer,
        ns4:FiwareAdvancedUi,
        ns4:FiwareCloudHosting,
        ns4:IDSRAMProcessLayer,
        ns4:RAMIFunctionalLayer,
        ns4:RAMIInformationLayer ;
    ns3:isPartOf ns4:IIRAFunctionalViewpoint ;
    ns6:note "Publications referred: 'IIC:PUB:G1:V1.80:20170131' '6.4 THE APPLICATION DOMAIN' 'Page 34' " ;
    ns4:isDescribedin ns4:IIRA ;
    ns5:alignsWith ns4:BdvaCloudAndHighPerformanceComputing,
        ns4:EdgecrossItSystemsLayer,
        ns4:FiwareAdvancedUi,
        ns4:FiwareCloudHosting,
        ns4:IDSRAMProcessLayer,
        ns4:RAMIFunctionalLayer,
        ns4:RAMIInformationLayer ;
    ns5:frames ns4:BdvaDataViualisationAndUserInteraction,
        ns4:DataProcessing,
        ns4:EndpointInvocation,
        ns4:Interoperability,
        ns4:SyntacticInteroperability .

ns8:Organization a owl:Class ;
    rdfs:label "Organization" .

ns4:ServiceComposition a owl:NamedIndividual,
        ns4:Concern ;
    rdfs:label "Service Composition"@en ;
    ns2:creator ns4:sebastian ;
    ns7:hasStakeholder <https://www.wikidata.org/wiki/Q1548249> ;
    rdfs:comment "2 to n Data Apps/Devices/Services are connected"@en,
        "In computing, service composability is a design principle, applied within the service-orientation design paradigm, that encourages the design of services that can be reused in multiple solutions that are themselves made up of composed services. The ability to recompose the service is ideally independent of the size and complexity of the service composition. This principle is directly responsible for the agility promised by SOA as it promotes composing new solutions by reusing existing services. (source: wikipedia)"@en ;
    rdfs:seeAlso "IoT-A Requirement UNI.014",
        "IoT-A Requirement UNI.031",
        "IoT-A Requirement UNI.043",
        "IoT-A Requirement UNI.089",
        "IoT-A Requirement UNI.094",
        "IoT-A Requirement UNI.234",
        "IoT-A Requirement UNI.244",
        "IoT-A Requirement UNI.245",
        "IoT-A Requirement UNI.247",
        "IoT-A Requirement UNI.251",
        "IoT-A Requirement UNI.253" ;
    ns4:hasDBpediaResource <http://dbpedia.org/resource/Service_composition> ;
    ns5:supports ns4:interoperability .

ns4:DataSovereignty a owl:NamedIndividual,
        ns4:Concern,
        ns4:StandardClassification ;
    rdfs:label "Data Sovereignty"@en ;
    ns2:creator ns4:sebastian ;
    ns4:hasDBpediaResource <http://dbpedia.org/resource/Cyber_sovereignty> ;
    ns4:hasWikipediaArticle <https://en.wikipedia.org/wiki/Data_sovereignty> .

ns4:The_Industrial_Internet_of_Things_Volume_G1_Reference_Architecture a owl:NamedIndividual,
        ns1:oaSpecificResource ;
    rdfs:label "Industrial Internet Architecture Version 1"@en ;
    ns6:note "The Industrial Internet of Things Volume G1: Reference Architecture IIC:PUB:G1:V1.80:20170131" ;
    ns4:hasOpenResource <https://www.iiconsortium.org/IIC_PUB_G1_V1.80_2017-01-31.pdf> .

ns4:DataProcessing a owl:NamedIndividual,
        ns4:Concern ;
    rdfs:label "Data Processing"@en ;
    ns2:creator ns4:sebastian ;
    ns7:hasStakeholder <https://www.wikidata.org/wiki/Q1548249> ;
    rdfs:comment "Data processing and analytic components from the App Store create flexible data processing pipelines."@en ;
    rdfs:seeAlso <https://dl.acm.org/citation.cfm?doid=3098208.3098210>,
        "IoT-A Requirement UNI.018" ;
    ns4:hasDBpediaResource <http://dbpedia.org/resource/Data_processing> .

ns4:FIWARE a owl:NamedIndividual,
        ns4:ArchitectureDescription,
        ns4:StandardizationFramework ;
    rdfs:label "FIWARE Architecture"@en ;
    ns2:creator ns4:sebastian ;
    ns3:associatedWith ns4:IDSRAMSystemLayer,
        ns4:IIRAImplementationViewpoint ;
    rdfs:comment "The FIWARE platform contains market-ready open source software, combining components that enable the connection to IoT with Context Information Management and Big Data services in the Cloud."@en ;
    ns4:hasOfficialResource <https://www.fiware.org/> ;
    ns4:hasPublisher ns4:Fiware ;
    ns5:alignsWith ns4:IDSRAMSystemLayer,
        ns4:IIRAImplementationViewpoint .

ns4:DataAnalytics a owl:NamedIndividual,
        ns4:Concern ;
    rdfs:label "Data Analytics"@en ;
    ns2:creator ns4:sebastian ;
    rdfs:comment "Analysis of data is a process of inspecting, cleaning, transforming, and modeling data with the goal of discovering useful information, suggesting conclusions, and supporting decision-making. Data analysis has multiple facets and approaches, encompassing diverse techniques under a variety of names, in different business, science, and social science domains. Data mining is a particular data analysis technique that focuses on modeling and knowledge discovery for predictive rather than purely descriptive purposes. Business intelligence covers data analysis that relies heavily on aggregation, focusing on business information. (source: wikipedia)"@en ;
    rdfs:seeAlso "IoT-A Requirement UNI.232" ;
    ns4:hasDBpediaResource <http://dbpedia.org/resource/Data_analysis> .

ns4:InformationDomain a owl:NamedIndividual .

ns4:RAMIFunctionalLayer a owl:NamedIndividual,
        <https://w3id.org/i40/rami#RAMIITLayer>,
        ns4:StandardClassification ;
    rdfs:label "RAMI Functional Layer"@en ;
    ns3:associatedWith ns4:BdvaDataAnalytics,
        ns4:BdvaDataViualisationAndUserInteraction,
        ns4:DtpSystemView,
        ns4:IDSRAMProcessLayer,
        ns4:IIRAApplicationDomain,
        ns4:IIRAOperationsDomain,
        ns4:IotaFunctionalViewpoint,
        ns4:IviManagementView,
        ns4:NgsiLdDataRepresentation,
        ns4:OceanSystemViewpoint,
        ns4:xRoadSystemComponents ;
    ns4:isDescribedin ns4:RAMI ;
    ns5:alignsWith ns4:BdvaDataAnalytics,
        ns4:BdvaDataViualisationAndUserInteraction,
        ns4:DtpSystemView,
        ns4:IDSRAMProcessLayer,
        ns4:IIRAApplicationDomain,
        ns4:IIRAOperationsDomain,
        ns4:IotaFunctionalViewpoint,
        ns4:IviManagementView,
        ns4:NgsiLdDataRepresentation,
        ns4:OceanSystemViewpoint,
        ns4:xRoadSystemComponents ;
    ns5:frames ns4:EndpointDescription,
        ns4:Interoperability,
        ns4:RoleCategorization,
        ns4:SemanticInteroperability,
        ns4:ServiceDescription .

ns4:RAMIIntegrationLayer a owl:NamedIndividual,
        <https://w3id.org/i40/rami#RAMIITLayer>,
        ns4:StandardClassification ;
    rdfs:label "RAMI Integration Layer"@en ;
    ns3:associatedWith ns4:DtpSystemView,
        ns4:EdgecrossEdgeComputingLayer,
        ns4:EdgecrossItSystemsLayer,
        ns4:FiwareIotServicesEnablement,
        ns4:IDSRAMSystemLayer,
        ns4:IIRAControlDomain,
        ns4:IotaEvolutionInteroperability,
        ns4:NgsiLdArchitecture,
        ns4:xRoadDeploymentView,
        ns4:xRoadProtocolsInterfaces ;
    ns4:isDescribedin ns4:RAMI ;
    ns5:alignsWith ns4:DtpSystemView,
        ns4:EdgecrossEdgeComputingLayer,
        ns4:EdgecrossItSystemsLayer,
        ns4:FiwareIotServicesEnablement,
        ns4:IDSRAMSystemLayer,
        ns4:IIRAControlDomain,
        ns4:IotaEvolutionInteroperability,
        ns4:NgsiLdArchitecture,
        ns4:xRoadDeploymentView,
        ns4:xRoadProtocolsInterfaces ;
    ns5:frames ns4:Interoperability,
        ns4:SemanticInteroperability,
        ns4:ThingDescription,
        ns4:ThingRepresentation,
        ns4:UserInteraction .

ns4:StandardizationFramework a owl:Class ;
    rdfs:label "Standarization Framework"@en ;
    ns2:creator ns4:irlan ;
    rdfs:comment "Describes existings Standardizations Initiatives, e.g, RAMI, NIST."@en ;
    ns6:altLabel "Reference Architecture"@en .

ns4:Viewpoint a owl:Class ;
    rdfs:label "Viewpoint" ;
    ns2:creator ns4:sebastian ;
    rdfs:comment "ISO 42010 definition of a Viewpoint"@en ;
    rdfs:seeAlso <https://www.iso.org/standard/50508.html> ;
    rdfs:subClassOf ns4:StandardClassification ;
    ns4:hasDBpediaResource <http://dbpedia.org/resource/ISO/IEC_42010> ;
    ns4:hasOfficialResource <http://www.iso-architecture.org/42010/> ;
    ns4:hasWikipediaArticle <https://en.wikipedia.org/wiki/ISO/IEC_42010#Conceptual_Model_-_Architecture_Viewpoint> .

ns4:IdentityManagement a owl:NamedIndividual,
        ns4:Concern ;
    rdfs:label "Identity Management"@en ;
    ns2:creator ns4:sebastian ;
    rdfs:comment "In computer security, identity and access management (IAM) is the security and business discipline that \"enables the right individuals to access the right resources at the right times and for the right reasons\".It addresses the need to ensure appropriate access to resources across increasingly heterogeneous technology environments and to meet increasingly rigorous compliance requirements. (source: wikipedia)"@en ;
    rdfs:seeAlso <https://ieeexplore.ieee.org/document/6188257>,
        <https://ieeexplore.ieee.org/document/7488250>,
        <https://ieeexplore.ieee.org/document/7919553>,
        "IoT-A Requirement UNI.048",
        "IoT-A Requirement UNI.432" ;
    ns4:hasDBpediaResource <http://dbpedia.org/resource/Identity_management> ;
    ns5:supports ns4:NonRepudiation .

ns4:Privacy a owl:NamedIndividual,
        ns4:Concern ;
    rdfs:label "Privacy"@en ;
    ns2:creator ns4:sebastian ;
    rdfs:comment "Information privacy, or data privacy (or data protection), is the relationship between collection and dissemination of data, technology, the public expectation of privacy, and the legal and political issues surrounding them. Privacy concerns exist wherever personally identifiable information or other sensitive information is collected, stored, used, and finally destroyed or deleted – in digital form or otherwise. Improper or non-existent disclosure control can be the root cause for privacy issues. Data privacy issues can arise in response to information from a wide range of sources, such as: * Healthcare records * Criminal justice investigations and proceedings * Financial institutions and transactions * Biological traits, such as genetic material * Residence and geographic records * Ethnicity * Privacy breach * Location-based service and geolocation * Web surfing behavior or user preferences using persistent cookies. (source: wikipedia)"@en ;
    rdfs:seeAlso <https://dl.acm.org/citation.cfm?doid=3098208.3098210>,
        <https://ieeexplore.ieee.org/document/6188257>,
        <https://ieeexplore.ieee.org/document/7919553>,
        "IoT-A Requirement UNI.423",
        "IoT-A Requirement UNI.424",
        "IoT-A Requirement UNI.606",
        "IoT-A Requirement UNI.623" ;
    ns4:hasDBpediaResource <http://dbpedia.org/resource/Information_privacy> ;
    ns5:supports ns4:DataSovereignty,
        ns4:Trustworthiness .

ns4:IIRAConnectivity a owl:NamedIndividual,
        ns4:IIRACrosscuttingFunction,
        ns4:StandardClassification ;
    rdfs:label "IIRA Connectivity"@en ;
    ns2:creator ns4:sebastian ;
    ns3:associatedWith ns4:BdvaDataProcessingArchitectures,
        ns4:DecisionMaker,
        ns4:DtpSystemView,
        ns4:FiwareApplicationsServicesAndDataDelivery,
        ns4:IEC_62541,
        ns4:IICF,
        ns4:IotaEvolutionInteroperability,
        ns4:LinkLayer,
        ns4:NgsiLdApiOperation,
        ns4:RAMICommunicationlayer,
        ns4:REST,
        ns4:oneM2M,
        <https://www.wikidata.org/wiki/Q1548249> ;
    ns3:isPartOf ns4:IIRAFunctionalViewpoint ;
    ns4:isDescribedin ns4:IIRA ;
    ns5:alignsWith ns4:BdvaDataProcessingArchitectures,
        ns4:DtpSystemView,
        ns4:FiwareApplicationsServicesAndDataDelivery,
        ns4:IotaEvolutionInteroperability,
        ns4:NgsiLdApiOperation,
        ns4:RAMICommunicationlayer ;
    ns5:frames ns4:Authentication,
        ns4:CardinalityOfDataSources,
        ns4:CardinalityOfParticipants,
        ns4:Communication,
        ns4:DataAccess,
        ns4:DataDiscovery,
        ns4:DynamicAdjustability,
        ns4:EndpointInvocation,
        ns4:Evolvability,
        ns4:Governance,
        ns4:IPv4Support,
        ns4:IPv6Support,
        ns4:Identification,
        ns4:IdentityManagement,
        ns4:IntegrityProtection,
        ns4:Interoperability,
        ns4:Multilaterism,
        ns4:NetworkPerformance,
        ns4:QualityOfService,
        ns4:Reliability,
        ns4:Resilience,
        ns4:Safety,
        ns4:Scalability,
        ns4:SecureCommunication,
        ns4:Security,
        ns4:SemanticInteroperability,
        ns4:ServiceChoreography,
        ns4:ServiceComposition,
        ns4:ServiceDeployment,
        ns4:ServiceDescription,
        ns4:ServiceDiscovery,
        ns4:ServiceLifecycleManagement,
        ns4:ServiceOrchestration,
        ns4:SyntacticInteroperability,
        ns4:TimeSynchronization,
        ns4:Trustworthiness,
        ns4:Unicast .

ns4:IIRA a owl:NamedIndividual,
        ns4:ArchitectureDescription,
        ns4:StandardizationFramework ;
    rdfs:label "Industrial Internet Reference Architecture"@en ;
    rdfs:comment "The IIRA addresses the need for a common architecture framework to develop interoperable IIoT systems for diverse applications across a broad spectrum of industrial verticals in the public and private sectors to achieve the true promise of IIoT."@en ;
    ns6:altLabel "IIRA" ;
    ns6:note "Publications referred: 1. The Industrial Internet of Things Volume G1: Reference Architecture (IIC:PUB:G1:V1.80:20170131)" ;
    ns4:hasOfficialResource <http://www.iiconsortium.org/IIRA.htm> ;
    ns4:hasPublisher ns4:IIC ;
    ns5:hasTargetConcern <http://purl.oclc.org/NET/mvco.owl#EndUser>,
        ns4:BusinessValue,
        ns4:DecisionMaker,
        ns4:Developer,
        ns4:MaintenanceCost,
        ns4:ProductLiability,
        ns4:ProductManager,
        ns4:ReturnOnInvestment,
        ns4:SystemEngineer,
        ns4:SystemOperator,
        <https://www.wikidata.org/wiki/Q1548249> .

ns4:IDSRAMSecurity a owl:NamedIndividual,
        ns4:IdsPerspective,
        ns4:StandardClassification ;
    rdfs:label "IDS RAM Security Perspective"@en ;
    ns3:associatedWith ns4:BdvaCyberSecurityTrust,
        ns4:BdvaDataProtection,
        ns4:FiwareSecurity,
        ns4:IIRASecurity,
        ns4:IIRASecurityFramework,
        ns4:IotaFunctionalViewpoint,
        ns4:IotaTrustSecurityPrivacy,
        ns4:RAMI ;
    rdfs:comment "The IDS Security Architecture provides means to identify participants, protect communication and data exchange transactions between them, and control the use of data after it has been sent."@en ;
    ns4:isDescribedin ns4:IDSRAMReferenceArchitectureModel ;
    ns5:alignsWith ns4:BdvaCyberSecurityTrust,
        ns4:BdvaDataProtection,
        ns4:FiwareSecurity,
        ns4:IIRASecurity,
        ns4:IIRASecurityFramework,
        ns4:IotaFunctionalViewpoint,
        ns4:IotaTrustSecurityPrivacy,
        ns4:OcfSecurity ;
    ns5:frames ns4:Authentication,
        ns4:Authorization,
        ns4:Communication,
        ns4:DataAccessControl,
        ns4:DataSovereignty,
        ns4:DataUsageControl,
        ns4:Identification,
        ns4:IdentityManagement,
        ns4:Privacy,
        ns4:SecureCommunication,
        ns4:Security,
        ns4:ServiceIsolation,
        ns4:Trustworthiness .

ns4:IIRAFunctionalViewpoint a owl:NamedIndividual,
        ns4:StandardClassification,
        ns4:Viewpoint ;
    rdfs:label "IIRA Functional Viewpoint"@en ;
    ns2:creator ns4:sebastian ;
    ns3:associatedWith ns4:IDSRAMReferenceArchitectureModel,
        ns4:IotaFunctionalViewpoint,
        ns4:OceanSystemViewpoint ;
    rdfs:comment "The IIRA Functional Viewpoint contains the IIRA Domains in order to describe technical relations and communications between the several dimensions of IoT devices."@en ;
    ns6:note "Publications referred: '(IIC:PUB:G1:V1.80:20170131' '3.5.3 FUNCTIONAL VIEWPOINT' 'Page 16' " ;
    ns4:isDescribedin ns4:IIRA ;
    ns5:alignsWith ns4:IDSRAMReferenceArchitectureModel,
        ns4:IotaFunctionalViewpoint,
        ns4:OceanSystemViewpoint ;
    ns5:frames <https://w3id.org/i40/rami#ProcessPlanning>,
        ns4:AccessPolicy,
        ns4:Actuation,
        ns4:Authentication,
        ns4:Authorization,
        ns4:Availability,
        ns4:BdvaDataViualisationAndUserInteraction,
        ns4:CardinalityOfDataSources,
        ns4:CardinalityOfParticipants,
        ns4:CloudComputing,
        ns4:Communication,
        ns4:DataAccess,
        ns4:DataAccessControl,
        ns4:DataAnalytics,
        ns4:DataAtRest,
        ns4:DataDiscovery,
        ns4:DataInMotion,
        ns4:DataProcessing,
        ns4:DataProtection,
        ns4:DataSovereignty,
        ns4:DynamicAdjustability,
        ns4:EndpointInvocation,
        ns4:Evolvability,
        ns4:Governance,
        ns4:IPv4Support,
        ns4:IPv6Support,
        ns4:Identification,
        ns4:IdentityManagement,
        ns4:IntegrityProtection,
        ns4:Interoperability,
        ns4:IoT,
        ns4:Multilaterism,
        ns4:NetworkPerformance,
        ns4:Privacy,
        ns4:QualityOfService,
        ns4:RealTimeAnalytics,
        ns4:Reliability,
        ns4:Resilience,
        ns4:Safety,
        ns4:Scalability,
        ns4:SecureCommunication,
        ns4:Security,
        ns4:SecurityConfiguration,
        ns4:SemanticInteroperability,
        ns4:Sensing,
        ns4:ServiceAccessControl,
        ns4:ServiceChoreography,
        ns4:ServiceComposition,
        ns4:ServiceDeployment,
        ns4:ServiceDescription,
        ns4:ServiceDiscovery,
        ns4:ServiceIsolation,
        ns4:ServiceLevelAgreements,
        ns4:ServiceLifecycleManagement,
        ns4:ServiceOrchestration,
        ns4:StreamProcessing,
        ns4:SyntacticInteroperability,
        ns4:TimeSynchronization,
        ns4:Trustworthiness,
        ns4:Unicast .

ns4:SyntacticInteroperability a owl:NamedIndividual,
        ns4:Concern ;
    rdfs:label "Syntactic Interoperability"@en ;
    ns2:creator ns4:sebastian ;
    rdfs:comment "If two or more systems are capable of communicating with each other, they exhibit syntactic interoperability when using specified data formats and communication protocols. XML or SQL standards are among the tools of syntactic interoperability. This is also true for lower-level data formats, such as ensuring alphabetical characters are stored in a same variation of ASCII or a Unicode format (for English or international text) in all the communicating systems. source: <https://en.wikipedia.org/wiki/Interoperability>"@en ;
    rdfs:seeAlso "IoT-A Requirement UNI.071",
        "IoT-A Requirement UNI.096",
        "IoT-A Requirement UNI.241",
        "IoT-A Requirement UNI.318",
        "IoT-A Requirement UNI.326",
        "IoT-A Requirement UNI.327",
        "IoT-A Requirement UNI.506",
        "IoT-A Requirement UNI.709",
        "UNI.327"@en ;
    ns6:note "Publications referred: '<https://doi.org/10.1016/j.jksuci.2016.10.003>' '2.8.2. Societal data service' 'Page 308'" ;
    ns4:hasWikipediaArticle <https://en.wikipedia.org/wiki/Unified_interoperability#Syntactic_interoperability> ;
    ns5:supports ns4:Interoperability .

ns4:European_BDV_SRIA_version_4_0 a owl:NamedIndividual,
        ns1:oaSpecificResource ;
    rdfs:label "BDV SRIA European Big Data Value Strategic Research and Innovation Agenda version 4.0 October 2017"@en ;
    ns4:hasOpenResource <http://bdva.eu/sites/default/files/BDVA_SRIA_v4_Ed1.1.pdf> .

ns4:TechnicalSpecification a owl:Class,
        owl:namedIndividial ;
    rdfs:label "Technical Specification"@en ;
    ns9:attributionURL "http://www.iec.ch" ;
    rdfs:comment "Specifies that a given Publication is a Technical Specification"@en,
        "Technical Specifications are often published when the subject under question is still under development or when insufficient consensus for approval of an International Standard is available.Technical Specifications approach International Standards in terms of detail and completeness, but have not yet passed through all approval stages either because consensus has not been reached or because standardization is seen to be premature."@en ;
    rdfs:isDefinedBy ns4:IEC ;
    rdfs:seeAlso <http://www.iec.ch/standardsdev/publications/ts.htm> ;
    rdfs:subClassOf ns4:Publication ;
    ns4:abbreviation "TS" .

ns4:BusinessContext a owl:NamedIndividual,
        ns4:Concern ;
    rdfs:label "Business Context"@en ;
    ns2:creator ns4:sebastian ;
    rdfs:comment "Electronic business, or e-business, is the application of information and communication technologies in support of all the activities of business. Commerce constitutes the exchange of products and services between businesses, groups and individuals and can be seen as one of the essential activities of any business. (source: wikipedia)"@en ;
    ns4:hasDBpediaResource <http://dbpedia.org/resource/Electronic_business> .

ns4:SemanticInteroperability a owl:NamedIndividual,
        ns4:Concern ;
    rdfs:label "Semantic Interoperability"@en ;
    ns2:creator ns4:sebastian ;
    ns7:hasStakeholder <http://dbpedia.org/ontology/developer> ;
    rdfs:comment """Beyond the ability of two or more computer systems to exchange information, semantic interoperability is the ability to automatically interpret the information exchanged meaningfully and accurately in order to produce useful results as defined by the end users of both systems. To achieve semantic interoperability, both sides must refer to a common information exchange reference model. 
source: <https://en.wikipedia.org/wiki/Interoperability>"""@en ;
    rdfs:seeAlso "IoT-A Requirement UNI.003",
        "IoT-A Requirement UNI.070",
        "IoT-A Requirement UNI.073",
        "IoT-A Requirement UNI.213",
        "IoT-A Requirement UNI.426",
        "IoT-A Requirement UNI.427" ;
    ns6:note "Publications referred: '<https://doi.org/10.1016/j.jksuci.2016.10.003>' '3.2. Direction toward Io<*>' 'Page 315'" ;
    ns4:hasDBpediaResource <http://dbpedia.org/resource/Semantic_interoperability> ;
    ns5:supports ns4:Interoperability .

ns4:MuhammadUsman a owl:NamedIndividual,
        ns8:Person ;
    rdfs:label "Muhammad Usman"@en .

ns4:IDSRAMProcessLayer a owl:NamedIndividual,
        ns4:IDSRAMLayer,
        ns4:StandardClassification ;
    rdfs:label "IDS RAM Process Layer"@en ;
    ns3:associatedWith ns4:BdvaDataAnalytics,
        ns4:BdvaDataManagement,
        ns4:BdvaDataProcessingArchitectures,
        ns4:DtpDeploymentView,
        ns4:FiwareApplicationsServicesAndDataDelivery,
        ns4:IIRAApplicationDomain,
        ns4:IIRAOperationsDomain,
        ns4:InformationDomain,
        ns4:InterfaceNetworksDevices,
        ns4:IotaFunctionalViewpoint,
        ns4:IotaInformationViewpoint,
        ns4:NgsiLdApiOperation,
        ns4:OceanSystemViewpoint,
        ns4:RAMIFunctionalLayer,
        ns4:xRoadProtocolsInterfaces,
        ns4:xRoadSystemComponents ;
    ns4:isDescribedin ns4:IDSRAMReferenceArchitectureModel ;
    ns5:alignsWith ns4:BdvaDataAnalytics,
        ns4:BdvaDataManagement,
        ns4:BdvaDataProcessingArchitectures,
        ns4:DtpDeploymentView,
        ns4:FiwareApplicationsServicesAndDataDelivery,
        ns4:IIRAApplicationDomain,
        ns4:IIRAOperationsDomain,
        ns4:InformationDomain,
        ns4:InterfaceNetworksDevices,
        ns4:IotaFunctionalViewpoint,
        ns4:IotaInformationViewpoint,
        ns4:NgsiLdApiOperation,
        ns4:OceanSystemViewpoint,
        ns4:RAMIFunctionalLayer,
        ns4:xRoadProtocolsInterfaces,
        ns4:xRoadSystemComponents ;
    ns5:frames ns4:ServiceChoreography,
        ns4:ServiceComposition,
        ns4:ServiceOrchestration .

ns4:OpenFog_Reference_Architecture_for_Fog_Computing a owl:NamedIndividual,
        ns1:oaSpecificResource ;
    rdfs:label "OpenFog Reference Architecture for Fog Computing"@en ;
    ns4:hasOpenResource <https://www.openfogconsortium.org/wp-content/uploads/OpenFog_Reference_Architecture_2_09_17-FINAL.pdf> .

ns4:Trustworthiness a owl:NamedIndividual,
        ns4:Concern ;
    rdfs:label "Trustworthiness"@en ;
    ns2:creator ns4:sebastian ;
    rdfs:comment "Trustworthiness is the degree of confidence one has that the system performs as expected in respect to all the key system characteristics in the face of environmental disruptions, human errors, system faults and attacks. source: IISF"@en ;
    rdfs:seeAlso <https://dl.acm.org/citation.cfm?doid=3180465.3180470>,
        <https://ieeexplore.ieee.org/document/6188257>,
        "IoT-A Requirement UNI.062",
        "IoT-A Requirement UNI.602",
        "IoT-A Requirement UNI.613" ;
    ns4:hasDBpediaResource <http://dbpedia.org/resource/Software_trustworthiness> .

ns4:Communication a owl:NamedIndividual,
        <https://w3id.org/i40/rami#AdminShellSubmodel>,
        ns4:Concern,
        ns4:StandardClassification ;
    rdfs:seeAlso "IoT-A Requirement UNI.021",
        "IoT-A Requirement UNI.095",
        "IoT-A Requirement UNI.303",
        "IoT-A Requirement UNI.306",
        "IoT-A Requirement UNI.307",
        "IoT-A Requirement UNI.308",
        "IoT-A Requirement UNI.309",
        "IoT-A Requirement UNI.310",
        "IoT-A Requirement UNI.311",
        "IoT-A Requirement UNI.312",
        "IoT-A Requirement UNI.313",
        "IoT-A Requirement UNI.315",
        "IoT-A Requirement UNI.318",
        "IoT-A Requirement UNI.321",
        "IoT-A Requirement UNI.324",
        "IoT-A Requirement UNI.716" ;
    ns4:isDescribedin ns4:AdministrationShell ;
    ns5:supports ns4:Interoperability .

ns4:Security a owl:NamedIndividual,
        ns4:Concern ;
    rdfs:label "Security"@en ;
    ns2:creator ns4:sebastian ;
    ns7:hasStakeholder <http://dbpedia.org/ontology/generalManager>,
        <https://www.wikidata.org/wiki/Q1548249> ;
    rdfs:comment "Information security, sometimes shortened to InfoSec, is the practice of defending information from unauthorized access, use, disclosure, disruption, modification, inspection, recording or destruction. It is a general term that can be used regardless of the form the data may take (e.g. electronic, physical). (source: wikipedia)"@en ;
    rdfs:seeAlso <https://dl.acm.org/citation.cfm?doid=3266237.3266263>,
        <https://ieeexplore.ieee.org/document/7919553>,
        "IoT-A Requirement UNI.040",
        "IoT-A Requirement UNI.507",
        "IoT-A Requirement UNI.626",
        "IoT-A Requirement UNI.719" ;
    ns4:hasDBpediaResource <http://dbpedia.org/resource/Information_security> ;
    ns5:supports ns4:Privacy .

ns4:IDSRAMSystemLayer a owl:NamedIndividual,
        ns4:IDSRAMLayer,
        ns4:StandardClassification ;
    rdfs:label "IDS RAM System Layer"@en ;
    ns2:creator ns4:sebastian ;
    ns3:associatedWith ns4:DtpSystemView,
        ns4:EdgecrossEdgeComputingLayer,
        ns4:EdgecrossItSystemsLayer,
        ns4:FIWARE,
        ns4:FiwareCloudHosting,
        ns4:FiwareIotServicesEnablement,
        ns4:IICFFrameworkLayer,
        ns4:IIRAControlDomain,
        ns4:IIRAImplementationViewpoint,
        ns4:IIRAPhysicalSystems,
        ns4:InterfaceNetworksDevices,
        ns4:IotaDeploymentOperationViewpoint,
        ns4:NgsiLdApiOperation,
        ns4:NgsiLdArchitecture,
        ns4:RAMICommunicationlayer,
        ns4:RAMIIntegrationLayer,
        ns4:xRoadDeploymentView ;
    ns4:isDescribedin ns4:IDSRAMReferenceArchitectureModel ;
    ns5:alignsWith ns4:DtpSystemView,
        ns4:EdgecrossEdgeComputingLayer,
        ns4:EdgecrossItSystemsLayer,
        ns4:FIWARE,
        ns4:FiwareCloudHosting,
        ns4:FiwareIotServicesEnablement,
        ns4:IICFFrameworkLayer,
        ns4:IIRAControlDomain,
        ns4:IIRAPhysicalSystems,
        ns4:InterfaceNetworksDevices,
        ns4:IotaDeploymentOperationViewpoint,
        ns4:NgsiLdApiOperation,
        ns4:NgsiLdArchitecture,
        ns4:RAMICommunicationlayer,
        ns4:RAMIIntegrationLayer,
        ns4:xRoadDeploymentView .

ns4:Interoperability a owl:NamedIndividual,
        ns4:Concern ;
    rdfs:label "Interoperability"@en ;
    ns7:hasStakeholder <https://w3id.org/i40/GeneralMAnager>,
        <https://www.wikidata.org/wiki/Q1548249> ;
    rdfs:comment "A systems ability to connect with other systems."@en,
        "Interoperability refers to the ability of two or more devices from the same vendor, or different vendors, to exchange information and use that information for correct co-operation [IEC61850-2010]."@en ;
    rdfs:seeAlso <https://dl.acm.org/citation.cfm?doid=3266237.3266263>,
        <https://ieeexplore.ieee.org/document/8249113>,
        "IoT-A Requirement UNI.008",
        "IoT-A Requirement UNI.010",
        "IoT-A Requirement UNI.023",
        "IoT-A Requirement UNI.042",
        "IoT-A Requirement UNI.047",
        "IoT-A Requirement UNI.093",
        "IoT-A Requirement UNI.094",
        "IoT-A Requirement UNI.232",
        "IoT-A Requirement UNI.712" ;
    ns4:hasDBpediaResource <http://dbpedia.org/resource/Interoperability> .

ns4:Standard a owl:Class ;
    rdfs:label "Standard"@en ;
    ns9:attributionName "Copyright © 2016 IEC Geneva, Switzerland." ;
    ns9:attributionURL <http://www.iec.ch> ;
    rdfs:comment "A document, established by consensus and approved by a recognized body, that provides, for common and repeated use, rules, guidelines or characteristics for activities or their results, aimed at the achievement of the optimum degree of order in a given context."@en ;
    rdfs:isDefinedBy ns4:IEC ;
    rdfs:seeAlso <http://www.iec.ch/standardsdev/publications/is.htm> ;
    rdfs:subClassOf ns4:Publication ;
    ns4:abbreviation "IS" .

ns8:Document a owl:Class ;
    rdfs:label "Document" .

ns4:Publication a owl:Class ;
    rdfs:label "Publication"@en ;
    rdfs:comment """Specifies a Publication. E.g., International Standards,Technical Specifications,Publicly Available Specifications,Amendments
                Technical Corrigenda,Interpretation Sheets,Technical Reports,Guides"""@en ;
    rdfs:isDefinedBy ns4:IEC ;
    rdfs:seeAlso <http://www.iec.ch/standardsdev/publications/> ;
    rdfs:subClassOf ns8:Document .

ns1:oaAnnotation a owl:Class ;
    rdfs:label "oa Annotation" .

ns4:StandardClassification a owl:Class ;
    rdfs:label "Standard Classification"@en ;
    rdfs:comment "Describes categorization areas that the different Standardizations Initiatives use to category Standards."@en .

ns4:Concern a owl:Class,
        owl:NamedIndividual ;
    rdfs:label "Concern" ;
    ns2:creator ns4:sebastian ;
    rdfs:comment "A concern regards a specific challenge or topic as defined by ISO42010. Each concern should at least be regarded by one view of an architecture."@en ;
    ns4:hasDBpediaResource <http://dbpedia.org/resource/ISO/IEC_42010> ;
    ns4:hasOfficialResource <http://www.iso-architecture.org/42010/> ;
    ns4:hasWikipediaArticle <https://en.wikipedia.org/wiki/ISO/IEC_42010#Conceptual_Model_-_Concern> .

ns1:oaRangeSelector a owl:Class ;
    rdfs:label "oa Range Selector" .

ns1:oaSpecificResource a owl:Class ;
    rdfs:label "oa Specific Resource" .

ns1:oaXPathSelector a owl:Class ;
    rdfs:label "oa X Path Selector" .

