<?xml version="1.0"?>
<?xml-stylesheet href="http://www.w3.org/2002/06/rdfs2html.xsl" type="application/xml"?>
<!DOCTYPE rdf:RDF [
   <!ENTITY cobra "http://daml.umbc.edu/ontologies/cobra/0.4/">
   <!ENTITY rdf    "http://www.w3.org/1999/02/22-rdf-syntax-ns#">
   <!ENTITY rdfs   "http://www.w3.org/2000/01/rdf-schema#">
   <!ENTITY xsd    "http://www.w3.org/2001/XMLSchema#"> 
   <!ENTITY owl    "http://www.w3.org/2002/07/owl#"> 
   <!ENTITY calc   "http://daml.umbc.edu/ontologies/cobra/0.4/calendarclock#">
   ]>
<!--
    Author: Harry Chen (mailto:harry.chen@umbc.edu)
            http://umbc.edu/~hchen4/

    Copyright 2003 Harry Chen, All Rights Reserved.
 
    This work is licensed under the Creative Commons Attribution
    License. To view a copy of this license, visit 
    http://creativecommons.org/licenses/by/1.0/ or send a letter to
    Creative Commons, 559 Nathan Abbott Way, Stanford, California
    94305, USA.  
   
    CoBrA Web Site: 
      http://cobra.umbc.edu

    This version: 
      http://daml.umbc.edu/ontologies/cobra/0.4/calendarclock

    Lastest version:
      http://daml.umbc.edu/ontologies/cobra/

    CVS Version: $Revision: 1.6 $, $Date: 2003/10/29 05:43:34 $
-->
<rdf:RDF  
   xmlns:rdf  = "&rdf;"
   xmlns:rdfs = "&rdfs;"
   xmlns:owl  = "&owl;"
   xmlns:xsd  = "&xsd;"
   xmlns      = "&calc;"
   xml:base   = "http://daml.umbc.edu/ontologies/cobra/0.4/calendarclock"> 
  
  <owl:Ontology rdf:about="&cobra;calendarclock"> 
    <owl:versionInfo>0.4</owl:versionInfo>
    <rdfs:label>COBRA-ONT Calendar/Clock Ontology</rdfs:label>
    <rdfs:comment>
      An ontology for describing calendar and clock time. 

      Parts of this ontology are adopted from the time-entry ontology
      developed by Feng Pan and Jerry R. Hobbs (USC/ISI) and DAML-Time.
    </rdfs:comment>
  </owl:Ontology>
    
  <owl:Class rdf:ID="CalendarDescription">
    <rdfs:label>CalendarDescription</rdfs:label>
    
    <rdfs:subClassOf>
      <owl:Restriction>
	<owl:onProperty rdf:resource="#dateOfMonth"/>
	<owl:maxCardinality rdf:datatype="&xsd;nonNegativeInteger">1</owl:maxCardinality>
      </owl:Restriction>
    </rdfs:subClassOf>

    <rdfs:subClassOf>
      <owl:Restriction>
	<owl:onProperty rdf:resource="#month"/>
	<owl:maxCardinality rdf:datatype="&xsd;nonNegativeInteger">1</owl:maxCardinality>
      </owl:Restriction>
    </rdfs:subClassOf>

    <rdfs:subClassOf>
      <owl:Restriction>
	<owl:onProperty rdf:resource="#year"/>
	<owl:maxCardinality rdf:datatype="&xsd;nonNegativeInteger">1</owl:maxCardinality>
      </owl:Restriction>
    </rdfs:subClassOf>
  </owl:Class>

  <owl:DatatypeProperty rdf:ID="dateOfMonth">
    <rdfs:label>dateOfMonth</rdfs:label>
    <rdfs:range rdf:resource="&xsd;gDay"/>
  </owl:DatatypeProperty>

  <owl:DatatypeProperty rdf:ID="month">
    <rdfs:label>month</rdfs:label>
    <rdfs:range rdf:resource="&xsd;gMonth"/>
  </owl:DatatypeProperty>

  <owl:DatatypeProperty rdf:ID="year">
    <rdfs:label>year</rdfs:label>
    <rdfs:range rdf:resource="&xsd;gYear"/>
  </owl:DatatypeProperty>

  <owl:Class rdf:ID="ClockDescription">
    <rdfs:label>ClockDescription</rdfs:label>
    
    <rdfs:subClassOf>
      <owl:Restriction>
	<owl:onProperty rdf:resource="#hourOfDay"/>
	<owl:maxCardinality rdf:datatype="&xsd;nonNegativeInteger">1</owl:maxCardinality>
      </owl:Restriction>
    </rdfs:subClassOf>

    <rdfs:subClassOf>
      <owl:Restriction>
	<owl:onProperty rdf:resource="#minute"/>
	<owl:maxCardinality rdf:datatype="&xsd;nonNegativeInteger">1</owl:maxCardinality>
      </owl:Restriction>
    </rdfs:subClassOf>

    <rdfs:subClassOf>
      <owl:Restriction>
	<owl:onProperty rdf:resource="#second"/>
	<owl:maxCardinality rdf:datatype="&xsd;nonNegativeInteger">1</owl:maxCardinality>
      </owl:Restriction>
    </rdfs:subClassOf>
  </owl:Class>
       
  <owl:DatatypeProperty rdf:ID="hourOfDay">
    <rdfs:label>hourOfDay</rdfs:label>
    <rdfs:comment>
      A non-negative integer that represents the hour of the day in
      the 24-hour clock (e.g., at 10:04:32 PM, the hourOfDay is 10)
    </rdfs:comment>
    <rdfs:range rdf:resource="&xsd;nonNegativeInteger"/>
  </owl:DatatypeProperty>

  <owl:DatatypeProperty rdf:ID="minute">
    <rdfs:label>minute</rdfs:label>
    <rdfs:comment>
      A non-negative integer that represents the minute within the
      hour (e.g., at 10:02:23 PM, the minute is 2).
    </rdfs:comment>
    <rdfs:range rdf:resource="&xsd;nonNegativeInteger"/>    
  </owl:DatatypeProperty>

  <owl:DatatypeProperty rdf:ID="second">
    <rdfs:label>second</rdfs:label>
    <rdfs:comment>
      A non-negative integer that represents the second within the
      minute (e.g., at 10:02:23 PM, the minute is 23).
    </rdfs:comment>
    <rdfs:range rdf:resource="&xsd;nonNegativeInteger"/>    
  </owl:DatatypeProperty>

</rdf:RDF>  
